@prefix rdfs: <http://www.w3.org/2000/01/rdf-schema#>.
@prefix owl: <http://www.w3.org/2002/07/owl#>.
@prefix xsd: <http://www.w3.org/2001/XMLSchema#>.
@prefix skos: <http://www.w3.org/2004/02/skos/core#>.
@prefix dct: <http://purl.org/dc/terms/>.
@prefix concept: <http://www.knora.org/ontology/shared/concept#>.
@prefix text: <http://www.knora.org/ontology/shared/text#>.
@prefix text-expression: <http://www.knora.org/ontology/shared/text-expression#>.
@prefix text-structure: <http://www.knora.org/ontology/shared/text-structure#>.
@prefix prosodic-structure: <http://www.knora.org/ontology/shared/prosodic-structure#>.
@prefix textedit: <http://www.knora.org/ontology/shared/text-editing#>.
@prefix scholarly-editing: <http://www.knora.org/ontology/shared/scholarly-editing#>.
@prefix infocar: <http://www.knora.org/ontology/shared/information-carrier#>.
@prefix litera: <http://www.knora.org/ontology/shared/literature#>.
@prefix ling: <http://www.knora.org/ontology/shared/linguistics#>.
@prefix lingmor: <http://www.knora.org/ontology/shared/linguistic-morphology#>.
@prefix indo: <http://www.knora.org/ontology/shared/indology#>.
@prefix knora-base: <http://www.knora.org/ontology/knora-base#>.

@base <http://www.knora.org/ontology/0041/atharvaveda>.
@prefix athar: <http://www.knora.org/ontology/0041/atharvaveda#>.

<http://www.knora.org/ontology/0041/atharvaveda>
	a owl:Ontology;
	dct:license <http://creativecommons.org/licenses/by/3.0/>;
	dct:title "An ontology about Atharvaveda"@en;
	dct:description """Formal description of specific concepts in the scientific study of Atharvaveda."""@en;
	dct:creator "Hans Cools, MD, knowledge engineer, ontologist, software developer, NIE-INE, Basel University, Switzerland"@en;
	dct:contributor
		"Magdalena Plamada, PhD, Zürich University, Switzerland"@en,
		"Reto Baumgartner, tool coordinator and software developer, NIE-INE, University of Zürich, Switzerland"@en;
	dct:publisher "Basel University, Switzerland"@en;

	knora-base:attachedToProject <http://rdfh.ch/projects/0041>.

#
# CLASSES
#

athar:Atharvaveda
	a owl:Class;
	rdfs:label "Atharvaveda"@sa, "Atharvaveda"@en, "Atharvaveda"@de;
	rdfs:comment """Fourth Veda, containing the knowledge of atharvāṇas, the procedures of beliefs and rituals addressing practical issues of daily life of the Vedic society in Hinduism, compiled about 1200 to 1000 BC."""@en;
	skos:note """The Atharvaveda contains 20 Kandas."""@en;
	rdfs:subClassOf indo:Veda.

athar:Paippalada-Samhita
	a owl:Class;
	rdfs:label "Paippalāda-Samhitā"@sa, "Paippalada-Samhita"@en, "Paippalada-Samhita"@de;
	rdfs:comment """One of the nine recensions of the Atharvaveda, along the different shakhas or Hindu theological schools, specialized in learning Vedic texts. Only this one and the Shaunakiya recension are extent."""@en;
	rdfs:subClassOf athar:Atharvaveda, textedit:Edition, [
		a owl:Restriction; owl:onProperty athar:paippaladaHasGenre; owl:minCardinality "0"^^xsd:nonNegativeInteger], [
		a owl:Restriction; owl:onProperty athar:paippaladaHasGenreValue; owl:minCardinality "0"^^xsd:nonNegativeInteger], [
		a owl:Restriction; owl:onProperty athar:paippaladaHasRecitingStyle; owl:minCardinality "0"^^xsd:nonNegativeInteger], [
		a owl:Restriction; owl:onProperty athar:paippaladaHasRecitingStyleValue; owl:minCardinality "0"^^xsd:nonNegativeInteger].

athar:Kanda
	a owl:Class;
	rdfs:label "Atharvaveda kāṇḍa"@sa, "Atharvaveda kanda"@en, "Atharvaveda Kanda"@de;
	rdfs:comment """Kande or verse section of the Atharvaveda."""@en;
	skos:note """The Atharvaveda contains 20 Kandas."""@en;
	rdfs:subClassOf prosodic-structure:VerseSection, indo:Expression, [
		a owl:Restriction; owl:onProperty athar:isKandaOfAtharvaveda; owl:minCardinality "0"^^xsd:nonNegativeInteger], [
		a owl:Restriction; owl:onProperty athar:isKandaOfAtharvavedaValue; owl:minCardinality "0"^^xsd:nonNegativeInteger].

athar:Sukta
	a owl:Class;
	rdfs:label "Atharvaveda sūkta"@sa, "Atharvaveda sukta"@en, "Atharvaveda-Sukta"@de;
	rdfs:comment """Sukta in the Atharvaveda."""@en;
	skos:note """The Atharvaveda contains 730 Suktas."""@en;
	rdfs:subClassOf litera:VerseSong, indo:Expression, text:HandwrittenText, [
		a owl:Restriction; owl:onProperty athar:isSuktaOfKanda; owl:minCardinality "0"^^xsd:nonNegativeInteger], [
		a owl:Restriction; owl:onProperty athar:isSuktaOfKandaValue; owl:minCardinality "0"^^xsd:nonNegativeInteger].

athar:Strophe
	a owl:Class;
	rdfs:label "Atharvaveda strophe"@en, "Atharvaveda-Strophe"@de;
	rdfs:comment """Group of verses or 2 half-strophes in the Atharvaveda."""@en;
	rdfs:subClassOf prosodic-structure:Strophe, text-expression:ExpressionPart, [
		a owl:Restriction; owl:onProperty indo:hasIndologicComment; owl:minCardinality "0"^^xsd:nonNegativeInteger], [
		a owl:Restriction; owl:onProperty athar:isStropheOfSukta; owl:minCardinality "0"^^xsd:nonNegativeInteger], [
		a owl:Restriction; owl:onProperty athar:isStropheOfSuktaValue; owl:minCardinality "0"^^xsd:nonNegativeInteger].

athar:HalfStrophe
	a owl:Class;
	rdfs:label "Atharvaveda half-strophe"@en, "Atharvaveda-Halbstrophe"@de;
	rdfs:comment """Half a strophe in the Atharvaveda."""@en;
	rdfs:subClassOf prosodic-structure:HalfStrophe.

athar:Verse
	a owl:Class;
	rdfs:label "Atharvaveda pada"@sa, "Atharvaveda verse"@en, "Atharvaveda-Vers"@de;
	rdfs:comment """Verse as part of a strophe in the Atharvaveda."""@en;
	skos:note """The Atharvaveda contains about 6000 verses."""@en;
	rdfs:subClassOf prosodic-structure:Verse, [
		a owl:Restriction; owl:onProperty athar:isVerseOfStrophe; owl:minCardinality "0"^^xsd:nonNegativeInteger], [
		a owl:Restriction; owl:onProperty athar:isVerseOfStropheValue; owl:minCardinality "0"^^xsd:nonNegativeInteger], [
		a owl:Restriction; owl:onProperty athar:isVerseOfHalfStrophe; owl:minCardinality "0"^^xsd:nonNegativeInteger], [
		a owl:Restriction; owl:onProperty athar:isVerseOfHalfStropheValue; owl:minCardinality "0"^^xsd:nonNegativeInteger].

athar:AdjectiveForm
	a owl:Class;
	rdfs:label "adjective form"@en, "Adjektivform"@de;
	rdfs:comment """Linguistic concept unifying occurrences of adjectives with identical literal and grammemes."""@en;
	rdfs:subClassOf lingmor:SyntacticWordForm, [
		a owl:Restriction; owl:onProperty lingmor:hasCase; owl:minCardinality "0"^^xsd:nonNegativeInteger], [
		a owl:Restriction; owl:onProperty lingmor:hasCaseValue; owl:minCardinality "0"^^xsd:nonNegativeInteger], [
		a owl:Restriction; owl:onProperty lingmor:hasGrammaticalGender; owl:minCardinality "0"^^xsd:nonNegativeInteger], [
		a owl:Restriction; owl:onProperty lingmor:hasGrammaticalGenderValue; owl:minCardinality "0"^^xsd:nonNegativeInteger], [
		a owl:Restriction; owl:onProperty lingmor:hasNumber; owl:minCardinality "0"^^xsd:nonNegativeInteger], [
		a owl:Restriction; owl:onProperty lingmor:hasNumberValue; owl:minCardinality "0"^^xsd:nonNegativeInteger], [
		a owl:Restriction; owl:onProperty athar:hasStem; owl:minCardinality "0"^^xsd:nonNegativeInteger], [
		a owl:Restriction; owl:onProperty athar:hasTermination; owl:minCardinality "0"^^xsd:nonNegativeInteger].

athar:AbsolutiveForm
	a owl:Class;
	rdfs:label "absolutive form"@en, "Absolutivform"@de;
	rdfs:comment """Linguistic concept unifying occurrences of absolutives with identical literal."""@en;
	rdfs:subClassOf lingmor:SyntacticWordForm.

athar:GerundForm
	a owl:Class;
	rdfs:label "gerund form"@en, "Gerundiumform"@de;
	rdfs:comment """Linguistic concept unifying occurrences of gerunds with identical literal and grammemes."""@en;
	rdfs:subClassOf lingmor:SyntacticWordForm, [
		a owl:Restriction; owl:onProperty lingmor:hasCase; owl:minCardinality "0"^^xsd:nonNegativeInteger], [
		a owl:Restriction; owl:onProperty lingmor:hasCaseValue; owl:minCardinality "0"^^xsd:nonNegativeInteger], [
		a owl:Restriction; owl:onProperty lingmor:hasGrammaticalGender; owl:minCardinality "0"^^xsd:nonNegativeInteger], [
		a owl:Restriction; owl:onProperty lingmor:hasGrammaticalGenderValue; owl:minCardinality "0"^^xsd:nonNegativeInteger], [
		a owl:Restriction; owl:onProperty lingmor:hasNumber; owl:minCardinality "0"^^xsd:nonNegativeInteger], [
		a owl:Restriction; owl:onProperty lingmor:hasNumberValue; owl:minCardinality "0"^^xsd:nonNegativeInteger], [
		a owl:Restriction; owl:onProperty athar:hasStem; owl:minCardinality "0"^^xsd:nonNegativeInteger], [
		a owl:Restriction; owl:onProperty athar:hasTermination; owl:minCardinality "0"^^xsd:nonNegativeInteger].

athar:InfinitiveForm
	a owl:Class;
	rdfs:label "infinitive form"@en, "Infinitivform"@de;
	rdfs:comment """Linguistic concept unifying occurrences of infinitives with identical literal."""@en;
	rdfs:subClassOf lingmor:SyntacticWordForm.

athar:NounForm
	a owl:Class;
	rdfs:label "noun form"@en, "Nomen-Form"@de;
	rdfs:comment """Linguistic concept unifying occurrences of nouns with identical literal and grammemes."""@en;
	rdfs:subClassOf lingmor:SyntacticWordForm, [
		a owl:Restriction; owl:onProperty lingmor:hasCase; owl:minCardinality "0"^^xsd:nonNegativeInteger], [
		a owl:Restriction; owl:onProperty lingmor:hasCaseValue; owl:minCardinality "0"^^xsd:nonNegativeInteger], [
		a owl:Restriction; owl:onProperty lingmor:hasComparisonDegree; owl:minCardinality "0"^^xsd:nonNegativeInteger], [
		a owl:Restriction; owl:onProperty lingmor:hasComparisonDegreeValue; owl:minCardinality "0"^^xsd:nonNegativeInteger], [
		a owl:Restriction; owl:onProperty lingmor:hasGrammaticalGender; owl:minCardinality "0"^^xsd:nonNegativeInteger], [
		a owl:Restriction; owl:onProperty lingmor:hasGrammaticalGenderValue; owl:minCardinality "0"^^xsd:nonNegativeInteger], [
		a owl:Restriction; owl:onProperty lingmor:hasNumber; owl:minCardinality "0"^^xsd:nonNegativeInteger], [
		a owl:Restriction; owl:onProperty lingmor:hasNumberValue; owl:minCardinality "0"^^xsd:nonNegativeInteger], [
		a owl:Restriction; owl:onProperty athar:hasStem; owl:minCardinality "0"^^xsd:nonNegativeInteger], [
		a owl:Restriction; owl:onProperty athar:hasTermination; owl:minCardinality "0"^^xsd:nonNegativeInteger].

athar:GenderedPronoundForm
	a owl:Class;
	rdfs:label "gendered pronoun form"@en, "Pronomen-Form mit Geschlecht"@de;
	rdfs:comment """Linguistic concept unifying occurrences of gendered pronouns with identical literal and grammemes."""@en;
	rdfs:subClassOf lingmor:SyntacticWordForm, [
		a owl:Restriction; owl:onProperty lingmor:hasCase; owl:minCardinality "0"^^xsd:nonNegativeInteger], [
		a owl:Restriction; owl:onProperty lingmor:hasCaseValue; owl:minCardinality "0"^^xsd:nonNegativeInteger], [
		a owl:Restriction; owl:onProperty lingmor:hasGrammaticalGender; owl:minCardinality "0"^^xsd:nonNegativeInteger], [
		a owl:Restriction; owl:onProperty lingmor:hasGrammaticalGenderValue; owl:minCardinality "0"^^xsd:nonNegativeInteger], [
		a owl:Restriction; owl:onProperty lingmor:hasNumber; owl:minCardinality "0"^^xsd:nonNegativeInteger], [
		a owl:Restriction; owl:onProperty lingmor:hasNumberValue; owl:minCardinality "0"^^xsd:nonNegativeInteger], [
		a owl:Restriction; owl:onProperty athar:hasStem; owl:minCardinality "0"^^xsd:nonNegativeInteger], [
		a owl:Restriction; owl:onProperty athar:hasTermination; owl:minCardinality "0"^^xsd:nonNegativeInteger].

athar:PassivePastParticipleForm
	a owl:Class;
	rdfs:label "past participle form"@en, "Pronomen-Form Vergangenheit"@de;
	rdfs:comment """Linguistic concept unifying occurrences of past participles with identical literal and grammemes."""@en;
	rdfs:subClassOf lingmor:SyntacticWordForm, [
		a owl:Restriction; owl:onProperty lingmor:hasCase; owl:minCardinality "0"^^xsd:nonNegativeInteger], [
		a owl:Restriction; owl:onProperty lingmor:hasCaseValue; owl:minCardinality "0"^^xsd:nonNegativeInteger], [
		a owl:Restriction; owl:onProperty lingmor:hasGrammaticalGender; owl:minCardinality "0"^^xsd:nonNegativeInteger], [
		a owl:Restriction; owl:onProperty lingmor:hasGrammaticalGenderValue; owl:minCardinality "0"^^xsd:nonNegativeInteger], [
		a owl:Restriction; owl:onProperty lingmor:hasNumber; owl:minCardinality "0"^^xsd:nonNegativeInteger], [
		a owl:Restriction; owl:onProperty lingmor:hasNumberValue; owl:minCardinality "0"^^xsd:nonNegativeInteger], [
		a owl:Restriction; owl:onProperty lingmor:hasTense; owl:minCardinality "0"^^xsd:nonNegativeInteger], [
		a owl:Restriction; owl:onProperty lingmor:hasTenseValue; owl:minCardinality "0"^^xsd:nonNegativeInteger], [
		a owl:Restriction; owl:onProperty lingmor:hasVerbalMood; owl:minCardinality "0"^^xsd:nonNegativeInteger], [
		a owl:Restriction; owl:onProperty lingmor:hasVerbalMoodValue; owl:minCardinality "0"^^xsd:nonNegativeInteger], [
		a owl:Restriction; owl:onProperty lingmor:hasVerbalVoice; owl:minCardinality "0"^^xsd:nonNegativeInteger], [
		a owl:Restriction; owl:onProperty lingmor:hasVerbalVoiceValue; owl:minCardinality "0"^^xsd:nonNegativeInteger], [
		a owl:Restriction; owl:onProperty athar:hasDerivation; owl:minCardinality "0"^^xsd:nonNegativeInteger], [
		a owl:Restriction; owl:onProperty athar:hasDerivationValue; owl:minCardinality "0"^^xsd:nonNegativeInteger], [
		a owl:Restriction; owl:onProperty athar:hasVerbStem; owl:minCardinality "0"^^xsd:nonNegativeInteger], [
		a owl:Restriction; owl:onProperty athar:hasVerbStemValue; owl:minCardinality "0"^^xsd:nonNegativeInteger], [
		a owl:Restriction; owl:onProperty athar:hasStem; owl:minCardinality "0"^^xsd:nonNegativeInteger], [
		a owl:Restriction; owl:onProperty athar:hasTermination; owl:minCardinality "0"^^xsd:nonNegativeInteger].

athar:UngenderedPronoundForm
	a owl:Class;
	rdfs:label "ungendered pronoun form"@en, "Pronomen-Form ohne Geschlecht"@de;
	rdfs:comment """Linguistic concept unifying occurrences of ungendered pronouns with identical literal grammemes."""@en;
	rdfs:subClassOf lingmor:SyntacticWordForm, [
		a owl:Restriction; owl:onProperty lingmor:hasCase; owl:minCardinality "0"^^xsd:nonNegativeInteger], [
		a owl:Restriction; owl:onProperty lingmor:hasCaseValue; owl:minCardinality "0"^^xsd:nonNegativeInteger], [
		a owl:Restriction; owl:onProperty lingmor:hasNumber; owl:minCardinality "0"^^xsd:nonNegativeInteger], [
		a owl:Restriction; owl:onProperty lingmor:hasNumberValue; owl:minCardinality "0"^^xsd:nonNegativeInteger], [
		a owl:Restriction; owl:onProperty lingmor:hasPerson; owl:minCardinality "0"^^xsd:nonNegativeInteger], [
		a owl:Restriction; owl:onProperty lingmor:hasPersonValue; owl:minCardinality "0"^^xsd:nonNegativeInteger], [
		a owl:Restriction; owl:onProperty athar:hasStem; owl:minCardinality "0"^^xsd:nonNegativeInteger], [
		a owl:Restriction; owl:onProperty athar:hasTermination; owl:minCardinality "0"^^xsd:nonNegativeInteger].

athar:FiniteVerbForm
	a owl:Class;
	rdfs:label "finite verb form"@en, "finite Verbform"@de;
	rdfs:comment """Linguistic concept unifying occurrences of finite verb forms with identical literal and grammemes."""@en;
	rdfs:subClassOf lingmor:SyntacticWordForm, [
		a owl:Restriction; owl:onProperty lingmor:hasNumber; owl:minCardinality "0"^^xsd:nonNegativeInteger], [
		a owl:Restriction; owl:onProperty lingmor:hasNumberValue; owl:minCardinality "0"^^xsd:nonNegativeInteger], [
		a owl:Restriction; owl:onProperty lingmor:hasPerson; owl:minCardinality "0"^^xsd:nonNegativeInteger], [
		a owl:Restriction; owl:onProperty lingmor:hasPersonValue; owl:minCardinality "0"^^xsd:nonNegativeInteger], [
		a owl:Restriction; owl:onProperty lingmor:hasTense; owl:minCardinality "0"^^xsd:nonNegativeInteger], [
		a owl:Restriction; owl:onProperty lingmor:hasTenseValue; owl:minCardinality "0"^^xsd:nonNegativeInteger], [
		a owl:Restriction; owl:onProperty lingmor:hasVerbalMood; owl:minCardinality "0"^^xsd:nonNegativeInteger], [
		a owl:Restriction; owl:onProperty lingmor:hasVerbalMoodValue; owl:minCardinality "0"^^xsd:nonNegativeInteger], [
		a owl:Restriction; owl:onProperty lingmor:hasVerbalVoice; owl:minCardinality "0"^^xsd:nonNegativeInteger], [
		a owl:Restriction; owl:onProperty lingmor:hasVerbalVoiceValue; owl:minCardinality "0"^^xsd:nonNegativeInteger], [
		a owl:Restriction; owl:onProperty athar:hasDerivation; owl:minCardinality "0"^^xsd:nonNegativeInteger], [
		a owl:Restriction; owl:onProperty athar:hasDerivationValue; owl:minCardinality "0"^^xsd:nonNegativeInteger], [
		a owl:Restriction; owl:onProperty athar:hasVerbStem; owl:minCardinality "0"^^xsd:nonNegativeInteger], [
		a owl:Restriction; owl:onProperty athar:hasVerbStemValue; owl:minCardinality "0"^^xsd:nonNegativeInteger], [
		a owl:Restriction; owl:onProperty athar:hasStem; owl:minCardinality "0"^^xsd:nonNegativeInteger], [
		a owl:Restriction; owl:onProperty athar:hasTermination; owl:minCardinality "0"^^xsd:nonNegativeInteger].

athar:Derivation
  a owl:Class;
 	rdfs:label "derivation"@en, "Derivation"@de;
	rdfs:comment """Derivation encodes the declension class of verbs."""@en;
	rdfs:subClassOf ling:Concept. #° lingmor:MorphologicalConcept

athar:VerbStem
  a owl:Class;
 	rdfs:label "verb stem"@en, "Verbstamm"@de;
	rdfs:comment """Verb stems encode additional specific meaning to a verb stem."""@en;
	rdfs:subClassOf ling:Concept. #° lingmor:MorphologicalConcept

athar:CompoundCase
	a owl:Class;
	rdfs:label "compound case"@en, "Kompositumteil"@de;
	rdfs:comment """Grammatical case indicating the part of a compound noun."""@en; #° subject
	rdfs:subClassOf lingmor:Case.



#
# PROPERTIES
#

athar:paippaladaHasGenre
	a owl:ObjectProperty;
	rdfs:label "Paippalada has genre"@en, "Paippalada hat Gattung"@de;
	rdfs:comment """Relating a Paippalada to its genre."""@en;
	rdfs:domain athar:Paippalada-Samhita;
	rdfs:range indo:Samhita;
	rdfs:subPropertyOf indo:vedaHasGenre;
	knora-base:subjectClassConstraint athar:Paippalada-Samhita;
	knora-base:objectClassConstraint indo:Samhita.

athar:paippaladaHasGenreValue
	a owl:ObjectProperty;
	rdfs:label "Paippalada has genre - statement"@en, "Paippalada hat Gattung - Festlegung"@de;
	rdfs:comment """Relating a Paippalada to a reification statement of the relation between the Paippalada and its genre."""@en;
	rdfs:subPropertyOf indo:vedaHasGenreValue;
	knora-base:subjectClassConstraint athar:Paippalada-Samhita;
	knora-base:objectClassConstraint knora-base:LinkValue.

athar:paippaladaHasRecitingStyle
	a owl:ObjectProperty;
	rdfs:label "Paippalada has reciting style"@en, "Paippalada hat Rezitationsstil"@de;
	rdfs:comment """Relating a Paippalada to a reciting style it has."""@en;
	rdfs:domain athar:Paippalada-Samhita;
	rdfs:range indo:Samhitapatha;
	rdfs:subPropertyOf indo:vedaHasRecitingStyle;
	knora-base:subjectClassConstraint athar:Paippalada-Samhita;
	knora-base:objectClassConstraint indo:Samhitapatha.

athar:paippaladaHasRecitingStyleValue
	a owl:ObjectProperty;
	rdfs:label "Veda has reciting style - statement"@en, "Veda hat Rezitationsstil - Festlegung"@de;
	rdfs:comment """Relating a Veda to a reification statement of the relation between the Veda and a reciting style it has."""@en;
	rdfs:subPropertyOf indo:vedaHasRecitingStyleValue;
	knora-base:subjectClassConstraint athar:Paippalada-Samhita;
	knora-base:objectClassConstraint knora-base:LinkValue.

athar:isKandaOfAtharvaveda
	a owl:ObjectProperty;
	rdfs:label "is kanda of Atharvaveda"@en, "ist Kanda einer Atharvaveda"@de;
	rdfs:comment """Relating a kanda to its Atharvaveda."""@en;
	rdfs:domain athar:Kanda;
	rdfs:range athar:Atharvaveda;
	rdfs:subPropertyOf concept:isPartOf;
	knora-base:subjectClassConstraint athar:Kanda;
	knora-base:objectClassConstraint athar:Atharvaveda.

athar:isKandaOfAtharvavedaValue
	a owl:ObjectProperty;
	rdfs:label "is kanda of Atharvaveda - statement"@en, "ist Kanda einer Atharvaveda - Festlegung"@de;
	rdfs:comment """Relating a kanda to a reification statement of the relation between the kanda and its Atharvaveda."""@en;
	rdfs:subPropertyOf concept:isPartOfValue;
	knora-base:subjectClassConstraint athar:Kanda;
	knora-base:objectClassConstraint knora-base:LinkValue.

athar:isSuktaOfKanda
	a owl:ObjectProperty;
	rdfs:label "is sukta of kanda"@en, "ist Sukta einer Kanda"@de;
	rdfs:comment """Relating an Atharvaveda sukta to its kanda."""@en;
	rdfs:domain athar:Sukta;
	rdfs:range athar:Kanda;
	rdfs:subPropertyOf concept:isPartOf;
	knora-base:subjectClassConstraint athar:Sukta;
	knora-base:objectClassConstraint athar:Kanda.

athar:isSuktaOfKandaValue
	a owl:ObjectProperty;
	rdfs:label "is sukta of kanda - statement"@en, "ist Sukta einer Kanda - Festlegung"@de;
	rdfs:comment """Relating an Atharvaveda sukta to a reification statement of the relation between the sukta and its kanda."""@en;
	rdfs:subPropertyOf concept:isPartOfValue;
	knora-base:subjectClassConstraint athar:Sukta;
	knora-base:objectClassConstraint knora-base:LinkValue.

athar:isStropheOfSukta
	a owl:ObjectProperty;
	rdfs:label "is strophe of sukta"@en, "ist Strophe einer Sukta"@de;
	rdfs:comment """Relating an Atharvaveda strophe to its sukta."""@en;
	rdfs:domain athar:Strophe;
	rdfs:range athar:Sukta;
	rdfs:subPropertyOf prosodic-structure:isStropheOfPoem;
	knora-base:subjectClassConstraint athar:Strophe;
	knora-base:objectClassConstraint athar:Sukta.

athar:isStropheOfSuktaValue
	a owl:ObjectProperty;
	rdfs:label "is strophe of sukta - statement"@en, "ist Strophe einer Sukta - Festlegung"@de;
	rdfs:comment """Relating an Atharvaveda strophe to a reification statement of the relation between the strophe and its sukta."""@en;
	rdfs:subPropertyOf prosodic-structure:isStropheOfPoemValue;
	knora-base:subjectClassConstraint athar:Strophe;
	knora-base:objectClassConstraint knora-base:LinkValue.

athar:isVerseOfStrophe
	a owl:ObjectProperty;
	rdfs:label "is verse of strophe"@en, "ist Vers einer Strophe"@de;
	rdfs:comment """Relating an Atharvaveda verse to a strophe it is part of."""@en;
	rdfs:domain athar:Verse;
	rdfs:range athar:Strophe;
	rdfs:subPropertyOf prosodic-structure:isVerseOfStrophe;
	knora-base:subjectClassConstraint athar:Verse;
	knora-base:objectClassConstraint athar:Strophe.

athar:isVerseOfStropheValue
	a owl:ObjectProperty;
	rdfs:label "is verse of strophe - statement"@en, "ist Vers einer Strophe - Festlegung"@de;
	rdfs:comment """Relating an Atharvaveda verse to a reification statement of the relation between the verse and a strophe it is part of."""@en;
	rdfs:subPropertyOf prosodic-structure:isVerseOfStropheValue;
	knora-base:subjectClassConstraint athar:Verse;
	knora-base:objectClassConstraint knora-base:LinkValue.

athar:isVerseOfHalfStrophe
	a owl:ObjectProperty;
	rdfs:label "is verse of half-strophe"@en, "ist Vers einer Halbstrophe"@de;
	rdfs:comment """Relating an Atharvaveda verse to a half-strophe it is part of."""@en;
	rdfs:domain athar:Verse;
	rdfs:range athar:HalfStrophe;
	rdfs:subPropertyOf prosodic-structure:isVerseOfHalfStrophe;
	knora-base:subjectClassConstraint athar:Verse;
	knora-base:objectClassConstraint athar:HalfStrophe.

athar:isVerseOfHalfStropheValue
	a owl:ObjectProperty;
	rdfs:label "is verse of strophe - statement"@en, "ist Vers einer Strophe - Festlegung"@de;
	rdfs:comment """Relating an Atharvaveda verse to a reification statement of the relation between the verse and a half-strophe it is part of."""@en;
	rdfs:subPropertyOf prosodic-structure:isVerseOfHalfStropheValue;
	knora-base:subjectClassConstraint athar:Verse;
	knora-base:objectClassConstraint knora-base:LinkValue.

athar:hasVerbStem
	a owl:ObjectProperty;
	rdfs:label "has verb stem"@en, "hat Verbastamm"@de;
	rdfs:comment """Relating a verb form to information about its stem."""@en;
	rdfs:domain lingmor:WordForm;
	rdfs:range athar:VerbStem;
	rdfs:subPropertyOf knora-base:hasLinkTo;
	knora-base:subjectClassConstraint lingmor:SyntacticWordForm;
	knora-base:objectClassConstraint athar:VerbStem.

athar:hasVerbStemValue
	a owl:ObjectProperty;
	rdfs:label "has stem type - statement"@en, "hat Verbstamm - Festlegung"@de;
	rdfs:comment """Relating a verb form to information about its stem - reification."""@en;
	rdfs:subPropertyOf knora-base:hasLinkToValue;
	knora-base:subjectClassConstraint lingmor:SyntacticWordForm;
	knora-base:objectClassConstraint knora-base:LinkValue.

athar:hasDerivation
	a owl:ObjectProperty;
	rdfs:label "has stem type"@en, "hat Stammtyp"@de;
	rdfs:comment """Relating a verb form to information about derivation."""@en;
	rdfs:domain lingmor:WordForm;
	rdfs:range lingmor:Derivation;
	rdfs:subPropertyOf knora-base:hasLinkTo;
	knora-base:subjectClassConstraint lingmor:SyntacticWordForm;
	knora-base:objectClassConstraint athar:Derivation.

athar:hasDerivationValue
	a owl:ObjectProperty;
	rdfs:label "has stem type - statement"@en, "hat Stammtyp - Festlegung"@de;
	rdfs:comment """Relating a verb form to information about derivation - reification."""@en;
	rdfs:subPropertyOf knora-base:hasLinkToValue;
	knora-base:subjectClassConstraint lingmor:SyntacticWordForm;
	knora-base:objectClassConstraint knora-base:LinkValue.

athar:hasStem
	a owl:ObjectProperty;
	rdfs:label "has stem"@en, "hat Stamm"@de;
	rdfs:comment """Relating a human natural language expression to a linguistic comment as a textual statement about the expression."""@en;
	rdfs:domain lingmor:SyntacticWordForm;
	rdfs:range rdfs:Literal;
	rdfs:subPropertyOf knora-base:hasValue;
	knora-base:subjectClassConstraint lingmor:SyntacticWordForm;
	knora-base:objectClassConstraint knora-base:TextValue.

athar:hasTermination
	a owl:ObjectProperty;
	rdfs:label "has termination"@en, "hat Endung"@de;
	rdfs:comment """Relating a human natural language expression to a linguistic comment as a textual statement about the expression."""@en;
	rdfs:domain lingmor:SyntacticWordForm;
	rdfs:range rdfs:Literal;
	rdfs:subPropertyOf knora-base:hasValue;
	knora-base:subjectClassConstraint lingmor:SyntacticWordForm;
	knora-base:objectClassConstraint knora-base:TextValue.