@prefix rdfs: <http://www.w3.org/2000/01/rdf-schema#>.
@prefix owl: <http://www.w3.org/2002/07/owl#>.
@prefix xsd: <http://www.w3.org/2001/XMLSchema#>.
@prefix skos: <http://www.w3.org/2004/02/skos/core#>.
@prefix dct: <http://purl.org/dc/terms/>.
@prefix concept: <http://www.knora.org/ontology/shared/concept#>.
@prefix text: <http://www.knora.org/ontology/shared/text#>.
@prefix text-expression: <http://www.knora.org/ontology/shared/text-expression#>.
@prefix text-structure: <http://www.knora.org/ontology/shared/text-structure#>.
@prefix prosodic-structure: <http://www.knora.org/ontology/shared/prosodic-structure#>.
@prefix textedit: <http://www.knora.org/ontology/shared/text-editing#>.
@prefix scholarly-editing: <http://www.knora.org/ontology/shared/scholarly-editing#>.
@prefix infocar: <http://www.knora.org/ontology/shared/information-carrier#>.
@prefix litera: <http://www.knora.org/ontology/shared/literature#>.
@prefix ling: <http://www.knora.org/ontology/shared/linguistics#>.
@prefix indo: <http://www.knora.org/ontology/shared/indology#>.
@prefix knora-base: <http://www.knora.org/ontology/knora-base#>.

@base <http://www.knora.org/ontology/0041/atharvaveda>.
@prefix athar: <http://www.knora.org/ontology/0041/atharvaveda#>.

<http://www.knora.org/ontology/0041/atharvaveda>
	a owl:Ontology;
	dct:license <http://creativecommons.org/licenses/by/3.0/>;
	dct:title "An ontology about Atharvaveda"@en;
	dct:description """Formal description of specific concepts in the scientific study of Atharvaveda."""@en;
	dct:creator "Hans Cools, MD, knowledge engineer, ontologist, software developer, NIE-INE, Basel University, Switzerland"@en;
	dct:contributor
		"Magdalena Plamada, PhD, Zürich University, Switzerland"@en,
		"Reto Baumgartner, tool coordinator and software developer, NIE-INE, University of Zürich, Switzerland"@en;
	dct:publisher "Basel University, Switzerland"@en;

	knora-base:attachedToProject <http://rdfh.ch/projects/0041>.

#
# CLASSES
#

athar:Atharvaveda
	a owl:Class;
	rdfs:label "Atharvaveda"@sa, "Atharvaveda"@en, "Atharvaveda"@de;
	rdfs:comment """Fourth Veda, containing the knowledge of atharvāṇas, the procedures of beliefs and rituals addressing practical issues of daily life of the Vedic society in Hinduism, compiled about 1200 to 1000 BC."""@en;
	skos:note """The Atharvaveda contains 20 Kandas."""@en;
	rdfs:subClassOf indo:Veda.

athar:Paippalada-Samhita
	a owl:Class;
	rdfs:label "Paippalāda-Samhitā"@sa, "Paippalada-Samhita"@en, "Paippalada-Samhita"@de;
	rdfs:comment """One of the nine recensions of the Atharvaveda, along the different shakhas or Hindu theological schools, specialized in learning Vedic texts. Only this one and the Shaunakiya recension are extent."""@en;
	rdfs:subClassOf athar:Atharvaveda, textedit:Edition, [
		a owl:Restriction; owl:onProperty athar:paippaladaHasGenre; owl:minCardinality "0"^^xsd:nonNegativeInteger], [
		a owl:Restriction; owl:onProperty athar:paippaladaHasGenreValue; owl:minCardinality "0"^^xsd:nonNegativeInteger], [
		a owl:Restriction; owl:onProperty athar:paippaladaHasRecitingStyle; owl:minCardinality "0"^^xsd:nonNegativeInteger], [
		a owl:Restriction; owl:onProperty athar:paippaladaHasRecitingStyleValue; owl:minCardinality "0"^^xsd:nonNegativeInteger].

athar:Kanda
	a owl:Class;
	rdfs:label "Atharvaveda kāṇḍa"@sa, "Atharvaveda kanda"@en, "Atharvaveda Kanda"@de;
	rdfs:comment """Kanda or verse section of the Atharvaveda."""@en;
	skos:note """The Atharvaveda contains 20 Kandas."""@en;
	rdfs:subClassOf prosodic-structure:VerseSection, indo:Expression, [
		a owl:Restriction; owl:onProperty athar:isKandaOfAtharvaveda; owl:minCardinality "0"^^xsd:nonNegativeInteger], [
		a owl:Restriction; owl:onProperty athar:isKandaOfAtharvavedaValue; owl:minCardinality "0"^^xsd:nonNegativeInteger].

athar:Sukta
	a owl:Class;
	rdfs:label "Atharvaveda sūkta"@sa, "Atharvaveda sukta"@en, "Atharvaveda-Sukta"@de;
	rdfs:comment """Sukta in the Atharvaveda."""@en;
	skos:note """The Atharvaveda contains 730 Suktas."""@en;
	rdfs:subClassOf litera:VerseSong, indo:Expression, text:HandwrittenText, [
		a owl:Restriction; owl:onProperty athar:isSuktaOfKanda; owl:minCardinality "0"^^xsd:nonNegativeInteger], [
		a owl:Restriction; owl:onProperty athar:isSuktaOfKandaValue; owl:minCardinality "0"^^xsd:nonNegativeInteger].

athar:Strophe
	a owl:Class;
	rdfs:label "Atharvaveda strophe"@en, "Atharvaveda-Strophe"@de;
	rdfs:comment """Group of verses or 2 half-strophes in the Atharvaveda."""@en;
	rdfs:subClassOf prosodic-structure:Strophe, text-expression:ExpressionPart, [
		a owl:Restriction; owl:onProperty indo:hasIndologicComment; owl:minCardinality "0"^^xsd:nonNegativeInteger], [
		a owl:Restriction; owl:onProperty athar:isStropheOfSukta; owl:minCardinality "0"^^xsd:nonNegativeInteger], [
		a owl:Restriction; owl:onProperty athar:isStropheOfSuktaValue; owl:minCardinality "0"^^xsd:nonNegativeInteger].

athar:HalfStrophe
	a owl:Class;
	rdfs:label "Atharvaveda half-strophe"@en, "Atharvaveda-Halbstrophe"@de;
	rdfs:comment """Half a strophe in the Atharvaveda."""@en;
	rdfs:subClassOf prosodic-structure:HalfStrophe.

athar:Verse
	a owl:Class;
	rdfs:label "Atharvaveda pada"@sa, "Atharvaveda verse"@en, "Atharvaveda-Vers"@de;
	rdfs:comment """Verse as part of a strophe in the Atharvaveda."""@en;
	skos:note """The Atharvaveda contains about 6000 verses."""@en;
	rdfs:subClassOf prosodic-structure:Verse, [
		a owl:Restriction; owl:onProperty athar:isVerseOfStrophe; owl:minCardinality "0"^^xsd:nonNegativeInteger], [
		a owl:Restriction; owl:onProperty athar:isVerseOfStropheValue; owl:minCardinality "0"^^xsd:nonNegativeInteger], [
		a owl:Restriction; owl:onProperty athar:isVerseOfHalfStrophe; owl:minCardinality "0"^^xsd:nonNegativeInteger], [
		a owl:Restriction; owl:onProperty athar:isVerseOfHalfStropheValue; owl:minCardinality "0"^^xsd:nonNegativeInteger].

#
# PROPERTIES
#

athar:paippaladaHasGenre
	a owl:ObjectProperty;
	rdfs:label "Paippalada has genre"@en, "Paippalada hat Gattung"@de;
	rdfs:comment """Relating a Paippalada to its genre."""@en;
	rdfs:subPropertyOf indo:vedaHasGenre;
	knora-base:subjectClassConstraint athar:Paippalada-Samhita;
	knora-base:objectClassConstraint indo:Samhita.

athar:paippaladaHasGenreValue
	a owl:ObjectProperty;
	rdfs:label "Paippalada has genre - statement"@en, "Paippalada hat Gattung - Festlegung"@de;
	rdfs:comment """Relating a Paippalada to a reification statement of the relation between the Paippalada and its genre."""@en;
	rdfs:subPropertyOf indo:vedaHasGenreValue;
	knora-base:subjectClassConstraint athar:Paippalada-Samhita;
	knora-base:objectClassConstraint knora-base:LinkValue.

athar:paippaladaHasRecitingStyle
	a owl:ObjectProperty;
	rdfs:label "Paippalada has reciting style"@en, "Paippalada hat Rezitationsstil"@de;
	rdfs:comment """Relating a Paippalada to a reciting style it has."""@en;
	rdfs:subPropertyOf indo:vedaHasRecitingStyle;
	knora-base:subjectClassConstraint athar:Paippalada-Samhita;
	knora-base:objectClassConstraint indo:Samhitapatha.

athar:paippaladaHasRecitingStyleValue
	a owl:ObjectProperty;
	rdfs:label "Veda has reciting style - statement"@en, "Veda hat Rezitationsstil - Festlegung"@de;
	rdfs:comment """Relating a Veda to a reification statement of the relation between the Veda and a reciting style it has."""@en;
	rdfs:subPropertyOf indo:vedaHasRecitingStyleValue;
	knora-base:subjectClassConstraint athar:Paippalada-Samhita;
	knora-base:objectClassConstraint knora-base:LinkValue.

athar:isKandaOfAtharvaveda
	a owl:ObjectProperty;
	rdfs:label "is kanda of Atharvaveda"@en, "ist Kanda einer Atharvaveda"@de;
	rdfs:comment """Relating a kanda to its Atharvaveda."""@en;
	rdfs:subPropertyOf concept:isPartOf;
	knora-base:subjectClassConstraint athar:Kanda;
	knora-base:objectClassConstraint athar:Atharvaveda.

athar:isKandaOfAtharvavedaValue
	a owl:ObjectProperty;
	rdfs:label "is kanda of Atharvaveda - statement"@en, "ist Kanda einer Atharvaveda - Festlegung"@de;
	rdfs:comment """Relating a kanda to a reification statement of the relation between the kanda and its Atharvaveda."""@en;
	rdfs:subPropertyOf concept:isPartOfValue;
	knora-base:subjectClassConstraint athar:Kanda;
	knora-base:objectClassConstraint knora-base:LinkValue.

athar:isSuktaOfKanda
	a owl:ObjectProperty;
	rdfs:label "is sukta of kanda"@en, "ist Sukta einer Kanda"@de;
	rdfs:comment """Relating an Atharvaveda sukta to its kanda."""@en;
	rdfs:subPropertyOf concept:isPartOf;
	knora-base:subjectClassConstraint athar:Sukta;
	knora-base:objectClassConstraint athar:Kanda.

athar:isSuktaOfKandaValue
	a owl:ObjectProperty;
	rdfs:label "is sukta of kanda - statement"@en, "ist Sukta einer Kanda - Festlegung"@de;
	rdfs:comment """Relating an Atharvaveda sukta to a reification statement of the relation between the sukta and its kanda."""@en;
	rdfs:subPropertyOf concept:isPartOfValue;
	knora-base:subjectClassConstraint athar:Sukta;
	knora-base:objectClassConstraint knora-base:LinkValue.

athar:isStropheOfSukta
	a owl:ObjectProperty;
	rdfs:label "is strophe of sukta"@en, "ist Strophe einer Sukta"@de;
	rdfs:comment """Relating an Atharvaveda strophe to its sukta."""@en;
	rdfs:subPropertyOf prosodic-structure:isStropheOfPoem;
	knora-base:subjectClassConstraint athar:Strophe;
	knora-base:objectClassConstraint athar:Sukta.

athar:isStropheOfSuktaValue
	a owl:ObjectProperty;
	rdfs:label "is strophe of sukta - statement"@en, "ist Strophe einer Sukta - Festlegung"@de;
	rdfs:comment """Relating an Atharvaveda strophe to a reification statement of the relation between the strophe and its sukta."""@en;
	rdfs:subPropertyOf prosodic-structure:isStropheOfPoemValue;
	knora-base:subjectClassConstraint athar:Strophe;
	knora-base:objectClassConstraint knora-base:LinkValue.

athar:isVerseOfStrophe
	a owl:ObjectProperty;
	rdfs:label "is verse of strophe"@en, "ist Vers einer Strophe"@de;
	rdfs:comment """Relating an Atharvaveda verse to a strophe it is part of."""@en;
	rdfs:subPropertyOf prosodic-structure:isVerseOfStrophe;
	knora-base:subjectClassConstraint athar:Verse;
	knora-base:objectClassConstraint athar:Strophe.

athar:isVerseOfStropheValue
	a owl:ObjectProperty;
	rdfs:label "is verse of strophe - statement"@en, "ist Vers einer Strophe - Festlegung"@de;
	rdfs:comment """Relating an Atharvaveda verse to a reification statement of the relation between the verse and a strophe it is part of."""@en;
	rdfs:subPropertyOf prosodic-structure:isVerseOfStropheValue;
	knora-base:subjectClassConstraint athar:Verse;
	knora-base:objectClassConstraint knora-base:LinkValue.

athar:isVerseOfHalfStrophe
	a owl:ObjectProperty;
	rdfs:label "is verse of half-strophe"@en, "ist Vers einer Halbstrophe"@de;
	rdfs:comment """Relating an Atharvaveda verse to a half-strophe it is part of."""@en;
	rdfs:subPropertyOf prosodic-structure:isVerseOfHalfStrophe;
	knora-base:subjectClassConstraint athar:Verse;
	knora-base:objectClassConstraint athar:HalfStrophe.

athar:isVerseOfHalfStropheValue
	a owl:ObjectProperty;
	rdfs:label "is verse of strophe - statement"@en, "ist Vers einer Strophe - Festlegung"@de;
	rdfs:comment """Relating an Atharvaveda verse to a reification statement of the relation between the verse and a half-strophe it is part of."""@en;
	rdfs:subPropertyOf prosodic-structure:isVerseOfHalfStropheValue;
	knora-base:subjectClassConstraint athar:Verse;
	knora-base:objectClassConstraint knora-base:LinkValue.