@prefix rdfs: <http://www.w3.org/2000/01/rdf-schema#>.
@prefix owl: <http://www.w3.org/2002/07/owl#>.
@prefix xsd: <http://www.w3.org/2001/XMLSchema#>.
@prefix skos: <http://www.w3.org/2004/02/skos/core#>.
@prefix dct: <http://purl.org/dc/terms/>.
@prefix event: <http://www.knora.org/ontology/shared/event#>.
@prefix human: <http://www.knora.org/ontology/shared/human#>.
@prefix org: <http://www.knora.org/ontology/shared/organization#>.
@prefix knora-base: <http://www.knora.org/ontology/knora-base#>.

@base <http://www.knora.org/ontology/shared/catholic-organization>.
@prefix cathorg: <http://www.knora.org/ontology/shared/catholic-organization#>.

<http://www.knora.org/ontology/shared/catholic-organization>
	a owl:Ontology;
	dct:license <http://creativecommons.org/licenses/by/3.0/>;
	dct:title "An ontology about catholic organization"@en;
	dct:description """Formal description of catholic organization, general subclasses, related classes, properties, and instances."""@en;
	dct:creator "Hans Cools, MD, knowledge engineer, ontologist, software developer, NIE-INE, Basel University, Switzerland"@en;
	dct:contributor "Prof. Dr. Ueli Zahnd, Faculty of Theology, University of Basel, Switzerland"@en, "Gabriel MÃ¼ller, Faculty of Theology, University of Basel, Switzerland"@en;

	knora-base:attachedToProject <http://www.knora.org/ontology/knora-base#DefaultSharedOntologiesProject>.

#
# CLASSES
#

cathorg:Organization
	a owl:Class;
	#rdfs:isDefinedBy <http://www.knora.org/ontology/shared/catholic-organization#>;
	rdfs:label "catholic organization"@en;
	rdfs:comment """Organization representing a catholic belief."""@en;
	rdfs:subClassOf org:ReligiousOrganization.

cathorg:Person
	a owl:Class;
	#rdfs:isDefinedBy <http://www.knora.org/ontology/shared/catholic-organization#>;
	rdfs:label "catholic person"@en, "katholische Person"@de, "personne catholique"@fr, "persona cattolica"@it;
	rdfs:comment """Person having a catholic belief."""@en;
	rdfs:subClassOf org:ReligiousPerson, [
		a owl:Restriction; owl:onProperty cathorg:isMemberOf; owl:minCardinality "0"^^xsd:nonNegativeInteger], [
		a owl:Restriction; owl:onProperty cathorg:isMemberOfValue; owl:minCardinality "0"^^xsd:nonNegativeInteger].

cathorg:Order
	a owl:Class;
	#rdfs:isDefinedBy <http://www.knora.org/ontology/shared/catholic-organization#>;
	rdfs:label "catholic order"@en, "katholische Orden"@de;
	rdfs:comment """Catholic organization whose member is male and celibatarian, founded by... ."""@en; #*
	rdfs:subClassOf cathorg:Organization.

cathorg:SecularClergy
	a owl:Class;
	#rdfs:isDefinedBy <http://www.knora.org/ontology/shared/catholic-organization#>;
	rdfs:label "secular clergy"@en;
	rdfs:comment """Catholic organization whose member does not take religious vows and does not live in an institution."""@en;
	rdfs:subClassOf cathorg:Organization.

#
# PROPERTIES
#

cathorg:isMemberOf
	a owl:ObjectProperty;
	rdfs:label "is member of catholic organization"@en, "ist Mitglied einer katholischen Organization"@de;
	rdfs:comment """Relating a person to a catholic organization the person is a member of."""@en;
	rdfs:domain cathorg:Person;
	rdfs:range cathorg:Organization;
	rdfs:subPropertyOf org:isMemberOfReligiousOrganization;
	knora-base:subjectClassConstraint cathorg:Person;
	knora-base:objectClassConstraint cathorg:Organization.

cathorg:isMemberOfValue
	a owl:ObjectProperty;
	rdfs:label "is member of catholic order - statement"@en, "ist Mitglied einem katholischen Orden - Festlegung"@de;
	rdfs:comment """Relating a person to a reification statement of the relation between the person and a catholic order the person is a member of."""@en;
	rdfs:subPropertyOf org:isMemberOfReligiousOrganizationValue;
	knora-base:subjectClassConstraint cathorg:Person;
	knora-base:objectClassConstraint knora-base:LinkValue.