@prefix rdf: <http://www.w3.org/1999/02/22-rdf-syntax-ns#>.
@prefix rdfs: <http://www.w3.org/2000/01/rdf-schema#>.
@prefix owl: <http://www.w3.org/2002/07/owl#>.
@prefix xsd: <http://www.w3.org/2001/XMLSchema#>.
@prefix skos: <http://www.w3.org/2004/02/skos/core#>.
@prefix dct: <http://purl.org/dc/terms/>.
@prefix foaf: <http://xmlns.com/foaf/0.1/>.
@prefix cidoc: <http://www.cidoc-crm.org/cidoc-crm/>.
@prefix frbroo: <http://iflastandards.info/ns/fr/frbr/frbroo/>.
@prefix event: <http://www.knora.org/ontology/0047/event#>.
@prefix human: <http://www.knora.org/ontology/0048/human#>.
@prefix document: <http://www.knora.org/ontology/005C/document#>.
@prefix text: <http://www.knora.org/ontology/0059/text#>.
@prefix infocar: <http://www.knora.org/ontology/004C/information-carrier#>.
@prefix publish: <http://www.knora.org/ontology/0056/publishing#>.
@prefix knora-base: <http://www.knora.org/ontology/knora-base#>.

@base <http://www.knora.org/ontology/0000/concept>.
@prefix concept: <http://www.knora.org/ontology/0000/concept#>.

<http://www.knora.org/ontology/0000/concept>
	a owl:Ontology;
	dct:title "An ontology about concept"@en;
	dct:description """Formal description of concept, its general subclasses, related classes and properties."""@en;
	dct:creator "Hans Cools, MD, knowledge engineer, ontologist, software developer, NIE-INE, Basel University, Switzerland"@en;
	dct:publisher "Basel University, Switzerland"@en;

	knora-base:attachedToProject <http://rdfh.ch/projects/0044>.

#
# CLASSES
#

concept:Concept #°
	a owl:Class;
	rdfs:label "concept"@en, "Konzept"@de;
	rdfs:comment """Abstract idea created by a person, as product of mental activity."""@en;
	rdfs:subClassOf human:Creation, frbroo:F6_Concept. # rdfs:subClassOf cidoc:E28_Conceptual_Object

concept:Fiction
	a owl:Class;
	rdfs:label "fiction"@en, "Fiktion"@de;
	rdfs:comment """Concept derived from imagination."""@en;
	rdfs:subClassOf concept:Concept.

concept:Nonfiction
	a owl:Class;
	rdfs:label "nonfiction"@en, "sachliches Konzept"@de;
	rdfs:comment """Concept based on fact."""@en;
	rdfs:subClassOf concept:Concept.

concept:Commonplace
	a owl:Class;
	rdfs:label "commonplace"@en, "Gemeinplatz"@de, "lieu commun"@fr;
	rdfs:comment """Concept generally known, not needing any further explanation, e.g. "Romeo and Julia"."""@en;
	rdfs:subClassOf concept:Concept.

concept:Motto
	a owl:Class;
	rdfs:label "motto"@en, "Motto"@de, "devise"@fr, "motto"@it;
	rdfs:comment """Concept chosen as encapsulating an ideal, principle, belief or goal of an individual or group."""@en;
	rdfs:subClassOf concept:Concept.

concept:SymbolicConcept
	a owl:Class;
	rdfs:label "symbolic concept"@en, "symbolisches Konzept"@de;
	rdfs:comment """Concept represented by one or more symbols."""@en;
	rdfs:subClassOf concept:Concept, cidoc:E90_Symbolic_Object, [
		a owl:Restriction; owl:onProperty concept:isPartOf; owl:minCardinality "0"^^xsd:nonNegativeInteger], [
		a owl:Restriction; owl:onProperty concept:isPartOfValue; owl:minCardinality "0"^^xsd:nonNegativeInteger].

concept:Identifier
	a owl:Class;
	rdfs:label "identifier"@en, "Identifikator"@de;
	rdfs:comment """Unique and permanent reference to a resource within a given context, and conforming to a formal identification system."""@en;
	rdfs:subClassOf concept:SymbolicConcept, cidoc:E42_Identifier, [ # rdfs:subClassOf cidoc:E41_Appellation
		a owl:Restriction; owl:onProperty concept:hasLiteral; owl:minCardinality "0"^^xsd:nonNegativeInteger].

concept:Set #°
	a owl:Class;
	rdfs:label "concept set"@en, "Konzeptsammlung"@de;
	rdfs:comment """Set of concepts."""@en;
	rdfs:subClassOf concept:SymbolicConcept.

concept:PropositionalConcept #°
	a owl:Class;
	rdfs:label "propositional concept"@en, "propositionales Konzept"@de;
	rdfs:comment """Concept represented by a statement bearing a truth value, e.g. a judgement or opinion."""@en;
	skos:note """Different from a linguistic proposition."""@en;
	rdfs:subClassOf concept:Concept, cidoc:E89_Propositional_Object.

concept:ThoughtBody
	a owl:Class;
	rdfs:label "body of thought"@en, "Gedankengut"@de;
	rdfs:comment """Group of coexisting propositional concepts."""@en;
	skos:note """Without the necessity of being logically coherent."""@en;
	skos:note """Related to belief system related to school of thought related to theory."""@en;
	rdfs:subClassOf concept:PropositionalConcept.

concept:Work
	a owl:Class;
	rdfs:label "conceptual work"@en, "konzeptuelles Werk"@de;
	rdfs:comment """Intellectual product as concept."""@en;
	rdfs:subClassOf concept:PropositionalConcept, frbroo:F1_Work, [
		a owl:Restriction; owl:onProperty text:hasTitle; owl:minCardinality "0"^^xsd:nonNegativeInteger].

concept:IndividualWork
	a owl:Class;
	rdfs:label "individual work"@en, "individuelles Werk"@de;
	rdfs:comment """Work as a complete whole realised in one self-contained expression."""@en;
	rdfs:subClassOf concept:Work, frbroo:F14_Individual_Work, [
		a owl:Restriction; owl:onProperty concept:isExpressedIn; owl:minCardinality "0"^^xsd:nonNegativeInteger], [
		a owl:Restriction; owl:onProperty concept:isExpressedInValue; owl:minCardinality "0"^^xsd:nonNegativeInteger].

concept:Information
	a owl:Class;
	rdfs:label "information"@en, "Information"@de;
	rdfs:comment """Symbolic propositional concept resolving uncertainty."""@en;
	rdfs:subClassOf concept:PropositionalConcept, concept:SymbolicConcept, cidoc:E73_Information_Object, [
		a owl:Restriction; owl:onProperty concept:informationHasSubject; owl:minCardinality "0"^^xsd:nonNegativeInteger], [
		a owl:Restriction; owl:onProperty concept:informationHasSubjectValue; owl:minCardinality "0"^^xsd:nonNegativeInteger], [
		a owl:Restriction; owl:onProperty infocar:isOnCarrier; owl:minCardinality "0"^^xsd:nonNegativeInteger], [
		a owl:Restriction; owl:onProperty infocar:isOnCarrierValue; owl:minCardinality "0"^^xsd:nonNegativeInteger], [
		a owl:Restriction; owl:onProperty infocar:isOnElectronicCarrier; owl:minCardinality "0"^^xsd:nonNegativeInteger], [
		a owl:Restriction; owl:onProperty infocar:isOnElectronicCarrierValue; owl:minCardinality "0"^^xsd:nonNegativeInteger], [
		a owl:Restriction; owl:onProperty concept:hasEncoder; owl:minCardinality "0"^^xsd:nonNegativeInteger], [
		a owl:Restriction; owl:onProperty concept:hasEncoderValue; owl:minCardinality "0"^^xsd:nonNegativeInteger].

concept:Procedure
	a owl:Class;
	rdfs:label "procedure"@en, "Vorgehen"@de;
	rdfs:comment """Plan to perform an action in one or more steps, in a certain manner to obtain a certain output under certain circumstances."""@en;
	rdfs:subClassOf concept:Information, cidoc:E29_Design_or_Procedure.

concept:ThoughtMethod #° part/SCO philosophy ?
	a owl:Class;
	rdfs:label "thought method"@en, "Methode des Denkens"@de;
	rdfs:comment """Way of analysing facts to form a judgment."""@en;
	rdfs:subClassOf concept:Information.

#
# PROPERTIES
#

concept:isPartOf
	a owl:ObjectProperty; #, owl:TransitiveProperty;
	rdfs:label "is part of"@en, "ist Teil von"@de;
	rdfs:comment "Relating a symbolic concept to another one it is part of."@en;
	rdfs:domain concept:SymbolicConcept;
	rdfs:range concept:SymbolicConcept;
	rdfs:subPropertyOf cidoc:P106i_forms_part_of, knora-base:hasLinkTo;
	knora-base:subjectClassConstraint concept:SymbolicConcept;
	knora-base:objectClassConstraint concept:SymbolicConcept.

concept:isPartOfValue
	a owl:ObjectProperty;
	rdfs:label "is part of - statement"@en, "ist Teil von - Festlegung"@de;
	rdfs:comment "Relating something to a reification statement of the relation between that something and something else it is part of."@en;
	rdfs:subPropertyOf knora-base:hasLinkToValue;
	knora-base:subjectClassConstraint concept:SymbolicConcept;
	knora-base:objectClassConstraint knora-base:LinkValue.

concept:isExpressedIn
	a owl:ObjectProperty;
	rdfs:label "is expressed in"@en, "ist ausgedruckt in"@de;
	rdfs:comment "Relating an individual work to an individual expression thereof."@en;
	rdfs:domain concept:IndividualWork;
	rdfs:range document:IndividualExpression;
	rdfs:subPropertyOf frbroo:R9_is_realised_in, knora-base:hasLinkTo;
	knora-base:subjectClassConstraint concept:IndividualWork;
	knora-base:objectClassConstraint document:IndividualExpression.

concept:isExpressedInValue
	a owl:ObjectProperty;
	rdfs:label "is expressed in - statement"@en, "ist ausgedruckt in - Festlegung"@de;
	rdfs:comment "Relating an individual work to a reification statement of the relation between the work and an individual expression thereof."@en;
	rdfs:subPropertyOf knora-base:hasLinkToValue;
	knora-base:subjectClassConstraint concept:IndividualWork;
	knora-base:objectClassConstraint knora-base:LinkValue.

concept:informationHasSubject
	a owl:ObjectProperty;
	rdfs:label "information has subject"@en, "Information hat Thema"@de;
	rdfs:comment """Relating information to a subject it is about."""@en;
	rdfs:domain concept:Information;
	rdfs:range rdfs:Resource;
	rdfs:subPropertyOf knora-base:hasLinkTo;
	knora-base:subjectClassConstraint concept:Information;
	knora-base:objectClassConstraint knora-base:Resource.

concept:informationHasSubjectValue
	a owl:ObjectProperty;
	rdfs:label "information has subject - statement"@en, "Information hat Thema - Festlegung"@de;
	rdfs:comment """Relating information to a reification statement of the relation between the information and a subject it is about."""@en;
	rdfs:subPropertyOf knora-base:hasLinkToValue;
	knora-base:subjectClassConstraint concept:Information;
	knora-base:objectClassConstraint knora-base:LinkValue.

# frbroo:R3_is_realised_in: more general: frbroo:F1_Work - frbroo:F22_Self-Contained_Expression

concept:hasDedicatedTo #°
	a owl:ObjectProperty;
	rdfs:label "has dedicated to"@en, "hat gewidmet"@de;
	rdfs:comment """Relating a person to another person to whom the former has dedicated something."""@en;
	rdfs:domain human:Person;
	rdfs:range human:Person;
	rdfs:subPropertyOf knora-base:hasLinkTo;
	knora-base:subjectClassConstraint human:Person;
	knora-base:objectClassConstraint human:Person.

concept:hasDedicatedToValue
	a owl:ObjectProperty;
	rdfs:label "has dedicated to - statement"@en, "hat gewidmet - Festlegung"@de;
	rdfs:comment """Relating a person to a reification statement of the relation between the person and another person to whom the former has dedicated something."""@en;
	rdfs:subPropertyOf knora-base:hasLinkToValue;
	knora-base:subjectClassConstraint human:Person;
	knora-base:objectClassConstraint knora-base:LinkValue.

concept:hasLiteral
	a owl:ObjectProperty;
	rdfs:label "has literal"@en, "hat Literale"@de;
	rdfs:comment """Relating a symbolic concept to a literal that expresses it."""@en;
	rdfs:domain concept:SymbolicConcept;
#	rdfs:range ling:Literal;
	rdfs:subPropertyOf knora-base:hasValue;
	knora-base:subjectClassConstraint concept:SymbolicConcept;
	knora-base:objectClassConstraint knora-base:TextValue.

concept:hasEncoder
	a owl:ObjectProperty;
	rdfs:label "information has encoder"@en, "Information hat Encoder"@de;
	rdfs:comment "Relating information to a person who encoded it."@en;
	rdfs:domain concept:Information;
#	rdfs:range [rdfs:subClassOf human:Person, [a owl:Restriction; owl:onProperty human:personHasRole; owl:someValuesFrom infocar:Encoder]];
	rdfs:subPropertyOf knora-base:hasLinkTo;
	knora-base:subjectClassConstraint concept:Information;
	knora-base:objectClassConstraint human:Person.

concept:hasEncoderValue
	a owl:ObjectProperty;
	rdfs:label "information has encoder - statement"@en, "Information hat Encoder - Festlegung"@de;
	rdfs:comment "Relating information to a reification statement of the relation between the information and a person who encoded it."@en;
	rdfs:subPropertyOf knora-base:hasLinkToValue;
	knora-base:subjectClassConstraint concept:Information;
	knora-base:objectClassConstraint knora-base:LinkValue.
