@prefix rdfs: <http://www.w3.org/2000/01/rdf-schema#>.
@prefix owl: <http://www.w3.org/2002/07/owl#>.
@prefix xsd: <http://www.w3.org/2001/XMLSchema#>.
@prefix skos: <http://www.w3.org/2004/02/skos/core#>.
@prefix dct: <http://purl.org/dc/terms/>.
@prefix human: <http://www.knora.org/ontology/shared/human#>.
@prefix language: <http://www.knora.org/ontology/shared/language#>.
@prefix teach: <http://www.knora.org/ontology/shared/teaching#>.
@prefix document: <http://www.knora.org/ontology/shared/document#>.
@prefix text: <http://www.knora.org/ontology/shared/text#>.
@prefix text-expression: <http://www.knora.org/ontology/shared/text-expression#>.
@prefix text-structure: <http://www.knora.org/ontology/shared/text-structure#>.
@prefix prosodic-structure: <http://www.knora.org/ontology/shared/prosodic-structure#>.
@prefix textedit: <http://www.knora.org/ontology/shared/text-editing#>.
@prefix scientific-editing: <http://www.knora.org/ontology/shared/scientific-editing#>.
@prefix publish: <http://www.knora.org/ontology/shared/publishing#>.
@prefix litera: <http://www.knora.org/ontology/shared/literature#>.
@prefix knora-base: <http://www.knora.org/ontology/knora-base#>.
@prefix salsah-gui: <http://www.knora.org/ontology/salsah-gui#>.

@base <http://www.knora.org/ontology/0060/delille>.
@prefix delille: <http://www.knora.org/ontology/0060/delille#>.

<http://www.knora.org/ontology/0060/delille>
	a owl:Ontology;
	dct:title "An ontology about Jacques Delille's poetry"@en; #*
	dct:description """Formal description of specific concepts in the scientific study of poetry of Jacques Delille, 22 June 1738 – 1 May 1813."""@en;
	dct:creator "Hans Cools, MD, knowledge engineer, ontologist, software developer, NIE-INE, Basel University, Switzerland"@en;
	dct:contributor "Roberta Padlina, tool coordinator and software developer, NIE-INE, University of Basel, Switzerland"@en;
	dct:publisher "University of Basel, Switzerland"@en;

	knora-base:attachedToProject <http://rdfh.ch/projects/0060>.

#
# CLASSES
#

delille:VersePoem
	a owl:Class;
	rdfs:label "Jacques Delille verse poem"@en, "Versgedicht Jacques Delilles"@de;
	rdfs:comment """Verse poem authored by Jacques Delille."""@en;
	rdfs:subClassOf litera:VersePoem, publish:Expression.

delille:TranslatedVersePoem
	a owl:Class;
	rdfs:label "Translated Jacques Delille verse poem"@en, "übersetzter gereimter Versgedicht Jacques Delilles"@de;
	rdfs:comment """Translated Jacques Delille verse poem."""@en;
	rdfs:subClassOf delille:VersePoem, language:PersonTranslation, text:Translation.

delille:EditedVersePoem
	a owl:Class;
	rdfs:label "edited Jacques Delille verse poem"@en, "ediertes Versgedicht Jacques Delilles"@de;
	rdfs:comment """Verse poem authored by Jacques Delille and edited."""@en;
	rdfs:subClassOf delille:VersePoem, textedit:Edition.

delille:Canto
	a owl:Class;
	rdfs:label "Jacques Delille canto"@en, "Canto Jacques Delilles"@de, "chant de Jacques Delille"@fr, "canto di Jacques Delille"@it;
	rdfs:comment """Group of strophes in a verse poem authored by Jacques Delille."""@en;
	rdfs:subClassOf prosodic-structure:VerseSection, text-expression:ExpressionPart.

# delille:RhymingVerse
#	a owl:Class;
#	rdfs:label "Jacques Delille rhyming verse"@en, "gereimter Vers Jacques Delilles"@de;
#	rdfs:comment """Rhyming verse in a verse poem authored by Jacques Delille."""@en;
#	rdfs:subClassOf text-structure:RhymingVerse.

# delille:Citation
#	a owl:Class;
#	rdfs:label "Citation of a Jacques Delille poem verse"@en, "Zitat eines Jacques Delilles Gedichtverses"@de; #, "de Jacques Delille"@fr, "di Jacques Delille"@it;
#	rdfs:comment """Citation of a Jacques Delille poem verse."""@en;
#	rdfs:subClassOf text:Citation.

# delille:CitationReference
#	a owl:Class;
#	rdfs:label "citation reference verse number"@en, "Zitatreferenz-Versnummer"@de;
#	rdfs:comment """Citation reference of a Jacques Delille poem verse as the latter's number."""@en;
#	rdfs:subClassOf text:CitationReference.

# delille:CitingExpression
#	a owl:Class;
#	rdfs:label "citing expression"@en, "zitierende Expression"@de; #, ""@fr, ""@it;
#	rdfs:comment """Publication text expression citing one or more verses of a poem authored by Jacques Delille."""@en;
#	rdfs:subClassOf publish:TextExpression.

delille:Dictionary
	a owl:Class;
	rdfs:label "citing dictionary"@en, "zitierendes Wörterbuch"@de; #, ""@fr, ""@it;
	rdfs:comment """Dictionary citing one or more verses of a poem authored by Jacques Delille."""@en;
	rdfs:subClassOf text-expression:Dictionary, publish:TextExpression.

delille:Manual
	a owl:Class;
	rdfs:label "citing teaching manual"@en, "zitierendes Lehrbuch"@de; #, ""@fr, ""@it;
	rdfs:comment """Teaching manual citing one or more verses of a poem authored by Jacques Delille."""@en;
	rdfs:subClassOf teach:Manual, publish:TextExpression.

delille:LiteraryExpression
	a owl:Class;
	rdfs:label "citing publication literary expression"@en, "zitierende literarische Publikation-Expression"@de; #, ""@fr, ""@it;
	rdfs:comment """Literary publication expression citing one or more verses of a poem authored by Jacques Delille."""@en;
	rdfs:subClassOf litera:Expression, publish:TextExpression.

delille:CitingPoem
	a owl:Class;
	rdfs:label "citing poem"@en, "zitierendes Gedicht"@de; #, ""@fr, ""@it;
	rdfs:comment """Poem citing one or more verses of a poem authored by Jacques Delille."""@en;
	rdfs:subClassOf litera:Poem, delille:LiteraryExpression.

delille:Novel
	a owl:Class;
	rdfs:label "citing novel"@en, "zitierender Roman"@de; #, ""@fr, ""@it;
	rdfs:comment """Novel citing one or more verses of a poem authored by Jacques Delille."""@en;
	rdfs:subClassOf litera:Novel, delille:LiteraryExpression.

delille:Nonfiction
	a owl:Class;
	rdfs:label "citing literary nonfiction"@en, "zitierende sachliche Literatur"@de; #, ""@fr, ""@it;
	rdfs:comment """Literary nonfiction citing one or more verses of a poem authored by Jacques Delille."""@en;
	rdfs:subClassOf litera:Nonfiction, delille:LiteraryExpression.

delille:ScientificExpression
	a owl:Class;
	rdfs:label "citing scientific publication expression"@en, "zitierende wissenschaftliche Publikation-Expression"@de;
	rdfs:comment """Scientific publication expression citing one or more verses of a poem authored by Jacques Delille."""@en;
	rdfs:subClassOf text-expression:ScientificExpression, publish:TextExpression.

delille:VulgarizedScientificExpression
	a owl:Class;
	rdfs:label "citing vulgarized scientific publication expression"@en, "zitierende vulgarisierte wissenschaftliche Publikation-Expression"@de;
	rdfs:comment """Vulgarized scientific publication expression citing one or more verses of a poem authored by Jacques Delille."""@en;
	rdfs:subClassOf text-expression:VulgarizedScientificExpression, publish:TextExpression.

delille:Catalogue
	a owl:Class;
	rdfs:label "citing catalogue"@en, "zitierende Katalog"@de;
	rdfs:comment """Catalogue citing one or more verses of a poem authored by Jacques Delille."""@en;
	rdfs:subClassOf document:Catalogue, publish:TextExpression.

delille:Commentary
	a owl:Class;
	rdfs:label "commentary"@en, "Kommentar"@de;
	rdfs:comment """Commentary on a citation of a verse of a poem authored by Jacques Delille."""@en;
	rdfs:subClassOf text-expression:Commentary, text-expression:ScientificExpression, publish:TextExpression.

delille:Argument
	a owl:Class;
	rdfs:label "argument"@en, "Argument"@de;
	rdfs:comment """Argument of a commentary on a citation of a verse of a poem authored by Jacques Delille."""@en;
	rdfs:subClassOf litera:Argument, publish:TextExpression.

# image

#
# PROPERTIES
#
