@prefix rdf: <http://www.w3.org/1999/02/22-rdf-syntax-ns#>.
@prefix rdfs: <http://www.w3.org/2000/01/rdf-schema#>.
@prefix owl: <http://www.w3.org/2002/07/owl#>.
@prefix xsd: <http://www.w3.org/2001/XMLSchema#>.
@prefix skos: <http://www.w3.org/2004/02/skos/core#>.
@prefix dct: <http://purl.org/dc/terms/>.
@prefix foaf: <http://xmlns.com/foaf/0.1/>.
@prefix cidoc: <http://www.cidoc-crm.org/cidoc-crm/>.
@prefix frbroo: <http://iflastandards.info/ns/fr/frbr/frbroo/>.
@prefix event: <http://www.knora.org/ontology/shared/event#>.
@prefix human: <http://www.knora.org/ontology/shared/human#>.
@prefix concept: <http://www.knora.org/ontology/shared/concept#>.
@prefix math: <http://www.knora.org/ontology/shared/mathematics#>.
@prefix ling: <http://www.knora.org/ontology/shared/linguistics#>.
@prefix text: <http://www.knora.org/ontology/shared/text#>.
@prefix text-structure: <http://www.knora.org/ontology/shared/text-structure#>.
@prefix note-structure: <http://www.knora.org/ontology/shared/note-structure#>.
@prefix infocar: <http://www.knora.org/ontology/shared/information-carrier#>.
@prefix publish: <http://www.knora.org/ontology/shared/publishing#>.
@prefix knora-base: <http://www.knora.org/ontology/knora-base#>.

@base <http://www.knora.org/ontology/shared/document>.
@prefix document: <http://www.knora.org/ontology/shared/document#>.

<http://www.knora.org/ontology/shared/document>
	a owl:Ontology;
	dct:license <http://creativecommons.org/licenses/by/3.0/>;
	dct:title "An ontology about document"@en;
	dct:description """Formal description of document, general subclasses, related classes and properties."""@en;
	dct:creator "Hans Cools, MD, knowledge engineer, ontologist, software developer, NIE-INE, Basel University, Switzerland"@en;
	dct:contributor "Roberta Padlina, tool coordinator and software developer, NIE-INE, University of Basel, Switzerland"@en;
	dct:publisher "Basel University, Switzerland"@en;
	knora-base:attachedToProject <http://www.knora.org/ontology/knora-base#DefaultSharedOntologiesProject>.

#
# CLASSES
#

document:Document
	a owl:Class;
	rdfs:label "document"@en, "Dokument"@de;
	rdfs:comment """Identifiable, immaterial, contained information, e.g. a text, a graphic, an image, an audiogram, a videogram, abstracted from its information carrier."""@en;
	rdfs:subClassOf concept:Information, [ # , cidoc:E31_Document: proposition about reality: narrower
#		a owl:Restriction; owl:onProperty document:hasContent; owl:minCardinality "0"^^xsd:nonNegativeInteger], [
#		a owl:Restriction; owl:onProperty document:hasContentValue; owl:minCardinality "0"^^xsd:nonNegativeInteger], [
		a owl:Restriction; owl:onProperty document:hasEncoder; owl:minCardinality "0"^^xsd:nonNegativeInteger], [
		a owl:Restriction; owl:onProperty document:hasEncoderValue; owl:minCardinality "0"^^xsd:nonNegativeInteger].

document:Element
	a owl:Class;
	rdfs:label "document element"@en, "Dokumentelement"@de;
	rdfs:comment """Information as part of a document."""@en;
	rdfs:subClassOf concept:Information, [
		a owl:Restriction; owl:onProperty document:isElementOfDocument; owl:minCardinality "0"^^xsd:nonNegativeInteger], [
		a owl:Restriction; owl:onProperty document:isElementOfDocumentValue; owl:minCardinality "0"^^xsd:nonNegativeInteger].

document:Structure
	a owl:Class;
	rdfs:label "document structure"@en, "Dokumentstruktur"@de;
	rdfs:comment """Structural element of a document."""@en;
	rdfs:subClassOf document:Element, [
		a owl:Restriction; owl:onProperty document:isStructureOfDocument; owl:minCardinality "0"^^xsd:nonNegativeInteger], [
		a owl:Restriction; owl:onProperty document:isStructureOfDocumentValue; owl:minCardinality "0"^^xsd:nonNegativeInteger].

document:Layout
	a owl:Class;
	rdfs:label "layout"@en, "Aufmachung"@de;
	rdfs:comment """Way in which the content of a page is set out."""@en;
	rdfs:subClassOf document:Element.

document:Space
	a owl:Class;
	rdfs:label "document space"@en, "Leerraum eines Dokumentes"@de;
	rdfs:comment """Empty space between document content structures, e.g. lines, columns, paragraphs, sections, strophes, images."""@en;
	rdfs:subClassOf document:Structure, [
#		a owl:Restriction; owl:onProperty document:isSpaceOfDocument; owl:allValuesFrom document:Document], [
		a owl:Restriction; owl:onProperty document:isSpaceOfDocument; owl:minCardinality "0"^^xsd:nonNegativeInteger], [
		a owl:Restriction; owl:onProperty document:isSpaceOfDocumentValue; owl:minCardinality "0"^^xsd:nonNegativeInteger].

document:VerticalSpace
	a owl:Class;
	rdfs:label "vertical document space"@en, "vertikaler Leerraum eines Dokumentes"@de;
	rdfs:comment """Document space with vertical orientation, e.g. between columns."""@en;
	rdfs:subClassOf document:Space.

document:HorizontalSpace
	a owl:Class;
	rdfs:label "horizontal document space"@en, "horizontaler Leerraum eines Dokumentes"@de;
	rdfs:comment """Document space with horizontal orientation, e.g. between lines."""@en;
	rdfs:subClassOf document:Space.

#Â° document:Reference

document:ContentStructure
	a owl:Class;
	rdfs:label "document content structure"@en, "Dokumentinhaltstruktur"@de;
	rdfs:comment """Content structure of a document."""@en;
	rdfs:subClassOf document:Structure, [
		a owl:Restriction; owl:onProperty document:contentStructureHasIdentifier; owl:minCardinality "0"^^xsd:nonNegativeInteger], [
		a owl:Restriction; owl:onProperty document:contentStructureHasIdentifierValue; owl:minCardinality "0"^^xsd:nonNegativeInteger], [
 		a owl:Restriction; owl:onProperty document:hasReference; owl:minCardinality "0"^^xsd:nonNegativeInteger], [
 		a owl:Restriction; owl:onProperty document:hasReferenceValue; owl:minCardinality "0"^^xsd:nonNegativeInteger], [
 		a owl:Restriction; owl:onProperty document:hasTextReference; owl:minCardinality "0"^^xsd:nonNegativeInteger], [
 		a owl:Restriction; owl:onProperty document:hasTextReferenceValue; owl:minCardinality "0"^^xsd:nonNegativeInteger], [
		a owl:Restriction; owl:onProperty document:hasFootnoteReference; owl:minCardinality "0"^^xsd:nonNegativeInteger], [
		a owl:Restriction; owl:onProperty document:hasFootnoteReferenceValue; owl:minCardinality "0"^^xsd:nonNegativeInteger], [
		a owl:Restriction; owl:onProperty document:hasEndnoteReference; owl:minCardinality "0"^^xsd:nonNegativeInteger], [
		a owl:Restriction; owl:onProperty document:hasEndnoteReferenceValue; owl:minCardinality "0"^^xsd:nonNegativeInteger], [
		a owl:Restriction; owl:onProperty document:hasExpressionReference; owl:minCardinality "0"^^xsd:nonNegativeInteger], [
		a owl:Restriction; owl:onProperty document:hasExpressionReferenceValue; owl:minCardinality "0"^^xsd:nonNegativeInteger].

document:ContentStructureIdentifier
	a owl:Class;
	rdfs:label "document content structure identifier"@en, "Dokumentinhaltstrukturidentifikator"@de;
	rdfs:comment """Identifier of a document content structure."""@en;
	rdfs:subClassOf document:Structure, concept:Identifier.

document:ContentStructureReference
	a owl:Class;
	rdfs:label "document content structure reference"@en, "Dokumentinhaltstrukturreferenz"@de;
	rdfs:comment """Reference as a document structure, referring from one document content structure to another via the identifier, e.g. a footnote reference from a text or image to the footnote identifier. The reference is linked to and has the same literal representation as the identifier of the content structure it refers to."""@en;
	rdfs:subClassOf document:Structure, concept:Identifier, [
		a owl:Restriction; owl:onProperty document:hasContentStructureIdentifier; owl:minCardinality "0"^^xsd:nonNegativeInteger], [
		a owl:Restriction; owl:onProperty document:hasContentStructureIdentifierValue; owl:minCardinality "0"^^xsd:nonNegativeInteger].

document:TextStructureReference
	a owl:Class;
	rdfs:label "text reference"@en, "Textreferenz"@de;
	rdfs:comment """Reference to text, e.g. a footnote reference."""@en;
	rdfs:subClassOf document:ContentStructureReference, [
		a owl:Restriction; owl:onProperty document:hasTextStructureIdentifier; owl:minCardinality "0"^^xsd:nonNegativeInteger], [
		a owl:Restriction; owl:onProperty document:hasTextStructureIdentifierValue; owl:minCardinality "0"^^xsd:nonNegativeInteger].

document:FootnoteReference
	a owl:Class;
	rdfs:label "footnote reference"@en, "Fussnotereferenz"@de;
	rdfs:comment """Reference to a footnote via the footnote identifier."""@en;
	rdfs:subClassOf document:TextStructureReference, [
		a owl:Restriction; owl:onProperty document:hasFootnoteIdentifier; owl:minCardinality "0"^^xsd:nonNegativeInteger], [
		a owl:Restriction; owl:onProperty document:hasFootnoteIdentifierValue; owl:minCardinality "0"^^xsd:nonNegativeInteger], [
		a owl:Restriction; owl:onProperty document:hasFootnoteNumber; owl:minCardinality "0"^^xsd:nonNegativeInteger], [
		a owl:Restriction; owl:onProperty document:hasFootnoteNumberValue; owl:minCardinality "0"^^xsd:nonNegativeInteger].

document:EndnoteReference
	a owl:Class;
	rdfs:label "endnote reference"@en, "Endnotereferenz"@de;
	rdfs:comment """Reference to an endnote."""@en;
	rdfs:subClassOf document:TextStructureReference, [
		a owl:Restriction; owl:onProperty document:hasEndnoteIdentifier; owl:minCardinality "0"^^xsd:nonNegativeInteger], [
		a owl:Restriction; owl:onProperty document:hasEndnoteIdentifierValue; owl:minCardinality "0"^^xsd:nonNegativeInteger], [
		a owl:Restriction; owl:onProperty document:hasEndnoteNumber; owl:minCardinality "0"^^xsd:nonNegativeInteger], [
		a owl:Restriction; owl:onProperty document:hasEndnoteNumberValue; owl:minCardinality "0"^^xsd:nonNegativeInteger].

document:ExpressionReference
	a owl:Class;
	rdfs:label "document expression reference"@en, "Dokument-Expression-Referenz"@de;
	rdfs:comment """Document structure referring from a document content structure to a document expression identifier, e.g. a siglum."""@en;
	rdfs:subClassOf document:Structure, concept:Identifier, [
		a owl:Restriction; owl:onProperty document:expressionReferenceHasIdentifier; owl:minCardinality "0"^^xsd:nonNegativeInteger], [
		a owl:Restriction; owl:onProperty document:expressionReferenceHasIdentifierValue; owl:minCardinality "0"^^xsd:nonNegativeInteger].

document:Column
	a owl:Class;
	rdfs:label "column"@en, "Spalte"@de;
	rdfs:comment """Content structure displaying information, e.g. text lines and graphs, as a column as part of a page."""@en;
	rdfs:subClassOf document:ContentStructure, [
#		a owl:Restriction; owl:onProperty document:isColumnOfPage; owl:allValuesFrom document:Page], [
		a owl:Restriction; owl:onProperty document:isColumnOfPage; owl:minCardinality "0"^^xsd:nonNegativeInteger], [
		a owl:Restriction; owl:onProperty document:isColumnOfPageValue; owl:minCardinality "0"^^xsd:nonNegativeInteger].

document:Page
	a owl:Class;
	rdfs:label "document page"@en, "Dokumentseite"@de;
	rdfs:comment """Content structure with information, e.g. text lines and graphs, as a page as part of a document expression, on an information carrier page."""@en;
	rdfs:subClassOf document:ContentStructure, [
#		a owl:Restriction; owl:onProperty document:isPageOfExpression; owl:allValuesFrom document:Document], [
		a owl:Restriction; owl:onProperty document:isPageOfExpression; owl:minCardinality "0"^^xsd:nonNegativeInteger], [
		a owl:Restriction; owl:onProperty document:isPageOfExpressionValue; owl:minCardinality "0"^^xsd:nonNegativeInteger], [
		a owl:Restriction; owl:onProperty document:pageHasIdentifier; owl:minCardinality "0"^^xsd:nonNegativeInteger], [
		a owl:Restriction; owl:onProperty document:pageHasIdentifierValue; owl:minCardinality "0"^^xsd:nonNegativeInteger], [		
		a owl:Restriction; owl:onProperty document:pageHasNumber; owl:minCardinality "0"^^xsd:nonNegativeInteger], [
		a owl:Restriction; owl:onProperty document:pageHasNumberValue; owl:minCardinality "0"^^xsd:nonNegativeInteger], [
		a owl:Restriction; owl:onProperty infocar:isPageOnCarrier; owl:minCardinality "0"^^xsd:nonNegativeInteger], [
		a owl:Restriction; owl:onProperty infocar:isPageOnCarrierValue; owl:minCardinality "0"^^xsd:nonNegativeInteger].

document:PageIdentifier
	a owl:Class;
	rdfs:label "document page identifier"@en, "Dokumentseiteidentifikator"@de;
	rdfs:comment """Identifier of a document page."""@en;
	rdfs:subClassOf document:ContentStructureIdentifier.

document:PageNumber
	a owl:Class;
	rdfs:label "document page number"@en, "Dokumentseitenummer"@de;
	rdfs:comment """Number of a document page."""@en;
	rdfs:subClassOf document:PageIdentifier, math:NaturalNumber.

document:TitlePage
	a owl:Class;
	rdfs:label "title page"@en, "Titelblatt"@de;
	rdfs:comment """Document page contianing a title."""@en;
	rdfs:subClassOf document:Page.

document:Marginal
	a owl:Class;
	rdfs:label "marginal"@en, "Marginale"@de;
	rdfs:comment """Information besides a text in the margin of a carrier, e.g. text, doodles, illuminations."""@en;
	rdfs:subClassOf document:ContentStructure.

document:Table #* tableHasTitle, tableHasField, tableHasRow, tableHasColumn
	a owl:Class;
	rdfs:label "table"@en, "Tabelle"@de;
	rdfs:comment """Two-dimensional structure composed of one or more fields or cell containing information and being part of a vertical column and a horizontal row, both with own identifier."""@en;
	rdfs:subClassOf document:ContentStructure, [
		a owl:Restriction; owl:onProperty document:isTableOfColumn; owl:minCardinality "0"^^xsd:nonNegativeInteger], [
		a owl:Restriction; owl:onProperty document:isTableOfColumnValue; owl:minCardinality "0"^^xsd:nonNegativeInteger].

document:Expression
	a owl:Class;
	rdfs:label "document expression"@en, "Dokument-Expression"@de;
	rdfs:comment """Document realisation of a work, conform FRBROO, e.g. a text, story, poem, play, musical, song, joke, choreographic notation, movement pattern, sound pattern, image, multimedia object, or any combination of them, having an objectively recognisable structure."""@en;
	rdfs:subClassOf document:Document, frbroo:F2_Expression, [
		a owl:Restriction; owl:onProperty document:expressionHasIdentifier; owl:minCardinality "0"^^xsd:nonNegativeInteger], [
		a owl:Restriction; owl:onProperty document:expressionHasIdentifierValue; owl:minCardinality "0"^^xsd:nonNegativeInteger], [	
		a owl:Restriction; owl:onProperty document:expressionHasTitle; owl:minCardinality "0"^^xsd:nonNegativeInteger], [
		a owl:Restriction; owl:onProperty document:expressionHasSubtitle; owl:minCardinality "0"^^xsd:nonNegativeInteger], [
		a owl:Restriction; owl:onProperty publish:hasPublishingState; owl:minCardinality "0"^^xsd:nonNegativeInteger], [
		a owl:Restriction; owl:onProperty publish:hasPublishingStateValue; owl:minCardinality "0"^^xsd:nonNegativeInteger], [
		a owl:Restriction; owl:onProperty publish:hasPublishing; owl:minCardinality "0"^^xsd:nonNegativeInteger], [
		a owl:Restriction; owl:onProperty publish:hasPublishingValue; owl:minCardinality "0"^^xsd:nonNegativeInteger], [
		a owl:Restriction; owl:onProperty publish:hasPublication; owl:minCardinality "0"^^xsd:nonNegativeInteger], [
		a owl:Restriction; owl:onProperty publish:hasPublicationValue; owl:minCardinality "0"^^xsd:nonNegativeInteger], [
		a owl:Restriction; owl:onProperty publish:hasElectronicPublication; owl:minCardinality "0"^^xsd:nonNegativeInteger], [
		a owl:Restriction; owl:onProperty publish:hasElectronicPublicationValue; owl:minCardinality "0"^^xsd:nonNegativeInteger], [
		a owl:Restriction; owl:onProperty publish:hasWebPublication; owl:minCardinality "0"^^xsd:nonNegativeInteger], [
		a owl:Restriction; owl:onProperty publish:hasWebPublicationValue; owl:minCardinality "0"^^xsd:nonNegativeInteger], [
		a owl:Restriction; owl:onProperty publish:hasFirstPublication; owl:minCardinality "0"^^xsd:nonNegativeInteger], [
		a owl:Restriction; owl:onProperty publish:hasFirstPublicationValue; owl:minCardinality "0"^^xsd:nonNegativeInteger], [		
		a owl:Restriction; owl:onProperty publish:hasLastPublication; owl:minCardinality "0"^^xsd:nonNegativeInteger], [
		a owl:Restriction; owl:onProperty publish:hasLastPublicationValue; owl:minCardinality "0"^^xsd:nonNegativeInteger], [
		a owl:Restriction; owl:onProperty publish:hasLastAuthorizedPublication; owl:minCardinality "0"^^xsd:nonNegativeInteger], [
		a owl:Restriction; owl:onProperty publish:hasLastAuthorizedPublicationValue; owl:minCardinality "0"^^xsd:nonNegativeInteger], [
		a owl:Restriction; owl:onProperty publish:hasUnauthorizedPublication; owl:minCardinality "0"^^xsd:nonNegativeInteger], [
		a owl:Restriction; owl:onProperty publish:hasUnauthorizedPublicationValue; owl:minCardinality "0"^^xsd:nonNegativeInteger], [
		a owl:Restriction; owl:onProperty publish:hasUnauthorizedRepublication; owl:minCardinality "0"^^xsd:nonNegativeInteger], [
		a owl:Restriction; owl:onProperty publish:hasUnauthorizedRepublicationValue; owl:minCardinality "0"^^xsd:nonNegativeInteger], [
		a owl:Restriction; owl:onProperty publish:hasPolyAuthorPublication; owl:minCardinality "0"^^xsd:nonNegativeInteger], [
		a owl:Restriction; owl:onProperty publish:hasPolyAuthorPublicationValue; owl:minCardinality "0"^^xsd:nonNegativeInteger], [
		a owl:Restriction; owl:onProperty publish:hasNachlassPublication; owl:minCardinality "0"^^xsd:nonNegativeInteger], [
		a owl:Restriction; owl:onProperty publish:hasNachlassPublicationValue; owl:minCardinality "0"^^xsd:nonNegativeInteger], [
		a owl:Restriction; owl:onProperty publish:hasNachlassPublicationDescription; owl:minCardinality "0"^^xsd:nonNegativeInteger].

document:IndividualExpression
	a owl:Class;
	rdfs:label "individual document expression"@en, "individuelle Dokument-Expression"@de;
	rdfs:comment """Document realisation of an individual work."""@en;
	rdfs:subClassOf document:Expression, frbroo:F22_Self-Contained_Expression, [
		a owl:Restriction; owl:onProperty document:isExpressionOfCycle; owl:minCardinality "0"^^xsd:nonNegativeInteger], [
		a owl:Restriction; owl:onProperty document:isExpressionOfCycleValue; owl:minCardinality "0"^^xsd:nonNegativeInteger].

document:ExpressionPart
	a owl:Class;
	rdfs:label "document expression part"@en, "Dokument-Expressionsteil"@de;
	rdfs:comment """Part of an individual document expression, considered as incomplete."""@en;
	rdfs:subClassOf document:Expression, frbroo:F23_Expression_Fragment, [
		a owl:Restriction; owl:onProperty document:isPartOfIndividualExpression; owl:minCardinality "0"^^xsd:nonNegativeInteger], [
		a owl:Restriction; owl:onProperty document:isPartOfIndividualExpressionValue; owl:minCardinality "0"^^xsd:nonNegativeInteger].

document:Draft
	a owl:Class;
	rdfs:label "document draft"@en, "Dokumententwurf"@de;
	rdfs:comment """Developmental document expression, subject to future modification."""@en;
	rdfs:subClassOf document:Expression, human:UnfinishedCreation. # Creation in a state of not having all envisioned features

document:PolyAuthorExpression
	a owl:Class;
	rdfs:label "poly-author document expression"@en, "Mehrautorentextdokument-Expression"@de;
	rdfs:comment """Document expression by different authors."""@en;
	rdfs:subClassOf document:Expression.

document:ExpressionIdentifier
	a owl:Class;
	rdfs:label "document expression identifier"@en, "Dokument-Expressionsidentifikator"@de;
	rdfs:comment """Identifier of a document expression."""@en;
	rdfs:subClassOf document:Structure, concept:Identifier.

# document:Witness

document:CollectedWorks
	a owl:Class;
	rdfs:label "collected works"@en, "gesammelte Werke"@de;
	rdfs:comment """Collection of individual document expressions of one author."""@en;
	rdfs:subClassOf document:Expression.

document:Cycle
	a owl:Class;
	rdfs:label "expression cycle"@en, "Expression-Zyklus"@de;
	rdfs:comment """Set of expressions belonging together, usually created around a certain theme, and intended to be experienced in a certain sequence."""@en;
	rdfs:subClassOf concept:Set.

document:Catalogue
	a owl:Class;
	rdfs:label "catalogue"@en, "Katalog"@de, "catalogue"@fr;
	rdfs:comment """List of descriptions of things, mostly ordered, e.g. alphabetically; e.g. library's book catalogue, exhibition's works of art catalogue, mail-order company's items for sale catalogue."""@en;
	rdfs:subClassOf document:IndividualExpression.

document:Encoder
	a owl:Class;
	rdfs:label "encoder"@en, "KodiererIn"@de, "codeur"@fr, "codificatore"@it;
	rdfs:comment """Role of a person converting a document into code, e.g. from text to XML."""@en;
	rdfs:subClassOf human:PersonCreator.

document:Code
	a owl:Class;
	rdfs:label "code document"@en,"Kode-Dokument"@de;
	rdfs:comment """Document as code."""@en;
	rdfs:subClassOf document:Document.

document:HypertextDocument
	a owl:Class;
	rdfs:label "hypertext document"@en,"Hypertext-Dokument"@de;
	rdfs:comment """Document written in Hypertext Markup Language (HTML)."""@en;
	rdfs:subClassOf document:Code.

document:HypertextElement
	a owl:Class;
	rdfs:label "hypertext document element"@en, "Hypertext-Dokumentelement"@de;
	rdfs:comment """Information as part of a hypertext document."""@en;
	rdfs:subClassOf document:Element, [
		a owl:Restriction; owl:onProperty document:isElementOfHypertextDocument; owl:minCardinality "0"^^xsd:nonNegativeInteger], [
		a owl:Restriction; owl:onProperty document:isElementOfHypertextDocumentValue; owl:minCardinality "0"^^xsd:nonNegativeInteger].

document:HypertextStructure
	a owl:Class;
	rdfs:label "hypertext document structure"@en, "Hypertext-Dokumentstruktur"@de;
	rdfs:comment """Structural element of a hypertext document."""@en;
	rdfs:subClassOf document:HypertextElement, document:Structure, [
		a owl:Restriction; owl:onProperty infocar:hasHyperlink; owl:minCardinality "0"^^xsd:nonNegativeInteger], [
		a owl:Restriction; owl:onProperty infocar:hasHyperlinkValue; owl:minCardinality "0"^^xsd:nonNegativeInteger].

#
# PROPERTIES
#

# document:hasContent
#	a owl:ObjectProperty;
#	rdfs:label "has content"@en, "hat Inhalt"@de;
#	rdfs:comment """Relating a document to its content."""@en;
#	rdfs:subPropertyOf knora-base:hasValue;
#	knora-base:subjectClassConstraint document:Document;
#	knora-base:objectClassConstraint knora-base:FileValue. # not instantiable in knora

# document:isLayoutOf
#	a owl:ObjectProperty;
#	rdfs:label "is layout of"@en, "ist Aufmachung von"@de;
#	rdfs:comment "Relating a layout to a document."@en;
#	rdfs:domain layout:Layout;
#	rdfs:range document:Document;
#	rdfs:subPropertyOf knora-base:hasLinkTo;
#	knora-base:subjectClassConstraint layout:Layout;
#	knora-base:objectClassConstraint document:Document.

document:hasEncoder
	a owl:ObjectProperty;
	rdfs:label "has encoder"@en, "hat Encoder"@de;
	rdfs:comment "Relating a document to a person who encoded it."@en;
	rdfs:domain document:Document;
#	rdfs:range [rdfs:subClassOf human:Person, [a owl:Restriction; owl:onProperty human:personHasRole; owl:someValuesFrom document:Encoder]];
	rdfs:subPropertyOf knora-base:hasLinkTo;
	knora-base:subjectClassConstraint document:Document;
	knora-base:objectClassConstraint human:Person.

document:hasEncoderValue
	a owl:ObjectProperty;
	rdfs:label "has encoder - statement"@en, "hat Encoder - Festlegung"@de;
	rdfs:comment "Relating a document to a reification statement of the relation between the document and a person who encoded it."@en;
	rdfs:subPropertyOf knora-base:hasLinkToValue;
	knora-base:subjectClassConstraint document:Document;
	knora-base:objectClassConstraint knora-base:LinkValue.

document:isElementOfDocument
	a owl:ObjectProperty;
	rdfs:label "is element of document"@en, "ist Element eines Dokumentes"@de;
	rdfs:comment """Relating a document element to a document it is part of."""@en;
	rdfs:domain document:Element;
	rdfs:range document:Document;
	rdfs:subPropertyOf concept:isPartOf;
	knora-base:subjectClassConstraint document:Element;
	knora-base:objectClassConstraint document:Document.

document:isElementOfDocumentValue
	a owl:ObjectProperty;
	rdfs:label "is element of document - statement"@en, "ist Element eines Dokumentes - Festlegung"@de;
	rdfs:comment """Relating a document element to a reification statement of the relation between the element and a document it is part of."""@en;
	rdfs:subPropertyOf concept:isPartOfValue;
	knora-base:subjectClassConstraint document:Element;
	knora-base:objectClassConstraint knora-base:LinkValue.

document:isStructureOfDocument
	a owl:ObjectProperty;
	rdfs:label "is structure of document"@en, "ist Struktur eines Dokumentes"@de;
	rdfs:comment """Relating a document structure to a document it is part of."""@en;
	rdfs:domain document:Structure;
	rdfs:range document:Document;
	rdfs:subPropertyOf document:isElementOfDocument;
	knora-base:subjectClassConstraint document:Structure;
	knora-base:objectClassConstraint document:Document.

document:isStructureOfDocumentValue
	a owl:ObjectProperty;
	rdfs:label "is structure of document - statement"@en, "ist Struktur eines Dokumentes - Festlegung"@de;
	rdfs:comment """Relating a document structure to a reification statement of the relation between the structure and a document it is part of."""@en;
	rdfs:subPropertyOf document:isElementOfDocumentValue;
	knora-base:subjectClassConstraint document:Structure;
	knora-base:objectClassConstraint knora-base:LinkValue.

document:isSpaceOfDocument
	a owl:ObjectProperty;
	rdfs:label "is space of document"@en, "ist Leerraum eines Dokumentes"@de;
	rdfs:comment """Relating a space to the document it is part of."""@en;
	rdfs:domain document:Space;
	rdfs:range document:Document;
	rdfs:subPropertyOf document:isStructureOfDocument;
	knora-base:subjectClassConstraint document:Space;
	knora-base:objectClassConstraint document:Document.

document:isSpaceOfDocumentValue
	a owl:ObjectProperty;
	rdfs:label "is space of document - statement"@en, "ist Leerraum eines Dokumentes - Festlegung"@de;
	rdfs:comment """Relating a space to a reification statement of the relation between the space and the document it is part of."""@en;
	rdfs:subPropertyOf document:isStructureOfDocumentValue;
	knora-base:subjectClassConstraint document:Space;
	knora-base:objectClassConstraint knora-base:LinkValue.

document:contentStructureHasIdentifier
	a owl:ObjectProperty;
	rdfs:label "document content structure has identifier"@en, "Dokumentinhaltstruktur hat Identifikator"@de;
	rdfs:comment """Relating a document content structure to its identifier."""@en;
	rdfs:domain document:ContentStructure;
	rdfs:range document:ContentStructureIdentifier;
	rdfs:subPropertyOf knora-base:hasLinkTo;
	knora-base:subjectClassConstraint document:ContentStructure;
	knora-base:objectClassConstraint document:ContentStructureIdentifier.

document:contentStructureHasIdentifierValue
	a owl:ObjectProperty;
	rdfs:label "document content structure has identifier - statement"@en, "Dokumentinhaltstruktur hat Identifikator - Festlegung"@de;
	rdfs:comment """Relating a document content structure to a reification statement of the relation between the content structure and its identifier."""@en;
	rdfs:subPropertyOf knora-base:hasLinkToValue;
	knora-base:subjectClassConstraint document:ContentStructure;
	knora-base:objectClassConstraint knora-base:LinkValue.

document:hasReference
	a owl:ObjectProperty;
	rdfs:label "document content structure has reference"@en, "Dokumentinhaltstruktur hat Referenz"@de;
	rdfs:comment """Relating a document content structure to a reference it has."""@en;
	rdfs:domain document:ContentStructure;
	rdfs:range document:ContentStructureReference;
	rdfs:subPropertyOf knora-base:hasLinkTo;
	knora-base:subjectClassConstraint document:ContentStructure;
	knora-base:objectClassConstraint document:ContentStructureReference.

document:hasReferenceValue
	a owl:ObjectProperty;
	rdfs:label "document content structure has reference - statement"@en, "Dokumentinhaltstruktur hat Referenz - Festlegung"@de;
	rdfs:comment """Relating a document content structure to a reification statement of the relation between the content structure and a reference it has."""@en;
	rdfs:subPropertyOf knora-base:hasLinkToValue;
	knora-base:subjectClassConstraint document:ContentStructure;
	knora-base:objectClassConstraint knora-base:LinkValue.

document:hasTextReference
	a owl:ObjectProperty;
	rdfs:label "has text reference"@en, "hat Textreferenz"@de;
	rdfs:comment """Relating a document content structure to a text reference it has."""@en;
	rdfs:domain document:ContentStructure;
	rdfs:range document:TextStructureReference;
	rdfs:subPropertyOf document:hasReference;
	knora-base:subjectClassConstraint document:ContentStructure;
	knora-base:objectClassConstraint document:TextStructureReference.

document:hasTextReferenceValue
	a owl:ObjectProperty;
	rdfs:label "has text reference - statement"@en, "hat Textreferenz - Festlegung"@de;
	rdfs:comment """Relating a document content structure to a reification statement of the relation between the content structure and a text reference it has."""@en;
	rdfs:subPropertyOf document:hasReferenceValue;
	knora-base:subjectClassConstraint document:ContentStructure;
	knora-base:objectClassConstraint knora-base:LinkValue.

document:hasFootnoteReference
	a owl:ObjectProperty;
	rdfs:label "has footnote reference"@en, "hat Fussnotereferenz"@de;
	rdfs:comment """Relating a document content structure to a footnote reference it has."""@en;
	rdfs:domain document:ContentStructure;
	rdfs:range document:FootnoteReference;
	rdfs:subPropertyOf document:hasTextReference;
	knora-base:subjectClassConstraint document:ContentStructure;
	knora-base:objectClassConstraint document:FootnoteReference.

document:hasFootnoteReferenceValue
	a owl:ObjectProperty;
	rdfs:label "has footnote reference - statement"@en, "hat Fussnotereferenz - Festlegung"@de;
	rdfs:comment """Relating a document content structure to a reification statement of the relation between the content structure and a footnote reference it has."""@en;
	rdfs:subPropertyOf document:hasTextReferenceValue;
	knora-base:subjectClassConstraint document:ContentStructure;
	knora-base:objectClassConstraint knora-base:LinkValue.

document:hasEndnoteReference
	a owl:ObjectProperty;
	rdfs:label "has endnote reference"@en, "hat Endnotereferenz"@de;
	rdfs:comment """Relating a document content structure to an endnote reference it has."""@en;
	rdfs:domain document:ContentStructure;
	rdfs:range document:EndnoteReference;
	rdfs:subPropertyOf document:hasTextReference;
	knora-base:subjectClassConstraint document:ContentStructure;
	knora-base:objectClassConstraint document:EndnoteReference.

document:hasEndnoteReferenceValue
	a owl:ObjectProperty;
	rdfs:label "has endnote reference - statement"@en, "hat Endnotereferenz - Festlegung"@de;
	rdfs:comment """Relating a document content structure to a reification statement of the relation between the content structure and an endnote reference it has."""@en;
	rdfs:subPropertyOf document:hasTextReferenceValue;
	knora-base:subjectClassConstraint document:ContentStructure;
	knora-base:objectClassConstraint knora-base:LinkValue.

document:hasExpressionReference
	a owl:ObjectProperty;
	rdfs:label "has expression reference"@en, "hat Expression-Referenz"@de;
	rdfs:comment """Relating a document content structure to an expression reference it has."""@en;
	rdfs:domain document:ContentStructure;
	rdfs:range document:ExpressionReference;
	rdfs:subPropertyOf knora-base:hasLinkTo;
	knora-base:subjectClassConstraint document:ContentStructure;
	knora-base:objectClassConstraint document:ExpressionReference.

document:hasExpressionReferenceValue
	a owl:ObjectProperty;
	rdfs:label "has expression reference - statement"@en, "hat Expression-Referenz - Festlegung"@de;
	rdfs:comment """Relating a document content structure to a reification statement of the relation between the content structure and an expression reference it has."""@en;
	rdfs:subPropertyOf knora-base:hasLinkToValue;
	knora-base:subjectClassConstraint document:ContentStructure;
	knora-base:objectClassConstraint knora-base:LinkValue.

document:hasContentStructureIdentifier
	a owl:ObjectProperty;
	rdfs:label "has document content structure identifier"@en, "hat Dokumentinhaltstrukturidentifikator"@de;
	rdfs:comment """Relating a document content structure reference to the identifier of another document content structure."""@en;
	rdfs:domain document:ContentStructureReference;
	rdfs:range document:ContentStructureIdentifier;
	rdfs:subPropertyOf knora-base:hasLinkTo;
	knora-base:subjectClassConstraint document:ContentStructureReference;
	knora-base:objectClassConstraint document:ContentStructureIdentifier.

document:hasContentStructureIdentifierValue
	a owl:ObjectProperty;
	rdfs:label "has document content structure identifier - statement"@en, "hat Dokumentinhaltstrukturidentifikator - Festlegung"@de;
	rdfs:comment """Relating a document content structure reference to a reification statement of the relation between that reference and the identifier of another document content structure."""@en;
	rdfs:subPropertyOf knora-base:hasLinkToValue;
	knora-base:subjectClassConstraint document:ContentStructureReference;
	knora-base:objectClassConstraint knora-base:LinkValue.

document:hasTextStructureIdentifier
	a owl:ObjectProperty;
	rdfs:label "has text identifier"@en, "hat Textidentifikator"@de;
	rdfs:comment """Relating a text reference to its text identifier."""@en;
	rdfs:domain document:TextStructureReference;
	rdfs:range text-structure:Identifier;
	rdfs:subPropertyOf document:hasContentStructureIdentifier;
	knora-base:subjectClassConstraint document:TextStructureReference;
	knora-base:objectClassConstraint text-structure:Identifier.

document:hasTextStructureIdentifierValue
	a owl:ObjectProperty;
	rdfs:label "has text identifier - statement"@en, "hat Textidentifikator - Festlegung"@de;
	rdfs:comment """Relating a text reference to a reification statement of the relation between that reference and its text identifier."""@en;
	rdfs:subPropertyOf document:hasContentStructureIdentifierValue;
	knora-base:subjectClassConstraint document:TextStructureReference;
	knora-base:objectClassConstraint knora-base:LinkValue.

document:hasFootnoteIdentifier
	a owl:ObjectProperty;
	rdfs:label "has footnote identifier"@en, "hat Fussnoteidentifikator"@de;
	rdfs:comment """Relating a footnote reference to its footnote identifier."""@en;
	rdfs:domain document:FootnoteReference;
	rdfs:range note-structure:FootnoteIdentifier;
	rdfs:subPropertyOf document:hasTextStructureIdentifier;
	knora-base:subjectClassConstraint document:FootnoteReference;
	knora-base:objectClassConstraint note-structure:FootnoteIdentifier.

document:hasFootnoteIdentifierValue
	a owl:ObjectProperty;
	rdfs:label "has footnote identifier - statement"@en, "hat Fussnoteidentifikator - Festlegung"@de;
	rdfs:comment """Relating a footnote reference to a reification statement of the relation between that reference and its footnote identifier."""@en;
	rdfs:subPropertyOf document:hasTextStructureIdentifierValue;
	knora-base:subjectClassConstraint document:FootnoteReference;
	knora-base:objectClassConstraint knora-base:LinkValue.

document:hasFootnoteNumber
	a owl:ObjectProperty;
	rdfs:label "has footnote number"@en, "hat Fussnotenummer"@de;
	rdfs:comment """Relating a footnote reference to its footnote number."""@en;
	rdfs:domain document:FootnoteReference;
	rdfs:range note-structure:FootnoteNumber;
	rdfs:subPropertyOf document:hasFootnoteIdentifier;
	knora-base:subjectClassConstraint document:FootnoteReference;
	knora-base:objectClassConstraint note-structure:FootnoteNumber.

document:hasFootnoteNumberValue
	a owl:ObjectProperty;
	rdfs:label "has footnote number - statement"@en, "hat Fussnotenummer - Festlegung"@de;
	rdfs:comment """Relating a footnote reference to a reification statement of the relation between the reference and its footnote number."""@en;
	rdfs:subPropertyOf document:hasFootnoteIdentifierValue;
	knora-base:subjectClassConstraint document:FootnoteReference;
	knora-base:objectClassConstraint knora-base:LinkValue.

document:hasEndnoteIdentifier
	a owl:ObjectProperty;
	rdfs:label "has endnote identifier"@en, "hat Endnoteidentifikator"@de;
	rdfs:comment """Relating an endnote reference to its endnote identifier."""@en;
	rdfs:domain document:EndnoteReference;
	rdfs:range note-structure:EndnoteIdentifier;
	rdfs:subPropertyOf document:hasTextStructureIdentifier;
	knora-base:subjectClassConstraint document:EndnoteReference;
	knora-base:objectClassConstraint note-structure:EndnoteIdentifier.

document:hasEndnoteIdentifierValue
	a owl:ObjectProperty;
	rdfs:label "has endnote identifier - statement"@en, "hat Endnoteidentifikator - Festlegung"@de;
	rdfs:comment """Relating an endnote reference to a reification statement of the relation between that reference and its endnote identifier."""@en;
	rdfs:subPropertyOf document:hasTextStructureIdentifierValue;
	knora-base:subjectClassConstraint document:EndnoteReference;
	knora-base:objectClassConstraint knora-base:LinkValue.

document:hasEndnoteNumber
	a owl:ObjectProperty;
	rdfs:label "has endnote number"@en, "hat Endnotenummer"@de;
	rdfs:comment """Relating an endnote reference to its endnote number."""@en;
	rdfs:domain document:EndnoteReference;
	rdfs:range note-structure:EndnoteNumber;
	rdfs:subPropertyOf document:hasEndnoteIdentifier;
	knora-base:subjectClassConstraint document:EndnoteReference;
	knora-base:objectClassConstraint note-structure:EndnoteNumber.

document:hasEndnoteNumberValue
	a owl:ObjectProperty;
	rdfs:label "has endnote number - statement"@en, "hat Endnotenummer - Festlegung"@de;
	rdfs:comment """Relating an endnote reference to a reification statement of the relation between the reference and its endnote number."""@en;
	rdfs:subPropertyOf document:hasEndnoteIdentifierValue;
	knora-base:subjectClassConstraint document:EndnoteReference;
	knora-base:objectClassConstraint knora-base:LinkValue.

document:isColumnOfPage
	a owl:ObjectProperty;
	rdfs:label "is column of document page"@en, "ist Spalte einer Dokumentseite"@de;
	rdfs:comment """Relating a column to a document page it is part of."""@en;
	rdfs:domain document:Column;
	rdfs:range document:Page;
	rdfs:subPropertyOf concept:isPartOf;
	knora-base:subjectClassConstraint document:Column;
	knora-base:objectClassConstraint document:Page.

document:isColumnOfPageValue
	a owl:ObjectProperty;
	rdfs:label "is column of document page - statement"@en, "ist Spalte einer Dokumentseite - Festlegung"@de;
	rdfs:comment """Relating a column to a reification statement of the relation between the column and a document page it is part of."""@en;
	rdfs:subPropertyOf concept:isPartOfValue;
	knora-base:subjectClassConstraint document:Column;
	knora-base:objectClassConstraint knora-base:LinkValue.

document:isPageOfExpression
	a owl:ObjectProperty;
	rdfs:label "is page of expression"@en, "ist Seite einer Expression"@de;
	rdfs:comment """Relating a document page to a document expression it is part of."""@en;
	rdfs:domain document:Page;
	rdfs:range document:Expression;
	rdfs:subPropertyOf concept:isPartOf;
	knora-base:subjectClassConstraint document:Page;
	knora-base:objectClassConstraint document:Expression.

document:isPageOfExpressionValue
	a owl:ObjectProperty;
	rdfs:label "is page of expression - statement"@en, "ist Seite einer Expression - Festlegung"@de;
	rdfs:comment """Relating a document page to a reification statement of the relation between the page and a document expression it is part of."""@en;
	rdfs:subPropertyOf concept:isPartOfValue;
	knora-base:subjectClassConstraint document:Page;
	knora-base:objectClassConstraint knora-base:LinkValue.

document:pageHasIdentifier
	a owl:ObjectProperty;
	rdfs:label "page has identifier"@en, "Seite hat Identifikator"@de;
	rdfs:comment """Relating a document page to its identifier."""@en;
	rdfs:domain document:Page;
	rdfs:range document:PageIdentifier;
	rdfs:subPropertyOf document:contentStructureHasIdentifier;
	knora-base:subjectClassConstraint document:Page;
	knora-base:objectClassConstraint document:PageIdentifier.

document:pageHasIdentifierValue
	a owl:ObjectProperty;
	rdfs:label "page has identifier - statement"@en, "Seite hat Identifikator - Festlegung"@de;
	rdfs:comment """Relating a document page to a reification statement of the relation between the page and its identifier."""@en;
	rdfs:subPropertyOf document:contentStructureHasIdentifierValue;
	knora-base:subjectClassConstraint document:Page;
	knora-base:objectClassConstraint knora-base:LinkValue.

document:pageHasNumber
	a owl:ObjectProperty;
	rdfs:label "page has number"@en, "Seite hat Nummer"@de;
	rdfs:comment """Relating a document page to its number."""@en;
	rdfs:domain document:Page;
	rdfs:range document:PageNumber;
	rdfs:subPropertyOf document:pageHasIdentifier;
	knora-base:subjectClassConstraint document:Page;
	knora-base:objectClassConstraint document:PageNumber.

document:pageHasNumberValue
	a owl:ObjectProperty;
	rdfs:label "page has number - statement"@en, "Seite hat Nummer - Festlegung"@de;
	rdfs:comment """Relating a document page to a reification statement of the relation between the page and its number."""@en;
	rdfs:subPropertyOf document:pageHasIdentifierValue;
	knora-base:subjectClassConstraint document:Page;
	knora-base:objectClassConstraint knora-base:LinkValue.

document:isTableOfColumn
	a owl:ObjectProperty;
	rdfs:label "is table of column"@en, "ist Tabelle einer Spalte"@de;
	rdfs:comment """Relating a table to a column it is part of."""@en;
	rdfs:domain document:Table;
	rdfs:range document:Column;
	rdfs:subPropertyOf concept:isPartOf; #Â°
	knora-base:subjectClassConstraint document:Table;
	knora-base:objectClassConstraint document:Column.

document:isTableOfColumnValue
	a owl:ObjectProperty;
	rdfs:label "is table of column - statement"@en, "ist Tabelle einer Spalte - Festlegung"@de;
	rdfs:comment """Relating a table to a reification statement of the relation between the table and a column it is part of."""@en;
	rdfs:subPropertyOf concept:isPartOfValue; #Â°
	knora-base:subjectClassConstraint document:Table;
	knora-base:objectClassConstraint knora-base:LinkValue.

document:expressionHasIdentifier
	a owl:ObjectProperty;
	rdfs:label "expression has identifier"@en, "Expression hat Identifikator"@de;
	rdfs:comment """Relating a document expression to its identifier."""@en;
	rdfs:domain document:Expression;
	rdfs:range document:ExpressionIdentifier;
	rdfs:subPropertyOf knora-base:hasLinkTo; #Â°
	knora-base:subjectClassConstraint document:Expression;
	knora-base:objectClassConstraint document:ExpressionIdentifier.

document:expressionHasIdentifierValue
	a owl:ObjectProperty;
	rdfs:label "expression has identifier - statement"@en, "Expression hat Identifikator - Festlegung"@de;
	rdfs:comment """Relating a document expression to a reification statement of the relation between the expression and its identifier."""@en;
	rdfs:subPropertyOf knora-base:hasLinkToValue; #Â°
	knora-base:subjectClassConstraint document:Expression;
	knora-base:objectClassConstraint knora-base:LinkValue.

document:expressionHasTitle
	a owl:ObjectProperty;
	rdfs:label "expression has title"@en, "Expression hat Titel"@de;
	rdfs:comment """Relating an expression to a title it has."""@en;
	rdfs:domain document:Expression;
#	rdfs:range rdfs:Literal;
	rdfs:subPropertyOf text:hasTitle;
	knora-base:subjectClassConstraint document:Expression;
	knora-base:objectClassConstraint knora-base:TextValue.

document:expressionHasSubtitle
	a owl:ObjectProperty;
	rdfs:label "expression has subtitle"@en, "Expression hat Untertitel"@de;
	rdfs:comment """Relating an expression to a subtitle it has."""@en;
	rdfs:domain document:Expression;
#	rdfs:range rdfs:Literal;
	rdfs:subPropertyOf text:hasSubtitle;
	knora-base:subjectClassConstraint document:Expression;
	knora-base:objectClassConstraint knora-base:TextValue.

document:isExpressionOfCycle
	a owl:ObjectProperty;
	rdfs:label "is expression of cycle"@en, "ist Expression eines Zyklus"@de;
	rdfs:comment """Relating an individual expression to a cycle it is part of."""@en;
	rdfs:domain document:IndividualExpression;
	rdfs:range document:Cycle;
	rdfs:subPropertyOf concept:isPartOf;
	knora-base:subjectClassConstraint document:IndividualExpression;
	knora-base:objectClassConstraint document:Cycle.

document:isExpressionOfCycleValue
	a owl:ObjectProperty;
	rdfs:label "is expression of cycle - statement"@en, "ist Expression eines Zyklus - Festlegung"@de;
	rdfs:comment """Relating an individual expression to a reification statement of the relation between the expression and a cycle it is part of."""@en;
	rdfs:subPropertyOf concept:isPartOfValue;
	knora-base:subjectClassConstraint document:IndividualExpression;
	knora-base:objectClassConstraint knora-base:LinkValue.

document:isPartOfIndividualExpression
	a owl:ObjectProperty;
	rdfs:label "is part of individual expression"@en, "ist Teil einer individuellen Expression"@de;
	rdfs:comment """Relating an expression part to an individual expression it is part of."""@en;
	rdfs:domain document:ExpressionPart;
	rdfs:range document:IndividualExpression;
	rdfs:subPropertyOf concept:isPartOf;
	knora-base:subjectClassConstraint document:ExpressionPart;
	knora-base:objectClassConstraint document:IndividualExpression.

document:isPartOfIndividualExpressionValue
	a owl:ObjectProperty;
	rdfs:label "is part of individual expression - statement"@en, "ist Teil einer individuellen Expression - Festlegung"@de;
	rdfs:comment """Relating an expression part to a reification statement of the relation between the expression part and an individual expression it is part of."""@en;
	rdfs:subPropertyOf concept:isPartOfValue;
	knora-base:subjectClassConstraint document:ExpressionPart;
	knora-base:objectClassConstraint knora-base:LinkValue.

document:expressionReferenceHasIdentifier
	a owl:ObjectProperty;
	rdfs:label "expression reference has identifier"@en, "Expression-Referenz hat Identifikator"@de;
	rdfs:comment """Relating a document expression reference to its identifier."""@en;
	rdfs:domain document:ExpressionReference;
	rdfs:range document:ExpressionIdentifier;
	rdfs:subPropertyOf knora-base:hasLinkTo; #Â°
	knora-base:subjectClassConstraint document:ExpressionReference;
	knora-base:objectClassConstraint document:ExpressionIdentifier.

document:expressionReferenceHasIdentifierValue
	a owl:ObjectProperty;
	rdfs:label "expression reference has identifier - statement"@en, "Expression-Referenz hat Identifikator - Festlegung"@de;
	rdfs:comment """Relating a document expression reference to a reification statement of the relation between that reference and its identifier."""@en;
	rdfs:subPropertyOf knora-base:hasLinkToValue; #Â°
	knora-base:subjectClassConstraint document:ExpressionReference;
	knora-base:objectClassConstraint knora-base:LinkValue.

document:isElementOfHypertextDocument
	a owl:ObjectProperty;
	rdfs:label "is element of hypertext  document"@en, "ist Element eines Hypertext-Dokumentes"@de;
	rdfs:comment """Relating a hypertext document element to a hypertext document it is part of."""@en;
	rdfs:domain document:HypertextElement;
	rdfs:range document:HypertextDocument;
	rdfs:subPropertyOf concept:isPartOf;
	knora-base:subjectClassConstraint document:HypertextElement;
	knora-base:objectClassConstraint document:HypertextDocument.

document:isElementOfHypertextDocumentValue
	a owl:ObjectProperty;
	rdfs:label "is element of hypertext hypertext hypertext document - statement"@en, "ist Element eines Hypertext-Dokumentes - Festlegung"@de;
	rdfs:comment """Relating a hypertext hypertext document element to a reification statement of the relation between the element and a hypertext document it is part of."""@en;
	rdfs:subPropertyOf concept:isPartOfValue;
	knora-base:subjectClassConstraint document:HypertextElement;
	knora-base:objectClassConstraint knora-base:LinkValue.