@prefix rdf: <http://www.w3.org/1999/02/22-rdf-syntax-ns#>.
@prefix rdfs: <http://www.w3.org/2000/01/rdf-schema#>.
@prefix owl: <http://www.w3.org/2002/07/owl#>.
@prefix xsd: <http://www.w3.org/2001/XMLSchema#>.
@prefix dct: <http://purl.org/dc/terms/>.
@prefix cidoc: <http://www.cidoc-crm.org/cidoc-crm/>.
@prefix human: <http://www.knora.org/ontology/shared/human#>.
@prefix concept: <http://www.knora.org/ontology/shared/concept#>.
@prefix document: <http://www.knora.org/ontology/shared/document#>.
@prefix text: <http://www.knora.org/ontology/shared/text#>.
@prefix infocar: <http://www.knora.org/ontology/shared/information-carrier#>.
@prefix knora-base: <http://www.knora.org/ontology/knora-base#>.

@base <http://www.knora.org/ontology/shared/image>.
@prefix image: <http://www.knora.org/ontology/shared/image#>.

<http://www.knora.org/ontology/shared/image>
	a owl:Ontology;
	dct:title "An ontology about image"@en;
	dct:description """Formal description of image as a visual resource in the broadest sense, its general subclasses, related classes, and properties."""@en;
	dct:creator "Hans Cools, MD, knowledge engineer, ontologist, software developer, NIE-INE, Basel University, Switzerland"@en;

	knora-base:attachedToProject <http://www.knora.org/ontology/knora-base#DefaultSharedOntologiesProject>. # <http://rdfh.ch/projects/004A>.

#
# CLASSES
#

image:Image
	a owl:Class;
	rdfs:label "image"@en,"Bild"@de;
	rdfs:comment """Visual representation of something."""@en;
	rdfs:subClassOf document:Document, cidoc:E38_Image. # rdfs:subClassOf cidoc:E36_Visual_Item rdfs:subClassOf cidoc:E73_Information_Object rdfs:subClassOf cidoc:E90_Symbolic_Object rdfs:subClassOf cidoc:E28_Conceptual_Object

image:ImageExpression
	a owl:Class;
	rdfs:label "image expression"@en,"Bildexpression"@de;
	rdfs:comment """Image as a document expression conform FRBROO."""@en;
	rdfs:subClassOf document:Expression, image:Image.

image:ImageCarrier
	a owl:Class;
	rdfs:label "image carrier"@en,"Bildtr채ger"@de;
	rdfs:comment """Image on a carrier."""@en;
	rdfs:subClassOf infocar:Carrier.

image:Photograph
	a owl:Class;
	rdfs:label "photograph"@en,"Foto"@de;
	rdfs:comment """Image made by exposing a photosensitive surface to light."""@en;
	rdfs:subClassOf image:ImageCarrier.

#
# PROPERTIES
#

image:imageDepicts
	a owl:ObjectProperty;
	rdfs:label "image depicts", "bildet ab"@de;
	rdfs:comment """Relating an image to what it depicts."""@en;
	rdfs:domain image:Image;
	rdfs:range rdfs:Resource;
	rdfs:subPropertyOf knora-base:hasLinkTo;
	knora-base:subjectClassConstraint image:Image;
	knora-base:objectClassConstraint knora-base:Resource.

image:imageDepictsValue
	a owl:ObjectProperty;
	rdfs:label "image depicts - statement", "bildet ab - Festlegung"@de;
	rdfs:comment """Relating an image to a reification statement of the relation between the image and what it depicts."""@en;
	rdfs:subPropertyOf knora-base:hasLinkToValue;
	knora-base:subjectClassConstraint image:Image;
	knora-base:objectClassConstraint knora-base:LinkValue.

image:hasPhotograph
	a owl:ObjectProperty;
	rdfs:label "has photograph", "hat Foto"@de;
	rdfs:comment """Relating something to a photograph thereof."""@en;
	rdfs:domain rdfs:Resource;
	rdfs:range image:Photograph;
	rdfs:subPropertyOf knora-base:hasLinkTo;
	knora-base:subjectClassConstraint knora-base:Resource;
	knora-base:objectClassConstraint image:Photograph.

image:hasPhotographValue
	a owl:ObjectProperty;
	rdfs:label "has photograph - statement", "hat Foto - Festlegung"@de;
	rdfs:comment """Relating something to a reification statement of the relation between that something and a photograph thereof."""@en;
	rdfs:subPropertyOf knora-base:hasLinkToValue;
	knora-base:subjectClassConstraint knora-base:Resource;
	knora-base:objectClassConstraint knora-base:LinkValue.

# image:isOnCarrier

# image:isOnCarrierValue

#image:hasPhotoRepresentation # can be activated when Knora2 is released
#	a owl:ObjectProperty;
#	rdfs:label "has photograph representation"@en, "hat Foto-Repr채sentation"@de;
#	rdfs:comment """Relating a resource to a photograph thereof."""@en;
#	rdfs:subPropertyOf knora-base:hasRepresentation; # cidoc:P138i_has_representation
#	knora-base:subjectClassConstraint knora-base:Resource;
#	knora-base:objectClassConstraint image:Photograph.

#image:hasPhotoRepresentationValue # can be activated when Knora2 is released
#	a owl:ObjectProperty;
#	rdfs:label "has photograph representation - statement"@en;
#	rdfs:comment """Relating a resource to a reification statement of the relation between the resource and a photograph thereof."""@en;
#	rdfs:subPropertyOf knora-base:hasRepresentationValue;
#	knora-base:subjectClassConstraint knora-base:Resource;
#	knora-base:objectClassConstraint knora-base:LinkValue.

image:hasPhotographIn
	a owl:ObjectProperty;
	rdfs:label "has photograph in", "hat Foto in"@de;
	rdfs:comment """Relating something to something else containing a photograph of the former."""@en;
	rdfs:subPropertyOf knora-base:hasLinkTo;
	knora-base:subjectClassConstraint knora-base:Resource;
	knora-base:objectClassConstraint knora-base:Resource.

image:hasPhotographInValue
	a owl:ObjectProperty;
	rdfs:label "has image in - statement", "hat Foto in - Festlegung"@de;
	rdfs:comment """Relating something to a reification statement of the relation between that something and something else containing a photograph of the former."""@en;
	rdfs:subPropertyOf knora-base:hasLinkToValue;
	knora-base:subjectClassConstraint knora-base:Resource;
	knora-base:objectClassConstraint knora-base:LinkValue.

image:hasPhotographSourceDescription
	a owl:ObjectProperty;
	rdfs:label "has photograph source description"@en, "hat Fotoquelle-Beschreibung"@de;
	rdfs:comment """Relating something to a description of a source of a photograph of that something."""@en;

	rdfs:subPropertyOf text:hasDescription;
	knora-base:subjectClassConstraint knora-base:Resource;
	knora-base:objectClassConstraint knora-base:TextValue.

image:hasPhotoRepresentation
	a owl:ObjectProperty;
	rdfs:label "has photo representation", "hat Foto-Repr채sentation"@de;
	rdfs:comment """Relating something to a digital container of metadata of a digital photograph of that something."""@en;
	rdfs:subPropertyOf knora-base:hasRepresentation;
	knora-base:subjectClassConstraint knora-base:Resource;
	knora-base:objectClassConstraint knora-base:StillImageRepresentation.

image:hasPhotoRepresentationValue
	a owl:ObjectProperty;
	rdfs:label "has photo representation - statement", "hat Foto-Repr채sentation - Festlegung"@de;
	rdfs:comment """Relating something to a reification statement of the relation between that something and a digital container of metadata of a digital photograph of that something."""@en;
	rdfs:subPropertyOf knora-base:hasRepresentationValue;
	knora-base:subjectClassConstraint knora-base:Resource;
	knora-base:objectClassConstraint knora-base:LinkValue.