@prefix rdf: <http://www.w3.org/1999/02/22-rdf-syntax-ns#>.
@prefix rdfs: <http://www.w3.org/2000/01/rdf-schema#>.
@prefix owl: <http://www.w3.org/2002/07/owl#>.
@prefix xsd: <http://www.w3.org/2001/XMLSchema#>.
@prefix dct: <http://purl.org/dc/terms/>.
@prefix cidoc: <http://www.cidoc-crm.org/cidoc-crm/>.
@prefix human: <http://www.knora.org/ontology/shared/human#>.
@prefix concept: <http://www.knora.org/ontology/shared/concept#>.
@prefix document: <http://www.knora.org/ontology/shared/document#>.
@prefix text: <http://www.knora.org/ontology/shared/text#>.
@prefix infocar: <http://www.knora.org/ontology/shared/information-carrier#>.
@prefix knora-base: <http://www.knora.org/ontology/knora-base#>.

@base <http://www.knora.org/ontology/shared/image>.
@prefix image: <http://www.knora.org/ontology/shared/image#>.

<http://www.knora.org/ontology/shared/image>
	a owl:Ontology;
	dct:license <http://creativecommons.org/licenses/by/3.0/>;
	dct:title "An ontology about image"@en;
	dct:description """Formal description of image as a visual resource in the broadest sense, its general subclasses, related classes, and properties."""@en;
	dct:creator "Hans Cools, MD, knowledge engineer, ontologist, software developer, NIE-INE, Basel University, Switzerland"@en;

	knora-base:attachedToProject <http://www.knora.org/ontology/knora-base#DefaultSharedOntologiesProject>.

#
# CLASSES
#

image:Image
	a owl:Class;
	rdfs:label "image"@en,"Bild"@de;
	rdfs:comment """Visual representation of something, abstracted from its carrier."""@en;
	rdfs:subClassOf document:Document, cidoc:E38_Image, [
		a owl:Restriction; owl:onProperty image:isImageOf; owl:minCardinality "0"^^xsd:nonNegativeInteger], [
		a owl:Restriction; owl:onProperty image:isImageOfValue; owl:minCardinality "0"^^xsd:nonNegativeInteger], [
		a owl:Restriction; owl:onProperty image:isOnCarrier; owl:minCardinality "0"^^xsd:nonNegativeInteger], [
		a owl:Restriction; owl:onProperty image:isOnCarrierValue; owl:minCardinality "0"^^xsd:nonNegativeInteger].

image:ImageExpression
	a owl:Class;
	rdfs:label "image expression"@en,"Bildexpression"@de;
	rdfs:comment """Image as a document expression conform FRBROO."""@en;
	rdfs:subClassOf document:Expression, image:Image.

image:ImageCarrier
	a owl:Class;
	rdfs:label "image carrier"@en,"Bildträger"@de;
	rdfs:comment """Image on a carrier."""@en;
	rdfs:subClassOf infocar:Carrier.

image:Photograph
	a owl:Class;
	rdfs:label "photograph"@en,"Foto"@de;
	rdfs:comment """Image made by exposing a photosensitive surface to light."""@en;
	rdfs:subClassOf image:Image, [
		a owl:Restriction; owl:onProperty image:isPhotographOf; owl:minCardinality "0"^^xsd:nonNegativeInteger], [
		a owl:Restriction; owl:onProperty image:isPhotographOfValue; owl:minCardinality "0"^^xsd:nonNegativeInteger].

# image:DigitalImage

#
# PROPERTIES
#

image:isImageOf
	a owl:ObjectProperty;
	rdfs:label "is image of", "ist Bild von"@de;
	rdfs:comment """Relating an image to what it depicts."""@en;
	rdfs:subPropertyOf concept:informationHasSubject;
	knora-base:subjectClassConstraint image:Image;
	knora-base:objectClassConstraint knora-base:Resource.

image:isImageOfValue
	a owl:ObjectProperty;
	rdfs:label "is image of - statement", "ist Bild von - Festlegung"@de;
	rdfs:comment """Relating an image to a reification statement of the relation between the image and what it depicts."""@en;
	rdfs:subPropertyOf concept:informationHasSubjectValue;
	knora-base:subjectClassConstraint image:Image;
	knora-base:objectClassConstraint knora-base:LinkValue.

image:isOnCarrier
	a owl:ObjectProperty;
	rdfs:label "is image on carrier", "ist Bild auf Träger"@de;
	rdfs:comment """Relating an image to a carrier it is on."""@en;
	rdfs:subPropertyOf infocar:isOnCarrier;
	knora-base:subjectClassConstraint image:Image;
	knora-base:objectClassConstraint image:ImageCarrier.

image:isOnCarrierValue
	a owl:ObjectProperty;
	rdfs:label "is image on carrier - statement", "ist Bild auf Träger - Festlegung"@de;
	rdfs:comment """Relating an image to a reification statement of the relation between the image and a carrier it is on."""@en;
	rdfs:subPropertyOf infocar:isOnCarrierValue;
	knora-base:subjectClassConstraint image:Image;
	knora-base:objectClassConstraint knora-base:LinkValue.

image:isPhotographOf
	a owl:ObjectProperty;
	rdfs:label "is photograph of", "ist Foto von"@de;
	rdfs:comment """Relating a photograph to what it depicts."""@en;
	rdfs:subPropertyOf image:isImageOf;
	knora-base:subjectClassConstraint image:Photograph;
	knora-base:objectClassConstraint knora-base:Resource.

image:isPhotographOfValue
	a owl:ObjectProperty;
	rdfs:label "is photograph of - statement", "ist Foto von - Festlegung"@de;
	rdfs:comment """Relating a photograph to a reification statement of the relation between the photograph and what it depicts."""@en;
	rdfs:subPropertyOf image:isImageOfValue;
	knora-base:subjectClassConstraint image:Photograph;
	knora-base:objectClassConstraint knora-base:LinkValue.

image:hasPhotographIn
	a owl:ObjectProperty;
	rdfs:label "has photograph in", "hat Foto in"@de;
	rdfs:comment """Relating something to something else containing a photograph of the former."""@en;
	rdfs:subPropertyOf knora-base:hasLinkTo;
	knora-base:subjectClassConstraint knora-base:Resource;
	knora-base:objectClassConstraint knora-base:Resource.

image:hasPhotographInValue
	a owl:ObjectProperty;
	rdfs:label "has image in - statement", "hat Foto in - Festlegung"@de;
	rdfs:comment """Relating something to a reification statement of the relation between that something and something else containing a photograph of the former."""@en;
	rdfs:subPropertyOf knora-base:hasLinkToValue;
	knora-base:subjectClassConstraint knora-base:Resource;
	knora-base:objectClassConstraint knora-base:LinkValue.

image:hasPhotographSourceDescription
	a owl:ObjectProperty;
	rdfs:label "has photograph source description"@en, "hat Fotoquelle-Beschreibung"@de;
	rdfs:comment """Relating something to a description of a source of a photograph of that something."""@en;

	rdfs:subPropertyOf text:hasDescription;
	knora-base:subjectClassConstraint knora-base:Resource;
	knora-base:objectClassConstraint knora-base:TextValue.