@prefix rdfs: <http://www.w3.org/2000/01/rdf-schema#>.
@prefix owl: <http://www.w3.org/2002/07/owl#>.
@prefix xsd: <http://www.w3.org/2001/XMLSchema#>.
@prefix skos: <http://www.w3.org/2004/02/skos/core#>.
@prefix dct: <http://purl.org/dc/terms/>.
@prefix text: <http://www.knora.org/ontology/shared/text#>.
@prefix text-structure: <http://www.knora.org/ontology/shared/text-structure#>.
@prefix litera: <http://www.knora.org/ontology/shared/literature#>.
@prefix knora-base: <http://www.knora.org/ontology/knora-base#>.

@base <http://www.knora.org/ontology/shared/indology>.
@prefix indo: <http://www.knora.org/ontology/shared/indology#>.

<http://www.knora.org/ontology/shared/indology>
	a owl:Ontology;
	dct:license <http://creativecommons.org/licenses/by/3.0/>;
	dct:title "An ontology about Indology"@en;
	dct:description """Formal description of Indology, general subclasses, related classes, and properties."""@en;
	dct:creator "Hans Cools, MD, knowledge engineer, ontologist, software developer, NIE-INE, Basel University, Switzerland"@en;
	dct:contributor "Magdalena Plamada, PhD, Zürich University, Switzerland"@en;
	dct:publisher "Basel University, Switzerland"@en;
	
	knora-base:attachedToProject <http://www.knora.org/ontology/knora-base#DefaultSharedOntologiesProject>.

#
# CLASSES
#

indo:Literature
	a owl:Class;
 	rdfs:label "Indian literature"@en, "indische Literatur"@de; # check
	rdfs:comment """Literature in Indian culture."""@en;
	rdfs:subClassOf litera:Literature.

indo:Expression
	a owl:Class;
	rdfs:label "Indian literary expression"@en, "indische literarische Expression"@de;
	rdfs:comment """Literary expression created in Indian culture."""@en, """Literarische Expression in indischer Kultur kreiert."""@de;
	rdfs:subClassOf litera:Expression.

indo:Veda
	a owl:Class;
	rdfs:label "Veda"@en, "Veda"@de;
	rdfs:comment """Hindu text written in Vedic Sanskrit, in a period dated roughly from 1700 to 400 BC."""@en;
	rdfs:subClassOf indo:Expression, [
		a owl:Restriction; owl:onProperty indo:vedaHasGenre; owl:minCardinality "0"^^xsd:nonNegativeInteger], [
		a owl:Restriction; owl:onProperty indo:vedaHasGenreValue; owl:minCardinality "0"^^xsd:nonNegativeInteger], [
		a owl:Restriction; owl:onProperty indo:vedaHasRecitingStyle; owl:minCardinality "0"^^xsd:nonNegativeInteger], [
		a owl:Restriction; owl:onProperty indo:vedaHasRecitingStyleValue; owl:minCardinality "0"^^xsd:nonNegativeInteger].

indo:VedaLiterature
	a owl:Class;
	rdfs:label "Veda literature"@en, "vedische indische Literatur"@de;
	rdfs:comment """Indian literature in a Veda."""@en;
	rdfs:subClassOf indo:Literature.  # owl:oneOf (Samhita Aranyaka Brahmana Upanishad)

indo:Samhita
	a owl:Class;
	rdfs:label "Samhita"@sa, "Samhita"@en, "Samhita"@de;
	rdfs:comment """One of the four text styles, and the oldest part, in a Veda, wherein text or verses are methodically put together."""@en;
	rdfs:subClassOf indo:VedaLiterature.

indo:Patha
	a owl:Class;
	rdfs:label "pāṭha"@sa, "patha"@en, "Patha"@de;
	rdfs:comment """Style to recite or chant a Vedic mantra in the oral tradition of the Vedas, enabling its memorization."""@en;
	skos:note """There are eleven Pathas, with increasing difficulty, divided in 3 simpler or natural, and 8 complex ones."""@en; # owl:oneOf (Samhitapatha Padapatha Kramapatha Jatapatha Maalaapatha Sikhapatha Rekhapatha Dhwajapatha Dandapatha Rathaapatha Ghanapatha)
	rdfs:subClassOf knora-base:Resource.

indo:Samhitapatha
	a owl:Class;
	rdfs:label "Samhita-pāṭha"@sa, "Samhitapatha"@en, "Samhitapatha"@de;
	rdfs:comment """One of the eleven Pathas, with continuous recitation of Sanskrit words bound by the phonetic rules of euphonic combination."""@en;
	rdfs:subClassOf indo:Patha.

indo:Padapatha
	a owl:Class;
	rdfs:label "Pada-pāṭha"@sa, "Padapatha"@en, "Padapatha"@de;
	rdfs:comment """One of the eleven Pathas, with a word by word recitation, marked by a conscious pause after every word, and after any special grammatical code embedded in the text; suppresses euphonic combination and restores each word in its original intended form."""@en;
	rdfs:subClassOf indo:Patha.

#
# PROPERTIES
#

indo:hasIndologicComment
	a owl:ObjectProperty;
	rdfs:label "has Indological comment"@en, "hat indologischer Kommentar"@de;
	rdfs:comment """Relating something to an Indological comment as a textual statement about that something."""@en;
	rdfs:subPropertyOf text:hasComment;
	knora-base:subjectClassConstraint knora-base:Resource;
	knora-base:objectClassConstraint knora-base:TextValue.

indo:vedaHasGenre
	a owl:ObjectProperty;
	rdfs:label "Veda has literary genre"@en, "Veda hat literarische Gattung"@de;
	rdfs:comment """Relating a Veda to a genre it has."""@en;
	rdfs:subPropertyOf litera:hasGenre;
	knora-base:subjectClassConstraint indo:Veda;
	knora-base:objectClassConstraint indo:VedaLiterature.

indo:vedaHasGenreValue
	a owl:ObjectProperty;
	rdfs:label "Veda has literary genre - statement"@en, "Veda hat literarische Gattung - Festlegung"@de;
	rdfs:comment """Relating a Veda to a reification statement of the relation between the Veda and a genre it has."""@en;
	rdfs:subPropertyOf litera:hasGenreValue;
	knora-base:subjectClassConstraint indo:Veda;
	knora-base:objectClassConstraint knora-base:LinkValue.

indo:vedaHasRecitingStyle
	a owl:ObjectProperty;
	rdfs:label "Veda has reciting style"@en, "Veda hat Rezitationsstil"@de;
	rdfs:comment """Relating a Veda to a reciting style it has."""@en;
	rdfs:subPropertyOf knora-base:hasLinkTo;
	knora-base:subjectClassConstraint indo:Veda;
	knora-base:objectClassConstraint indo:Patha.

indo:vedaHasRecitingStyleValue
	a owl:ObjectProperty;
	rdfs:label "Veda has reciting style - statement"@en, "Veda hat Rezitationsstil - Festlegung"@de;
	rdfs:comment """Relating a Veda to a reification statement of the relation between the Veda and a reciting style it has."""@en;
	rdfs:subPropertyOf knora-base:hasLinkToValue;
	knora-base:subjectClassConstraint indo:Veda;
	knora-base:objectClassConstraint knora-base:LinkValue.