@prefix rdfs: <http://www.w3.org/2000/01/rdf-schema#>.
@prefix owl: <http://www.w3.org/2002/07/owl#>.
@prefix xsd: <http://www.w3.org/2001/XMLSchema#>.
@prefix skos: <http://www.w3.org/2004/02/skos/core#>.
@prefix dct: <http://purl.org/dc/terms/>.
@prefix foaf: <http://xmlns.com/foaf/0.1/>.
@prefix cidoc: <http://www.cidoc-crm.org/cidoc-crm/>.
@prefix frbroo: <http://iflastandards.info/ns/fr/frbr/frbroo/>.
@prefix physical: <http://www.knora.org/ontology/shared/physical-resource#>.
@prefix event: <http://www.knora.org/ontology/shared/event#>.
@prefix human: <http://www.knora.org/ontology/shared/human#>.
@prefix concept: <http://www.knora.org/ontology/shared/concept#>.
@prefix document: <http://www.knora.org/ontology/shared/document#>.
@prefix text: <http://www.knora.org/ontology/shared/text#>.
@prefix device: <http://www.knora.org/ontology/shared/device#>.
@prefix ling: <http://www.knora.org/ontology/shared/linguistics#>.
@prefix knora-base: <http://www.knora.org/ontology/knora-base#>.

@base <http://www.knora.org/ontology/shared/information-carrier>.
@prefix infocar: <http://www.knora.org/ontology/shared/information-carrier#>.

<http://www.knora.org/ontology/shared/information-carrier>
	a owl:Ontology;
	dct:title "An ontology about information carrier"@en;
	dct:description """Formal description of information carrier in broadest sense, general subclasses, related classes, and properties."""@en;
	dct:creator "Hans Cools, MD, knowledge engineer, ontologist, software developer, NIE-INE, Basel University, Switzerland"@en;
	dct:publisher "Basel University, Switzerland"@en;

	knora-base:attachedToProject <http://www.knora.org/ontology/knora-base#DefaultSharedOntologiesProject>. # <http://rdfh.ch/projects/004C>.

#
# CLASSES
#

infocar:Carrier
 	a owl:Class;
 	rdfs:label "information carrier"@en,"Informationsträger"@de, "support d'information"@fr;
 	rdfs:comment """Carrier of information created by a person."""@en;
	skos:note """Includes both F4_Manifestation_Singleton and F5_Item as declared in FRBROO."""@en;
	rdfs:subClassOf human:PhysicalCreation, cidoc:E84_Information_Carrier, [
		a owl:Restriction; owl:onProperty infocar:carrierHasDescription; owl:minCardinality "0"^^xsd:nonNegativeInteger], [
		a owl:Restriction; owl:onProperty infocar:hasSender; owl:minCardinality "0"^^xsd:nonNegativeInteger], [
		a owl:Restriction; owl:onProperty infocar:hasSenderValue; owl:minCardinality "0"^^xsd:nonNegativeInteger], [
		a owl:Restriction; owl:onProperty infocar:hasReceiver; owl:minCardinality "0"^^xsd:nonNegativeInteger], [
		a owl:Restriction; owl:onProperty infocar:hasReceiverValue; owl:minCardinality "0"^^xsd:nonNegativeInteger].

infocar:Set
	a owl:Class;
	rdfs:label "information carrier set"@en, "Informationsträger-Reihe"@de, "ensemble des supports d'information"@fr;
	rdfs:comment """Information carriers belonging together, e.g. a partitioned work, a nachlass."""@en;
	rdfs:subClassOf human:PhysicalCreation. #, [
#		a owl:Restriction; owl:onProperty infocar:hasCarrierDescription; owl:minCardinality "0"^^xsd:nonNegativeInteger].

infocar:Collection
	a owl:Class;
	rdfs:label "information carrier collection"@en, "Informationsträger-Kollektion"@de, "collection des supports d'information"@fr;
	rdfs:comment """Information carriers brought together, e.g. an archive."""@en;
	rdfs:subClassOf human:PhysicalCreation, [
		a owl:Restriction; owl:onProperty infocar:hasCarrierDescription; owl:minCardinality "0"^^xsd:nonNegativeInteger].

infocar:Copy
	a owl:Class;
	rdfs:label "information carrier copy"@en, "Informationsträgerkopie"@de;
	rdfs:comment """Carrier with a copy of information."""@en;
	rdfs:subClassOf infocar:Carrier, human:Copy.

infocar:Leaf
	a owl:Class;
	rdfs:label "leaf"@en, "Blatt"@de;
	rdfs:comment """Sheet of a writable substance, e.g. paper, parchment, treated plant leaf."""@en;
	rdfs:subClassOf infocar:Carrier, [
		a owl:Restriction; owl:onProperty infocar:isLeafOfBook; owl:minCardinality "0"^^xsd:nonNegativeInteger], [
		a owl:Restriction; owl:onProperty infocar:isLeafOfBookValue; owl:minCardinality "0"^^xsd:nonNegativeInteger].

# fold, Falte, cf. Gedicht Heinrich Heine

infocar:Page
	a owl:Class;
	rdfs:label "page"@en, "Seite"@de;
	rdfs:comment """One of the 2 surfaces of a leaf, e.g. a manuscript, or of a leaf as part of a bundled set of leafs, e.g. a book."""@en;
	rdfs:subClassOf infocar:Carrier, [
		a owl:Restriction; owl:onProperty infocar:isPageOfLeaf; owl:minCardinality "0"^^xsd:nonNegativeInteger], [
		a owl:Restriction; owl:onProperty infocar:isPageOfLeafValue; owl:minCardinality "0"^^xsd:nonNegativeInteger], [
		a owl:Restriction; owl:onProperty infocar:isPageOfBook; owl:minCardinality "0"^^xsd:nonNegativeInteger], [
		a owl:Restriction; owl:onProperty infocar:isPageOfBookValue; owl:minCardinality "0"^^xsd:nonNegativeInteger], [
		a owl:Restriction; owl:onProperty infocar:pageHasNumber; owl:minCardinality "0"^^xsd:nonNegativeInteger].

infocar:Book
	a owl:Class;
	rdfs:label "book"@en, "Buch"@de;
	rdfs:comment """Set of leafs, e.g. sheets of paper or parchment, binded together along one side, with a front and back cover."""@en;
	rdfs:subClassOf infocar:Carrier.

infocar:Binding
	a owl:Class;
	rdfs:label "binding"@en, "Einband"@de;
	rdfs:comment """Material holding the leafs and covers of a book together."""@en;
	rdfs:subClassOf infocar:Carrier, [
		a owl:Restriction; owl:onProperty infocar:isBindingOfBook; owl:minCardinality "0"^^xsd:nonNegativeInteger], [
		a owl:Restriction; owl:onProperty infocar:isBindingOfBookValue; owl:minCardinality "0"^^xsd:nonNegativeInteger].

infocar:PartitionedWork
	a owl:Class;
	rdfs:label "partitioned work"@en, "partitioniertes Werk"@de;
	rdfs:comment """Set of volumes carrying a common expression, e.g. a dictionary."""@en;
	rdfs:subClassOf infocar:Set.

infocar:Volume
	a owl:Class;
	rdfs:label "volume"@en, "Band"@de;
	rdfs:comment """One of a set of books, carrying a part of the common expression of the set."""@en;
	rdfs:subClassOf infocar:Book, [
		a owl:Restriction; owl:onProperty infocar:isVolumeOfWork; owl:minCardinality "0"^^xsd:nonNegativeInteger], [
		a owl:Restriction; owl:onProperty infocar:isVolumeOfWorkValue; owl:minCardinality "0"^^xsd:nonNegativeInteger], [		
		a owl:Restriction; owl:onProperty infocar:volumeHasNumber; owl:minCardinality "0"^^xsd:nonNegativeInteger].

infocar:Nachlass
	a owl:Class;
	rdfs:label "nachlass"@en, "Nachlass"@de;
	rdfs:comment """Set of information carriers as materialized expressions of a person as existing after the person's death and unpublished during life."""@en;
	rdfs:subClassOf infocar:Set, cidoc:E78_Collection.

infocar:NachlassElement
	a owl:Class;
	rdfs:label "nachlass element"@en, "Nachlass-Element"@de;
	rdfs:comment """Element of a nachlass."""@en;
	rdfs:subClassOf infocar:Carrier, [
		a owl:Restriction; owl:onProperty infocar:isPartOfNachlass; owl:minCardinality "0"^^xsd:nonNegativeInteger], [
		a owl:Restriction; owl:onProperty infocar:isPartOfNachlassValue; owl:minCardinality "0"^^xsd:nonNegativeInteger].

infocar:Archive
	a owl:Class;
	rdfs:label "archive"@en, "Archiv"@de, "archive"@fr, "archivio"@it;
	rdfs:comment """Set of information carriers ordered along a method."""@en;
	rdfs:subClassOf infocar:Collection, cidoc:E78_Collection.

infocar:ArchiveElement
	a owl:Class;
	rdfs:label "archive element"@en, "Archiv-Element"@de;
	rdfs:comment """Element of an archive, which can be a single file or a file group."""@en;
	rdfs:subClassOf infocar:Carrier, [
		a owl:Restriction; owl:onProperty infocar:isPartOfArchive; owl:minCardinality "0"^^xsd:nonNegativeInteger], [
		a owl:Restriction; owl:onProperty infocar:isPartOfArchiveValue; owl:minCardinality "0"^^xsd:nonNegativeInteger], [
		a owl:Restriction; owl:onProperty infocar:hasArchiveSignature; owl:minCardinality "0"^^xsd:nonNegativeInteger].

infocar:WritingUtensil
	a owl:Class;
	rdfs:label "writing utensil"@en, "Schreibzeug"@de;
	rdfs:comment """Object to write with."""@en;
	rdfs:subClassOf human:PhysicalCreation.

infocar:Pencil
	a owl:Class;
	rdfs:label "pencil"@en, "Bleistift"@de;
	rdfs:comment """Elongated cylindrical(-like) utensil for writing or drawing, containing a thin rod of graphite."""@en;
	rdfs:subClassOf infocar:WritingUtensil.

infocar:ColouredPencil
	a owl:Class;
	rdfs:label "coloured pencil"@en, "Farbstift"@de, "crayon de couleur"@en, "matita colorata"@de;
	rdfs:comment """Elongated cylindrical(-like) utensil for writing or drawing, containing a pigmented wax- or oil-based core."""@en;
	rdfs:subClassOf infocar:WritingUtensil.

infocar:Pen
	a owl:Class;
	rdfs:label "pen"@en, "Tintenstift"@de;
	rdfs:comment """Elongated cylindrical(-like) hollow object containing ink for writing or drawing."""@en;
	rdfs:subClassOf infocar:WritingUtensil.

infocar:FountainPen
	a owl:Class;
	rdfs:label "fountain pen"@en, "Füller"@de;
	rdfs:comment """Pen with refillable reservoir for fluid ink for feeding a metal nib."""@en;
	rdfs:subClassOf infocar:Pen.

infocar:Typewriter
	a owl:Class;
	rdfs:label "typewriter"@en, "Schreibmaschine"@de;
	rdfs:comment """Writing device with moving parts for letter printing."""@en; # mechanical or electronic 
	rdfs:subClassOf infocar:WritingUtensil.

infocar:Manuscript
	a owl:Class;
	rdfs:label "manuscript"@en, "Manuskript"@de;
	rdfs:comment """Carrier with a handwritten text."""@en;
	rdfs:subClassOf infocar:Carrier, frbroo:F4_Manifestation_Singleton, [
		a owl:Restriction; owl:onProperty infocar:manuscriptHasIdentifier; owl:minCardinality "0"^^xsd:nonNegativeInteger], [
		a owl:Restriction; owl:onProperty infocar:manuscriptHasIdentifierValue; owl:minCardinality "0"^^xsd:nonNegativeInteger], [
		a owl:Restriction; owl:onProperty infocar:manuscriptHasAddress; owl:minCardinality "0"^^xsd:nonNegativeInteger], [
		a owl:Restriction; owl:onProperty infocar:manuscriptHasAddressValue; owl:minCardinality "0"^^xsd:nonNegativeInteger], [
		a owl:Restriction; owl:onProperty infocar:isManuscriptOfCollection; owl:minCardinality "0"^^xsd:nonNegativeInteger], [
		a owl:Restriction; owl:onProperty infocar:isManuscriptOfCollectionValue; owl:minCardinality "0"^^xsd:nonNegativeInteger].

infocar:ManuscriptIdentifier
	a owl:Class;
	rdfs:label "manuscript identifier"@en, "Manuskript-Identifikator"@de;
	rdfs:comment """Identifier of a manuscript."""@en;
#	rdfs:seeAlso <https://www.tei-c.org/release/doc/tei-p5-doc/en/html/ref-msIdentifier.html>;
	rdfs:subClassOf concept:Identifier.

infocar:ManuscriptAddress
	a owl:Class;
	rdfs:label "manuscript address"@en, "Manuskript-Adresse"@de;
	rdfs:comment """Address of a manuscript."""@en;
#	rdfs:seeAlso <https://www.tei-c.org/release/doc/tei-p5-doc/en/html/ref-msIdentifier.html>;
	rdfs:subClassOf concept:SymbolicConcept, [
		a owl:Restriction; owl:onProperty infocar:manuscriptAddressHasLocation; owl:minCardinality "0"^^xsd:nonNegativeInteger], [
		a owl:Restriction; owl:onProperty infocar:manuscriptAddressHasLibrary; owl:minCardinality "0"^^xsd:nonNegativeInteger], [
		a owl:Restriction; owl:onProperty infocar:manuscriptAddressHasCollection; owl:minCardinality "0"^^xsd:nonNegativeInteger].
#		a owl:Restriction; owl:onProperty infocar:manuscriptAddressHasShelfMark; owl:minCardinality "0"^^xsd:nonNegativeInteger].

infocar:ManuscriptCollection
	a owl:Class;
	rdfs:label "manuscript collection"@en, "Manuskriptkollektion"@de, "collection des manuscrits"@fr;
	rdfs:comment """Collection of manuscripts."""@en;
	rdfs:subClassOf infocar:Collection.

infocar:PalmLeafManuscript
	a owl:Class;
	rdfs:label "palm-leaf manuscript"@en, "Palmblattmanuskript"@de;
	rdfs:comment """Palm leaf manuscript."""@en;
	skos:Note """Dried and smoke treated palm leaves were used as writing carrier in the Indian subcontinent and Southeast since at least the 5th century BC, possibly much earlier."""@en;
	rdfs:subClassOf infocar:Leaf, infocar:Manuscript.

infocar:NoteCarrier
	a owl:Class;
	rdfs:label "note carrier"@en,"Notizträger"@de;
	rdfs:comment """Carrier whereon notes are written, e.g. a first registration of thoughts."""@en;
	rdfs:subClassOf infocar:Carrier, frbroo:F4_Manifestation_Singleton.

infocar:Notebook
	a owl:Class;
	rdfs:label "notebook"@en,"Notizbuch"@de;
	rdfs:comment """Book wherein notes are written."""@en;
	rdfs:subClassOf infocar:Book, infocar:NoteCarrier.

infocar:Typescript
	a owl:Class;
	rdfs:label "typescript"@en, "Typoskript"@de;
	rdfs:comment """Carrier with a typewritten text."""@en;
	rdfs:subClassOf infocar:Carrier, frbroo:F4_Manifestation_Singleton.

infocar:TextCopy
	a owl:Class;
	rdfs:label "text copy"@en, "Textkopie"@de;
	rdfs:comment """Carrier with a copy of a text."""@en;
	rdfs:subClassOf infocar:Copy.

infocar:Transcript
	a owl:Class;
	rdfs:label "transcript"@en, "Transkript"@de;
#	ling:hasSynonym "Abschrift"@de;
	rdfs:comment """Text copy created by character, by any method, e.g. handwriting, typewriting, digitizing."""@en; # printing
	rdfs:subClassOf infocar:TextCopy, frbroo:F4_Manifestation_Singleton, [
		a owl:Restriction; owl:onProperty infocar:hasTranscriber; owl:minCardinality "0"^^xsd:nonNegativeInteger], [
		a owl:Restriction; owl:onProperty infocar:hasTranscriberValue; owl:minCardinality "0"^^xsd:nonNegativeInteger].

infocar:ManualTranscript
	a owl:Class;
	rdfs:label "manual transcript"@en, "manuelles Transkript"@de;
	rdfs:comment """Handwritten transcript."""@en;
	rdfs:subClassOf infocar:Transcript, infocar:Manuscript.

infocar:Printing
	a owl:Class;
	rdfs:label "printing"@en, "Drucken"@de;
	rdfs:comment """Action of putting an expression on a carrier, e.g. with ink on paper."""@en;
	rdfs:subClassOf human:Procedure, frbroo:F32_Carrier_Production_Event.

infocar:AgentPrinter
	a owl:Class;
	rdfs:label "agent printer"@en, "Agent-Drucker"@de;
	rdfs:comment """Role of a human agent, person or organization, printing an expression."""@en;
	rdfs:subClassOf human:AgentRole.

infocar:PersonPrinter
	a owl:Class;
	rdfs:label "person printer"@en, "Person-Drucker"@de;
	rdfs:comment """Role of a person printing an expression."""@en;
	rdfs:subClassOf human:PersonCreator, infocar:AgentPrinter.

infocar:Print
	a owl:Class;
	rdfs:label "print"@en, "Druck"@de;
	rdfs:comment """Something printed on a carrier."""@en;
	rdfs:subClassOf infocar:Carrier, [
		a owl:Restriction; owl:onProperty infocar:hasPrinter; owl:minCardinality "0"^^xsd:nonNegativeInteger], [
		a owl:Restriction; owl:onProperty infocar:hasPrinterValue; owl:minCardinality "0"^^xsd:nonNegativeInteger], [
		a owl:Restriction; owl:onProperty infocar:isPartOfPrintRun; owl:minCardinality "0"^^xsd:nonNegativeInteger], [
		a owl:Restriction; owl:onProperty infocar:isPartOfPrintRunValue; owl:minCardinality "0"^^xsd:nonNegativeInteger].

infocar:PrintRun
	a owl:Class;
	rdfs:label "print run"@en, "Druckauflage"@de, "Tirage"@fr, "Tiratura"@it;
	rdfs:comment """Set of prints of the same expression, created at one time."""@en;
	skos:note """When applicable, all the prints have the same ISBN, but a different bar code."""@en;
	rdfs:subClassOf infocar:Set.

infocar:FirstPrint
	a owl:Class;
	rdfs:label "first print"@en, "Erstdruck"@de;
	rdfs:comment """Earliest print of an expression."""@en;
	rdfs:subClassOf infocar:Print.

infocar:Diary
	a owl:Class;
	rdfs:label "diary"@en,"Tagebuch"@de;
	rdfs:comment """information carrier with periodically, usually daily, described personal experiences and observations."""@en;
	rdfs:subClassOf infocar:Carrier.

infocar:PersonSender
	a owl:Class;
	rdfs:label "person sender"@en, "Person-Sender"@de;
	rdfs:comment """Role of a person sending information on a carrier."""@en;
	rdfs:subClassOf human:PersonSender.

infocar:PersonReceiver
	a owl:Class;
	rdfs:label "person receiver"@en, "Person-Empfänger"@de;
	rdfs:comment """Role of a person receiving information on carrier."""@en;
	rdfs:subClassOf human:PersonReceiver.

infocar:Letter
	a owl:Class;
	rdfs:label "letter"@en, "Brief"@de, "lettre"@fr, "lettera"@it;
	rdfs:comment """Written text, e.g. on a leaf, intended to be sent from (a) person(s) or (an) Organization(s) to another one, e.g. through a postal system."""@en;
	rdfs:subClassOf infocar:Carrier, frbroo:F4_Manifestation_Singleton, [
		a owl:Restriction; owl:onProperty infocar:letterFollows; owl:minCardinality "0"^^xsd:nonNegativeInteger], [
		a owl:Restriction; owl:onProperty infocar:letterFollowsValue; owl:minCardinality "0"^^xsd:nonNegativeInteger], [
		a owl:Restriction; owl:onProperty infocar:letterPrecedes; owl:minCardinality "0"^^xsd:nonNegativeInteger], [
		a owl:Restriction; owl:onProperty infocar:letterPrecedesValue; owl:minCardinality "0"^^xsd:nonNegativeInteger].

infocar:Postcard
	a owl:Class;
	rdfs:label "postcard"@en, "Postkarte"@de, "carte postale"@fr, "cartolina"@it;
	rdfs:comment """Card with one side, usually with a printed structure, used for writing a message, an address and applying a postage stamp, to be sent through a postal system."""@en;
	rdfs:subClassOf infocar:Carrier, frbroo:F4_Manifestation_Singleton.

infocar:Convolute
	a owl:Class;
	rdfs:label "information carrier convolute"@en, "Informationsträger-Konvolut"@de;
	rdfs:comment """Set of information carriers, e.g. handwritten drafts, manuscripts, typoscripts or prints, with a commonality, e.g. being of the same author."""@en;
	rdfs:subClassOf infocar:Collection, [
		a owl:Restriction; owl:onProperty infocar:convoluteHasTitle; owl:minCardinality "0"^^xsd:nonNegativeInteger], [
		a owl:Restriction; owl:onProperty infocar:convoluteHasDescription; owl:minCardinality "0"^^xsd:nonNegativeInteger], [
		a owl:Restriction; owl:onProperty infocar:convoluteHasSizeDescription; owl:minCardinality "0"^^xsd:nonNegativeInteger], [
		a owl:Restriction; owl:onProperty infocar:convoluteHasOriginDescription; owl:minCardinality "0"^^xsd:nonNegativeInteger], [
		a owl:Restriction; owl:onProperty infocar:convoluteHasContentRepresentation; owl:minCardinality "0"^^xsd:nonNegativeInteger], [
		a owl:Restriction; owl:onProperty infocar:containsEarlierStagesOf; owl:minCardinality "0"^^xsd:nonNegativeInteger], [
		a owl:Restriction; owl:onProperty infocar:containsEarlierStagesOfValue; owl:minCardinality "0"^^xsd:nonNegativeInteger], [
		a owl:Restriction; owl:onProperty infocar:containsEarlierStagesOfPublication; owl:minCardinality "0"^^xsd:nonNegativeInteger], [
		a owl:Restriction; owl:onProperty infocar:containsEarlierStagesOfPublicationValue; owl:minCardinality "0"^^xsd:nonNegativeInteger], [
		a owl:Restriction; owl:onProperty infocar:containsLaterStagesOf; owl:minCardinality "0"^^xsd:nonNegativeInteger], [
		a owl:Restriction; owl:onProperty infocar:containsLaterStagesOfValue; owl:minCardinality "0"^^xsd:nonNegativeInteger].

infocar:ConvoluteElement
	a owl:Class;
	rdfs:label "convolute element"@en, "Konvolut-Element"@de;
	rdfs:comment """Element of an information carrier convolute."""@en;
	rdfs:subClassOf infocar:Carrier, [
		a owl:Restriction; owl:onProperty infocar:isPartOfConvolute; owl:minCardinality "0"^^xsd:nonNegativeInteger], [
		a owl:Restriction; owl:onProperty infocar:isPartOfConvoluteValue; owl:minCardinality "0"^^xsd:nonNegativeInteger].

infocar:ElectronicCarrier #° data or information storage device
	a owl:Class;
	rdfs:label "electronic information carrier"@en,"elektronischer Informationsträger"@de;
	rdfs:comment """Electronic machine carrying electronic information."""@en;
	rdfs:subClassOf device:ElectronicMachine, infocar:Carrier.

infocar:ElectronicBook
	a owl:Class;
	rdfs:label "electronic book"@en,"elektronisches Buch"@de;
	rdfs:comment """Electronic information carrier with a text structure as in a book."""@en;
	rdfs:subClassOf infocar:ElectronicCarrier.

infocar:WebPage
	a owl:Class;
	rdfs:label "web page"@en, "Webseite"@de;
	rdfs:comment """Electronic carrier page on the World Wide Web."""@en;
	skos:note """Not necessarily published, i.e. made public."""@en;
	rdfs:subClassOf infocar:ElectronicCarrier, [
		a owl:Restriction; owl:onProperty infocar:webPageHasName; owl:minCardinality "0"^^xsd:nonNegativeInteger], [
		a owl:Restriction; owl:onProperty infocar:webPageHasURL; owl:minCardinality "0"^^xsd:nonNegativeInteger].

infocar:Hyperlink # software
	a owl:Class;
	rdfs:label "hyperlink"@en,"Hyperlink"@de;
	rdfs:comment """Link from a hypertext document structure to another location, activated by clicking on a highlighted word or image."""@en;
	rdfs:subClassOf knora-base:Resource, [
		a owl:Restriction; owl:onProperty infocar:hyperlinkHasName; owl:minCardinality "0"^^xsd:nonNegativeInteger], [
		a owl:Restriction; owl:onProperty infocar:hyperlinkHasURL; owl:minCardinality "0"^^xsd:nonNegativeInteger].

#
# PROPERTIES
#

infocar:carrierHasDescription
	a owl:ObjectProperty;
	rdfs:label "has description"@en, "hat Beschreibung"@de;
	rdfs:comment """Relating an information carrier to a description thereof."""@en;
	rdfs:subPropertyOf text:hasDescription;
	knora-base:subjectClassConstraint infocar:Carrier;
	knora-base:objectClassConstraint knora-base:TextValue.

infocar:isOnCarrier
	a owl:ObjectProperty;
	rdfs:label "is on carrier"@en, "ist auf Träger"@de;
	rdfs:comment "Relating information to a carrier it is on."@en;
	rdfs:domain concept:Information;
	rdfs:range infocar:Carrier;
	rdfs:subPropertyOf knora-base:hasLinkTo;
	knora-base:subjectClassConstraint concept:Information;
	knora-base:objectClassConstraint infocar:Carrier.

infocar:isOnCarrierValue
	a owl:ObjectProperty;
	rdfs:label "is on carrier - statement"@en, "ist auf Träger - Festlegung"@de;
	rdfs:comment "Relating information to a reification statement of the relation between the information and a carrier it is on."@en;
	rdfs:subPropertyOf knora-base:hasLinkToValue;
	knora-base:subjectClassConstraint concept:Information;
	knora-base:objectClassConstraint knora-base:LinkValue.

infocar:isOnElectronicCarrier
	a owl:ObjectProperty;
	rdfs:label "is on electronic carrier"@en, "ist auf elektronischen Träger"@de;
	rdfs:comment "Relating information to an electronic carrier it is on."@en;
	rdfs:domain concept:Information;
	rdfs:range infocar:ElectronicCarrier;
	rdfs:subPropertyOf infocar:isOnCarrier;
	knora-base:subjectClassConstraint concept:Information;
	knora-base:objectClassConstraint infocar:ElectronicCarrier.

infocar:isOnElectronicCarrierValue
	a owl:ObjectProperty;
	rdfs:label "is on electronic carrier - statement"@en, "ist auf elektronischen Träger - Festlegung"@de;
	rdfs:comment "Relating information to a reification statement of the relation between the information and an electronic carrier it is on."@en;
	rdfs:subPropertyOf infocar:isOnCarrierValue;
	knora-base:subjectClassConstraint concept:Information;
	knora-base:objectClassConstraint knora-base:LinkValue.

infocar:isPageOnCarrier
	a owl:ObjectProperty;
	rdfs:label "is page on carrier"@en, "ist Seite auf Träger"@de;
	rdfs:comment """Relating a document page to a carrier page it is on."""@en;
	rdfs:domain document:Page;
	rdfs:range infocar:Page;
	rdfs:subPropertyOf infocar:isOnCarrier;
	knora-base:subjectClassConstraint document:Page;
	knora-base:objectClassConstraint infocar:Page.

infocar:isPageOnCarrierValue
	a owl:ObjectProperty;
	rdfs:label "is page on carrier - statement"@en, "ist Seite auf Träger - Festlegung"@de;
	rdfs:comment """Relating a document page to a reification statement of the relation between the page and a carrier page it is on."""@en;
	rdfs:subPropertyOf infocar:isOnCarrierValue;
	knora-base:subjectClassConstraint document:Page;
	knora-base:objectClassConstraint knora-base:LinkValue.

infocar:isTextOnPage
	a owl:ObjectProperty;
	rdfs:label "is text on page"@en, "ist Text auf Seite"@de;
	rdfs:comment """Relating a text to a carrier page it is on."""@en;
	rdfs:domain text:Text;
	rdfs:range infocar:Page;
	rdfs:subPropertyOf infocar:isOnCarrier;
	knora-base:subjectClassConstraint text:Text;
	knora-base:objectClassConstraint infocar:Page.

infocar:isTextOnPageValue
	a owl:ObjectProperty;
	rdfs:label "is text on page - statement"@en, "ist Text auf Seite - Festlegung"@de;
	rdfs:comment """Relating a text to a reification statement of the relation between the text and a carrier page it is on."""@en;
	rdfs:subPropertyOf infocar:isOnCarrierValue;
	knora-base:subjectClassConstraint text:Text;
	knora-base:objectClassConstraint knora-base:LinkValue.

infocar:isWrittenWith
	a owl:ObjectProperty;
	rdfs:label "is written with"@en, "ist geschrieben mit"@de;
	rdfs:comment "Relating a text to a utensil it is written with."@en;
	rdfs:subPropertyOf knora-base:hasLinkTo;
	knora-base:subjectClassConstraint text:WrittenText;
	knora-base:objectClassConstraint infocar:WritingUtensil.

infocar:isWrittenWithValue
	a owl:ObjectProperty;
	rdfs:label "is is written with - statement"@en, "ist geschrieben mit - Festlegung"@de;
	rdfs:comment "Relating a text to a reification statement of the relation between the text and a utensil it is written with."@en;
	rdfs:subPropertyOf knora-base:hasLinkToValue;
	knora-base:subjectClassConstraint text:WrittenText;
	knora-base:objectClassConstraint knora-base:LinkValue.

infocar:hasCarrierDescription
	a owl:ObjectProperty;
	rdfs:label "has information carrier description"@en, "hat Textträger-Beschreibung"@de;
	rdfs:comment """Relating an information carrier collection to a description of an information carrier it contains."""@en;
	rdfs:domain infocar:Collection;
	rdfs:range rdfs:Literal;
	rdfs:subPropertyOf text:hasDescription;
	knora-base:subjectClassConstraint infocar:Collection;
	knora-base:objectClassConstraint knora-base:TextValue.

infocar:isPageOfLeaf
	a owl:ObjectProperty;
	rdfs:label "is page of leaf"@en, "ist Seite eines Blattes"@de;
	rdfs:comment """Relating a page to its leaf, single or in a book."""@en;
	rdfs:domain infocar:Page;
	rdfs:range infocar:Leaf;
	rdfs:subPropertyOf physical:isPartOf;
	knora-base:subjectClassConstraint infocar:Page;
	knora-base:objectClassConstraint infocar:Leaf. # owl:disjointUnionOf (infocar:Leaf infocar:Book) # exclusive OR

infocar:isPageOfLeafValue
	a owl:ObjectProperty;
	rdfs:label "is page of leaf - statement"@en, "ist Seite eines Blattes - Festlegung"@de;
	rdfs:comment """Relating a page to a reification statement of the relation between the page and its leaf, single or in a book."""@en;
	rdfs:subPropertyOf physical:isPartOfValue;
	knora-base:subjectClassConstraint infocar:Page;
	knora-base:objectClassConstraint knora-base:LinkValue.

infocar:isPageOfBook
	a owl:ObjectProperty;
	rdfs:label "is page of book"@en, "ist Seite eines Buchs"@de;
	rdfs:comment """Relating a page to a book its leaf is part of."""@en;
	rdfs:domain infocar:Page;
	rdfs:range infocar:Book;
	rdfs:subPropertyOf physical:isPartOf; # owl:propertyChainAxiom (infocar:isPageOfLeaf infocar:isLeafOfBook)
	knora-base:subjectClassConstraint infocar:Page;
	knora-base:objectClassConstraint infocar:Book.

infocar:isPageOfBookValue
	a owl:ObjectProperty;
	rdfs:label "is page of book - statement"@en, "ist Seite eines Buchs - Festlegung"@de;
	rdfs:comment """Relating a page to a reification statement of the relation between the page and a book its leaf is part of."""@en;
	rdfs:subPropertyOf physical:isPartOfValue;
	knora-base:subjectClassConstraint infocar:Page;
	knora-base:objectClassConstraint knora-base:LinkValue.

infocar:pageHasNumber
	a owl:ObjectProperty;
	rdfs:label "page has number"@en, "Seite hat Nummer"@de;
	rdfs:comment """Relating a page to a number it has."""@en;
	rdfs:subPropertyOf knora-base:hasValue;
	knora-base:subjectClassConstraint infocar:Page;
	knora-base:objectClassConstraint knora-base:IntValue.

infocar:isLeafOfBook
	a owl:ObjectProperty;
	rdfs:label "is leaf of book"@en, "ist Blatt eines Buchs"@de;
	rdfs:comment """Relating a leaf to a book it is part of."""@en;
	rdfs:domain infocar:Leaf;
	rdfs:range infocar:Book;
	rdfs:subPropertyOf physical:isPartOf;
	knora-base:subjectClassConstraint infocar:Leaf;
	knora-base:objectClassConstraint infocar:Book.

infocar:isLeafOfBookValue
	a owl:ObjectProperty;
	rdfs:label "is leaf of book - statement"@en, "ist Blatt eines Buchs - Festlegung"@de;
	rdfs:comment """Relating a leaf to a reification statement of the relation between the leaf and a book it is part of."""@en;
	rdfs:subPropertyOf physical:isPartOfValue;
	knora-base:subjectClassConstraint infocar:Leaf;
	knora-base:objectClassConstraint knora-base:LinkValue.

infocar:isBindingOfBook
	a owl:ObjectProperty;
	rdfs:label "is binding of book"@en, "ist Einband eines Buchs"@de;
	rdfs:comment """Relating a binding to a book it is part of."""@en;
	rdfs:domain infocar:Binding;
	rdfs:range infocar:Book;
	rdfs:subPropertyOf physical:isPartOf;
	knora-base:subjectClassConstraint infocar:Binding;
	knora-base:objectClassConstraint infocar:Book.

infocar:isBindingOfBookValue
	a owl:ObjectProperty;
	rdfs:label "is binding of book - statement"@en, "ist Einband eines Buchs - Festlegung"@de;
	rdfs:comment """Relating a binding to a reification statement of the relation between the binding and a book it is part of."""@en;
	rdfs:subPropertyOf physical:isPartOfValue;
	knora-base:subjectClassConstraint infocar:Binding;
	knora-base:objectClassConstraint knora-base:LinkValue.

infocar:isVolumeOfWork
	a owl:ObjectProperty;
	rdfs:label "is volume of work"@en, "ist Band eines Werkes"@de;
	rdfs:comment """Relating a volume to a work it is part of."""@en;
	rdfs:domain infocar:Volume;
	rdfs:range infocar:PartitionedWork;
	rdfs:subPropertyOf physical:isPartOf;
	knora-base:subjectClassConstraint infocar:Volume;
	knora-base:objectClassConstraint infocar:PartitionedWork.

infocar:isVolumeOfWorkValue
	a owl:ObjectProperty;
	rdfs:label "is volume of work - statement"@en, "ist Band eines Werkes - Festlegung"@de;
	rdfs:comment """Relating a volume to a reification statement of the relation between the volume and a work it is part of."""@en;
	rdfs:subPropertyOf physical:isPartOfValue;
	knora-base:subjectClassConstraint infocar:Volume;
	knora-base:objectClassConstraint knora-base:LinkValue.

infocar:volumeHasNumber
	a owl:ObjectProperty;
	rdfs:label "volume has number"@en, "Band hat Nummer"@de;
	rdfs:comment "Relating a volume to its sequence number."@en;
	rdfs:domain infocar:Volume;
	rdfs:range xsd:nonNegativeInteger;
	rdfs:subPropertyOf knora-base:hasValue;
	knora-base:subjectClassConstraint infocar:Volume;
	knora-base:objectClassConstraint knora-base:IntValue.

infocar:isPartOfNachlass
	a owl:ObjectProperty;
	rdfs:label "is part of nachlass"@en, "ist Teil eines Nachlasses"@de;
	rdfs:comment """Relating an element of a nachlass to the nachlass."""@en;
	rdfs:domain infocar:NachlassElement;
	rdfs:range infocar:Nachlass;
	rdfs:subPropertyOf physical:isPartOf;
	knora-base:subjectClassConstraint infocar:NachlassElement;
	knora-base:objectClassConstraint infocar:Nachlass.

infocar:isPartOfNachlassValue
	a owl:ObjectProperty;
	rdfs:label "is part of nachlass - statement"@en, "ist Teil eines Nachlasses - Festlegung"@de;
	rdfs:comment """Relating an element of a nachlass to a reification statement of the relation between the element and the nachlass."""@en;
	rdfs:subPropertyOf physical:isPartOfValue;
	knora-base:subjectClassConstraint infocar:NachlassElement;
	knora-base:objectClassConstraint knora-base:LinkValue.

infocar:isPartOfArchive
	a owl:ObjectProperty;
	rdfs:label "is part of archive"@en, "ist Teil eines Archivs"@de;
	rdfs:comment """Relating an element of an archive to the archive."""@en;
	rdfs:domain infocar:ArchiveElement;
	rdfs:range infocar:Archive;
	rdfs:subPropertyOf physical:isPartOf;
	knora-base:subjectClassConstraint infocar:ArchiveElement;
	knora-base:objectClassConstraint infocar:Archive.

infocar:isPartOfArchiveValue
	a owl:ObjectProperty;
	rdfs:label "is part of archive - statement"@en, "ist Teil eines Archivs - Festlegung"@de;
	rdfs:comment """Relating an element of an archive to a reification statement of the relation between the element and the archive."""@en;
	rdfs:subPropertyOf physical:isPartOfValue;
	knora-base:subjectClassConstraint infocar:ArchiveElement;
	knora-base:objectClassConstraint knora-base:LinkValue.

infocar:hasArchiveSignature
	a owl:ObjectProperty;
	rdfs:label "has archive signature"@en, "hat Archivsignatur"@de;
	rdfs:comment """Relating an element of an archive to its signature as identifier."""@en;
	rdfs:domain infocar:ArchiveElement;
	rdfs:range rdfs:Literal;
	rdfs:subPropertyOf text:hasIdentifier;
	knora-base:subjectClassConstraint infocar:ArchiveElement;
	knora-base:objectClassConstraint knora-base:TextValue.

infocar:manuscriptHasIdentifier
	a owl:ObjectProperty;
	rdfs:label "manuscript has identifier"@en, "Manuskript hat Identifikator"@de;
	rdfs:comment """Relating a manuscript to its identifier."""@en;
	rdfs:domain infocar:Manuscript;
	rdfs:range infocar:ManuscriptIdentifier;
	rdfs:subPropertyOf knora-base:hasLinkTo;
	knora-base:subjectClassConstraint infocar:Manuscript;
	knora-base:objectClassConstraint infocar:ManuscriptIdentifier.

infocar:manuscriptHasIdentifierValue
	a owl:ObjectProperty;
	rdfs:label "manuscript has identifier - statement"@en, "Manuskript hat Identifikator - Festlegung"@de;
	rdfs:comment """Relating a manuscript to a reification statement of the relation between the manuscript and its identifier."""@en;
	rdfs:subPropertyOf knora-base:hasLinkToValue;
	knora-base:subjectClassConstraint infocar:Manuscript;
	knora-base:objectClassConstraint knora-base:LinkValue.

infocar:manuscriptHasAddress
	a owl:ObjectProperty;
	rdfs:label "manuscript has address"@en, "Manuskript hat Adresse"@de;
	rdfs:comment """Relating a manuscript to its address."""@en;
	rdfs:domain infocar:Manuscript;
	rdfs:range infocar:ManuscriptAddress;
	rdfs:subPropertyOf knora-base:hasLinkTo;
	knora-base:subjectClassConstraint infocar:Manuscript;
	knora-base:objectClassConstraint infocar:ManuscriptAddress.

infocar:manuscriptHasAddressValue
	a owl:ObjectProperty;
	rdfs:label "manuscript has address - statement"@en, "Manuskript hat Adresse - Festlegung"@de;
	rdfs:comment """Relating a manuscript to a reification statement of the relation between the manuscript and its address."""@en;
	rdfs:subPropertyOf knora-base:hasLinkToValue;
	knora-base:subjectClassConstraint infocar:Manuscript;
	knora-base:objectClassConstraint knora-base:LinkValue.

infocar:manuscriptAddressHasLocation
	a owl:ObjectProperty;
	rdfs:label "manuscript address has location"@en, "Manuskript-Adresse hat Ort"@de;
	rdfs:comment """Relating a manuscript address to its location name."""@en;
	rdfs:domain infocar:ManuscriptAddress;
	rdfs:range rdfs:Literal;
	rdfs:subPropertyOf text:hasName;
	knora-base:subjectClassConstraint infocar:ManuscriptAddress;
	knora-base:objectClassConstraint knora-base:TextValue.

infocar:manuscriptAddressHasLibrary
	a owl:ObjectProperty;
	rdfs:label "manuscript address has library"@en, "Manuskript-Adresse hat Bibliothek"@de;
	rdfs:comment """Relating a manuscript address to its library name."""@en;
	rdfs:domain infocar:ManuscriptAddress;
	rdfs:range rdfs:Literal;
	rdfs:subPropertyOf text:hasName;
	knora-base:subjectClassConstraint infocar:ManuscriptAddress;
	knora-base:objectClassConstraint knora-base:TextValue.

infocar:manuscriptAddressHasCollection
	a owl:ObjectProperty;
	rdfs:label "manuscript address has collection"@en, "Manuskript-Adresse hat Kollektion"@de;
	rdfs:comment """Relating a manuscript address to its collection name."""@en;
	rdfs:domain infocar:ManuscriptAddress;
	rdfs:range rdfs:Literal;
	rdfs:subPropertyOf text:hasName;
	knora-base:subjectClassConstraint infocar:ManuscriptAddress;
	knora-base:objectClassConstraint knora-base:TextValue.

infocar:isManuscriptOfCollection
	a owl:ObjectProperty;
	rdfs:label "is manuscript of collection"@en, "ist Manuskript einer Kollektion"@de;
	rdfs:comment "Relating a manuscript to a collection it is part of."@en;
	rdfs:domain infocar:Manuscript;
	rdfs:range infocar:ManuscriptCollection;
	rdfs:subPropertyOf physical:isPartOf;
	knora-base:subjectClassConstraint infocar:Manuscript;
	knora-base:objectClassConstraint infocar:ManuscriptCollection.

infocar:isManuscriptOfCollectionValue
	a owl:ObjectProperty;
	rdfs:label "is manuscript of collection - statement"@en, "ist Manuskript einer Kollektion - Festlegung"@de;
	rdfs:comment "Relating a manuscript to a reification statement of the relation between the manuscript and a collection it is part of."@en;
	rdfs:subPropertyOf physical:isPartOfValue;
	knora-base:subjectClassConstraint infocar:Manuscript;
	knora-base:objectClassConstraint knora-base:LinkValue.

infocar:isInManuscript
	a owl:ObjectProperty;
	rdfs:label "is in manuscript"@en, "ist in Manuskript"@de;
	rdfs:comment "Relating a handwritten text to the manuscript that carries it."@en;
	rdfs:domain text:HandwrittenText;
	rdfs:range infocar:Manuscript;
	rdfs:subPropertyOf infocar:isOnCarrier;
	knora-base:subjectClassConstraint text:HandwrittenText;
	knora-base:objectClassConstraint infocar:Manuscript.

infocar:isInManuscriptValue
	a owl:ObjectProperty;
	rdfs:label "is in manuscript - statement"@en, "ist in Manuskript - Festlegung"@de;
	rdfs:comment "Relating a handwritten text to a reification statement of the relation between the handwritten text and the manuscript that carries it."@en;
	rdfs:subPropertyOf infocar:isOnCarrierValue;
	knora-base:subjectClassConstraint text:HandwrittenText;
	knora-base:objectClassConstraint knora-base:LinkValue.

infocar:isInTypescript
	a owl:ObjectProperty;
	rdfs:label "is in typescript"@en, "ist in Typoskript"@de;
	rdfs:comment "Relating a typewritten text to the typescript that carries it."@en;
	rdfs:domain text:TypewrittenText;
	rdfs:range infocar:Typescript;
	rdfs:subPropertyOf infocar:isOnCarrier;
	knora-base:subjectClassConstraint text:TypewrittenText;
	knora-base:objectClassConstraint infocar:Typescript.

infocar:isInTypescriptValue
	a owl:ObjectProperty;
	rdfs:label "is in typescript - statement"@en, "ist in Typoskript - Festlegung"@de;
	rdfs:comment "Relating a typewritten text to a reification statement of the relation between the typewritten text and the typescript that carries it."@en;
	rdfs:subPropertyOf infocar:isOnCarrierValue;
	knora-base:subjectClassConstraint text:TypewrittenText;
	knora-base:objectClassConstraint knora-base:LinkValue.

infocar:isInTextCopy
	a owl:ObjectProperty;
	rdfs:label "is in text copy"@en, "ist in Textkopie"@de;
	rdfs:comment "Relating a copied text to its carrier."@en;
	rdfs:domain text:CopiedText;
	rdfs:range infocar:TextCopy;
	rdfs:subPropertyOf infocar:isOnCarrier;
	knora-base:subjectClassConstraint text:CopiedText;
	knora-base:objectClassConstraint infocar:TextCopy.

infocar:isInTextCopyValue
	a owl:ObjectProperty;
	rdfs:label "is in text copy - statement"@en, "ist in Textkopie - Festlegung"@de;
	rdfs:comment "Relating a copied text to a reification statement of the relation between the copied text and its carrier."@en;
	rdfs:subPropertyOf infocar:isOnCarrierValue;
	knora-base:subjectClassConstraint text:CopiedText;
	knora-base:objectClassConstraint knora-base:LinkValue.

infocar:isInTranscript
	a owl:ObjectProperty;
	rdfs:label "is in transcript"@en, "ist in Abschrift"@de;
	rdfs:comment "Relating a transcribed text to a transcript that carries it."@en;
	rdfs:domain text:TranscribedText;
	rdfs:range infocar:Transcript;
	rdfs:subPropertyOf infocar:isOnCarrier;
	knora-base:subjectClassConstraint text:TranscribedText;
	knora-base:objectClassConstraint infocar:Transcript.

infocar:isInTranscriptValue
	a owl:ObjectProperty;
	rdfs:label "is in transcript - statement"@en, "ist in Abschrift - Festlegung"@de;
	rdfs:comment "Relating a transcribed text to a reification statement of the relation between the text and the transcript that carries it."@en;
	rdfs:subPropertyOf infocar:isOnCarrierValue;
	knora-base:subjectClassConstraint text:TranscribedText;
	knora-base:objectClassConstraint knora-base:LinkValue.

infocar:isInPrint
	a owl:ObjectProperty;
	rdfs:label "is in print"@en, "ist in Druck"@de;
	rdfs:comment "Relating a printed text to a print that carries it."@en;
	rdfs:domain text:PrintedText;
	rdfs:range infocar:Print;
	rdfs:subPropertyOf infocar:isOnCarrier;
	knora-base:subjectClassConstraint text:PrintedText;
	knora-base:objectClassConstraint infocar:Print.

infocar:isInPrintValue
	a owl:ObjectProperty;
	rdfs:label "is in print - statement"@en, "ist in Druck - Festlegung"@de;
	rdfs:comment "Relating a printed text to a reification statement of the relation between the text and a print that carries it."@en;
	rdfs:subPropertyOf infocar:isOnCarrierValue;
	knora-base:subjectClassConstraint text:PrintedText;
	knora-base:objectClassConstraint knora-base:LinkValue.

infocar:entryIsInDiary
	a owl:ObjectProperty;
	rdfs:label "entry is in diary"@en, "Eintrag ist in Tagebuch"@de;
	rdfs:comment """Relating a diary entry to a diary it is in."""@en;
	rdfs:domain text:DiaryEntry;
	rdfs:range infocar:Diary;
	rdfs:subPropertyOf infocar:isOnCarrier;
	knora-base:subjectClassConstraint text:DiaryEntry;
	knora-base:objectClassConstraint infocar:Diary.

infocar:entryIsInDiaryValue
	a owl:ObjectProperty;
	rdfs:label "entry is in diary - statement"@en, "Eintrag ist in Tagebuch - Festlegung"@de;
	rdfs:comment """Relating a diary entry to a reification statement of the relation between the entry and a diary it is in."""@en;
	rdfs:subPropertyOf infocar:isOnCarrierValue;
	knora-base:subjectClassConstraint text:DiaryEntry;
	knora-base:objectClassConstraint knora-base:LinkValue.

infocar:hasDiaryEnteringDate
	a owl:ObjectProperty;
	rdfs:label "has diary entering date"@en, "hat Tagebucheintragsdatum"@de;
	rdfs:comment """Relating a diary entry to its date of entering in a diary."""@en;
	rdfs:subPropertyOf human:creationHasDate;
	knora-base:subjectClassConstraint text:DiaryEntry;
	knora-base:objectClassConstraint knora-base:DateValue.

infocar:isInDiary
	a owl:ObjectProperty;
	rdfs:label "is in diary"@en, "ist in Tagebuch"@de;
	rdfs:comment """Relating a diary expression to a diary it is in."""@en;
	rdfs:domain text:DiaryExpression;
	rdfs:range infocar:Diary;
	rdfs:subPropertyOf infocar:isOnCarrier;
	knora-base:subjectClassConstraint text:DiaryExpression;
	knora-base:objectClassConstraint infocar:Diary.

infocar:isInDiaryValue
	a owl:ObjectProperty;
	rdfs:label "is in diary - statement"@en, "ist in Tagebuch - Festlegung"@de;
	rdfs:comment """Relating a diary expression to a reification statement of the relation between the expression and a diary it is in."""@en;
	rdfs:subPropertyOf infocar:isOnCarrierValue;
	knora-base:subjectClassConstraint text:DiaryExpression;
	knora-base:objectClassConstraint knora-base:LinkValue.

infocar:isInLetter
	a owl:ObjectProperty;
	rdfs:label "is in letter"@en, "ist in Brief"@de;
	rdfs:comment """Relating a letter expression to a letter it is in."""@en;
	rdfs:domain text:LetterExpression;
	rdfs:range infocar:Letter;
	rdfs:subPropertyOf infocar:isOnCarrier;
	knora-base:subjectClassConstraint text:LetterExpression;
	knora-base:objectClassConstraint infocar:Letter.

infocar:isInLetterValue
	a owl:ObjectProperty;
	rdfs:label "is in letter - statement"@en, "ist in Brief - Festlegung"@de;
	rdfs:comment """Relating a letter expression to a reification statement of the relation between the letter expression and a letter it is in."""@en;
	rdfs:subPropertyOf infocar:isOnCarrierValue;
	knora-base:subjectClassConstraint text:LetterExpression;
	knora-base:objectClassConstraint knora-base:LinkValue.

infocar:hasSender
	a owl:ObjectProperty;
	rdfs:label "has sender"@en, "hat Absender"@de;
	rdfs:comment """Relating an information carrier to a human agent - a person or a group - that sent it."""@en;
	rdfs:domain infocar:Carrier;
#	rdfs:range [rdfs:subClassOf human:Agent, [a owl:Restriction; owl:onProperty human:agentHasRole; owl:someValuesFrom infocar:Sender]];
	rdfs:subPropertyOf physical:hasSender;
	knora-base:subjectClassConstraint infocar:Carrier;
	knora-base:objectClassConstraint human:Agent.

infocar:hasSenderValue
	a owl:ObjectProperty;
	rdfs:label "has sender - statement"@en, "hat Absender - Festlegung"@de;
	rdfs:comment """Relating an information carrier to a reification statement of the relation between that something and a human agent - a person or a group - that sent it."""@en;
	rdfs:subPropertyOf physical:hasSenderValue;
	knora-base:subjectClassConstraint infocar:Carrier;
	knora-base:objectClassConstraint knora-base:LinkValue.

infocar:hasReceiver
	a owl:ObjectProperty;
	rdfs:label "has receiver"@en, "hat Empfänger"@de;
	rdfs:comment """Relating an information carrier to a human agent - a person or a group - that received it."""@en;
	rdfs:domain infocar:Carrier;
#	rdfs:range [rdfs:subClassOf human:Agent, [a owl:Restriction; owl:onProperty human:agentHasRole; owl:someValuesFrom infocar:Receiver]];
	rdfs:subPropertyOf physical:hasReceiver;
	knora-base:subjectClassConstraint infocar:Carrier;
	knora-base:objectClassConstraint human:Agent.

infocar:hasReceiverValue
	a owl:ObjectProperty;
	rdfs:label "has receiver - statement"@en, "hat Empfänger - Festlegung"@de;
	rdfs:comment """Relating an information carrier to a reification statement of the relation between that something and a human agent - a person or a group - that received it."""@en;
	rdfs:subPropertyOf physical:hasReceiverValue;
	knora-base:subjectClassConstraint infocar:Carrier;
	knora-base:objectClassConstraint knora-base:LinkValue.

infocar:hasTranscriber
	a owl:ObjectProperty;
	rdfs:label "has transcriber"@en, "hat TranskribiererIn"@de;
	rdfs:comment """Relating a transcript to a person who created it."""@en;
	rdfs:domain infocar:Transcript;
#	rdfs:range [rdfs:subClassOf human:Person, [a owl:Restriction; owl:onProperty human:personHasRole; owl:someValuesFrom text:Transcriber]];
	rdfs:subPropertyOf human:hasCreator;
	knora-base:subjectClassConstraint infocar:Transcript;
	knora-base:objectClassConstraint human:Person.

infocar:hasTranscriberValue
	a owl:ObjectProperty;
	rdfs:label "has transcriber - statement"@en, "hat TranskribiererIn - Festlegung"@de;
	rdfs:comment """Relating a transcript to a reification statement of the relation between the transcript and a person who created it."""@en;
	rdfs:subPropertyOf human:hasCreatorValue;
	knora-base:subjectClassConstraint infocar:Transcript;
	knora-base:objectClassConstraint knora-base:LinkValue.

infocar:convoluteHasTitle
	a owl:ObjectProperty;
	rdfs:label "convolute has title"@en, "Konvolut hat Titel"@de;
	rdfs:comment """Relating a convolute to its titel."""@en;
	rdfs:subPropertyOf text:hasTitle;
	knora-base:subjectClassConstraint infocar:Convolute;
	knora-base:objectClassConstraint knora-base:TextValue.

infocar:convoluteHasDescription
	a owl:ObjectProperty;
	rdfs:label "convolute has description"@en, "Konvolut hat Beschreibung"@de;
	rdfs:comment """Relating a convolute to a description thereof."""@en;
	rdfs:subPropertyOf text:hasDescription;
	knora-base:subjectClassConstraint infocar:Convolute;
	knora-base:objectClassConstraint knora-base:TextValue.

infocar:convoluteHasSizeDescription
	a owl:ObjectProperty;
	rdfs:label "convolute has size description"@en, "Konvolutgrösse hat Beschreibung"@de;
	rdfs:comment """Relating a convolute to a description of its size."""@en;
	rdfs:subPropertyOf text:hasDescription;
	knora-base:subjectClassConstraint infocar:Convolute;
	knora-base:objectClassConstraint knora-base:TextValue.

infocar:convoluteHasOriginDescription
	a owl:ObjectProperty;
	rdfs:label "convolute has origin description"@en, "Konvolut hat Herkunftbeschreibung"@de;
	rdfs:comment """Relating a text convolute to a description of its origin."""@en;
	rdfs:subPropertyOf text:hasDescription;
	knora-base:subjectClassConstraint infocar:Convolute;
	knora-base:objectClassConstraint knora-base:TextValue.

infocar:convoluteHasContentRepresentation
	a owl:ObjectProperty;
	rdfs:label "convolute has content representation"@en, "Konvolut hat Inhaltrepräsentation"@de;
	rdfs:comment """Relating a convolute to a description of its content representation."""@en;
	rdfs:subPropertyOf text:hasDescription;
	knora-base:subjectClassConstraint infocar:Convolute;
	knora-base:objectClassConstraint knora-base:TextValue.

infocar:containsEarlierStagesOf
	a owl:ObjectProperty; # , owl:TransitiveProperty;
	rdfs:label "contains earlier stages of"@en, "enthält frühere Stufen von"@de;
	rdfs:comment """Relating a convolute to another one whose information carriers bear later stages of the texts on the carriers of the former."""@en;
	rdfs:subPropertyOf knora-base:hasLinkTo;
	knora-base:subjectClassConstraint infocar:Convolute;
	knora-base:objectClassConstraint infocar:Convolute.

infocar:containsEarlierStagesOfValue
	a owl:ObjectProperty;
	rdfs:label "contains earlier stages of - statement"@en, "enthält frühere Stufen von - Festlegung"@de;
	rdfs:comment """Relating a convolute to a reification statement of the relation between the convolute and another one whose information carriers bear later stages of the texts on the carriers of the former."""@en;
	rdfs:subPropertyOf knora-base:hasLinkToValue;
	knora-base:subjectClassConstraint infocar:Convolute;
	knora-base:objectClassConstraint knora-base:LinkValue.

infocar:containsEarlierStagesOfPublication
	a owl:ObjectProperty; # , owl:TransitiveProperty;
	rdfs:label "contains earlier stages of publication"@en, "enthält frühere Stufen von Publikation"@de;
	rdfs:comment """Relating a convolute to another one whose information carriers bear later publication stages of the texts on the carriers of the former."""@en;
	rdfs:subPropertyOf infocar:containsEarlierStagesOf;
	knora-base:subjectClassConstraint infocar:Convolute;
	knora-base:objectClassConstraint infocar:Convolute.

infocar:containsEarlierStagesOfPublicationValue
	a owl:ObjectProperty;
	rdfs:label "contains earlier stages of publication - statement"@en, "enthält frühere Stufen von Herausgabe - Festlegung"@de;
	rdfs:comment """Relating a convolute to a reification statement of the relation between the convolute and another one whose information carriers bear later publication stages of the texts on the carriers of the former."""@en;
	rdfs:subPropertyOf infocar:containsEarlierStagesOfValue;
	knora-base:subjectClassConstraint infocar:Convolute;
	knora-base:objectClassConstraint knora-base:LinkValue.

infocar:containsLaterStagesOf
	a owl:ObjectProperty; # , owl:TransitiveProperty;
	rdfs:label "contains later stages of"@en, "enthält spätere Stufen von"@de;
	rdfs:comment """Relating a convolute to another one whose information carriers bear earlier stages of the texts on the carriers of the former."""@en;
	rdfs:subPropertyOf knora-base:hasLinkTo;
	knora-base:subjectClassConstraint infocar:Convolute;
	knora-base:objectClassConstraint infocar:Convolute.

infocar:containsLaterStagesOfValue
	a owl:ObjectProperty;
	rdfs:label "contains later stages of - statement"@en, "enthält spätere Stufen von - Festlegung"@de;
	rdfs:comment """Relating a convolute to a reification statement of the relation between the convolute and another one whose information carriers bear later stages of the texts on the carriers of the former."""@en;
	rdfs:subPropertyOf knora-base:hasLinkToValue;
	knora-base:subjectClassConstraint infocar:Convolute;
	knora-base:objectClassConstraint knora-base:LinkValue.

infocar:hasPrinter
	a owl:ObjectProperty;
	rdfs:label "has printer"@en, "hat Drucker"@de;
	rdfs:comment """Relating a print to its printer."""@en;
	rdfs:domain infocar:Print;
#	rdfs:range [rdfs:subClassOf human:Agent, [a owl:Restriction; owl:onProperty human:agentHasRole; owl:someValuesFrom infocar:AgentPrinter]];
	rdfs:subPropertyOf human:hasCreator;
	knora-base:subjectClassConstraint infocar:Print;
	knora-base:objectClassConstraint human:Agent.

infocar:hasPrinterValue
	a owl:ObjectProperty;
	rdfs:label "has printer - statement"@en, "hat Drucker - Festlegung"@de;
	rdfs:comment """Relating a print to a reification statement of the relation between the print and its printer."""@en;
	rdfs:subPropertyOf human:hasCreatorValue;
	knora-base:subjectClassConstraint infocar:Print;
	knora-base:objectClassConstraint knora-base:LinkValue.

infocar:isPartOfPrintRun
	a owl:ObjectProperty;
	rdfs:label "is part of print run"@en, "ist Teil einer Druckauflage"@de;
	rdfs:comment """Relating a print to the run it is part of."""@en;
	rdfs:subPropertyOf physical:isPartOf;
	knora-base:subjectClassConstraint infocar:Print;
	knora-base:objectClassConstraint infocar:PrintRun.

infocar:isPartOfPrintRunValue
	a owl:ObjectProperty;
	rdfs:label "is part of print run - statement"@en, "ist Teil einer Druckauflage - Festlegung"@de;
	rdfs:comment """Relating a print to a reification statement of the relation between the print and the run it is part of."""@en;
	rdfs:subPropertyOf physical:isPartOfValue;
	knora-base:subjectClassConstraint infocar:Print;
	knora-base:objectClassConstraint knora-base:LinkValue.

infocar:letterFollows
	a owl:ObjectProperty;
	rdfs:label "letter follows"@en, "Brief folgt nach"@de;
	rdfs:comment """Relating a letter to another letter that precedes the former."""@en;
	rdfs:domain infocar:Letter;
	rdfs:range infocar:Letter;
	rdfs:subPropertyOf knora-base:hasLinkTo;
	knora-base:subjectClassConstraint infocar:Letter;
	knora-base:objectClassConstraint infocar:Letter.

infocar:letterFollowsValue
	a owl:ObjectProperty;
	rdfs:label "letter follows - statement"@en, "Brief folgt nach - Festlegung"@de;
	rdfs:comment """Relating a letter to a reification statement of the relation between the letter and another letter that precedes the former."""@en;
	rdfs:subPropertyOf knora-base:hasLinkToValue;
	knora-base:subjectClassConstraint infocar:Letter;
	knora-base:objectClassConstraint knora-base:LinkValue.

infocar:letterPrecedes
	a owl:ObjectProperty;
	rdfs:label "letter precedes"@en, "Brief geht voraus an"@de;
	rdfs:comment """Relating a letter to another letter that follows the former."""@en;
	rdfs:domain infocar:Letter;
	rdfs:range infocar:Letter;
	rdfs:subPropertyOf knora-base:hasLinkTo;
	knora-base:subjectClassConstraint infocar:Letter;
	knora-base:objectClassConstraint infocar:Letter.

infocar:letterPrecedesValue
	a owl:ObjectProperty;
	rdfs:label "letter precedes - statement"@en, "Brief geht voraus an - Festlegung"@de;
	rdfs:comment """Relating a letter to a reification statement of the relation between the letter and another letter that follows the former."""@en;
	rdfs:subPropertyOf knora-base:hasLinkToValue;
	knora-base:subjectClassConstraint infocar:Letter;
	knora-base:objectClassConstraint knora-base:LinkValue.

infocar:isPartOfConvolute
	a owl:ObjectProperty;
	rdfs:label "is part of convolute"@en, "ist Teil eines Konvoluts"@de;
	rdfs:comment """Relating an element of a convolute to the convolute."""@en;
	rdfs:domain infocar:ConvoluteElement;
	rdfs:range infocar:Convolute;
	rdfs:subPropertyOf physical:isPartOf;
	knora-base:subjectClassConstraint infocar:ConvoluteElement;
	knora-base:objectClassConstraint infocar:Convolute.

infocar:isPartOfConvoluteValue
	a owl:ObjectProperty;
	rdfs:label "is part of convolute - statement"@en, "ist Teil eines Konvoluts - Festlegung"@de;
	rdfs:comment """Relating an element of a convolute to a reification statement of the relation between the element and the convolute."""@en;
	rdfs:subPropertyOf physical:isPartOfValue;
	knora-base:subjectClassConstraint infocar:ConvoluteElement;
	knora-base:objectClassConstraint knora-base:LinkValue.

infocar:webPageHasName
	a owl:ObjectProperty;
	rdfs:label "web page has name"@en, "Webseite hat Name"@de;
	rdfs:comment """Relating a web page to a name it has."""@en;
	rdfs:domain infocar:WebPage;
	rdfs:range rdfs:Literal;
	rdfs:subPropertyOf text:hasName;
	knora-base:subjectClassConstraint infocar:WebPage;
	knora-base:objectClassConstraint knora-base:TextValue.

infocar:webPageHasURL
	a owl:ObjectProperty;
	rdfs:label "web page has URL"@en, "Webseite hat URL"@de;
	rdfs:comment """Relating a web page to a URL it has."""@en;
	rdfs:domain infocar:Hyperlink;
	rdfs:range xsd:anyURI;
	rdfs:subPropertyOf knora-base:hasValue;
	knora-base:subjectClassConstraint infocar:WebPage;
	knora-base:objectClassConstraint knora-base:UriValue.

infocar:hasHyperlink
	a owl:ObjectProperty;
	rdfs:label "has hyperlink"@en, "hat Hyperlink"@de;
	rdfs:comment """Relating a document structure to a hyperlink it has on an electronic carrier."""@en;
	rdfs:domain document:Structure;
	rdfs:range infocar:Hyperlink;
	rdfs:subPropertyOf knora-base:hasLinkTo;
	knora-base:subjectClassConstraint document:Structure;
	knora-base:objectClassConstraint infocar:Hyperlink.

infocar:hasHyperlinkValue
	a owl:ObjectProperty;
	rdfs:label "has hyperlink - statement"@en, "hat Hyperlink - Festlegung"@de;
	rdfs:comment """Relating document structure to a reification statement of the relation between the document structure and a hyperlink it has on an electronic carrier."""@en;
	rdfs:subPropertyOf knora-base:hasLinkToValue;
	knora-base:subjectClassConstraint document:Structure;
	knora-base:objectClassConstraint knora-base:LinkValue.

infocar:hyperlinkHasName
	a owl:ObjectProperty;
	rdfs:label "hyperlink has name"@en, "Hyperlink hat Name"@de;
	rdfs:comment """Relating a hyperlink to a name it has."""@en;
	rdfs:domain infocar:Hyperlink;
	rdfs:range rdfs:Literal;
	rdfs:subPropertyOf text:hasName;
	knora-base:subjectClassConstraint infocar:Hyperlink;
	knora-base:objectClassConstraint knora-base:TextValue.

infocar:hyperlinkHasURL
	a owl:ObjectProperty;
	rdfs:label "hyperlink has URL"@en, "Hyperlink hat URL"@de;
	rdfs:comment """Relating a hyperlink to a URL it has."""@en;
	rdfs:domain infocar:Hyperlink;
	rdfs:range xsd:anyURI;
	rdfs:subPropertyOf knora-base:hasValue;
	knora-base:subjectClassConstraint infocar:Hyperlink;
	knora-base:objectClassConstraint knora-base:UriValue.