@prefix rdfs: <http://www.w3.org/2000/01/rdf-schema#>.
@prefix owl: <http://www.w3.org/2002/07/owl#>.
@prefix xsd: <http://www.w3.org/2001/XMLSchema#>.
@prefix dct: <http://purl.org/dc/terms/>.
@prefix skos: <http://www.w3.org/2004/02/skos/core#>.
@prefix physical: <http://www.knora.org/ontology/0055/physical-resource#>.
@prefix event: <http://www.knora.org/ontology/0047/event#>.
@prefix human: <http://www.knora.org/ontology/0048/human#>.
@prefix concept: <http://www.knora.org/ontology/0044/concept#>.
@prefix language: <http://www.knora.org/ontology/004F/language#>.
@prefix document: <http://www.knora.org/ontology/005C/document#>.
@prefix text: <http://www.knora.org/ontology/0059/text#>.
@prefix text-structure: <http://www.knora.org/ontology/005B/text-structure#>.
@prefix textedit: <http://www.knora.org/ontology/005A/text-editing#>.
@prefix infocar: <http://www.knora.org/ontology/004C/information-carrier#>.
@prefix image: <http://www.knora.org/ontology/004A/image#>.
@prefix litera: <http://www.knora.org/ontology/0050/literature#>.
@prefix publish: <http://www.knora.org/ontology/0056/publishing#>.
@prefix knora-base: <http://www.knora.org/ontology/knora-base#>.

@base <http://www.knora.org/ontology/004D/kuno-raeber>.
@prefix kuno-raeber: <http://www.knora.org/ontology/004D/kuno-raeber#>.

<http://www.knora.org/ontology/004D/kuno-raeber>
	a owl:Ontology;
	dct:title "An ontology about the lyric of Kuno Raeber"@en;
	dct:description """Formal description of elements in the online publication of the lyric work of the Swiss poet Kuno Raeber."""@en;
	dct:creator "Hans Cools, MD, knowledge engineer, ontologist, software developer, NIE-INE, Basel University, Switzerland"@en;

	knora-base:attachedToProject <http://rdfh.ch/projects/004D>.

#
# CLASSES
#

kuno-raeber:Work
	a owl:Class;
	rdfs:label "Kuno Raeber work"@en, "Werk Kuno Raebers"@de;
	rdfs:comment """Work by Kuno Raeber."""@en;
	rdfs:subClassOf concept:IndividualWork.

kuno-raeber:Text
	a owl:Class;
	rdfs:label "Kuno Raeber text expression"@en, "Text-Expression Kuno Raebers"@de;
	rdfs:comment """Text expression authored by Kuno Raeber."""@en;
	rdfs:subClassOf text:IndividualExpression, [
		a owl:Restriction; owl:onProperty text:hasAlias; owl:minCardinality "0"^^xsd:nonNegativeInteger], [
		a owl:Restriction; owl:onProperty text:hasDetailDescription; owl:minCardinality "0"^^xsd:nonNegativeInteger], [
		a owl:Restriction; owl:onProperty text:hasSpecialDescription; owl:minCardinality "0"^^xsd:nonNegativeInteger], [
#		a owl:Restriction; owl:onProperty kuno-raeber:isFinalVersion; owl:minCardinality "0"^^xsd:nonNegativeInteger], [
		a owl:Restriction; owl:onProperty kuno-raeber:isInSwissGerman; owl:minCardinality "0"^^xsd:nonNegativeInteger], [
		a owl:Restriction; owl:onProperty kuno-raeber:isPartOfCycle; owl:minCardinality "0"^^xsd:nonNegativeInteger], [
		a owl:Restriction; owl:onProperty knora-base:seqnum; owl:minCardinality "0"^^xsd:nonNegativeInteger].

kuno-raeber:Prologue
	a owl:Class;
	rdfs:label "Kuno Raeber prologue"@en, "Vorwort Kuno Raebers"@de;
	rdfs:comment """Prologue authored by Kuno Raeber."""@en;
	rdfs:subClassOf text-structure:Prologue, text:Nonfiction, kuno-raeber:Text.

kuno-raeber:Epilogue
	a owl:Class;
	rdfs:label "Kuno Raeber epilogue"@en, "Nachwort Kuno Raebers"@de;
	rdfs:comment """Epilogue authored by Kuno Raeber."""@en;
	rdfs:subClassOf text-structure:Epilogue, text:Nonfiction, kuno-raeber:Text.

kuno-raeber:Poem
	a owl:Class;
	rdfs:label "Kuno Raeber poem"@en, "Gedicht Kuno Raebers"@de;
	rdfs:comment """Poem authored by Kuno Raeber."""@en;
	rdfs:subClassOf litera:Poem, kuno-raeber:Text, [
		a owl:Restriction; owl:onProperty kuno-raeber:poemHasTitle; owl:minCardinality "0"^^xsd:nonNegativeInteger], [
		a owl:Restriction; owl:onProperty kuno-raeber:hasSameEditionAsIn; owl:minCardinality "0"^^xsd:nonNegativeInteger], [
		a owl:Restriction; owl:onProperty kuno-raeber:hasSameEditionAsInValue; owl:minCardinality "0"^^xsd:nonNegativeInteger], [
		a owl:Restriction; owl:onProperty kuno-raeber:hasReferencePoem; owl:minCardinality "0"^^xsd:nonNegativeInteger], [
		a owl:Restriction; owl:onProperty kuno-raeber:hasReferencePoemValue; owl:minCardinality "0"^^xsd:nonNegativeInteger], [
		a owl:Restriction; owl:onProperty kuno-raeber:hasReferenceTitle; owl:minCardinality "0"^^xsd:nonNegativeInteger], [
		a owl:Restriction; owl:onProperty kuno-raeber:hasStrophe; owl:minCardinality "0"^^xsd:nonNegativeInteger].

kuno-raeber:ScientificEdition
	a owl:Class;
	rdfs:label "Kuno Raeber text scientific edition"@en, "wissenschaftliche Edition eines Kuno Raeber Textes"@de;
	rdfs:comment """Scientific edition of a text authored by Kuno Raeber."""@en, """Wissenschaftliche Edition eines von Kuno Raeber verfassten Texts."""@de;
	rdfs:subClassOf textedit:ScientificEdition, [
		a owl:Restriction; owl:onProperty language:hasContent; owl:minCardinality "0"^^xsd:nonNegativeInteger], [
		a owl:Restriction; owl:onProperty kuno-raeber:hasPageIndicator; owl:minCardinality "0"^^xsd:nonNegativeInteger], [
		a owl:Restriction; owl:onProperty kuno-raeber:hasPageNumberIndicator; owl:minCardinality "0"^^xsd:nonNegativeInteger], [
		a owl:Restriction; owl:onProperty kuno-raeber:hasColumnIndicator; owl:minCardinality "0"^^xsd:nonNegativeInteger].

kuno-raeber:DiplomaticTranscription
	a owl:Class;
	rdfs:label "Kuno Raeber text diplomatic transcription"@en, "diplomatische Umschrift eines Kuno Raeber Textes"@de;
	rdfs:comment """Diplomatic transcription of a text authored by Kuno Raeber."""@en, """Diplomatische Umschrift eines von Kuno Raeber verfassten Texts."""@de;
	rdfs:subClassOf textedit:DiplomaticTranscription, [
		a owl:Restriction; owl:onProperty language:hasContent; owl:minCardinality "0"^^xsd:nonNegativeInteger], [ # needed due to restriction in dhl-knora
		a owl:Restriction; owl:onProperty knora-base:seqnum; owl:minCardinality "0"^^xsd:nonNegativeInteger].

kuno-raeber:HandwrittenPoem
	a owl:Class;
	rdfs:label "Kuno Raeber handwritten poem"@en, "handgeschriebenes Gedicht Kuno Raebers"@de;
	rdfs:comment """Handwritten poem authored by Kuno Raeber."""@en, """Handgeschriebenes Gedicht Kuno Raebers."""@de;
	rdfs:subClassOf kuno-raeber:Poem, text:HandwrittenText, [
		a owl:Restriction; owl:onProperty kuno-raeber:isOnPage; owl:minCardinality "0"^^xsd:nonNegativeInteger], [
		a owl:Restriction; owl:onProperty kuno-raeber:isOnPageValue; owl:minCardinality "0"^^xsd:nonNegativeInteger].

kuno-raeber:PoemNote
	a owl:Class;
	rdfs:label "Kuno Raeber poem note"@en, "Gedichtnotiz Kuno Raebers"@de;
	rdfs:comment """Poem note authored by Kuno Raeber."""@en, """Gedichtnotiz Kuno Raebers."""@de;
	rdfs:subClassOf kuno-raeber:HandwrittenPoem, human:FirstVersion, [
		a owl:Restriction; owl:onProperty kuno-raeber:isInNotebook; owl:minCardinality "0"^^xsd:nonNegativeInteger], [
		a owl:Restriction; owl:onProperty kuno-raeber:isInNotebookValue; owl:minCardinality "0"^^xsd:nonNegativeInteger].

kuno-raeber:PostcardPoem
	a owl:Class;
	rdfs:label "Kuno Raeber postcard poem"@en, "Postkarten-Gedicht Kuno Raebers"@de;
	rdfs:comment """Postcard poem authored by Kuno Raeber."""@en, """Postkarten-Gedicht Kuno Raebers."""@de;
	rdfs:subClassOf kuno-raeber:HandwrittenPoem, [
		a owl:Restriction; owl:onProperty kuno-raeber:isOnPostcard; owl:minCardinality "0"^^xsd:nonNegativeInteger], [
		a owl:Restriction; owl:onProperty kuno-raeber:isOnPostcardValue; owl:minCardinality "0"^^xsd:nonNegativeInteger], [
		a owl:Restriction; owl:onProperty publish:hasNachlassPublicationDescription; owl:minCardinality "0"^^xsd:nonNegativeInteger].

kuno-raeber:TypewrittenPoem
	a owl:Class;
	rdfs:label "Kuno Raeber typewritten poem"@en, "maschinengeschriebenes Gedicht Kuno Raebers"@de;
	rdfs:comment """Typewritten poem authored by Kuno Raeber."""@en, """Maschinengeschriebenes Gedicht Kuno Raebers."""@de;
	rdfs:subClassOf kuno-raeber:Poem, text:TypewrittenText.

kuno-raeber:PublicationPoem
	a owl:Class;
	rdfs:label "Kuno Raeber publication poem"@en, "Publikation-Gedicht Kuno Raebers"@de;
	rdfs:comment """Poem authored by Kuno Raeber, as published."""@en, """Gedicht Kuno Raebers wie publiziert."""@de;
	rdfs:subClassOf kuno-raeber:Poem, publish:Expression, [
		a owl:Restriction; owl:onProperty kuno-raeber:isInPolyAuthorPublicationConvolute; owl:minCardinality "0"^^xsd:nonNegativeInteger], [
		a owl:Restriction; owl:onProperty kuno-raeber:isInPolyAuthorPublicationConvoluteValue; owl:minCardinality "0"^^xsd:nonNegativeInteger].

kuno-raeber:DiaryEntry
	a owl:Class;
	rdfs:label "Kuno Raeber diary entry"@en, "Tagebucheintrag Kuno Raebers"@de;
	rdfs:comment """Diary entry authored by Kuno Raeber."""@en;
	rdfs:subClassOf text:DiaryEntry, kuno-raeber:Text, [
		a owl:Restriction; owl:onProperty kuno-raeber:isInDiary; owl:minCardinality "0"^^xsd:nonNegativeInteger], [
		a owl:Restriction; owl:onProperty kuno-raeber:isInDiaryValue; owl:minCardinality "0"^^xsd:nonNegativeInteger], [
		a owl:Restriction; owl:onProperty kuno-raeber:isInDiaryConvolute; owl:minCardinality "0"^^xsd:nonNegativeInteger], [
		a owl:Restriction; owl:onProperty kuno-raeber:isInDiaryConvoluteValue; owl:minCardinality "0"^^xsd:nonNegativeInteger].

kuno-raeber:LetterExpression
	a owl:Class;
	rdfs:label "Kuno Raeber letter expression"@en, "Brief-Expression Kuno Raebers"@de;
	rdfs:comment """Letter expression written by Kuno Raeber."""@en;
	rdfs:subClassOf text:LetterExpression, text:WrittenText, kuno-raeber:Text, [
		a owl:Restriction; owl:onProperty text:hasSpecialDescription; owl:minCardinality "0"^^xsd:nonNegativeInteger].

kuno-raeber:Page
	a owl:Class;
	rdfs:label "Kuno Raeber page"@en, "Seite Kuno Raebers"@de;
	rdfs:comment """Page with a handwritten poem by Kuno Raeber."""@en, """Seite mit einem handgeschriebenen Gedicht Kuno Raebers."""@de;
	rdfs:subClassOf infocar:Page, [
		a owl:Restriction; owl:onProperty knora-base:hasRepresentation; owl:minCardinality "0"^^xsd:nonNegativeInteger].

kuno-raeber:Convolute
	a owl:Class;
	rdfs:label "Kuno Raeber convolute"@en, "Konvolut Kuno Raebers"@de;
	rdfs:comment """Convolute of which the elements are authored by Kuno Raeber."""@en;
	rdfs:subClassOf infocar:Convolute, [
		a owl:Restriction; owl:onProperty text:hasComment; owl:minCardinality "0"^^xsd:nonNegativeInteger].

kuno-raeber:PoemNotebook
	a owl:Class;
	rdfs:label "Kuno Raeber poem notebook"@en, "Gedichten-Notizbuch Kuno Raebers"@de;
	rdfs:comment """Notebook with poem drafts authored by Kuno Raeber."""@en;
	rdfs:subClassOf infocar:Manuscript, infocar:Notebook, kuno-raeber:Convolute, infocar:ArchiveElement, [
		a owl:Restriction; owl:onProperty knora-base:hasRepresentation; owl:minCardinality "0"^^xsd:nonNegativeInteger], [
		a owl:Restriction; owl:onProperty kuno-raeber:containsEarlierStagesOfManuscriptConvolute; owl:minCardinality "0"^^xsd:nonNegativeInteger], [
		a owl:Restriction; owl:onProperty kuno-raeber:containsEarlierStagesOfManuscriptConvoluteValue; owl:minCardinality "0"^^xsd:nonNegativeInteger], [
		a owl:Restriction; owl:onProperty kuno-raeber:containsEarlierStagesOfTypescriptConvolute; owl:minCardinality "0"^^xsd:nonNegativeInteger], [
		a owl:Restriction; owl:onProperty kuno-raeber:containsEarlierStagesOfTypescriptConvoluteValue; owl:minCardinality "0"^^xsd:nonNegativeInteger].

kuno-raeber:Manuscript
	a owl:Class;
	rdfs:label "Kuno Raeber manuscript"@en, "Manuskript Kuno Raebers"@de;
	rdfs:comment """Manuscript authored by Kuno Raeber."""@en;
	rdfs:subClassOf infocar:Leaf, infocar:Manuscript, infocar:ConvoluteElement, infocar:ArchiveElement, [
		a owl:Restriction; owl:onProperty kuno-raeber:isPartOfManuscriptConvolute; owl:minCardinality "0"^^xsd:nonNegativeInteger], [
		a owl:Restriction; owl:onProperty kuno-raeber:isPartOfManuscriptConvoluteValue; owl:minCardinality "0"^^xsd:nonNegativeInteger].

kuno-raeber:PoemManuscript
	a owl:Class;
	rdfs:label "Kuno Raeber poem manuscript"@en, "Gedicht-Manuskript Kuno Raebers"@de;
	rdfs:comment """Manuscript with a poem authored by Kuno Raeber."""@en;
	rdfs:subClassOf kuno-raeber:Manuscript.

kuno-raeber:ManuscriptConvolute
	a owl:Class;
	rdfs:label "Kuno Raeber poem manuscript convolute"@en, "Gedicht-Manuskriptenkonvolut Kuno Raebers"@de;
	rdfs:comment """Poem manuscript convolute with poems authored by Kuno Raeber."""@en;
	rdfs:subClassOf kuno-raeber:Convolute, infocar:ArchiveElement, [
		a owl:Restriction; owl:onProperty kuno-raeber:containsLaterStagesOfNotebook; owl:minCardinality "0"^^xsd:nonNegativeInteger], [
		a owl:Restriction; owl:onProperty kuno-raeber:containsLaterStagesOfNotebookValue; owl:minCardinality "0"^^xsd:nonNegativeInteger], [	
		a owl:Restriction; owl:onProperty kuno-raeber:containsEarlierStagesOfTypescriptConvolute; owl:minCardinality "0"^^xsd:nonNegativeInteger], [
		a owl:Restriction; owl:onProperty kuno-raeber:containsEarlierStagesOfTypescriptConvoluteValue; owl:minCardinality "0"^^xsd:nonNegativeInteger].

kuno-raeber:PoemPostcard
	a owl:Class;
	rdfs:label "Kuno Raeber poem postcard"@en, "Gedicht-Postkarte Kuno Raebers"@de;
	rdfs:comment """Postcard with a poem authored by Kuno Raeber."""@en;
	rdfs:subClassOf infocar:Manuscript, infocar:Postcard, infocar:ArchiveElement, infocar:ConvoluteElement, [
		a owl:Restriction; owl:onProperty kuno-raeber:isPartOfPostcardConvolute; owl:minCardinality "0"^^xsd:nonNegativeInteger], [
		a owl:Restriction; owl:onProperty kuno-raeber:isPartOfPostcardConvoluteValue; owl:minCardinality "0"^^xsd:nonNegativeInteger], [
		a owl:Restriction; owl:onProperty knora-base:hasRepresentation; owl:minCardinality "0"^^xsd:nonNegativeInteger].

kuno-raeber:PoemPostcardConvolute
	a owl:Class;
	rdfs:label "Kuno Raeber poem postcard convolute"@en, "Gedicht-Postkartenkonvolut Kuno Raebers"@de;
	rdfs:comment """Poem postcard convolute with poems authored by Kuno Raeber."""@en;
	rdfs:subClassOf kuno-raeber:Convolute, [
		a owl:Restriction; owl:onProperty knora-base:hasRepresentation; owl:minCardinality "0"^^xsd:nonNegativeInteger], [
		a owl:Restriction; owl:onProperty kuno-raeber:containsLaterStagesOfNotebook; owl:minCardinality "0"^^xsd:nonNegativeInteger], [
		a owl:Restriction; owl:onProperty kuno-raeber:containsLaterStagesOfNotebookValue; owl:minCardinality "0"^^xsd:nonNegativeInteger].

kuno-raeber:Typescript
	a owl:Class;
	rdfs:label "Kuno Raeber typescript"@en, "Typoskript Kuno Raebers"@de;
	rdfs:comment """Typescript by Kuno Raeber."""@en;
	rdfs:subClassOf infocar:Leaf, infocar:Typescript, infocar:ConvoluteElement, infocar:ArchiveElement, [
		a owl:Restriction; owl:onProperty kuno-raeber:isPartOfTypescriptConvolute; owl:minCardinality "0"^^xsd:nonNegativeInteger], [
		a owl:Restriction; owl:onProperty kuno-raeber:isPartOfTypescriptConvoluteValue; owl:minCardinality "0"^^xsd:nonNegativeInteger].

kuno-raeber:PoemTypescript
	a owl:Class;
	rdfs:label "Kuno Raeber poem typescript"@en, "Gedicht-Typoskript Kuno Raebers"@de;
	rdfs:comment """Poem typescript by Kuno Raeber."""@en;
	rdfs:subClassOf kuno-raeber:Typescript.

kuno-raeber:TypescriptConvolute
	a owl:Class;
	rdfs:label "Kuno Raeber typescript convolute"@en, "Typoskriptenonvolut Kuno Raebers"@de;
	rdfs:comment """Typescript convolute with poems authored by Kuno Raeber."""@en;
	rdfs:subClassOf kuno-raeber:Convolute, infocar:ArchiveElement, [
		a owl:Restriction; owl:onProperty kuno-raeber:containsLaterStagesOfNotebook; owl:minCardinality "0"^^xsd:nonNegativeInteger], [
		a owl:Restriction; owl:onProperty kuno-raeber:containsLaterStagesOfNotebookValue; owl:minCardinality "0"^^xsd:nonNegativeInteger], [
		a owl:Restriction; owl:onProperty kuno-raeber:containsLaterStagesOfManuscriptConvolute; owl:minCardinality "0"^^xsd:nonNegativeInteger], [
		a owl:Restriction; owl:onProperty kuno-raeber:containsLaterStagesOfManuscriptConvoluteValue; owl:minCardinality "0"^^xsd:nonNegativeInteger].

kuno-raeber:TypescriptConvoluteWithImage # to be removed when knora-base:hasRepresentation will be implemented in Knora
	a owl:Class;
	rdfs:label "Kuno Raeber poem typescript convolute with image"@en, "Gedicht-Typoskriptenonvolut mit Bild Kuno Raebers"@de;
	rdfs:comment """Poem typescript convolute with poems authored by Kuno Raeber, mit bild."""@en;
	rdfs:subClassOf kuno-raeber:TypescriptConvolute, [
		a owl:Restriction; owl:onProperty knora-base:hasRepresentation; owl:minCardinality "0"^^xsd:nonNegativeInteger].

kuno-raeber:PrintedPoemBookPublication
	a owl:Class;
	rdfs:label "Kuno Raeber printed poem book publication"@en, "gedruckte Gedichtenbuchausgabe Kuno Raebers"@de;
	rdfs:comment """Printed publication of a book  with poems authored by Kuno Raeber."""@en;
	rdfs:subClassOf infocar:Book, publish:PrintedPublication, kuno-raeber:Convolute, [
		a owl:Restriction; owl:onProperty knora-base:hasRepresentation; owl:minCardinality "0"^^xsd:nonNegativeInteger], [
		a owl:Restriction; owl:onProperty kuno-raeber:containsLaterStagesOfNotebook; owl:minCardinality "0"^^xsd:nonNegativeInteger], [
		a owl:Restriction; owl:onProperty kuno-raeber:containsLaterStagesOfNotebookValue; owl:minCardinality "0"^^xsd:nonNegativeInteger], [
		a owl:Restriction; owl:onProperty kuno-raeber:containsLaterStagesOfManuscriptConvolute; owl:minCardinality "0"^^xsd:nonNegativeInteger], [
		a owl:Restriction; owl:onProperty kuno-raeber:containsLaterStagesOfManuscriptConvoluteValue; owl:minCardinality "0"^^xsd:nonNegativeInteger], [
		a owl:Restriction; owl:onProperty kuno-raeber:containsLaterStagesOfTypescriptConvolute; owl:minCardinality "0"^^xsd:nonNegativeInteger], [
		a owl:Restriction; owl:onProperty kuno-raeber:containsLaterStagesOfTypescriptConvoluteValue; owl:minCardinality "0"^^xsd:nonNegativeInteger].

kuno-raeber:PolyAuthorPublication
	a owl:Class;
	rdfs:label "Kuno Raeber poly-author publication"@en, "Mehrautorenpublikationen Kuno Raebers"@de;
	rdfs:comment """Publication with a poem authored by Kuno Raeber among expressions by other authors."""@en;
	rdfs:subClassOf publish:PolyAuthorPublication, [
		a owl:Restriction; owl:onProperty kuno-raeber:hasContentPartInPolyAuthorPublicationConvolute; owl:minCardinality "0"^^xsd:nonNegativeInteger], [
		a owl:Restriction; owl:onProperty kuno-raeber:hasContentPartInPolyAuthorPublicationConvoluteValue; owl:minCardinality "0"^^xsd:nonNegativeInteger].

kuno-raeber:PolyAuthorPublicationConvolute
	a owl:Class;
	rdfs:label "Kuno Raeber poly-author publication convolute"@en, "Mehrautorenpublikationen-Konvolut Kuno Raebers"@de;
	rdfs:comment """Convolute of poems authored by Kuno Raeber as published among expressions by other authors."""@en;
	rdfs:subClassOf kuno-raeber:Convolute.

kuno-raeber:Diary
	a owl:Class;
	rdfs:label "Kuno Raeber diary"@en,"Tagebuch Kuno Raebers"@de;
	rdfs:comment """Diary with entries authored by Kuno Raeber."""@en;
	skos:note """Different from kuno-raeber:DiaryConvolute - in contrast to kuno-raeber:PoemNotebook - because only selections from different diaries are published online."""@en;
	rdfs:subClassOf infocar:Diary, infocar:Manuscript, infocar:Book, infocar:ArchiveElement.

kuno-raeber:DiaryConvolute
	a owl:Class;
	rdfs:label "Kuno Raeber diary convolute"@en,"Tagebuch-Konvolut Kuno Raebers"@de;
	rdfs:comment """Convolute of diaries with entries authored by Kuno Raeber."""@en;
	rdfs:subClassOf kuno-raeber:Convolute, infocar:ArchiveElement.

kuno-raeber:Letter
	a owl:Class;
	rdfs:label "Kuno Raeber letter"@en,"Brief Kuno Raebers"@de;
	rdfs:comment """Letter written by or to Kuno Raeber."""@en;
	rdfs:subClassOf infocar:Letter, infocar:ArchiveElement, [
		a owl:Restriction; owl:onProperty kuno-raeber:isPartOfLetterConvolute; owl:minCardinality "0"^^xsd:nonNegativeInteger], [
		a owl:Restriction; owl:onProperty kuno-raeber:isPartOfLetterConvoluteValue; owl:minCardinality "0"^^xsd:nonNegativeInteger].

kuno-raeber:LetterConvolute
	a owl:Class;
	rdfs:label "Kuno Raeber letter convolute"@en,"Briefekonvolut Kuno Raebers"@de;
	rdfs:comment """Convolute of letters written by and to Kuno Raeber."""@en;
	rdfs:subClassOf kuno-raeber:Convolute, infocar:ArchiveElement.

kuno-raeber:NachlassPublication
	a owl:Class;
	rdfs:label "Kuno Raeber nachlass publication"@en, "Nachlass-Publication Kuno Raebers"@de;
	rdfs:comment """Publication of a Nachlass of Kuno Raeber."""@en;
	rdfs:subClassOf publish:NachlassPublication, infocar:Volume, publish:PrintedPublication.

#
# PROPERTIES
#

kuno-raeber:poemHasTitle
	a owl:ObjectProperty;
	rdfs:label "poem has title"@en, "Gedicht hat Titel"@de;
	rdfs:comment """Relating a poem by Kuno Raeber to a title it has."""@en;
	rdfs:domain kuno-raeber:Poem;
	rdfs:range knora-base:TextValue;
	rdfs:subPropertyOf text:expressionHasTitle;
	knora-base:subjectClassConstraint kuno-raeber:Poem;
	knora-base:objectClassConstraint knora-base:TextValue.

kuno-raeber:hasPageIndicator
	a owl:ObjectProperty;
	rdfs:label "has page indicator"@en, "hat Seite-Indikator"@de;
	rdfs:comment """Relating a derived text expression by Kuno Raeber to a diacritical sign that indicates where a page starts."""@en;
	rdfs:domain kuno-raeber:ScientificEdition;
	rdfs:range knora-base:TextValue;
	rdfs:subPropertyOf knora-base:hasValue;
	knora-base:subjectClassConstraint kuno-raeber:ScientificEdition;
	knora-base:objectClassConstraint knora-base:TextValue.

kuno-raeber:hasPageNumberIndicator
	a owl:ObjectProperty;
	rdfs:label "has page number indicator"@en, "hat Seitennummer-Indikator"@de;
	rdfs:comment """Relating a derived text expression by Kuno Raeber to a diacritical sign that indicates the number of a page."""@en;
	rdfs:domain kuno-raeber:ScientificEdition;
	rdfs:range knora-base:TextValue;
	rdfs:subPropertyOf knora-base:hasValue;
	knora-base:subjectClassConstraint kuno-raeber:ScientificEdition;
	knora-base:objectClassConstraint knora-base:TextValue.

kuno-raeber:hasColumnIndicator
	a owl:ObjectProperty;
	rdfs:label "has column indicator"@en, "hat Spalte-Indikator"@de;
	rdfs:comment """Relating a derived text expression by Kuno Raeber to a diacritical sign that indicates where on a page a column starts."""@en;
	rdfs:domain kuno-raeber:ScientificEdition;
	rdfs:range knora-base:TextValue;
	rdfs:subPropertyOf knora-base:hasValue;
	knora-base:subjectClassConstraint kuno-raeber:ScientificEdition;
	knora-base:objectClassConstraint knora-base:TextValue.

kuno-raeber:isOnPage # to be removed when knora-base:hasRepresentation will be implemented in Knora
	a owl:ObjectProperty;
	rdfs:label "is on page"@en, "ist auf Seite"@de;
	rdfs:comment """Relating a handwritten poem by Kuno Raeber to a carrier page it is on."""@en;
	rdfs:domain kuno-raeber:HandwrittenPoem;
	rdfs:range kuno-raeber:Page;
	rdfs:subPropertyOf infocar:isTextOnPage;
	knora-base:subjectClassConstraint kuno-raeber:HandwrittenPoem;
	knora-base:objectClassConstraint kuno-raeber:Page.

kuno-raeber:isOnPageValue # to be removed when knora-base:hasRepresentation will be implemented in Knora
	a owl:ObjectProperty;
	rdfs:label "is on page - statement"@en, "ist auf Seite - Festlegung"@de;
	rdfs:comment """Relating a handwritten poem by Kuno Raeber to a reification statement of the relation between the poem and a carrier page it is on."""@en;
	rdfs:subPropertyOf infocar:isTextOnPageValue;
	knora-base:subjectClassConstraint kuno-raeber:HandwrittenPoem;
	knora-base:objectClassConstraint knora-base:LinkValue.

kuno-raeber:isInNotebook
	a owl:ObjectProperty;
	rdfs:label "is in notebook"@en, "ist in Notizbuch"@de;
	rdfs:comment """Relating a poem note by Kuno Raeber to a notebook it is in."""@en;
	rdfs:domain kuno-raeber:PoemNote;
	rdfs:range kuno-raeber:PoemNotebook;
	rdfs:subPropertyOf infocar:isInManuscript;
	knora-base:subjectClassConstraint kuno-raeber:PoemNote;
	knora-base:objectClassConstraint kuno-raeber:PoemNotebook.

kuno-raeber:isInNotebookValue
	a owl:ObjectProperty;
	rdfs:label "is in notebook - statement"@en, "ist in Notizbuch - Festlegung"@de;
	rdfs:comment """Relating a poem note by Kuno Raeber to a reification statement of the relation between the poem note and a notebook it is in."""@en;
	rdfs:subPropertyOf infocar:isInManuscriptValue;
	knora-base:subjectClassConstraint kuno-raeber:PoemNote;
	knora-base:objectClassConstraint knora-base:LinkValue.

kuno-raeber:isOnPostcard
	a owl:ObjectProperty;
	rdfs:label "is on postcard"@en, "ist auf Postkarte"@de;
	rdfs:comment """Relating a poem by Kuno Raeber to a postcard it is on."""@en;
	rdfs:domain kuno-raeber:PostcardPoem;
	rdfs:range kuno-raeber:PoemPostcard;
	rdfs:subPropertyOf infocar:isInManuscript;
	knora-base:subjectClassConstraint kuno-raeber:PostcardPoem;
	knora-base:objectClassConstraint kuno-raeber:PoemPostcard.

kuno-raeber:isOnPostcardValue
	a owl:ObjectProperty;
	rdfs:label "is on postcard - statement"@en, "ist auf Postkarte - Festlegung"@de;
	rdfs:comment """Relating a poem by Kuno Raeber to a reification statement of the relation between the poem and a postcard it is on."""@en;
	rdfs:subPropertyOf infocar:isInManuscriptValue;
	knora-base:subjectClassConstraint kuno-raeber:PostcardPoem;
	knora-base:objectClassConstraint knora-base:LinkValue.

kuno-raeber:isInPolyAuthorPublicationConvolute
	a owl:ObjectProperty;
	rdfs:label "is in poly-author publication convolute"@en, "ist in Mehrautorenpublikationen-Konvolut"@de;
	rdfs:comment """Relating a publication poem by Kuno Raeber to a poly-author publication it is in."""@en;
	rdfs:domain kuno-raeber:PublicationPoem;
	rdfs:range kuno-raeber:PolyAuthorPublicationConvolute;
	rdfs:subPropertyOf knora-base:hasLinkTo;
	knora-base:subjectClassConstraint kuno-raeber:PublicationPoem;
	knora-base:objectClassConstraint kuno-raeber:PolyAuthorPublicationConvolute.

kuno-raeber:isInPolyAuthorPublicationConvoluteValue
	a owl:ObjectProperty;
	rdfs:label "is in poly-author publication convolute - statement"@en, "ist in Mehrautorenpublikationen-Konvolut - Festlegung"@de;
	rdfs:comment """Relating a publication poem by Kuno Raeber to a reification statement of the relation between the poem and a poly-author publication it is in."""@en;
	rdfs:subPropertyOf knora-base:hasLinkToValue;
	knora-base:subjectClassConstraint kuno-raeber:PublicationPoem;
	knora-base:objectClassConstraint knora-base:LinkValue.

kuno-raeber:isPartOfManuscriptConvolute
	a owl:ObjectProperty;
	rdfs:label "is part of manuscript convolute"@en, "ist Teil von Manuskriptkonvolut"@de;
	rdfs:comment """Relating a manuscript by Kuno Raeber to the convolute it is part of."""@en;
	rdfs:domain kuno-raeber:Manuscript;
	rdfs:range kuno-raeber:ManuscriptConvolute;
	rdfs:subPropertyOf infocar:isPartOfConvolute;
	knora-base:subjectClassConstraint kuno-raeber:Manuscript;
	knora-base:objectClassConstraint kuno-raeber:ManuscriptConvolute.

kuno-raeber:isPartOfManuscriptConvoluteValue
	a owl:ObjectProperty;
	rdfs:label "is part of manuscript convolute - statement"@en, "ist Teil von Manuskriptkonvolut - Festlegung"@de;
	rdfs:comment """Relating a poem manuscript by Kuno Raeber to a reification statement of the relation between the poem manuscript and the convolute it is part of."""@en;
	rdfs:subPropertyOf infocar:isPartOfConvoluteValue;
	knora-base:subjectClassConstraint kuno-raeber:Manuscript;
	knora-base:objectClassConstraint knora-base:LinkValue.

kuno-raeber:isPartOfPostcardConvolute
	a owl:ObjectProperty;
	rdfs:label "is part of postcard convolute"@en, "ist Teil von Postkartekonvolut"@de;
	rdfs:comment """Relating a poem postcard by Kuno Raeber to the convolute it is part of."""@en;
	rdfs:domain kuno-raeber:PoemPostcard;
	rdfs:range kuno-raeber:PoemPostcardConvolute;
	rdfs:subPropertyOf infocar:isPartOfConvolute;
	knora-base:subjectClassConstraint kuno-raeber:PoemPostcard;
	knora-base:objectClassConstraint kuno-raeber:PoemPostcardConvolute.

kuno-raeber:isPartOfPostcardConvoluteValue
	a owl:ObjectProperty;
	rdfs:label "is part of postcard convolute - statement"@en, "ist Teil von Postkartekonvolut - Festlegung"@de;
	rdfs:comment """Relating a poem postcard by Kuno Raeber to a reification statement of the relation between the poem postcard and the convolute it is part of."""@en;
	rdfs:subPropertyOf infocar:isPartOfConvoluteValue;
	knora-base:subjectClassConstraint kuno-raeber:PoemPostcard;
	knora-base:objectClassConstraint knora-base:LinkValue.
		
kuno-raeber:isPartOfTypescriptConvolute
	a owl:ObjectProperty;
	rdfs:label "is part of typescript convolute"@en, "ist Teil von Typoskriptkonvolut"@de;
	rdfs:comment """Relating a typescript by Kuno Raeber to the convolute it is part of."""@en;
	rdfs:domain kuno-raeber:Typescript;
	rdfs:range kuno-raeber:TypescriptConvolute;
	rdfs:subPropertyOf infocar:isPartOfConvolute;
	knora-base:subjectClassConstraint kuno-raeber:Typescript;
	knora-base:objectClassConstraint kuno-raeber:TypescriptConvolute.

kuno-raeber:isPartOfTypescriptConvoluteValue
	a owl:ObjectProperty;
	rdfs:label "is part of typescript convolute - statement"@en, "ist Teil von Typoskriptkonvolut - Festlegung"@de;
	rdfs:comment """Relating a typescript by Kuno Raeber to a reification statement of the relation between the typescript and the convolute it is part of."""@en;
	rdfs:subPropertyOf infocar:isPartOfConvoluteValue;
	knora-base:subjectClassConstraint kuno-raeber:Typescript;
	knora-base:objectClassConstraint knora-base:LinkValue.

kuno-raeber:containsEarlierStagesOfManuscriptConvolute
	a owl:ObjectProperty;
	rdfs:label "contains earlier stages of manuscript convolute"@en, "enthält Vorstufen von Manuskriptenkonvolut"@de;
	rdfs:comment """Relating a convolute to another one containing manuscripts with later stages of poems by Kuno Raeber of the former convolute."""@en;
	rdfs:domain kuno-raeber:PoemNotebook;
	rdfs:range kuno-raeber:ManuscriptConvolute;
	rdfs:subPropertyOf infocar:containsEarlierStagesOf;
	knora-base:subjectClassConstraint kuno-raeber:PoemNotebook;
	knora-base:objectClassConstraint kuno-raeber:ManuscriptConvolute.

kuno-raeber:containsEarlierStagesOfManuscriptConvoluteValue
	a owl:ObjectProperty;
	rdfs:label "contains earlier stages of manuscript convolute - statement"@en, "enthält Vorstufen von Manuskriptenkonvolut - Festlegung"@de;
	rdfs:comment """Relating a convolute to a reification statement of the relation between the convolute and another one containing manuscripts with later stages of poems by Kuno Raeber of the former convolute."""@en;
	rdfs:subPropertyOf infocar:containsEarlierStagesOfValue;
	knora-base:subjectClassConstraint kuno-raeber:PoemNotebook;
	knora-base:objectClassConstraint knora-base:LinkValue.

kuno-raeber:containsEarlierStagesOfTypescriptConvolute
	a owl:ObjectProperty;
	rdfs:label "contains earlier stages of typescript convolute"@en, "enthält Vorstufen von Typoskriptenonvolut"@de;
	rdfs:comment """Relating a convolute to another one containing typescripts with later stages of poems by Kuno Raeber of the former convolute."""@en;
	rdfs:domain kuno-raeber:Convolute;
	rdfs:range kuno-raeber:TypescriptConvolute;
	rdfs:subPropertyOf infocar:containsEarlierStagesOf;
	knora-base:subjectClassConstraint kuno-raeber:Convolute;
	knora-base:objectClassConstraint kuno-raeber:TypescriptConvolute.

kuno-raeber:containsEarlierStagesOfTypescriptConvoluteValue
	a owl:ObjectProperty;
	rdfs:label "contains earlier stages of typescript convolute - statement"@en, "enthält Vorstufen von Typoskriptenonvolut - Festlegung"@de;
	rdfs:comment """Relating a convolute to a reification statement of the relation between the convolute and another one containing typescripts with later stages of poems by Kuno Raeber of the former convolute."""@en;
	rdfs:subPropertyOf infocar:containsEarlierStagesOfValue;
	knora-base:subjectClassConstraint kuno-raeber:Convolute;
	knora-base:objectClassConstraint knora-base:LinkValue.

kuno-raeber:containsLaterStagesOfNotebook
	a owl:ObjectProperty;
	rdfs:label "contains later stages of notebook"@en, "enthält spätere Stufen von Notizbuch"@de;
	rdfs:comment """Relating a convolute to a notebook containing earlier stages of poems by Kuno Raeber of the former convolute."""@en;
	rdfs:domain kuno-raeber:Convolute;
	rdfs:range kuno-raeber:PoemNotebook;
	rdfs:subPropertyOf infocar:containsLaterStagesOf;
	knora-base:subjectClassConstraint kuno-raeber:Convolute;
	knora-base:objectClassConstraint kuno-raeber:PoemNotebook.

kuno-raeber:containsLaterStagesOfNotebookValue
	a owl:ObjectProperty;
	rdfs:label "contains later stages of notebook - statement"@en, "enthält spätere Stufen von Notizbuch - Festlegung"@de;
	rdfs:comment """Relating a convolute to a reification statement of the relation between the convolute and a notebook containing earlier stages of poems by Kuno Raeber of the former convolute."""@en;
	rdfs:subPropertyOf infocar:containsLaterStagesOfValue;
	knora-base:subjectClassConstraint kuno-raeber:Convolute;
	knora-base:objectClassConstraint knora-base:LinkValue.

kuno-raeber:containsLaterStagesOfManuscriptConvolute
	a owl:ObjectProperty;
	rdfs:label "contains later stages of manuscript convolute"@en, "enthält spätere Stufen von Manuskriptenkonvolut"@de;
	rdfs:comment """Relating a convolute to another one containing manuscripts with earlier stages of poems by Kuno Raeber of the former convolute."""@en;
	rdfs:domain kuno-raeber:Convolute;
	rdfs:range kuno-raeber:ManuscriptConvolute;
	rdfs:subPropertyOf infocar:containsLaterStagesOf;
	knora-base:subjectClassConstraint kuno-raeber:Convolute;
	knora-base:objectClassConstraint kuno-raeber:ManuscriptConvolute.

kuno-raeber:containsLaterStagesOfManuscriptConvoluteValue
	a owl:ObjectProperty;
	rdfs:label "contains later stages of manuscript convolute - statement"@en, "enthält spätere Stufen von Manuskriptenkonvolut - Festlegung"@de;
	rdfs:comment """Relating a convolute to a reification statement of the relation between the convolute and another one containing manuscripts with earlier stages of poems by Kuno Raeber of the former convolute."""@en;
	rdfs:subPropertyOf infocar:containsLaterStagesOfValue;
	knora-base:subjectClassConstraint kuno-raeber:Convolute;
	knora-base:objectClassConstraint knora-base:LinkValue.

kuno-raeber:containsLaterStagesOfTypescriptConvolute
	a owl:ObjectProperty;
	rdfs:label "contains later stages of typescript convolute"@en, "enthält spätere Stufen von Typoskriptenonvolut"@de;
	rdfs:comment """Relating a convolute to another one containing typescripts with earlier stages of poems by Kuno Raeber of the former convolute."""@en;
	rdfs:domain kuno-raeber:PrintedPoemBookPublication;
	rdfs:range kuno-raeber:TypescriptConvolute;
	rdfs:subPropertyOf infocar:containsLaterStagesOf;
	knora-base:subjectClassConstraint kuno-raeber:PrintedPoemBookPublication;
	knora-base:objectClassConstraint kuno-raeber:TypescriptConvolute.

kuno-raeber:containsLaterStagesOfTypescriptConvoluteValue
	a owl:ObjectProperty;
	rdfs:label "contains later stages of typescript convolute - statement"@en, "enthält spätere Stufen von Typoskriptenonvolut - Festlegung"@de;
	rdfs:comment """Relating a convolute to a reification statement of the relation between the convolute and another one containing typescripts with earlier stages of poems by Kuno Raeber of the former convolute."""@en;
	rdfs:subPropertyOf infocar:containsLaterStagesOfValue;
	knora-base:subjectClassConstraint kuno-raeber:PrintedPoemBookPublication;
	knora-base:objectClassConstraint knora-base:LinkValue.

kuno-raeber:isInDiary
	a owl:ObjectProperty;
	rdfs:label "entry is in diary"@en, "Eintrag ist in Tagebuch"@de;
	rdfs:comment """Relating a diary entry by Kuno Raeber to the diary it is in."""@en;
	rdfs:domain kuno-raeber:DiaryEntry;
	rdfs:range kuno-raeber:Diary;
	rdfs:subPropertyOf infocar:entryIsInDiary;
	knora-base:subjectClassConstraint kuno-raeber:DiaryEntry;
	knora-base:objectClassConstraint kuno-raeber:Diary.

kuno-raeber:isInDiaryValue
	a owl:ObjectProperty;
	rdfs:label "entry is in diary - statement"@en, "Eintrag ist in Tagebuch - Festlegung"@de;
	rdfs:comment """Relating a diary entry by Kuno Raeber to a reification statement of the relation between the entry and the diary it is in."""@en;
	rdfs:subPropertyOf infocar:entryIsInDiaryValue;
	knora-base:subjectClassConstraint kuno-raeber:DiaryEntry;
	knora-base:objectClassConstraint knora-base:LinkValue.

kuno-raeber:isInDiaryConvolute
	a owl:ObjectProperty;
	rdfs:label "is in diary convolute"@en, "ist in Tagebuch-Konvolut"@de;
	rdfs:comment """Relating a diary entry by Kuno Raeber to a diary convolute it is in."""@en;
	rdfs:domain kuno-raeber:DiaryEntry;
	rdfs:range kuno-raeber:DiaryConvolute;
	rdfs:subPropertyOf knora-base:hasLinkTo;
	knora-base:subjectClassConstraint kuno-raeber:DiaryEntry;
	knora-base:objectClassConstraint kuno-raeber:DiaryConvolute.

kuno-raeber:isInDiaryConvoluteValue
	a owl:ObjectProperty;
	rdfs:label "is in diary convolute - statement"@en, "ist in Tagebuch-Konvolut - Festlegung"@de;
	rdfs:comment """Relating a diary entry by Kuno Raeber to a reification statement of the relation between the diary entry and a diary convolute it is in."""@en;
	rdfs:subPropertyOf knora-base:hasLinkToValue;
	knora-base:subjectClassConstraint kuno-raeber:DiaryEntry;
	knora-base:objectClassConstraint knora-base:LinkValue.

kuno-raeber:isPartOfLetterConvolute
	a owl:ObjectProperty;
	rdfs:label "is part of letter convolute"@en, "ist Teil eines Briefe-Konvolut"@de;
	rdfs:comment """Relating a letter by Kuno Raeber to a convolute it is in."""@en;
	rdfs:domain kuno-raeber:Letter;
	rdfs:range kuno-raeber:LetterConvolute;
	rdfs:subPropertyOf physical:isPartOf;
	knora-base:subjectClassConstraint kuno-raeber:Letter;
	knora-base:objectClassConstraint kuno-raeber:LetterConvolute.

kuno-raeber:isPartOfLetterConvoluteValue
	a owl:ObjectProperty;
	rdfs:label "is part of letter convolute - statement"@en, "ist Teil eines Briefe-Konvolut - Festlegung"@de;
	rdfs:comment """Relating a letter by Kuno Raeber to a reification statement of the relation between the letter and a convolute it is in."""@en;
	rdfs:subPropertyOf physical:isPartOfValue;
	knora-base:subjectClassConstraint kuno-raeber:Letter;
	knora-base:objectClassConstraint knora-base:LinkValue.

kuno-raeber:hasSameEditionAsIn
	a owl:ObjectProperty;
	rdfs:label "has same edition as in"@en, "hat gleiche Edition als in "@de;
	rdfs:comment """Relating a poem by Kuno Raeber to a convolute containing a poem with the same edition."""@en;
	rdfs:domain kuno-raeber:Poem;
	rdfs:range kuno-raeber:Convolute;
	rdfs:subPropertyOf knora-base:hasLinkTo;
	knora-base:subjectClassConstraint kuno-raeber:Poem;
	knora-base:objectClassConstraint kuno-raeber:Convolute.

kuno-raeber:hasSameEditionAsInValue
	a owl:ObjectProperty;
	rdfs:label "has same edition as in - statement"@en, "hat gleiche Edition als in - Festlegung"@de;
	rdfs:comment """Relating a poem by Kuno Raeber to a reification statement of the relation between the poem and a convolute containing a poem with the same edition."""@en;
	rdfs:subPropertyOf knora-base:hasLinkToValue;
	knora-base:subjectClassConstraint kuno-raeber:Poem;
	knora-base:objectClassConstraint knora-base:LinkValue.

kuno-raeber:hasReferencePoem
	 a owl:ObjectProperty;
	rdfs:label "has reference poem"@en, "hat Bezugsgedicht"@de;
	rdfs:comment "Relating a poem to another one as its reference."@en;
	rdfs:domain kuno-raeber:Poem;
	rdfs:range kuno-raeber:Poem;
	rdfs:subPropertyOf text:hasReferenceText;
	knora-base:subjectClassConstraint kuno-raeber:Poem;
	knora-base:objectClassConstraint kuno-raeber:Poem.

kuno-raeber:hasReferencePoemValue
	a owl:ObjectProperty;
	rdfs:label "has reference poem - statement"@en, "hat Bezugsgedicht - Festlegung"@de;
	rdfs:comment "Relating a poem to a reification statement of the relation between the poem and another one as its reference."@en;
	rdfs:subPropertyOf text:hasReferenceTextValue;
	knora-base:subjectClassConstraint kuno-raeber:Poem;
	knora-base:objectClassConstraint knora-base:LinkValue.

kuno-raeber:hasReferenceTitle
	a owl:ObjectProperty;
	rdfs:label "has reference title"@en, "hat Bezugstitel"@de;
	rdfs:comment """Relating a poem to a title of a reference poem."""@en;
	rdfs:domain kuno-raeber:Poem;
	rdfs:range rdfs:Literal;
	rdfs:subPropertyOf text:hasTitle;
	knora-base:subjectClassConstraint kuno-raeber:Poem;
	knora-base:objectClassConstraint knora-base:TextValue.

kuno-raeber:hasContentPartInPolyAuthorPublicationConvolute
	a owl:ObjectProperty;
	rdfs:label "has part in poly-author publication convolute"@en, "ist Teilweise in einem Mehrautorenpublikationen-Konvolut"@de;
	rdfs:comment "Relating a poly-author publication to a convolute it has part of its content in."@en;
	rdfs:domain kuno-raeber:PolyAuthorPublication;
	rdfs:range kuno-raeber:PolyAuthorPublicationConvolute;
	rdfs:subPropertyOf knora-base:hasLinkTo;
	knora-base:subjectClassConstraint kuno-raeber:PolyAuthorPublication;
	knora-base:objectClassConstraint kuno-raeber:PolyAuthorPublicationConvolute.

kuno-raeber:hasContentPartInPolyAuthorPublicationConvoluteValue
	a owl:ObjectProperty;
	rdfs:label "has part in poly-author publication convolute - statement"@en, "ist Teilweise in einem Mehrautorenpublikationen-Konvolut - Festlegung"@de;
	rdfs:comment "Relating a poly-author publication to a reification statement of the relation between the publication and a convolute it has part of its content in."@en;
	rdfs:subPropertyOf knora-base:hasLinkToValue;
	knora-base:subjectClassConstraint kuno-raeber:PolyAuthorPublication;
	knora-base:objectClassConstraint knora-base:LinkValue.

# kuno-raeber:isFinalVersion
#	a owl:ObjectProperty;
#	rdfs:label "is final version"@en, "ist Endfassung"@de;
#	rdfs:comment """Relating a text by Kuno Raeber to being a last version or not."""@en;
#	rdfs:domain kuno-raeber:Text;
#	rdfs:range xsd:boolean;
#	rdfs:subPropertyOf knora-base:hasValue;
#	knora-base:subjectClassConstraint kuno-raeber:Text;
#	knora-base:objectClassConstraint knora-base:BooleanValue.

kuno-raeber:isInSwissGerman
	a owl:ObjectProperty;
	rdfs:label "is in Swiss German"@en, "ist auf Schweizerdeutsch"@de;
	rdfs:comment """Relating a text by Kuno Raeber to being expressed in Swiss German or not."""@en;
	rdfs:domain kuno-raeber:Text;
	rdfs:range xsd:boolean;
	rdfs:subPropertyOf knora-base:hasValue;
	knora-base:subjectClassConstraint kuno-raeber:Text;
	knora-base:objectClassConstraint knora-base:BooleanValue.

kuno-raeber:isPartOfCycle
	a owl:ObjectProperty;
	rdfs:label "is part of cycle"@en, "ist Teil eines Zyklus"@de;
	rdfs:comment """Relating a text by Kuno Raeber to being part of a cycle or not."""@en;
	rdfs:domain kuno-raeber:Text;
	rdfs:range xsd:boolean;
	rdfs:subPropertyOf knora-base:hasValue;
	knora-base:subjectClassConstraint kuno-raeber:Text;
	knora-base:objectClassConstraint knora-base:BooleanValue.

kuno-raeber:hasStrophe
	a owl:ObjectProperty;
	rdfs:label "has strophe"@en, "hat Strophe"@de;
	rdfs:comment """Relating a poem by Kuno Raeber to having a strophe or not."""@en;
	rdfs:domain kuno-raeber:Poem;
	rdfs:range xsd:boolean;
	rdfs:subPropertyOf knora-base:hasValue;
	knora-base:subjectClassConstraint kuno-raeber:Poem;
	knora-base:objectClassConstraint knora-base:BooleanValue.