@prefix rdfs: <http://www.w3.org/2000/01/rdf-schema#>.
@prefix owl: <http://www.w3.org/2002/07/owl#>.
@prefix xsd: <http://www.w3.org/2001/XMLSchema#>.
@prefix skos: <http://www.w3.org/2004/02/skos/core#>.
@prefix dct: <http://purl.org/dc/terms/>.
@prefix foaf: <http://xmlns.com/foaf/0.1/>.
@prefix unicore: <http://purl.uniprot.org/core/>.
@prefix cidoc: <http://www.cidoc-crm.org/cidoc-crm/>.
@prefix frbroo: <http://iflastandards.info/ns/fr/frbr/frbroo/>.
@prefix event: <http://www.knora.org/ontology/shared/event#>.
@prefix agent: <http://www.knora.org/ontology/shared/agent#>.
@prefix human: <http://www.knora.org/ontology/shared/human#>.
@prefix creating: <http://www.knora.org/ontology/shared/creating#>.
@prefix concept: <http://www.knora.org/ontology/shared/concept#>.
@prefix text: <http://www.knora.org/ontology/shared/text#>.
@prefix device: <http://www.knora.org/ontology/shared/device#>.
@prefix ling: <http://www.knora.org/ontology/shared/linguistics#>.
@prefix knora-base: <http://www.knora.org/ontology/knora-base#>.

@base <http://www.knora.org/ontology/shared/language>.
@prefix language: <http://www.knora.org/ontology/shared/language#>.

<http://www.knora.org/ontology/shared/language>
	a owl:Ontology;
	dct:license <http://creativecommons.org/licenses/by/3.0/>;
	dct:title "An ontology about language"@en;
	dct:description """Formal description of language, general subclasses, related classes and properties."""@en;
	dct:creator "Hans Cools, MD, knowledge engineer, ontologist, software developer, NIE-INE, Basel University, Switzerland"@en;
	dct:publisher "Basel University, Switzerland"@en;

	knora-base:attachedToProject <http://www.knora.org/ontology/knora-base#DefaultSharedOntologiesProject>.

#
# CLASSES
#

language:Language
	a owl:Class;
	rdfs:label "language"@en, "Sprache"@de;
	rdfs:comment """Dynamic set of sensory carriers, e.g. a sign, symbol, word, including sound and gesture, to express meaning, and used along rules or grammar model, e.g. syntax for serialization."""@en;
	rdfs:subClassOf dct:LinguisticSystem, knora-base:Resource, [
		a owl:Restriction; owl:onProperty knora-base:seqnum; owl:minCardinality "0"^^xsd:nonNegativeInteger].

language:HumanLanguage
	a owl:Class;
	rdfs:label "human language"@en, "menschliche Sprache"@de;
	rdfs:comment """Language of a human."""@en;
	skos:note """Also formal language, e.g. computer programming language."""@en;
	rdfs:subClassOf language:Language. #*, human:Ability.

language:HumanNaturalLanguage
	a owl:Class;
	rdfs:label "human natural language"@en, "menschliche naturliche Sprache"@de;
	rdfs:comment """Language naturally evolved in humans."""@en;
	skos:note """Excluded is formal language, e.g. computer programming language."""@en;
	rdfs:subClassOf language:HumanLanguage, [
		a owl:Restriction; owl:onProperty language:hasCode; owl:minCardinality "0"^^xsd:nonNegativeInteger].
#	owl:disjointWith language:FormalLanguage.

language:GeneralHumanNaturalLanguage
	a owl:Class;
	rdfs:label "general human natural language"@en, "algemeine menschliche naturliche Sprache"@de;
	rdfs:comment """Language naturally evolved in humans and used as official language in one or more countries."""@en; #°
	rdfs:subClassOf language:HumanNaturalLanguage, [
		a owl:Restriction; owl:onProperty language:hasDialect; owl:minCardinality "0"^^xsd:nonNegativeInteger], [
		a owl:Restriction; owl:onProperty language:hasDialectValue; owl:minCardinality "0"^^xsd:nonNegativeInteger].

language:English
	a owl:Class;
	rdfs:label "English"@en, "Englisch"@de;
	rdfs:comment """The language developed and spoken in the United Kingdom, also an official language in 66 other countries, and spoken in other parts of the world."""@en;
	rdfs:subClassOf language:GeneralHumanNaturalLanguage.

language:French
	a owl:Class;
	rdfs:label "French"@en, "Französisch"@de, "français"@fr, "francese"@it;
	rdfs:comment """The language developed and spoken in France, also an official language in 29 other countries, and spoken in other parts of the world."""@en;
	rdfs:subClassOf language:GeneralHumanNaturalLanguage.

language:German
	a owl:Class;
	rdfs:label "German"@en, "Deutsch"@de, "allemand"@fr, "tedesco"@it;
	rdfs:comment """The language developed and spoken in Germany and Austria, also an official language in 5 other countries, and spoken in other parts of the world."""@en;
	rdfs:subClassOf language:GeneralHumanNaturalLanguage.

language:Italian
	a owl:Class;
	rdfs:label "Italian"@en, "Italienisch"@de, "italien"@fr, "italiana"@it;
	rdfs:comment """The language developed and spoken in Italy, also an official language in 2 other countries and a state, and spoken in other parts of the world."""@en;
	rdfs:subClassOf language:GeneralHumanNaturalLanguage.

language:SwissGerman
	a owl:Class;
	rdfs:label "Swiss German"@en, "Schweizerdeutsch"@de;
	rdfs:comment """Any of the Alemannic dialects spoken in the German-speaking part of Switzerland and in some Alpine communities in Northern Italy bordering Switzerland."""@en;
	rdfs:subClassOf language:GeneralHumanNaturalLanguage, [
		a owl:Restriction; owl:onProperty language:swissGermanHasDialect; owl:minCardinality "0"^^xsd:nonNegativeInteger], [
		a owl:Restriction; owl:onProperty language:swissGermanHasDialectValue; owl:minCardinality "0"^^xsd:nonNegativeInteger].

language:HumanNaturalLanguageExpression
	a owl:Class;
	rdfs:label "human natural language expression"@en, "menschliche naturliche sprachliche Äusserung"@de;
	rdfs:comment """Expression in a human natural language."""@en;
	skos:note """Different from the FRBROO based document:Expression."""@en;
	rdfs:subClassOf concept:Information, cidoc:E33_Linguistic_Object, [
		a owl:Restriction; owl:onProperty language:hasContent; owl:minCardinality "0"^^xsd:nonNegativeInteger], [
		a owl:Restriction; owl:onProperty language:expressedInNaturalLanguage; owl:minCardinality "0"^^xsd:nonNegativeInteger], [
		a owl:Restriction; owl:onProperty language:expressedInNaturalLanguageValue; owl:minCardinality "0"^^xsd:nonNegativeInteger], [
		a owl:Restriction; owl:onProperty language:expressedInDialect; owl:minCardinality "0"^^xsd:nonNegativeInteger], [
		a owl:Restriction; owl:onProperty language:expressedInDialectValue; owl:minCardinality "0"^^xsd:nonNegativeInteger], [
		a owl:Restriction; owl:onProperty language:hasTranslator; owl:minCardinality "0"^^xsd:nonNegativeInteger], [
		a owl:Restriction; owl:onProperty language:hasTranslatorValue; owl:minCardinality "0"^^xsd:nonNegativeInteger], [
		a owl:Restriction; owl:onProperty language:hasPersonTranslator; owl:minCardinality "0"^^xsd:nonNegativeInteger], [
		a owl:Restriction; owl:onProperty language:hasPersonTranslatorValue; owl:minCardinality "0"^^xsd:nonNegativeInteger], [
		a owl:Restriction; owl:onProperty language:hasMachineTranslator; owl:minCardinality "0"^^xsd:nonNegativeInteger], [
		a owl:Restriction; owl:onProperty language:hasMachineTranslatorValue; owl:minCardinality "0"^^xsd:nonNegativeInteger], [
		a owl:Restriction; owl:onProperty language:hasTranslation; owl:minCardinality "0"^^xsd:nonNegativeInteger], [
		a owl:Restriction; owl:onProperty language:hasTranslationValue; owl:minCardinality "0"^^xsd:nonNegativeInteger], [
		a owl:Restriction; owl:onProperty language:isTranslatedInto; owl:minCardinality "0"^^xsd:nonNegativeInteger], [
		a owl:Restriction; owl:onProperty language:isTranslatedIntoValue; owl:minCardinality "0"^^xsd:nonNegativeInteger], [
		a owl:Restriction; owl:onProperty ling:hasComment; owl:minCardinality "0"^^xsd:nonNegativeInteger].

language:Dialect
	a owl:Class;
	rdfs:label "dialect"@en, "Mundart"@de;
	rdfs:comment """Regional variant of a standard human natural language."""@en;
	rdfs:subClassOf language:HumanNaturalLanguage.

language:BaselGerman
	a owl:Class;
	rdfs:label "Basel German"@en, "Baseldeutsch"@de;
	rdfs:comment """Dialect of the city of Basel, Switzerland."""@en;
	rdfs:subClassOf language:Dialect.

language:AgentTranslator
	a owl:Class;
	rdfs:label "agent translator"@en, "Agent-Übersetzer"@de;
	rdfs:comment """Role of an agent, person or machine, transferring a human natural language expression in another natural language."""@en;
	rdfs:subClassOf agent:Creator.

language:PersonTranslator
	a owl:Class;
	rdfs:label "person-translator"@en, "Person-Übersetzer"@de;
	rdfs:comment """Translator as role of a person."""@en;
	rdfs:subClassOf language:AgentTranslator, creating:PersonCreator.

language:MachineTranslator
	a owl:Class;
	rdfs:label "machine-translator"@en, "Maschine-Übersetzer"@de;
	rdfs:comment """Translator as role of a machine."""@en;
	rdfs:subClassOf language:AgentTranslator.

language:Translation
	a owl:Class;
	rdfs:label "translation"@en, "Übersetzung"@de, "traduction"@fr, "traduzione"@it;
	rdfs:comment """Human natural language expression transferred from another natural language."""@en;
	skos:note """Can follow the original to a degree, hence differ from another translation; e.g. a free translation gives a general meaning."""@en;
	rdfs:seeAlso <https://www.abc-clio.com/ODLIS/odlis_t.aspx>;
	rdfs:subClassOf language:HumanNaturalLanguageExpression, [
		a owl:Restriction; owl:onProperty language:translationHasTranslator; owl:minCardinality "0"^^xsd:nonNegativeInteger], [
		a owl:Restriction; owl:onProperty language:translationHasTranslatorValue; owl:minCardinality "0"^^xsd:nonNegativeInteger].

language:PersonTranslation
	a owl:Class;
	rdfs:label "person's translation"@en, "Übersetzung einer Person"@de;
	rdfs:comment """Translation done by a person."""@en;
	rdfs:subClassOf language:Translation, creating:CreationDerivative, [
		a owl:Restriction; owl:onProperty language:translationHasPersonTranslator; owl:minCardinality "0"^^xsd:nonNegativeInteger], [
		a owl:Restriction; owl:onProperty language:translationHasPersonTranslatorValue; owl:minCardinality "0"^^xsd:nonNegativeInteger].

language:MachineTranslation
	a owl:Class;
	rdfs:label "machine translation"@en, "Maschinenübersetzung"@de, "traduction automatique"@fr, "traduzione automatica"@it;
	rdfs:comment """Translation done by a digital electronic computer using translation software."""@en;
	rdfs:subClassOf language:Translation.

#
# PROPERTIES
#

language:hasCode
	a owl:ObjectProperty;
	rdfs:label "language has code"@en, "Sprache hat Kode"@de;
	rdfs:comment """Relating a language to a code (object) representing that language."""@en;
	rdfs:domain language:HumanNaturalLanguage;
	rdfs:range skos:Concept;
	rdfs:subPropertyOf knora-base:hasValue; # skos:exactMatch
	knora-base:subjectClassConstraint language:HumanNaturalLanguage;
	knora-base:objectClassConstraint knora-base:TextValue. 

language:hasContent
	a owl:ObjectProperty;
	rdfs:label "has content"@en, "hat Inhalt"@de;
	rdfs:comment """Relating a human natural language expression to its content."""@en;
	rdfs:domain language:HumanNaturalLanguageExpression;
	rdfs:range rdfs:Literal;
	rdfs:subPropertyOf concept:hasLiteral;
	knora-base:subjectClassConstraint language:HumanNaturalLanguageExpression;
	knora-base:objectClassConstraint knora-base:TextValue.

language:hasDialect
	a owl:ObjectProperty;
	rdfs:label "has dialect"@en, "hat Dialekt"@de;
	rdfs:comment """Relating a human natural language to a dialect it has."""@en;
	rdfs:domain language:HumanNaturalLanguage;
	rdfs:range language:Dialect;
	rdfs:subPropertyOf knora-base:hasLinkTo;
	knora-base:subjectClassConstraint language:HumanNaturalLanguage;
	knora-base:objectClassConstraint language:Dialect.

language:hasDialectValue
	a owl:ObjectProperty;
	rdfs:label "has dialect - statement"@en, "hat Dialekt - Festlegung"@de;
	rdfs:comment """Relating a human natural language to a reification statement of the relation between the natural language and a dialect it has."""@en;
	rdfs:subPropertyOf knora-base:hasLinkToValue;
	knora-base:subjectClassConstraint language:HumanNaturalLanguage;
	knora-base:objectClassConstraint knora-base:LinkValue.

language:swissGermanHasDialect
	a owl:ObjectProperty;
	rdfs:label "Swiss German has dialect"@en, "Schweizerdeutsch hat Dialekt"@de;
	rdfs:comment """Relating Swiss German to a dialect it has."""@en;
	rdfs:domain language:SwissGerman;
	rdfs:range language:Dialect;
	rdfs:subPropertyOf knora-base:hasLinkTo;
	knora-base:subjectClassConstraint language:SwissGerman;
	knora-base:objectClassConstraint language:Dialect.

language:swissGermanHasDialectValue
	a owl:ObjectProperty;
	rdfs:label "Swiss German has dialect - statement"@en, "Schweizerdeutsch hat Dialekt - Festlegung"@de;
	rdfs:comment """Relating Swiss German to a reification statement of the relation between Swiss German and a dialect it has."""@en;
	rdfs:subPropertyOf knora-base:hasLinkToValue;
	knora-base:subjectClassConstraint language:SwissGerman;
	knora-base:objectClassConstraint knora-base:LinkValue.

language:expressedInNaturalLanguage
	a owl:ObjectProperty;
	rdfs:label "expressed in natural language"@en, "geäußert in naturlichen Sprache"@de;
	rdfs:comment """Relating a human expression to a natural language wherein it is expressed."""@en;
	rdfs:domain language:HumanNaturalLanguageExpression;
	rdfs:range language:HumanNaturalLanguage;
	rdfs:subPropertyOf cidoc:P72_has_language, knora-base:hasLinkTo;
	knora-base:subjectClassConstraint language:HumanNaturalLanguageExpression;
	knora-base:objectClassConstraint language:HumanNaturalLanguage.

language:expressedInNaturalLanguageValue
	a owl:ObjectProperty;
	rdfs:label "expressed in natural language - statement"@en, "geäußert in naturlichen Sprache - Festlegung"@de;
	rdfs:comment """Relating a human expression to a reification statement of the relation between the expression and a natural language wherein it is expressed."""@en;
	rdfs:subPropertyOf knora-base:hasLinkToValue;
	knora-base:subjectClassConstraint language:HumanNaturalLanguageExpression;
	knora-base:objectClassConstraint knora-base:LinkValue.

language:expressedInDialect
	a owl:ObjectProperty;
	rdfs:label "expressed in dialect"@en, "geäußert in Mundart"@de;
	rdfs:comment """Relating a human expression to a dialect it is expressed in."""@en;
	rdfs:domain language:HumanNaturalLanguageExpression;
	rdfs:range language:Dialect;
	rdfs:subPropertyOf knora-base:hasLinkTo;
	knora-base:subjectClassConstraint language:HumanNaturalLanguageExpression;
	knora-base:objectClassConstraint language:Dialect.

language:expressedInDialectValue
	a owl:ObjectProperty;
	rdfs:label "expressed in dialect - statement"@en, "geäußert in Mundart - Festlegung"@de;
	rdfs:comment "Relating a human expression to a reification statement of the relation between the expression and a dialect it is expressed in."@en;
	rdfs:subPropertyOf knora-base:hasLinkToValue;
	knora-base:subjectClassConstraint language:HumanNaturalLanguageExpression;
	knora-base:objectClassConstraint knora-base:LinkValue.

language:hasTranslator
	a owl:ObjectProperty;
	rdfs:label "has translator"@en, "hat Übersetzer"@de;
	rdfs:comment """Relating a natural language expression to an agent that translated it."""@en;
	rdfs:domain language:HumanNaturalLanguageExpression;
	rdfs:range agent:Agent; # [rdfs:subClassOf human:Person, [a owl:Restriction; owl:onProperty agent:hasRole; owl:someValuesFrom language:Translator]];
	rdfs:subPropertyOf knora-base:hasLinkTo;
	knora-base:subjectClassConstraint language:HumanNaturalLanguageExpression;
	knora-base:objectClassConstraint agent:Agent.

language:hasTranslatorValue
	a owl:ObjectProperty;
	rdfs:label "has translator - statement"@en, "hat Übersetzer - Festlegung"@de;
	rdfs:comment """Relating a natural language expression to a reification statement of the relation between the expression and an agent that translated it."""@en;
	rdfs:subPropertyOf knora-base:hasLinkToValue;
	knora-base:subjectClassConstraint language:HumanNaturalLanguageExpression;
	knora-base:objectClassConstraint knora-base:LinkValue.

language:hasPersonTranslator
	a owl:ObjectProperty;
	rdfs:label "has person-translator"@en, "hat Person-Übersetzer"@de;
	rdfs:comment """Relating a natural language expression to a person who translated it."""@en;
	rdfs:domain language:HumanNaturalLanguageExpression;
	rdfs:range human:Person; # [rdfs:subClassOf human:Person, [a owl:Restriction; owl:onProperty human:personHasRole; owl:someValuesFrom language:PersonTranslator]];
	rdfs:subPropertyOf language:hasTranslator;
	knora-base:subjectClassConstraint language:HumanNaturalLanguageExpression;
	knora-base:objectClassConstraint human:Person.

language:hasPersonTranslatorValue
	a owl:ObjectProperty;
	rdfs:label "has person-translator - statement"@en, "hat Person-Übersetzer - Festlegung"@de;
	rdfs:comment """Relating a natural language expression to a reification statement of the relation between the expression and a person who translated it."""@en;
	rdfs:subPropertyOf language:hasTranslatorValue;
	knora-base:subjectClassConstraint language:HumanNaturalLanguageExpression;
	knora-base:objectClassConstraint knora-base:LinkValue.

language:translationHasTranslator
	a owl:ObjectProperty;
	rdfs:label "translation has translator"@en, "Übersetzung hat Übersetzer"@de;
	rdfs:comment """Relating a translation to an agent that created it."""@en;
	rdfs:domain language:Translation;
	rdfs:range agent:Agent; # [rdfs:subClassOf human:Person, [a owl:Restriction; owl:onProperty agent:hasRole; owl:someValuesFrom language:Translator]];
	rdfs:subPropertyOf knora-base:hasLinkTo;
	knora-base:subjectClassConstraint language:Translation;
	knora-base:objectClassConstraint agent:Agent.

language:translationHasTranslatorValue
	a owl:ObjectProperty;
	rdfs:label "translation has translator - statement"@en, "Übersetzung hat Übersetzer - Festlegung"@de;
	rdfs:comment """Relating a translation to a reification statement of the relation between the translation and an agent that created it."""@en;
	rdfs:subPropertyOf knora-base:hasLinkToValue;
	knora-base:subjectClassConstraint language:Translation;
	knora-base:objectClassConstraint knora-base:LinkValue.

language:translationHasPersonTranslator
	a owl:ObjectProperty;
	rdfs:label "translation has person-translator"@en, "Übersetzung hat Person-Übersetzer"@de;
	rdfs:comment """Relating a translation to a person who created it."""@en;
	rdfs:domain language:PersonTranslation;
	rdfs:range human:Person; # [rdfs:subClassOf human:Person, [a owl:Restriction; owl:onProperty human:personHasRole; owl:someValuesFrom language:PersonTranslator]];
	rdfs:subPropertyOf language:translationHasTranslator;
	knora-base:subjectClassConstraint language:PersonTranslation;
	knora-base:objectClassConstraint human:Person.

language:translationHasPersonTranslatorValue
	a owl:ObjectProperty;
	rdfs:label "translation has person-translator - statement"@en, "Übersetzung hat Person-Übersetzer - Festlegung"@de;
	rdfs:comment """Relating a translation to a reification statement of the relation between the translation and a person who created it."""@en;
	rdfs:subPropertyOf language:translationHasTranslatorValue;
	knora-base:subjectClassConstraint language:PersonTranslation;
	knora-base:objectClassConstraint knora-base:LinkValue.

language:hasMachineTranslator
	a owl:ObjectProperty;
	rdfs:label "has machine-translator"@en, "hat Maschine-Übersetzer"@de;
	rdfs:comment """Relating a natural language expression to a machine that translated it."""@en;
	rdfs:domain language:HumanNaturalLanguageExpression;
	rdfs:range device:DigitalElectronicComputer; # [rdfs:subClassOf device:DigitalElectronicComputer, [a owl:Restriction; owl:onProperty human:personHasRole; owl:someValuesFrom language:Translator]];
	rdfs:subPropertyOf language:hasTranslator;
	knora-base:subjectClassConstraint language:HumanNaturalLanguageExpression;
	knora-base:objectClassConstraint device:DigitalElectronicComputer.

language:hasMachineTranslatorValue
	a owl:ObjectProperty;
	rdfs:label "has machine-translator - statement"@en, "hat Maschine-Übersetzer - Festlegung"@de;
	rdfs:comment """Relating a natural language expression to a reification statement of the relation between the expression and a machine that translated it."""@en;
	rdfs:subPropertyOf language:hasTranslatorValue;
	knora-base:subjectClassConstraint language:HumanNaturalLanguageExpression;
	knora-base:objectClassConstraint knora-base:LinkValue.

language:hasTranslation
	a owl:ObjectProperty;
	rdfs:label "has translation"@en, "hat Übersetzung"@de;
	rdfs:comment """Relating a human natural language expression to another one in another natural language into which it is translated."""@en;
	rdfs:domain language:HumanNaturalLanguageExpression;
	rdfs:range language:Translation;
	rdfs:subPropertyOf knora-base:hasLinkTo;
	knora-base:subjectClassConstraint language:HumanNaturalLanguageExpression;
	knora-base:objectClassConstraint language:Translation.

language:hasTranslationValue
	a owl:ObjectProperty;
	rdfs:label "has translation - statement"@en, "hat Übersetzung - Festlegung"@de;
	rdfs:comment """Relating a human natural language expression to a reification statement of the relation between the expression and another one in another natural language into which it is translated."""@en;
	rdfs:subPropertyOf knora-base:hasLinkToValue;
	knora-base:subjectClassConstraint language:HumanNaturalLanguageExpression;
	knora-base:objectClassConstraint knora-base:LinkValue.

language:isTranslatedInto
	a owl:ObjectProperty;
	rdfs:label "is translated in"@en, "ist übersetzt in"@de;
	rdfs:comment """Relating a human natural language expression to the language it is translated in."""@en;
	rdfs:domain language:HumanNaturalLanguageExpression;
	rdfs:range language:HumanNaturalLanguage;
	rdfs:subPropertyOf language:expressedInNaturalLanguage;
	knora-base:subjectClassConstraint language:HumanNaturalLanguageExpression;
	knora-base:objectClassConstraint language:HumanNaturalLanguage.

language:isTranslatedIntoValue
	a owl:ObjectProperty;
	rdfs:label "is translated in - statement"@en, "ist übersetzt in - Festlegung"@de;
	rdfs:comment """Relating a human natural language expression to a reification statement of the relation between the expression and the language it is translated in."""@en;
	rdfs:subPropertyOf language:expressedInNaturalLanguageValue;
	knora-base:subjectClassConstraint language:HumanNaturalLanguageExpression;
	knora-base:objectClassConstraint knora-base:LinkValue.