@prefix rdfs: <http://www.w3.org/2000/01/rdf-schema#>.
@prefix owl: <http://www.w3.org/2002/07/owl#>.
@prefix xsd: <http://www.w3.org/2001/XMLSchema#>.
@prefix skos: <http://www.w3.org/2004/02/skos/core#>.
@prefix dct: <http://purl.org/dc/terms/>.
@prefix text: <http://www.knora.org/ontology/shared/text#>.
@prefix textedit: <http://www.knora.org/ontology/shared/text-editing#>.
@prefix infocar: <http://www.knora.org/ontology/shared/information-carrier#>.
@prefix knora-base: <http://www.knora.org/ontology/knora-base#>.

@base <http://www.knora.org/ontology/0064/lavater>.
@prefix lavater: <http://www.knora.org/ontology/0064/lavater#>.

<http://www.knora.org/ontology/0064/lavater>
	a owl:Ontology;
	dct:title "An ontology about Johann Caspar Lavater's correspondence"@en;
	dct:description """Formal description of specific concepts in the scientific study of correspondence of Johann Caspar Lavater, 15 November 1741 - 2 January 1801."""@en;
	dct:creator "Hans Cools, MD, knowledge engineer, ontologist, software developer, NIE-INE, Basel University, Switzerland"@en;
	dct:contributor "Reto Baumgartner, tool coordinator and software developer, NIE-INE, University of ZÃ¼rich, Switzerland"@en;
	dct:publisher "Basel University, Switzerland"@en;

	knora-base:attachedToProject <http://rdfh.ch/projects/0064>.

#
# CLASSES
#

lavater:LetterExpression
	a owl:Class;
	rdfs:label "Johann Caspar Lavater letter expression"@en, "Brief-Expression Johann Caspar Lavaters"@de;
	rdfs:comment """Letter expression either authored by or written to by Johann Caspar Lavater."""@en;
	rdfs:subClassOf text:LetterExpression, text:HandwrittenText.

lavater:EditedLetter
	a owl:Class;
	rdfs:label "edited Johann Caspar Lavater letter"@en, "edierter Brief Johann Caspar Lavaters"@de;
	rdfs:comment """Letter either authored or received by Johann Caspar Lavater, and critically edited."""@en;
	rdfs:subClassOf textedit:CriticalEdition.

lavater:Letter
	a owl:Class;
	rdfs:label "Johann Caspar Lavater letter"@en, "Johann Caspar Lavater-Brief"@de, "lettre de Johann Caspar Lavater"@fr, "lettera di Johann Caspar Lavater"@it;
	rdfs:comment """Letter send by or to Johann Caspar Lavater."""@en;
	rdfs:subClassOf infocar:Letter, infocar:ConvoluteElement, infocar:ArchiveElement.

lavater:Page
	a owl:Class;
	rdfs:label "Johann Caspar Lavater letter page"@en, "Seite eines Briefes Johann Caspar Lavaters"@de;
	rdfs:comment """Page of a letter of Johann Caspar Lavater."""@en;
	rdfs:subClassOf infocar:Page. #, [
#		a owl:Restriction; owl:onProperty knora-base:hasRepresentation; owl:minCardinality "0"^^xsd:nonNegativeInteger], [
#		a owl:Restriction; owl:onProperty knora-base:hasRepresentationValue; owl:minCardinality "0"^^xsd:nonNegativeInteger].

lavater:LetterConvolute
	a owl:Class;
	rdfs:label "Johann Caspar Lavater letter convolute"@en,"Briefekonvolut Johann Caspar Lavaters"@de;
	rdfs:comment """Convolute of letters send by and to Johann Caspar Lavater."""@en;
	rdfs:subClassOf infocar:Convolute, infocar:ArchiveElement.
