@prefix rdfs: <http://www.w3.org/2000/01/rdf-schema#>.
@prefix owl: <http://www.w3.org/2002/07/owl#>.
@prefix xsd: <http://www.w3.org/2001/XMLSchema#>.
@prefix skos: <http://www.w3.org/2004/02/skos/core#>.
@prefix dct: <http://purl.org/dc/terms/>.
@prefix foaf: <http://xmlns.com/foaf/0.1/>.
@prefix cidoc: <http://www.cidoc-crm.org/cidoc-crm/>.
@prefix frbroo: <http://iflastandards.info/ns/fr/frbr/frbroo/>.
@prefix event: <http://www.knora.org/ontology/shared/event#>.
@prefix human: <http://www.knora.org/ontology/shared/human#>.
@prefix language: <http://www.knora.org/ontology/shared/language#>.
@prefix concept: <http://www.knora.org/ontology/shared/concept#>.
@prefix math: <http://www.knora.org/ontology/shared/mathematics#>.
@prefix document: <http://www.knora.org/ontology/shared/document#>.
@prefix text: <http://www.knora.org/ontology/shared/text#>.
@prefix text-structure: <http://www.knora.org/ontology/shared/text-structure#>.
@prefix textedit: <http://www.knora.org/ontology/shared/text-editing#>.
@prefix publish: <http://www.knora.org/ontology/shared/publishing#>.
@prefix litera: <http://www.knora.org/ontology/shared/literature#>.
@prefix ling: <http://www.knora.org/ontology/shared/linguistics#>.
@prefix lingmor: <http://www.knora.org/ontology/shared/linguistic-morphology#>.
@prefix knora-base: <http://www.knora.org/ontology/knora-base#>.

@base <http://www.knora.org/ontology/shared/note-structure>.
@prefix note-structure: <http://www.knora.org/ontology/shared/note-structure#>.

<http://www.knora.org/ontology/shared/note-structure>
	a owl:Ontology;
	dct:title "An ontology about note structure"@en;
	dct:description """Formal description of note structure, subclasses, related classes, and properties."""@en;
	skos:note """Extension of the text structure ontology."""@en;
	dct:creator "Hans Cools, MD, knowledge engineer, ontologist, software developer, NIE-INE, Basel University, Switzerland"@en;
	dct:contributor "Roberta Padlina, tool coordinator and software developer, NIE-INE, Basel University, Switzerland"@en;
	dct:contributor "Reto Baumgartner, tool coordinator and software developer, NIE-INE, University of ZÃ¼rich, Switzerland"@en;
	dct:publisher "Basel University, Switzerland"@en;

	knora-base:attachedToProject <http://www.knora.org/ontology/knora-base#DefaultSharedOntologiesProject>.

#
# CLASSES
#

note-structure:Note
	a owl:Class;
	rdfs:label "note structure"@en, "Notiz-Struktur"@de;
	rdfs:comment """Text with note structure, not necessarily having sentences or being syntactically correct; e.g. a first registration of thought, or a remark added to another text."""@en;
	rdfs:subClassOf text-structure:CompositionalContentStructure, [
		a owl:Restriction; owl:onProperty note-structure:isNoteStructureOfExpression; owl:minCardinality "0"^^xsd:nonNegativeInteger], [
		a owl:Restriction; owl:onProperty note-structure:isNoteStructureOfExpressionValue; owl:minCardinality "0"^^xsd:nonNegativeInteger].

note-structure:MarginalNote
	a owl:Class;
	rdfs:label "marginal note"@en, "Marginale Notiz"@de;
	rdfs:comment """Note written besides a text in the margin of a carrier."""@en;
	rdfs:subClassOf note-structure:Note, text:WrittenText, document:Marginal.

note-structure:InterlinearNote
	a owl:Class;
	rdfs:label "interlinear note"@en, "interlineare Notiz"@de;
	rdfs:comment """Note written between text lines."""@en;
	rdfs:subClassOf note-structure:Note, text:WrittenText.

note-structure:Gloss
	a owl:Class;
	rdfs:label "gloss"@en, "Glosse"@de;
	rdfs:comment """Explanatory note, e.g. interlinear or marginal."""@en;
	rdfs:subClassOf note-structure:Note, [
		a owl:Restriction; owl:onProperty note-structure:isGlossOfExpression; owl:minCardinality "0"^^xsd:nonNegativeInteger], [
		a owl:Restriction; owl:onProperty note-structure:isGlossOfExpressionValue; owl:minCardinality "0"^^xsd:nonNegativeInteger].

note-structure:MarginalGloss
	a owl:Class;
	rdfs:label "marginal gloss"@en, "marginale Glosse"@de;
	rdfs:comment """Gloss as a marginal note."""@en;
	rdfs:subClassOf note-structure:Gloss, note-structure:MarginalNote.

note-structure:InterlinearGloss
	a owl:Class;
	rdfs:label "interlinear gloss"@en, "interlineare Glosse"@de;
	rdfs:comment """Gloss as an interlinear note."""@en;
	rdfs:subClassOf note-structure:Gloss, note-structure:InterlinearNote.

note-structure:Footnote
	a owl:Class;
	rdfs:label "footnote structure"@en, "Fussnotestruktur"@de;
	rdfs:comment """Note on information on a page at the end of that page, seperate from the main content."""@en;
	rdfs:subClassOf note-structure:Note, [
		a owl:Restriction; owl:onProperty note-structure:footnoteHasIdentifier; owl:minCardinality "0"^^xsd:nonNegativeInteger], [
		a owl:Restriction; owl:onProperty note-structure:footnoteHasIdentifierValue; owl:minCardinality "0"^^xsd:nonNegativeInteger], [
		a owl:Restriction; owl:onProperty note-structure:footnoteHasNumber; owl:minCardinality "0"^^xsd:nonNegativeInteger], [
		a owl:Restriction; owl:onProperty note-structure:footnoteHasNumberValue; owl:minCardinality "0"^^xsd:nonNegativeInteger].

note-structure:FootnoteIdentifier
	a owl:Class;
	rdfs:label "footnote identifier"@en, "Fussnoteidentifikator"@de;
	rdfs:comment """Identifier of a footnote."""@en;
	rdfs:subClassOf text-structure:Identifier.

note-structure:FootnoteNumber
	a owl:Class;
	rdfs:label "footnote number"@en, "Fussnotenummer"@de;
	rdfs:comment """Number of a footnote."""@en;
	rdfs:subClassOf note-structure:FootnoteIdentifier, math:Number.

note-structure:Endnote
	a owl:Class;
	rdfs:label "endnote structure"@en, "Endnotestruktur"@de;
	rdfs:comment """Note on information on a page at the end of the document, seperate from the main content."""@en;
	rdfs:subClassOf note-structure:Note, [
		a owl:Restriction; owl:onProperty note-structure:endnoteHasIdentifier; owl:minCardinality "0"^^xsd:nonNegativeInteger], [
		a owl:Restriction; owl:onProperty note-structure:endnoteHasIdentifierValue; owl:minCardinality "0"^^xsd:nonNegativeInteger], [
		a owl:Restriction; owl:onProperty note-structure:endnoteHasNumber; owl:minCardinality "0"^^xsd:nonNegativeInteger], [
		a owl:Restriction; owl:onProperty note-structure:endnoteHasNumberValue; owl:minCardinality "0"^^xsd:nonNegativeInteger].

note-structure:EndnoteIdentifier
	a owl:Class;
	rdfs:label "endnote identifier"@en, "Endnoteidentifikator"@de;
	rdfs:comment """Identifier of an endnote."""@en;
	rdfs:subClassOf text-structure:Identifier.

note-structure:EndnoteNumber
	a owl:Class;
	rdfs:label "endnote number"@en, "Endnotenummer"@de;
	rdfs:comment """Number of an endnote."""@en;
	rdfs:subClassOf note-structure:EndnoteIdentifier, math:Number.

#
# PROPERTIES
#

note-structure:isNoteStructureOfExpression
	a owl:ObjectProperty;
	rdfs:label "is note of expression"@en, "ist Notiz einer Expression"@de;
	rdfs:comment """Relating a note structure to a text expression it is part of."""@en;
	rdfs:domain note-structure:Note;
	rdfs:range text:Expression;
	rdfs:subPropertyOf text-structure:isPartOfTextExpression;
	knora-base:subjectClassConstraint note-structure:Note;
	knora-base:objectClassConstraint text:Expression.

note-structure:isNoteStructureOfExpressionValue
	a owl:ObjectProperty;
	rdfs:label "is note of expression - statement"@en, "ist Notiz einer Expression - Festlegung"@de;
	rdfs:comment """Relating a note structure to a reification statement of the relation between the note and a text expression it is part of."""@en;
	rdfs:subPropertyOf text-structure:isPartOfTextExpressionValue;
	knora-base:subjectClassConstraint note-structure:Note;
	knora-base:objectClassConstraint knora-base:LinkValue.

note-structure:isGlossOfExpression
	a owl:ObjectProperty;
	rdfs:label "is gloss of expression"@en, "ist Glosse einer Expression"@de;
	rdfs:comment """Relating a gloss to a text expression it is part of."""@en;
	rdfs:domain note-structure:Gloss;
	rdfs:range text:Expression;
	rdfs:subPropertyOf note-structure:isNoteStructureOfExpression;
	knora-base:subjectClassConstraint note-structure:Gloss;
	knora-base:objectClassConstraint text:Expression.

note-structure:isGlossOfExpressionValue
	a owl:ObjectProperty;
	rdfs:label "is gloss of expression - statement"@en, "ist Glosse einer Expression - Festlegung"@de;
	rdfs:comment """Relating a gloss to a reification statement of the relation between the gloss and a text expression it is part of."""@en;
	rdfs:subPropertyOf note-structure:isNoteStructureOfExpressionValue;
	knora-base:subjectClassConstraint note-structure:Gloss;
	knora-base:objectClassConstraint knora-base:LinkValue.

note-structure:footnoteHasIdentifier
	a owl:ObjectProperty;
	rdfs:label "footnote has identifier"@en, "Fussnote hat Identifikator"@de;
	rdfs:comment """Relating a footnote to an identifier (as resource) it has."""@en;
	rdfs:domain note-structure:Footnote;
	rdfs:range note-structure:FootnoteIdentifier;
	rdfs:subPropertyOf text-structure:hasIdentifier;
	knora-base:subjectClassConstraint note-structure:Footnote;
	knora-base:objectClassConstraint note-structure:FootnoteIdentifier.

note-structure:footnoteHasIdentifierValue
	a owl:ObjectProperty;
	rdfs:label "footnote has identifier - statement"@en, "Fussnote hat Identifikator - Festlegung"@de;
	rdfs:comment """Relating a footnote to a reification statement of the relation between the footnote and an identifier (as resource) it has."""@en;
	rdfs:subPropertyOf text-structure:hasIdentifierValue;
	knora-base:subjectClassConstraint note-structure:Footnote;
	knora-base:objectClassConstraint knora-base:LinkValue.

note-structure:footnoteHasNumber
	a owl:ObjectProperty;
	rdfs:label "footnote has number"@en, "Fussnote hat Nummer"@de;
	rdfs:comment """Relating a footnote to a natural number (as resource) it has."""@en;
	rdfs:domain note-structure:Footnote;
	rdfs:range note-structure:FootnoteNumber;
	rdfs:subPropertyOf note-structure:footnoteHasIdentifier;
	knora-base:subjectClassConstraint note-structure:Footnote;
	knora-base:objectClassConstraint note-structure:FootnoteNumber.

note-structure:footnoteHasNumberValue
	a owl:ObjectProperty;
	rdfs:label "footnote has number - statement"@en, "Fussnote hat Nummer - Festlegung"@de;
	rdfs:comment """Relating a footnote to a reification statement of the relation between the footnote and a natural number (as resource) it has."""@en;
	rdfs:subPropertyOf note-structure:footnoteHasIdentifierValue;
	knora-base:subjectClassConstraint note-structure:Footnote;
	knora-base:objectClassConstraint knora-base:LinkValue.

note-structure:endnoteHasIdentifier
	a owl:ObjectProperty;
	rdfs:label "endnote has identifier"@en, "Endnote hat Identifikator"@de;
	rdfs:comment """Relating an endnote to an identifier (as resource) it has."""@en;
	rdfs:domain note-structure:Endnote;
	rdfs:range note-structure:EndnoteIdentifier;
	rdfs:subPropertyOf text-structure:hasIdentifier;
	knora-base:subjectClassConstraint note-structure:Endnote;
	knora-base:objectClassConstraint note-structure:EndnoteIdentifier.

note-structure:endnoteHasIdentifierValue
	a owl:ObjectProperty;
	rdfs:label "endnote has identifier - statement"@en, "Endnote hat Identifikator - Festlegung"@de;
	rdfs:comment """Relating an endnote to a reification statement of the relation between the endnote and an identifier (as resource) it has."""@en;
	rdfs:subPropertyOf text-structure:hasIdentifierValue;
	knora-base:subjectClassConstraint note-structure:Endnote;
	knora-base:objectClassConstraint knora-base:LinkValue.

note-structure:endnoteHasNumber
	a owl:ObjectProperty;
	rdfs:label "endnote has number"@en, "Endnote hat Nummer"@de;
	rdfs:comment """Relating an endnote to a number (as resource) it has."""@en;
	rdfs:domain note-structure:Endnote;
	rdfs:range note-structure:EndnoteNumber;
	rdfs:subPropertyOf note-structure:endnoteHasIdentifier;
	knora-base:subjectClassConstraint note-structure:Endnote;
	knora-base:objectClassConstraint note-structure:EndnoteNumber.

note-structure:endnoteHasNumberValue
	a owl:ObjectProperty;
	rdfs:label "endnote has number - statement"@en, "Endnote hat Nummer - Festlegung"@de;
	rdfs:comment """Relating an endnote to a reification statement of the relation between the endnote and a natural number (as resource) it has."""@en;
	rdfs:subPropertyOf note-structure:endnoteHasIdentifierValue;
	knora-base:subjectClassConstraint note-structure:Endnote;
	knora-base:objectClassConstraint knora-base:LinkValue.