@prefix rdfs: <http://www.w3.org/2000/01/rdf-schema#>.
@prefix owl: <http://www.w3.org/2002/07/owl#>.
@prefix xsd: <http://www.w3.org/2001/XMLSchema#>.
@prefix skos: <http://www.w3.org/2004/02/skos/core#>.
@prefix dct: <http://purl.org/dc/terms/>.
@prefix foaf: <http://xmlns.com/foaf/0.1/>.
@prefix cidoc: <http://www.cidoc-crm.org/cidoc-crm/>.
@prefix frbroo: <http://iflastandards.info/ns/fr/frbr/frbroo/>.
@prefix event: <http://www.knora.org/ontology/0047/event#>.
@prefix physical: <http://www.knora.org/ontology/0055/physical-resource#>.
@prefix agent: <http://www.knora.org/ontology/0040/agent#>.
@prefix human: <http://www.knora.org/ontology/0048/human#>.
@prefix text: <http://www.knora.org/ontology/0059/text#>.
@prefix knora-base: <http://www.knora.org/ontology/knora-base#>.

@base <http://www.knora.org/ontology/0000/organization>.
@prefix org: <http://www.knora.org/ontology/0000/organization#>.

<http://www.knora.org/ontology/0000/organization>
	a owl:Ontology;
	dct:title "An ontology about person organization"@en;
	dct:description """Formal description of organization involving persons, general subclasses, related classes and properties."""@en;
	dct:creator "Hans Cools, MD, knowledge engineer, ontologist, software developer, NIE-INE, Basel University, Switzerland"@en;
	dct:publisher "Basel University, Switzerland"@en;

	knora-base:attachedToProject <http://rdfh.ch/projects/0051>.

#
# CLASSES
#

org:Organization
	a owl:Class;
	#rdfs:isDefinedBy <http://www.knora.org/ontology/0000/organization#>;
	rdfs:label "person organization"@en, "Personensorganisation"@de; #*
	rdfs:comment """Organized group of persons."""@en;
	skos:note """An organization can be a legal person."""@en;
#	owl:disjointWith human:Person; # from FOAF
	rdfs:subClassOf human:Group, agent:Organization, foaf:Organization, frbroo:F11_Corporate_Body, [ # rdfs:subClassOf cidoc:E74_Group
		a owl:Restriction; owl:onProperty org:hasName; owl:minCardinality "0"^^xsd:nonNegativeInteger], [
		a owl:Restriction; owl:onProperty org:actsIn; owl:minCardinality "0"^^xsd:nonNegativeInteger], [
		a owl:Restriction; owl:onProperty org:actsInValue; owl:minCardinality "0"^^xsd:nonNegativeInteger], [
		a owl:Restriction; owl:onProperty org:hasRole; owl:minCardinality "0"^^xsd:nonNegativeInteger], [
		a owl:Restriction; owl:onProperty org:hasRoleValue; owl:minCardinality "0"^^xsd:nonNegativeInteger].

org:Role
	a owl:Class;
	#rdfs:isDefinedBy <http://www.knora.org/ontology/0000/organization#>;
	rdfs:label "organization's role"@en;
	rdfs:comment """Role of a person organization."""@en;
	rdfs:subClassOf human:GroupRole.

org:Creator
	a owl:Class;
	rdfs:label "organization creator"@en, "Organisation-Erschafferin"@de;
	rdfs:comment """Publisher as role of an organization."""@en;
	rdfs:subClassOf human:AgentCreator, org:Role.

org:Administration
	a owl:Class;
	#rdfs:isDefinedBy <http://www.knora.org/ontology/0000/organization#>;
	rdfs:label "administration"@en, "Verwaltung"@de;
	rdfs:comment """Role of an organization administering a group of people on any level, e.g. international, national, regional or city level."""@en;
	rdfs:subClassOf org:Role.

org:ReligiousOrganization #* OR to group religions
	a owl:Class;
	#rdfs:isDefinedBy <http://www.knora.org/ontology/0000/organization#>;
	rdfs:label "religious organization"@en, "religiöse Organisation"@de;
	rdfs:comment """Organization of religious persons."""@en;
	rdfs:subClassOf org:Organization.

org:ReligiousPerson
	a owl:Class;
	rdfs:label "religious person"@en, "religiöse Person"@de, "personne réligieuse"@fr; # "persona"@it;
	rdfs:comment """Person having religious faith or believing."""@en;
	rdfs:subClassOf human:Person, [
		a owl:Restriction; owl:onProperty org:isMemberOfReligiousOrganization; owl:minCardinality "0"^^xsd:nonNegativeInteger], [
		a owl:Restriction; owl:onProperty org:isMemberOfReligiousOrganizationValue; owl:minCardinality "0"^^xsd:nonNegativeInteger].

org:PoliticalOrganization
	a owl:Class;
	#rdfs:isDefinedBy <http://www.knora.org/ontology/0000/organization#>;
	rdfs:label "political organization"@en, "politische Organisation"@de;
	rdfs:comment """Organization being involved in politics."""@en;
	rdfs:subClassOf org:Organization.

org:Politician
	a owl:Class;
	#rdfs:isDefinedBy <http://www.knora.org/ontology/0000/organization#>;
	rdfs:label "politician role"@en, "Politiker-Rolle"@de;
	rdfs:comment """Occupational role of being professionally involved in politics, especially as a holder of an elected office."""@en;
	rdfs:subClassOf human:OccupationalRole.

org:Company
	a owl:Class;
	#rdfs:isDefinedBy <http://www.knora.org/ontology/0000/organization#>;
	rdfs:label "company"@en, "Betrieb"@de;
	rdfs:comment """Organization having primarily an economical role."""@en;
	rdfs:subClassOf org:Organization.

org:MemoryInstitution
	a owl:Class;
	rdfs:label "memory institution"@en, "Gedächtnisinstitution"@de;
	rdfs:comment """Organization having a role of maintaining a repository of public knowledge, such as a library, an archive, museum, sites and monuments record, clearinghouse, a provider of a digital library, and a data aggregation service, which serve as memories for given societies or mankind."""@en;
	rdfs:subClassOf org:Organization.

org:Museum # humans + equipment: computers + meters + moist regulators etc.
	a owl:Class;
	rdfs:label "museum"@en, "Museum"@de;
	rdfs:comment """Organization having roles of preserving and exhibiting objects of historical, scientific, artistic, or cultural interest in a special building also called museum."""@en;
	rdfs:subClassOf org:MemoryInstitution. # hasRole Preservator, Exhibitioner

org:Library
	a owl:Class;
	rdfs:label "library"@en, "Bibliothek"@de, "bibliothèque"@fr, "biblioteca"@it;
	rdfs:comment """Organization having a role of maintaining and making accessible information carriers to a defined community for reference or borrowing. An information carrier can be a book, periodical, newspaper, manuscript, film, map, print, also in microform, CD, cassette, videotape, DVD, Blu-ray Disc, e-book, audiobook, database, and other document format."""@en;
	rdfs:subClassOf org:MemoryInstitution.

org:MasonicLodge
	a owl:Class;
	#rdfs:isDefinedBy <http://www.knora.org/ontology/0000/organization#>;
	rdfs:label "Masonic lodge"@en, "Freimaurerloge"@de;
	rdfs:comment """Organizational unit of Freemasonry."""@en;
	rdfs:subClassOf org:Organization.

#
# PROPERTIES
#

org:hasName
	a owl:ObjectProperty;
	rdfs:label "person organization has name"@en, "Personensorganisation hat Name"@de;
	rdfs:comment """Relating a person organization to a name of that organization."""@en;
	rdfs:domain org:Organization;
	rdfs:range rdfs:Literal;
	rdfs:subPropertyOf text:hasName;
	knora-base:subjectClassConstraint org:Organization;
	knora-base:objectClassConstraint knora-base:TextValue.

org:actsIn
	a owl:ObjectProperty;
	#rdfs:isDefinedBy <http://www.knora.org/ontology/0000/organization#>;
	rdfs:label "person organization acts in"@en, "Personensorganisation agiert in"@de;
	rdfs:comment """Relating a person organization to an action it acts in."""@en;
	rdfs:domain org:Organization;
	rdfs:range human:Action;
	rdfs:subPropertyOf human:actsIn;
	knora-base:subjectClassConstraint org:Organization;
	knora-base:objectClassConstraint human:Action.

org:actsInValue
	a owl:ObjectProperty;
	#rdfs:isDefinedBy <http://www.knora.org/ontology/0000/organization#>;
	rdfs:label "person organization acts in - statement"@en, "Personensorganisation agiert in - Festlegung"@de;
	rdfs:comment """Relating a person organization to a reification statement of the relation between the organization and an action it is acting in."""@en;
	rdfs:subPropertyOf human:actsInValue;
	knora-base:subjectClassConstraint org:Organization;
	knora-base:objectClassConstraint knora-base:LinkValue.

org:hasRole
	a owl:ObjectProperty;
	#rdfs:isDefinedBy <http://www.knora.org/ontology/0000/organization#>;
	rdfs:label "person organization has role"@en, "Personensorganisation hat Rolle"@de;
	rdfs:comment """Relating a person organization to a role it has."""@en;
	rdfs:domain org:Organization;
	rdfs:range org:Role;
	rdfs:subPropertyOf human:groupHasRole;
	knora-base:subjectClassConstraint org:Organization;
	knora-base:objectClassConstraint org:Role.

org:hasRoleValue
	a owl:ObjectProperty;
	#rdfs:isDefinedBy <http://www.knora.org/ontology/0000/organization#>;
	rdfs:label "person organization has role - statement"@en, "Personensorganisation hat Rolle - Festlegung"@de;
	rdfs:comment """Relating a person organization to a reification statement of the relation between the organization and a role it has."""@en;
	rdfs:subPropertyOf human:groupHasRoleValue;
	knora-base:subjectClassConstraint org:Organization;
	knora-base:objectClassConstraint knora-base:LinkValue.

org:isMemberOf
	a owl:ObjectProperty;
	#rdfs:isDefinedBy <http://www.knora.org/ontology/0000/organization#>;
	rdfs:label "is member of person organization"@en, "ist Mitglied einer Personensorganisation"@de;
	rdfs:comment """Relating a person to an organization the person is a member of."""@en;
	rdfs:domain human:Person;
	rdfs:range org:Organization;
	rdfs:subPropertyOf human:isMemberOf;
	knora-base:subjectClassConstraint human:Person;
	knora-base:objectClassConstraint org:Organization.

org:isMemberOfValue
	a owl:ObjectProperty;
	#rdfs:isDefinedBy <http://www.knora.org/ontology/0000/organization#>;
	rdfs:label "is member of person organization - statement"@en, "ist Mitglied einer Personensorganisation - Festlegung"@de;
	rdfs:comment """Relating a person to a reification statement of the relation between the person and an organization the person is a member of."""@en;
	rdfs:subPropertyOf human:isMemberOfValue;
	knora-base:subjectClassConstraint human:Person;
	knora-base:objectClassConstraint knora-base:LinkValue.

# org:organizationIsMemberOf

org:isMemberOfReligiousOrganization
	a owl:ObjectProperty;
	#rdfs:isDefinedBy <http://www.knora.org/ontology/0000/organization#>;
	rdfs:label "is member of religious organization"@en, "ist Mitglied einer religiösen Organization"@de;
	rdfs:comment """Relating a person to a religious organization the person is a member of."""@en;
	rdfs:domain org:ReligiousPerson;
	rdfs:range org:ReligiousOrganization;
	rdfs:subPropertyOf org:isMemberOf;
	knora-base:subjectClassConstraint org:ReligiousPerson;
	knora-base:objectClassConstraint org:ReligiousOrganization.

org:isMemberOfReligiousOrganizationValue
	a owl:ObjectProperty;
	#rdfs:isDefinedBy <http://www.knora.org/ontology/0000/organization#>;
	rdfs:label "is member of religious organization - statement"@en, "ist Mitglied einer religiösen Organization - Festlegung"@de;
	rdfs:comment """Relating a person to a reification statement of the relation between the person and a religious organization the person is a member of."""@en;
	rdfs:subPropertyOf org:isMemberOfValue;
	knora-base:subjectClassConstraint org:ReligiousPerson;
	knora-base:objectClassConstraint knora-base:LinkValue.

org:isMemberOfAdministration
	a owl:ObjectProperty;
	#rdfs:isDefinedBy <http://www.knora.org/ontology/0000/organization#>;
	rdfs:label "is member of administration"@en, "ist Mitglied einer Verwaltung"@de;
	rdfs:comment """Relating a person to an administration organization the person is a member of."""@en;
	rdfs:domain human:Person;
#	rdfs:range [rdfs:subClassOf org:Organization, [a owl:Restriction; owl:onProperty org:hasRole; owl:someValuesFrom org:Administration]];
	rdfs:subPropertyOf org:isMemberOf;
	knora-base:subjectClassConstraint human:Person;
	knora-base:objectClassConstraint org:Organization.

org:isMemberOfAdministrationValue
	a owl:ObjectProperty;
	#rdfs:isDefinedBy <http://www.knora.org/ontology/0000/organization#>;
	rdfs:label "is member of administration - statement"@en, "ist Mitglied einer Verwaltung - Festlegung"@de;
	rdfs:comment """Relating a person to a reification statement of the relation between the person and an administration organization the person is a member of."""@en;
	rdfs:subPropertyOf org:isMemberOfValue;
	knora-base:subjectClassConstraint human:Person;
	knora-base:objectClassConstraint knora-base:LinkValue.

org:isMemberOfCompany
	a owl:ObjectProperty;
	#rdfs:isDefinedBy <http://www.knora.org/ontology/0000/organization#>;
	rdfs:label "is member of company"@en, "ist Mitglied einer Firme"@de;
	rdfs:comment """Relating a person to a company the person is a member of."""@en;
	rdfs:domain human:Person;
	rdfs:range org:Company;
	rdfs:subPropertyOf org:isMemberOf;
	knora-base:subjectClassConstraint human:Person;
	knora-base:objectClassConstraint org:Company.

org:isMemberOfCompanyValue
	a owl:ObjectProperty;
	#rdfs:isDefinedBy <http://www.knora.org/ontology/0000/organization#>;
	rdfs:label "is member of company - statement"@en, "ist Mitglied einer Firme - Festlegung"@de;
	rdfs:comment """Relating a person to a reification statement of the relation between the person and a company the person is a member of."""@en;
	rdfs:subPropertyOf org:isMemberOfValue;
	knora-base:subjectClassConstraint human:Person;
	knora-base:objectClassConstraint knora-base:LinkValue.