@prefix rdfs: <http://www.w3.org/2000/01/rdf-schema#>.
@prefix owl: <http://www.w3.org/2002/07/owl#>.
@prefix xsd: <http://www.w3.org/2001/XMLSchema#>.
@prefix skos: <http://www.w3.org/2004/02/skos/core#>.
@prefix dct: <http://purl.org/dc/terms/>.
@prefix concept: <http://www.knora.org/ontology/shared/concept#>.
@prefix math: <http://www.knora.org/ontology/shared/mathematics#>.
@prefix document: <http://www.knora.org/ontology/shared/document#>.
@prefix text: <http://www.knora.org/ontology/shared/text#>.
@prefix textedit: <http://www.knora.org/ontology/shared/text-editing#>.
@prefix text-structure: <http://www.knora.org/ontology/shared/text-structure#>.
@prefix infocar: <http://www.knora.org/ontology/shared/information-carrier#>.
@prefix publish: <http://www.knora.org/ontology/shared/publishing#>.
@prefix litera: <http://www.knora.org/ontology/shared/literature#>.
@prefix knora-base: <http://www.knora.org/ontology/knora-base#>.

@base <http://www.knora.org/ontology/0067/parzival>.
@prefix parzival: <http://www.knora.org/ontology/0067/parzival#>.

<http://www.knora.org/ontology/0067/parzival>
	a owl:Ontology;
	dct:title """An ontology about Wolfram von Eschenbach's "Parzival" """@en;
	dct:description """Formal description of specific concepts in the critical and digital edition of Wolfram von Eschenbach's "Parzival"."""@en;
	dct:creator "Hans Cools, MD, knowledge engineer, ontologist, software developer, NIE-INE, Basel University, Switzerland"@en;
	dct:contributor "Reinhard Priber, tool coordinator and software developer, NIE-INE, University of ZÃ¼rich, Switzerland"@en;
	dct:publisher "Basel University, Switzerland"@en;

	knora-base:attachedToProject <http://rdfh.ch/projects/0067>.

#
# CLASSES
#

parzival:VerseNovel
	a owl:Class;
	rdfs:label """version of 'Parzival'"""@en, """Version 'Parzivals'"""@de;
	rdfs:comment """Any version of Wolfram Von Eschenbach's verse novel 'Parzival'."""@en;
	rdfs:subClassOf litera:VerseNovel.

parzival:CopiedVerseNovel
	a owl:Class;
	rdfs:label """copied version of 'Parzival'"""@en, """kopierte Version 'Parzivals'"""@de;
	rdfs:comment """Copied version of Wolfram Von Eschenbach's verse novel 'Parzival'."""@en;
	rdfs:subClassOf litera:VerseNovel, textedit:Witness.

parzival:HandwrittenTranscribedVerseNovel
	a owl:Class;
	rdfs:label """handwritten transcribed version of 'Parzival'"""@en, """handtranskribierte Version 'Parzivals'"""@de;
	rdfs:comment """Handwritten transcribed version of Wolfram Von Eschenbach's verse novel 'Parzival'."""@en;
	rdfs:subClassOf parzival:CopiedVerseNovel, text:HandwrittenText, text:TranscribedText.

parzival:HandwrittenTranscribedVerseNovelFragment
	a owl:Class;
	rdfs:label """handwritten transcribed fragment of 'Parzival'"""@en, """handtranskribiertes Fragment 'Parzivals'"""@de;
	rdfs:comment """Fragment of a handwritten transcribed version of Wolfram Von Eschenbach's verse novel 'Parzival'."""@en;
	rdfs:subClassOf text:HandwrittenText, text:TranscribedText, text:ExpressionPart.

parzival:PrintedVerseNovel
	a owl:Class;
	rdfs:label """printed version of 'Parzival'"""@en, """gedruckte Version 'Parzivals'"""@de;
	rdfs:comment """Printed version of Wolfram Von Eschenbach's verse novel 'Parzival'."""@en;
	rdfs:subClassOf parzival:CopiedVerseNovel, text:PrintedText.

parzival:VerseNovelCopy
	a owl:Class;
	rdfs:label """copy of 'Parzival'"""@en, """Kopie 'Parzivals'"""@de;
	rdfs:comment """Copy of Wolfram Von Eschenbach's verse novel 'Parzival'."""@en;
	rdfs:subClassOf infocar:Copy, infocar:Book.

parzival:ManualVerseNovelTranscript
	a owl:Class;
	rdfs:label """manual transcript of 'Parzival'"""@en, """manuelles Transkript 'Parzivals'"""@de;
	rdfs:comment """Manual transcript of Wolfram Von Eschenbach's verse novel 'Parzival'."""@en;
	rdfs:subClassOf parzival:VerseNovelCopy, infocar:ManualTranscript, infocar:Codex.

parzival:ManualVerseNovelTranscriptFragment
	a owl:Class;
	rdfs:label """manual transcript fragment of 'Parzival'"""@en, """manuelles Transkriptfragment 'Parzivals'"""@de;
	rdfs:comment """Manual transcript fragment of Wolfram Von Eschenbach's verse novel 'Parzival'."""@en;
	rdfs:subClassOf infocar:ManualTranscript, infocar:Fragment.

parzival:VerseNovelPrint
	a owl:Class;
	rdfs:label """print of 'Parzival'"""@en, """Druck von 'Parzival'"""@de;
	rdfs:comment """Print of Wolfram Von Eschenbach's verse novel 'Parzival'."""@en;
	rdfs:subClassOf parzival:VerseNovelCopy, infocar:Print, infocar:Book.

parzival:DocumentPage
	a owl:Class;
	rdfs:label """document page of 'Parzival'"""@en, """Dokumentseite von 'Parzival'"""@de;
	rdfs:comment """Document page of Wolfram Von Eschenbach's verse novel 'Parzival'."""@en;
	rdfs:subClassOf document:Page, document:ExpressionPart.

parzival:TextPage
	a owl:Class;
	rdfs:label """text page of 'Parzival'"""@en, """Textseite von 'Parzival'"""@de;
	rdfs:comment """Text page of Wolfram Von Eschenbach's verse novel 'Parzival'."""@en;
	rdfs:subClassOf text-structure:Page, text:ExpressionPart.

parzival:Page
	a owl:Class;
	rdfs:label "page of 'Parzival'"@en, "Seite 'Parzivals'"@de;
	rdfs:comment """Page of a manual transcript of 'Parzival'."""@en, """Seite eines Manuellen Transkripts 'Parzivals'."""@de;
	rdfs:subClassOf infocar:Page, [
		a owl:Restriction; owl:onProperty knora-base:hasRepresentation; owl:minCardinality "0"^^xsd:nonNegativeInteger], [
		a owl:Restriction; owl:onProperty knora-base:hasRepresentationValue; owl:minCardinality "0"^^xsd:nonNegativeInteger].

parzival:Verse
	a owl:Class;
	rdfs:label """verse of 'Parzival'"""@en, """Vers von 'Parzival'"""@de;
	rdfs:comment """Verse in Wolfram Von Eschenbach's verse novel 'Parzival', or a version or derivative thereof."""@en;
	rdfs:subClassOf text-structure:Verse, [
		a owl:Restriction; owl:onProperty parzival:isVerseOfDreissiger; owl:minCardinality "0"^^xsd:nonNegativeInteger], [
		a owl:Restriction; owl:onProperty parzival:isVerseOfDreissigerValue; owl:minCardinality "0"^^xsd:nonNegativeInteger].

# verse ohne Dreissiger

parzival:Dreissiger
	a owl:Class;
	rdfs:label "dreissiger"@en, "Dreissiger"@de, "dreissiger"@fr, "dreissiger"@it;
	rdfs:comment """Set of about 30 verses in Wolfram Von Eschenbach's verse novel 'Parzival', or a version or derivative thereof."""@en;
	rdfs:seeAlso """Bumke Joachim, "Wolfram von Eschenbach", Springer-Verlag, Stuttgart, 2004."""@en;
	rdfs:subClassOf text-structure:ProsodicStructure, text:ExpressionPart, [
		a owl:Restriction; owl:onProperty parzival:isDreissigerOfNovel; owl:minCardinality "0"^^xsd:nonNegativeInteger], [
		a owl:Restriction; owl:onProperty parzival:isDreissigerOfNovelValue; owl:minCardinality "0"^^xsd:nonNegativeInteger], [
		a owl:Restriction; owl:onProperty parzival:dreissigerHasNumber; owl:minCardinality "0"^^xsd:nonNegativeInteger], [
		a owl:Restriction; owl:onProperty parzival:dreissigerHasNumberValue; owl:minCardinality "0"^^xsd:nonNegativeInteger].

parzival:DreissigerNumber
	a owl:Class;
	rdfs:label "dreissiger number"@en, "Dreissigernummer"@de;
	rdfs:comment """Number of a dreissiger."""@en;
	rdfs:subClassOf text-structure:Identifier, math:NaturalNumber.

parzival:VerseSection
	a owl:Class;
	rdfs:label """verse section of 'Parzival'"""@en, """Versabschnitt von 'Parzival'"""@de;
	rdfs:comment """Verse section of about 50 dreissiger in Wolfram Von Eschenbach's verse novel 'Parzival', or a version or derivative thereof."""@en;
	rdfs:subClassOf text-structure:VerseSection, [
		a owl:Restriction; owl:onProperty parzival:isSectionOfNovel; owl:minCardinality "0"^^xsd:nonNegativeInteger], [
		a owl:Restriction; owl:onProperty parzival:isSectionOfNovelValue; owl:minCardinality "0"^^xsd:nonNegativeInteger].

parzival:CriticalEdition
	a owl:Class;
	rdfs:label """critical text edition of 'Parzival'"""@en, """kritische Textedition von 'Parzival'"""@de;
	rdfs:comment """Critical text edition of a transcript of Wolfram Von Eschenbach's verse novel 'Parzival'."""@en;
	rdfs:subClassOf textedit:CriticalEdition, publish:Expression.

parzival:ScientificEdition
	a owl:Class;
	rdfs:label """scientific text edition of 'Parzival'"""@en, """wissenschaftliche Textedition von 'Parzival'"""@de;
	rdfs:comment """Scientific text edition of a transcript of Wolfram Von Eschenbach's verse novel 'Parzival'."""@en;
	rdfs:subClassOf textedit:ScientificEdition, publish:Expression.

#
# PROPERTIES
#

parzival:isVerseOfDreissiger
	a owl:ObjectProperty;
	rdfs:label "is verse of dreissiger"@en, "ist Vers eines Dreissigers"@de;
	rdfs:comment """Relating a verse to a dreissiger it is part of."""@en;
	rdfs:domain parzival:Verse;
	rdfs:range parzival:Dreissiger;
	rdfs:subPropertyOf concept:isPartOf;
	knora-base:subjectClassConstraint parzival:Verse;
	knora-base:objectClassConstraint parzival:Dreissiger.

parzival:isVerseOfDreissigerValue
	a owl:ObjectProperty;
	rdfs:label "is verse of dreissiger - statement"@en, "ist Vers eines Dreissigers - Festlegung"@de;
	rdfs:comment """Relating a verse to a reification statement of the relation between the verse and a dreissiger it is part of."""@en;
	rdfs:subPropertyOf concept:isPartOfValue;
	knora-base:subjectClassConstraint parzival:Verse;
	knora-base:objectClassConstraint knora-base:LinkValue.

parzival:isDreissigerOfNovel
	a owl:ObjectProperty;
	rdfs:label "is dreissiger of verse novel"@en, "ist Dreissiger eines Versromans"@de;
	rdfs:comment """Relating a dreissiger to a verse novel it is part of."""@en;
	rdfs:domain parzival:Dreissiger;
	rdfs:range parzival:VerseNovel;
	rdfs:subPropertyOf concept:isPartOf;
	knora-base:subjectClassConstraint parzival:Dreissiger;
	knora-base:objectClassConstraint parzival:VerseNovel.

parzival:isDreissigerOfNovelValue
	a owl:ObjectProperty;
	rdfs:label "is dreissiger of verse novel - statement"@en, "ist Dreissiger eines Versromans - Festlegung"@de;
	rdfs:comment """Relating a dreissiger to a reification statement of the relation between the dreissiger and a verse novel it is part of."""@en;
	rdfs:subPropertyOf concept:isPartOfValue;
	knora-base:subjectClassConstraint parzival:Dreissiger;
	knora-base:objectClassConstraint knora-base:LinkValue.

parzival:dreissigerHasNumber
	a owl:ObjectProperty;
	rdfs:label "dreissiger has number"@en, "Dreissiger hat Nummer"@de;
	rdfs:comment """Relating a dreissiger to its number."""@en;
	rdfs:domain parzival:Dreissiger;
	rdfs:range parzival:DreissigerNumber;
	rdfs:subPropertyOf text-structure:hasIdentifier;
	knora-base:subjectClassConstraint parzival:Dreissiger;
	knora-base:objectClassConstraint parzival:DreissigerNumber.

parzival:dreissigerHasNumberValue
	a owl:ObjectProperty;
	rdfs:label "dreissiger has number - statement"@en, "Dreissiger hat Nummer - Festlegung"@de;
	rdfs:comment """Relating a dreissiger to a reification statement of the relation between the dreissiger and its number."""@en;
	rdfs:subPropertyOf text-structure:hasIdentifierValue;
	knora-base:subjectClassConstraint parzival:Dreissiger;
	knora-base:objectClassConstraint knora-base:LinkValue.

parzival:isSectionOfNovel
	a owl:ObjectProperty;
	rdfs:label """is verse section of verse novel 'Parzival'"""@en, """ist Versabschnitt des Versromans 'Parzival'"""@de;
	rdfs:comment """Relating a verse section to a version of Wolfram Von Eschenbach's verse novel 'Parzival'."""@en;
	rdfs:domain parzival:VerseSection;
	rdfs:range parzival:VerseNovel;
	rdfs:subPropertyOf text-structure:isVerseSectionOfVerseNovel;
	knora-base:subjectClassConstraint parzival:VerseSection;
	knora-base:objectClassConstraint parzival:VerseNovel.

parzival:isSectionOfNovelValue
	a owl:ObjectProperty;
	rdfs:label """is verse section of verse novel 'Parzival' - statement"""@en, """ist Versabschnitts des Versromans 'Parzival' - Festlegung"""@de;
	rdfs:comment """Relating a verse section to a reification statement of the relation between the verse section and a version of Wolfram Von Eschenbach's verse novel 'Parzival'."""@en;
	rdfs:subPropertyOf text-structure:isVerseSectionOfVerseNovelValue;
	knora-base:subjectClassConstraint parzival:VerseSection;
	knora-base:objectClassConstraint knora-base:LinkValue.