@prefix rdfs: <http://www.w3.org/2000/01/rdf-schema#>.
@prefix owl: <http://www.w3.org/2002/07/owl#>.
@prefix xsd: <http://www.w3.org/2001/XMLSchema#>.
@prefix skos: <http://www.w3.org/2004/02/skos/core#>.
@prefix dct: <http://purl.org/dc/terms/>.
@prefix foaf: <http://xmlns.com/foaf/0.1/>.
@prefix cidoc: <http://www.cidoc-crm.org/cidoc-crm/>.
@prefix frbroo: <http://iflastandards.info/ns/fr/frbr/frbroo/>.
@prefix event: <http://www.knora.org/ontology/shared/event#>.
@prefix human: <http://www.knora.org/ontology/shared/human#>.
@prefix language: <http://www.knora.org/ontology/shared/language#>.
@prefix concept: <http://www.knora.org/ontology/shared/concept#>.
@prefix document: <http://www.knora.org/ontology/shared/document#>.
@prefix text: <http://www.knora.org/ontology/shared/text#>.
@prefix text-structure: <http://www.knora.org/ontology/shared/text-structure#>.
@prefix infocar: <http://www.knora.org/ontology/shared/information-carrier#>.
@prefix publish: <http://www.knora.org/ontology/shared/publishing#>.
@prefix litera: <http://www.knora.org/ontology/shared/literature#>.
@prefix ling: <http://www.knora.org/ontology/shared/linguistics#>.
@prefix knora-base: <http://www.knora.org/ontology/knora-base#>.

@base <http://www.knora.org/ontology/shared/text-editing>.
@prefix textedit: <http://www.knora.org/ontology/shared/text-editing#>.

<http://www.knora.org/ontology/shared/text-editing>
	a owl:Ontology;
	dct:title "An ontology about text editing"@en;
	dct:description """Formal description of text editing, general subclasses, related classes, and properties."""@en;
	dct:creator "Hans Cools, MD, knowledge engineer, ontologist, software developer, NIE-INE, Basel University, Switzerland"@en;
	dct:contributor "Roberta Padlina, tool coordinator, NIE-INE, Basel University, Switzerland"@en;
	dct:publisher "Basel University, Switzerland"@en;
#	rdfs:seeAlso <https://digitallatin.github.io/guidelines/LDLT-Guidelines.html>;

	knora-base:attachedToProject <http://www.knora.org/ontology/knora-base#DefaultSharedOntologiesProject>. # <http://rdfh.ch/projects/005A>.

#
# CLASSES
#

textedit:Editor
	a owl:Class;
	rdfs:label "text editor"@en, "Text-Editor"@de;
	rdfs:comment """Role of a person changing a text."""@en;
	rdfs:subClassOf human:PersonCreator.

textedit:Edition
	a owl:Class;
	rdfs:label "text edition"@en, "Text-Edition"@de;
	rdfs:comment """Changed text as a result of editing."""@en;
	rdfs:subClassOf text:Text , [ # human:CreationVersion
		a owl:Restriction; owl:onProperty textedit:hasEditor; owl:minCardinality "0"^^xsd:nonNegativeInteger], [
		a owl:Restriction; owl:onProperty textedit:hasEditorValue; owl:minCardinality "0"^^xsd:nonNegativeInteger], [
		a owl:Restriction; owl:onProperty textedit:hasEditorialSymbol; owl:minCardinality "0"^^xsd:nonNegativeInteger].

textedit:EditorialSymbol
	a owl:Class;
	rdfs:label "editorial symbol"@en, "editorisches Zeichen"@de;
	rdfs:comment """Symbol in an edition indicating a textual aspect of the original text."""@en;
	rdfs:subClassOf ling:Literal.

# textedit:Compilator

textedit:Glossator
	a owl:Class;
	rdfs:label "glossator"@la, "glossator"@en, "Glossator"@de;
	rdfs:comment """Role of a person adding glosses to a text."""@en;
	rdfs:subClassOf textedit:Editor.

textedit:Redactor
	a owl:Class;
	rdfs:label "redactor"@la, "redactor"@en, "Redactor"@de;
	rdfs:comment """Editor assembling parts of texts to a new coherent text."""@en;
	rdfs:subClassOf textedit:Editor.

textedit:Abbreviator
	a owl:Class;
	rdfs:label "abbreviator"@en, "KurzfasserIn"@de, "abbreviator"@la;
	rdfs:comment """Editor shortening a text."""@en;
	rdfs:subClassOf textedit:Editor.

textedit:Abbreviation # derivative?
	a owl:Class;
	rdfs:label "abbreviation"@en, "Kurzfassung"@de;
	rdfs:comment """Shortened edition."""@en;
	rdfs:subClassOf textedit:Edition.

textedit:Paraphrase # derivative? # scientific?
	a owl:Class;
	rdfs:label "paraphrase"@en, "Paraphrase"@de;
	rdfs:comment """Edition restating a text clarifying its meaning."""@en;
	rdfs:subClassOf textedit:Edition.

textedit:LiteralExposition # derivative? # scientific?
	a owl:Class;
	rdfs:label "literal exposition"@en, "wörtliche Auslegung"@de;
	rdfs:comment """Edition providing background information on word level to a text in clarifying its meaning."""@en;
	rdfs:subClassOf textedit:Edition.

textedit:Transliteration
	a owl:Class;
	rdfs:label "transliteration"@en, "Transliteration"@de, "translittération"@fr, "traslitterazione"@it;
	rdfs:comment """Written text transferred in another alphabet using the closest corresponding symbols, e.g. letters."""@en;
	skos:note """Primarily representing the symbols, not the sounds."""@en;
	rdfs:subClassOf text:WrittenText, textedit:Edition.

textedit:DerivedTextExpression
	a owl:Class;
	rdfs:label "derived text expression"@en, "abgeleitete Textexpression"@de;
	rdfs:comment """Text expression derived from another text expression with content changed beyond a version."""@en;
	rdfs:subClassOf text:Expression, human:CreationDerivative, textedit:Edition.

textedit:EditionScientist
	a owl:Class;
	rdfs:label "edition scientist"@en, "EditionswissenschaftlerIn"@de;
	rdfs:comment """Role of a person practicing edition science."""@en;
	rdfs:subClassOf human:Scientist.

textedit:ScientificEditor
	a owl:Class;
	rdfs:label "scientific editor"@en, "wissenschaftliche Editor"@de, "éditrice scientifique"@fr;
	rdfs:comment """Role of a person editing scientific text."""@en;
	skos:note """Different from an editor of scientific literature, who is not necessarily a scientist."""@en;
	rdfs:subClassOf textedit:Editor, textedit:EditionScientist.

textedit:ScientificEdition
	a owl:Class;
	rdfs:label "scientific edition"@en, "wissenschaftliche Edition"@de;
	rdfs:comment """Derived text expression edited for scientific purpose."""@en;
	rdfs:subClassOf textedit:DerivedTextExpression , [
		a owl:Restriction; owl:onProperty textedit:hasScientificEditor; owl:minCardinality "0"^^xsd:nonNegativeInteger], [
		a owl:Restriction; owl:onProperty textedit:hasScientificEditorValue; owl:minCardinality "0"^^xsd:nonNegativeInteger].

textedit:DiplomaticTranscription
	a owl:Class;
	rdfs:label "diplomatic transcription"@en, "diplomatische Umschrift"@de;
#	ling:hasSynonym "Lesehilfe"@de;
	rdfs:comment """Transcription of a text with diacritical signs indicating visual textual properties to describe the textual state."""@en;
	skos:note """Mostly autographs or juridical; without interpretation""";
	rdfs:subClassOf textedit:ScientificEdition, [
		a owl:Restriction; owl:onProperty textedit:hasPageIndicator; owl:minCardinality "0"^^xsd:nonNegativeInteger], [
		a owl:Restriction; owl:onProperty textedit:hasPageNumberIndicator; owl:minCardinality "0"^^xsd:nonNegativeInteger], [
		a owl:Restriction; owl:onProperty textedit:hasColumnIndicator; owl:minCardinality "0"^^xsd:nonNegativeInteger], [
		a owl:Restriction; owl:onProperty textedit:isDiplomaticTranscriptionOfTextOnPage; owl:minCardinality "0"^^xsd:nonNegativeInteger], [
		a owl:Restriction; owl:onProperty textedit:isDiplomaticTranscriptionOfTextOnPageValue; owl:minCardinality "0"^^xsd:nonNegativeInteger].

# textedit:Diplomatic-InterpretativeTranscription

textedit:CriticalEditor
	a owl:Class;
	rdfs:label "critical text editor"@en, "kritische Text-Editor"@de;
	rdfs:comment """Role of being a scientist editing a text expression in a critical scientific way."""@en;
	rdfs:subClassOf human:Scientist, human:PersonCreator.

textedit:CriticalEdition
	a owl:Class;
	rdfs:label "critical text edition"@en, "kritische Textedition"@de;
	rdfs:comment """Edition to which a critical editor added evidence and interpretation of a text creation and historical transmission, using a critical apparatus, allowing readers to assess the editor's choice."""@en;
	rdfs:subClassOf textedit:ScientificEdition, [
		a owl:Restriction; owl:onProperty textedit:hasCriticalEditor; owl:minCardinality "0"^^xsd:nonNegativeInteger], [
		a owl:Restriction; owl:onProperty textedit:hasCriticalEditorValue; owl:minCardinality "0"^^xsd:nonNegativeInteger].

# textedit:Variorum rdfs:subClassOf textedit:CriticalEdition

textedit:GeneticEdition
	a owl:Class;
	rdfs:label "genetic edition"@en, "genetische Edition"@de, "édition génétique"@fr, "edizione genetica"@it;
	rdfs:comment """Critical edition accounting for the modifications by the author."""@en;
	rdfs:subClassOf textedit:CriticalEdition.

textedit:ConstitutedEdition
	a owl:Class;
	rdfs:label "constituted text edition"@en, "konstituierter Text Edition"@de;
#	ling:hasSynonym "Lesetext"@de;
	rdfs:comment """Plain text expression as endresult of critical editing of another text expression."""@en;
	rdfs:subClassOf textedit:ScientificEdition.

textedit:EditorialStructure
	a owl:Class;
	rdfs:label "editorial text structure"@en, "editorische Textstruktur"@de;
	rdfs:comment """Scientific text structure depending on editorial purpose, e.g. an editing apparatus."""@en;
	rdfs:subClassOf text-structure:ScientificStructure.	

textedit:Apparatus
	a owl:Class;
	rdfs:label "editing apparatus"@en, "Edierungsapparatus"@de, "apparatus editionis"@la;
	rdfs:comment """Editorial compositional structure to analyse text in a scientific edition along certain criteria."""@en;
	rdfs:subClassOf textedit:EditorialStructure, text-structure:CompositionalContentStructure, [
		a owl:Restriction; owl:onProperty textedit:isApparatusOf; owl:minCardinality "0"^^xsd:nonNegativeInteger], [
		a owl:Restriction; owl:onProperty textedit:isApparatusOfValue; owl:minCardinality "0"^^xsd:nonNegativeInteger].

textedit:ApparatusEntry
	a owl:Class;
	rdfs:label "editing apparatus entry"@en, "Edierungsapparateintrag"@de; #, "entrée d'apparat éditionel"@fr, "iscrizione del apparato"@it;
	rdfs:comment """Entry of an editing apparatus."""@en;
	rdfs:subClassOf textedit:EditorialStructure, text-structure:CompositionalContentStructure, [
		a owl:Restriction; owl:onProperty textedit:isEntryOfApparatus; owl:minCardinality "0"^^xsd:nonNegativeInteger], [
		a owl:Restriction; owl:onProperty textedit:isEntryOfApparatusValue; owl:minCardinality "0"^^xsd:nonNegativeInteger], [
		a owl:Restriction; owl:onProperty textedit:hasApparatusEnteringDate; owl:minCardinality "0"^^xsd:nonNegativeInteger].

textedit:DoctrinalApparatus
	a owl:Class;
	rdfs:label "doctrinal apparatus"@en, "doktrinal Apparat"@de;
#	ling:hasSynonym textedit:HistoricalApparatus;
	rdfs:comment """Editing apparatus commmenting on the content of a scientific text edition in a historical and doctrinal context."""@en; # info about theory
	rdfs:subClassOf textedit:Apparatus, [
		a owl:Restriction; owl:onProperty textedit:isDoctrinalApparatusOf; owl:minCardinality "0"^^xsd:nonNegativeInteger], [
		a owl:Restriction; owl:onProperty textedit:isDoctrinalApparatusOfValue; owl:minCardinality "0"^^xsd:nonNegativeInteger].

textedit:DoctrinalApparatusEntry
	a owl:Class;
	rdfs:label "doctrinal apparatus entry"@en, "doktrinaler Apparateintrag"@de; #, "entrée d'apparat doctrine"@fr, "iscrizione del apparato doctrino"@it;
	rdfs:comment """Entry of a doctrinal apparatus."""@en;
	rdfs:subClassOf textedit:ApparatusEntry, [
		a owl:Restriction; owl:onProperty textedit:isEntryOfDoctrinalApparatus; owl:minCardinality "0"^^xsd:nonNegativeInteger], [
		a owl:Restriction; owl:onProperty textedit:isEntryOfDoctrinalApparatusValue; owl:minCardinality "0"^^xsd:nonNegativeInteger].

textedit:ApparatusFontium
	a owl:Class;
	rdfs:label "apparatus fontium"@en, "Apparatus Fontium"@de, "apparatus fontium"@la;
	rdfs:comment """Editing apparatus containing references to one or more citations."""@en;
	rdfs:subClassOf textedit:Apparatus, [
		a owl:Restriction; owl:onProperty textedit:isApparatusFontiumOf; owl:minCardinality "0"^^xsd:nonNegativeInteger], [
		a owl:Restriction; owl:onProperty textedit:isApparatusFontiumOfValue; owl:minCardinality "0"^^xsd:nonNegativeInteger].

textedit:ApparatusFontiumEntry
	a owl:Class;
	rdfs:label "apparatus fontium entry"@en, "Apparatus Fontium-Eintrag"@de; #, "entrée d'apparat "@fr, "iscrizione del apparato "@it;
	rdfs:comment """Entry of an apparatus fontium."""@en;
	rdfs:subClassOf textedit:ApparatusEntry, [
		a owl:Restriction; owl:onProperty textedit:isEntryOfApparatusFontium; owl:minCardinality "0"^^xsd:nonNegativeInteger], [
		a owl:Restriction; owl:onProperty textedit:isEntryOfApparatusFontiumValue; owl:minCardinality "0"^^xsd:nonNegativeInteger].

# textedit:hasCitationReference

textedit:CriticalApparatus
	a owl:Class;
	rdfs:label "critical apparatus"@en, "textkritischer Apparat"@de, "apparat critique"@fr, "apparato critico"@it, "apparatus criticus"@la;
	rdfs:comment """Editing apparatus to a critical text edition providing information of textual versions."""@en;
	rdfs:subClassOf textedit:Apparatus, [
		a owl:Restriction; owl:onProperty textedit:isCriticalApparatusOf; owl:minCardinality "0"^^xsd:nonNegativeInteger], [
		a owl:Restriction; owl:onProperty textedit:isCriticalApparatusOfValue; owl:minCardinality "0"^^xsd:nonNegativeInteger].

textedit:CriticalApparatusEntry
	a owl:Class;
	rdfs:label "critical apparatus entry"@en, "textkritischer Apparateintrag"@de, "entrée d'apparat critique"@fr, "iscrizione del apparato critico"@it;
	rdfs:comment """Entry of critical apparatus."""@en;
	rdfs:subClassOf textedit:ApparatusEntry, [
		a owl:Restriction; owl:onProperty textedit:isEntryOfCriticalApparatus; owl:minCardinality "0"^^xsd:nonNegativeInteger], [
		a owl:Restriction; owl:onProperty textedit:isEntryOfCriticalApparatusValue; owl:minCardinality "0"^^xsd:nonNegativeInteger].

textedit:StructureApparatus
	a owl:Class;
	rdfs:label "text structure apparatus"@en, "Textstruktur-Apparat"@de;
	rdfs:comment """Editing apparatus to a critical text edition providing information of text structure."""@en;
	rdfs:subClassOf textedit:Apparatus.

textedit:StructureApparatusEntry
	a owl:Class;
	rdfs:label "structure apparatus entry"@en, "Textstruktur-Apparateintrag"@de; #, "entrée d'apparat de structure"@fr, "iscrizione del apparato del "@it;
	rdfs:comment """Entry of text structure apparatus."""@en;
	rdfs:subClassOf textedit:ApparatusEntry, [
		a owl:Restriction; owl:onProperty textedit:isEntryOfStructureApparatus; owl:minCardinality "0"^^xsd:nonNegativeInteger], [
		a owl:Restriction; owl:onProperty textedit:isEntryOfStructureApparatusValue; owl:minCardinality "0"^^xsd:nonNegativeInteger].

textedit:StructureDescription
	a owl:Class;
	rdfs:label "text structure description"@en, "Textstrukturdeskription"@de;
	rdfs:comment """Description of a text structure in a structure apparatus."""@en;
	rdfs:subClassOf textedit:EditorialStructure, [
		a owl:Restriction; owl:onProperty textedit:isStructureDescriptionOfEntry; owl:minCardinality "0"^^xsd:nonNegativeInteger], [
		a owl:Restriction; owl:onProperty textedit:isStructureDescriptionOfEntryValue; owl:minCardinality "0"^^xsd:nonNegativeInteger], [
		a owl:Restriction; owl:onProperty textedit:structureDescriptionHasContent; owl:minCardinality "0"^^xsd:nonNegativeInteger].

textedit:Reading
	a owl:Class;
	rdfs:label "reading"@en, "Textinterpretation"@de, "lezione"@it, "lectio"@la;
	rdfs:comment """Copy of one or more words or phrases of a witness."""@en;
	rdfs:subClassOf textedit:EditorialStructure, text:CopiedText, [
		a owl:Restriction; owl:onProperty textedit:hasSiglum; owl:minCardinality "0"^^xsd:nonNegativeInteger], [
		a owl:Restriction; owl:onProperty textedit:hasSiglumValue; owl:minCardinality "0"^^xsd:nonNegativeInteger].

textedit:Siglum
	a owl:Class;
	rdfs:label "siglum"@en, "Siglum"@de, "siglum"@fr, "siglum"@it;
	rdfs:comment """One or more symbols as a reference to an expression as original or witness."""@en;
	rdfs:subClassOf document:ExpressionReference, [
		a owl:Restriction; owl:onProperty textedit:isSiglumOfScientificEdition; owl:minCardinality "0"^^xsd:nonNegativeInteger], [
		a owl:Restriction; owl:onProperty textedit:isSiglumOfScientificEditionValue; owl:minCardinality "0"^^xsd:nonNegativeInteger], [
		a owl:Restriction; owl:onProperty textedit:siglumHasIdentifier; owl:minCardinality "0"^^xsd:nonNegativeInteger], [
		a owl:Restriction; owl:onProperty textedit:siglumHasIdentifierValue; owl:minCardinality "0"^^xsd:nonNegativeInteger], [
		a owl:Restriction; owl:onProperty textedit:siglumHasWitnessIdentifier; owl:minCardinality "0"^^xsd:nonNegativeInteger], [
		a owl:Restriction; owl:onProperty textedit:siglumHasWitnessIdentifierValue; owl:minCardinality "0"^^xsd:nonNegativeInteger].

textedit:Witness
	a owl:Class;
	rdfs:label "witness text"@en, "Textzeuge"@de;
	rdfs:comment """Copy of a text studied in a critical edition, as comparison or proof of existance of the original by looking for features of originality, possibly enabling the original's reconstruction."""@en;
	rdfs:subClassOf text:CopiedText, text:Expression, [
		a owl:Restriction; owl:onProperty textedit:witnessHasIdentifier; owl:minCardinality "0"^^xsd:nonNegativeInteger], [
		a owl:Restriction; owl:onProperty textedit:witnessHasIdentifierValue; owl:minCardinality "0"^^xsd:nonNegativeInteger], [
		a owl:Restriction; owl:onProperty textedit:isWitnessOf; owl:minCardinality "0"^^xsd:nonNegativeInteger], [
		a owl:Restriction; owl:onProperty textedit:isWitnessOfValue; owl:minCardinality "0"^^xsd:nonNegativeInteger].

textedit:WitnessIdentifier
	a owl:Class;
	rdfs:label "witness text identifier"@en, "Textzeugeidentifikator"@de;
	rdfs:comment """Identifier of a witness text expression."""@en;
	rdfs:subClassOf document:ExpressionIdentifier.

textedit:Lemma
	a owl:Class;
	rdfs:label "lemma"@en, "Lemma"@de, "lemma"@fr, "lemma"@it;
	rdfs:comment """Editorial structure with a copy of one or more words or phrases in an apparatus entry referring to its edition text, and possibly as appearing in a witness or created by an editor, and judged by the editor to be authentic, accurate, and/or authoritative, and compaired with variants referring to other witnesses"""@en;
	skos:note """In an apparatus entry a lemma is mostly seperated from a variant or editorial explanation by a right square bracket ']'."""@en;
	rdfs:subClassOf textedit:EditorialStructure, [
		a owl:Restriction; owl:onProperty textedit:isLemmaOfCriticalEntry; owl:minCardinality "0"^^xsd:nonNegativeInteger], [
		a owl:Restriction; owl:onProperty textedit:isLemmaOfCriticalEntryValue; owl:minCardinality "0"^^xsd:nonNegativeInteger], [
		a owl:Restriction; owl:onProperty textedit:isLemmaOfDoctrinalEntry; owl:minCardinality "0"^^xsd:nonNegativeInteger], [
		a owl:Restriction; owl:onProperty textedit:isLemmaOfDoctrinalEntryValue; owl:minCardinality "0"^^xsd:nonNegativeInteger], [
		a owl:Restriction; owl:onProperty textedit:lemmaHasReference; owl:minCardinality "0"^^xsd:nonNegativeInteger], [
		a owl:Restriction; owl:onProperty textedit:lemmaHasReferenceValue; owl:minCardinality "0"^^xsd:nonNegativeInteger], [
		a owl:Restriction; owl:onProperty textedit:lemmaHasVariant; owl:minCardinality "0"^^xsd:nonNegativeInteger], [
		a owl:Restriction; owl:onProperty textedit:lemmaHasVariantValue; owl:minCardinality "0"^^xsd:nonNegativeInteger], [
		a owl:Restriction; owl:onProperty textedit:lemmaHasComment; owl:minCardinality "0"^^xsd:nonNegativeInteger], [
		a owl:Restriction; owl:onProperty textedit:lemmaHasCommentValue; owl:minCardinality "0"^^xsd:nonNegativeInteger].

textedit:WitnessedLemma
	a owl:Class;
	rdfs:label "witnessed lemma"@en, "bezeugtes Lemma"@de; #, "lemma"@fr, "lemma"@it;
	rdfs:comment """Lemma with a witness."""@en;
	rdfs:subClassOf textedit:Lemma.

textedit:Conjecture
	a owl:Class;
	rdfs:label "conjecture"@en, "Konjektur"@de;
	rdfs:comment """Witness-independent lemma expressly proposed to be of interest but absent in the main text of an edition."""@en;
	rdfs:subClassOf textedit:Lemma.

textedit:Emendation
	a owl:Class;
	rdfs:label "emendation"@en, "Emendation"@de, "émendation"@fr, "emendazione"@it;
	rdfs:comment """Conjecture accepted by the editor in the main text of an edition."""@en;
	rdfs:subClassOf textedit:Conjecture.

textedit:Variant
	a owl:Class;
	rdfs:label "variant"@en, "Variant"@de, "variante"@fr, "variante"@it;
	rdfs:comment """Reading of a critical apparatus entry, judged by an editor to be unsatisfactory for linguistic and/or stylistic reasons, but of interest for establishing the text, and as such varying from what the editor has judged to be the lemma."""@en;
	skos:note """Absence in a witness of respective part is commented."""@en;
	rdfs:subClassOf textedit:Reading, [
		a owl:Restriction; owl:onProperty textedit:isVariantOfEntry; owl:minCardinality "0"^^xsd:nonNegativeInteger], [
		a owl:Restriction; owl:onProperty textedit:isVariantOfEntryValue; owl:minCardinality "0"^^xsd:nonNegativeInteger], [
		a owl:Restriction; owl:onProperty textedit:variantHasReference; owl:minCardinality "0"^^xsd:nonNegativeInteger], [
		a owl:Restriction; owl:onProperty textedit:variantHasReferenceValue; owl:minCardinality "0"^^xsd:nonNegativeInteger], [
		a owl:Restriction; owl:onProperty textedit:variantHasComment; owl:minCardinality "0"^^xsd:nonNegativeInteger], [
		a owl:Restriction; owl:onProperty textedit:variantHasCommentValue; owl:minCardinality "0"^^xsd:nonNegativeInteger].

textedit:EditorialComment
	a owl:Class;
	rdfs:label "editorial comment"@en, "editorische Kommentar"@de; #, ""@fr, ""@it;
	rdfs:comment """Comment in a scientific edition."""@en;
	rdfs:subClassOf textedit:EditorialStructure, [
		a owl:Restriction; owl:onProperty textedit:isCommentOn; owl:minCardinality "0"^^xsd:nonNegativeInteger], [
		a owl:Restriction; owl:onProperty textedit:isCommentOnValue; owl:minCardinality "0"^^xsd:nonNegativeInteger], [
		a owl:Restriction; owl:onProperty textedit:isCommentOfScientificEdition; owl:minCardinality "0"^^xsd:nonNegativeInteger], [
		a owl:Restriction; owl:onProperty textedit:isCommentOfScientificEditionValue; owl:minCardinality "0"^^xsd:nonNegativeInteger], [
		a owl:Restriction; owl:onProperty textedit:isCommentOfEntry; owl:minCardinality "0"^^xsd:nonNegativeInteger], [
		a owl:Restriction; owl:onProperty textedit:isCommentOfEntryValue; owl:minCardinality "0"^^xsd:nonNegativeInteger], [
		a owl:Restriction; owl:onProperty textedit:commentHasReference; owl:minCardinality "0"^^xsd:nonNegativeInteger], [
		a owl:Restriction; owl:onProperty textedit:commentHasReferenceValue; owl:minCardinality "0"^^xsd:nonNegativeInteger], [
		a owl:Restriction; owl:onProperty textedit:commentHasContent; owl:minCardinality "0"^^xsd:nonNegativeInteger].

#
# PROPERTIES
#

textedit:hasEditor
	a owl:ObjectProperty;
	rdfs:label "edition has editor"@en, "Edition hat Editor"@de;
	rdfs:comment """Relating an edition to a person who created it."""@en;
	rdfs:domain textedit:Edition;
#	rdfs:range [rdfs:subClassOf human:Person, [a owl:Restriction; owl:onProperty human:personHasRole; owl:someValuesFrom textedit:Editor]];
	rdfs:subPropertyOf knora-base:hasLinkTo;
	knora-base:subjectClassConstraint textedit:Edition;
	knora-base:objectClassConstraint human:Person.

textedit:hasEditorValue
	a owl:ObjectProperty;
	rdfs:label "edition has editor - statement"@en, "Edition hat Editor - Festlegung"@de;
	rdfs:comment """Relating an edition to a reification statement of the relation between the edition and a person who created it."""@en;
	rdfs:subPropertyOf knora-base:hasLinkToValue;
	knora-base:subjectClassConstraint textedit:Edition;
	knora-base:objectClassConstraint knora-base:LinkValue.

textedit:hasEditorialSymbol
	a owl:ObjectProperty;
	rdfs:label "has editorial symbol"@en, "hat editorisches Zeichen"@de;
	rdfs:comment """Relating an edition to a symbol indicating a textual aspect of the original text."""@en;
	rdfs:domain textedit:Edition;
#	rdfs:range textedit:EditorialSymbol;
	rdfs:subPropertyOf language:hasContent;
	knora-base:subjectClassConstraint textedit:Edition;
	knora-base:objectClassConstraint knora-base:TextValue.

textedit:hasRedactor
	a owl:ObjectProperty;
	rdfs:label "has redactor"@en, "hat Redaktor"@de;
	rdfs:comment """Relating a text to a person who redacted it."""@en;
	rdfs:domain text:Text;
#	rdfs:range [rdfs:subClassOf human:Person, [a owl:Restriction; owl:onProperty human:personHasRole; owl:someValuesFrom textedit:Redactor]];
	rdfs:subPropertyOf knora-base:hasLinkTo;
	knora-base:subjectClassConstraint text:Text;
	knora-base:objectClassConstraint human:Person.

textedit:hasRedactorValue
	a owl:ObjectProperty;
	rdfs:label "has redactor - statement"@en, "hat Redaktor - Festlegung"@de;
	rdfs:comment """Relating a text to a reification statement of the relation between the text and a person who redacted it."""@en;
	rdfs:subPropertyOf knora-base:hasLinkToValue;
	knora-base:subjectClassConstraint text:Text;
	knora-base:objectClassConstraint knora-base:LinkValue.

textedit:hasGlossator
	a owl:ObjectProperty;
	rdfs:label "has glossator"@en, "hat Glossator"@de;
	rdfs:comment """Relating a text to a person who glossed it."""@en;
	rdfs:domain text:Text;
#	rdfs:range [rdfs:subClassOf human:Person, [a owl:Restriction; owl:onProperty human:personHasRole; owl:someValuesFrom text:Glossator]];
	rdfs:subPropertyOf knora-base:hasLinkTo;
	knora-base:subjectClassConstraint text:Text;
	knora-base:objectClassConstraint human:Person.

textedit:hasGlossatorValue
	a owl:ObjectProperty;
	rdfs:label "has glossator - statement"@en, "hat Glossator - Festlegung"@de;
	rdfs:comment """Relating a text to a reification statement of the relation between the text and a person who glossed it."""@en;
	rdfs:subPropertyOf knora-base:hasLinkToValue;
	knora-base:subjectClassConstraint text:Text;
	knora-base:objectClassConstraint knora-base:LinkValue.

textedit:hasAbbreviator
	a owl:ObjectProperty;
	rdfs:label "has abbreviator"@en, "hat Abkurzer"@de;
	rdfs:comment """Relating a text to a person who abbreviated it."""@en;
	rdfs:domain text:Text;
#	rdfs:range [rdfs:subClassOf human:Person, [a owl:Restriction; owl:onProperty human:personHasRole; owl:someValuesFrom text:Abbreviator]];
	rdfs:subPropertyOf knora-base:hasLinkTo;
	knora-base:subjectClassConstraint text:Text;
	knora-base:objectClassConstraint human:Person.

textedit:hasAbbreviatorValue
	a owl:ObjectProperty;
	rdfs:label "has abbreviator - statement"@en, "hat Abkurzer - Festlegung"@de;
	rdfs:comment """Relating a text to a reification statement of the relation between the text and a person who abbreviated it."""@en;
	rdfs:subPropertyOf knora-base:hasLinkToValue;
	knora-base:subjectClassConstraint text:Text;
	knora-base:objectClassConstraint knora-base:LinkValue.

textedit:hasEdition
	a owl:ObjectProperty;
	rdfs:label "text has edition"@en, "Text hat Edition"@de;
	rdfs:comment "Relating a text to an edition it has."@en;
	rdfs:domain text:Text;
	rdfs:range textedit:Edition;
	rdfs:subPropertyOf knora-base:hasLinkTo;
	knora-base:subjectClassConstraint text:Text;
	knora-base:objectClassConstraint textedit:Edition.

textedit:hasEditionValue
	a owl:ObjectProperty;
	rdfs:label "text has edition - statement"@en, "Text hat Edition - Festlegung"@de;
	rdfs:comment "Relating a text to a reification statement of the relation between the text and an edition thereof."@en;
	rdfs:subPropertyOf knora-base:hasLinkToValue;
	knora-base:subjectClassConstraint text:Text;
	knora-base:objectClassConstraint knora-base:LinkValue.

textedit:hasSameEditionAs
	a owl:ObjectProperty;
	rdfs:label "has same edition as"@en, "hat gleiche Edition als"@de;
	rdfs:comment """Relating two texts with a same edition."""@en;
	rdfs:domain text:Text;
	rdfs:range text:Text;
	rdfs:subPropertyOf knora-base:hasLinkTo;
	knora-base:subjectClassConstraint text:Text;
	knora-base:objectClassConstraint text:Text.

textedit:hasSameEditionAsValue
	a owl:ObjectProperty;
	rdfs:label "has same edition as - statement"@en, "hat gleiche Edition als - Festlegung"@de;
	rdfs:comment """Relating a text to a reification statement of the relation between the text and another one with a same edition."""@en;
	rdfs:subPropertyOf knora-base:hasLinkToValue;
	knora-base:subjectClassConstraint text:Text;
	knora-base:objectClassConstraint knora-base:LinkValue.

textedit:hasTransliteration
	a owl:ObjectProperty;
	rdfs:label "has transliteration"@en, "hat Transliteration"@de;
	rdfs:comment """Relating a text to a transliteration thereof."""@en;
	rdfs:domain text:Text;
	rdfs:range textedit:Transliteration;
	rdfs:subPropertyOf knora-base:hasLinkTo;
	knora-base:subjectClassConstraint text:Text;
	knora-base:objectClassConstraint textedit:Transliteration.

textedit:hasTransliterationValue
	a owl:ObjectProperty;
	rdfs:label "has transliteration - statement"@en, "hat Transliteration - Festlegung"@de;
	rdfs:comment """Relating a text to a reification statement of the relation between the text and a transliteration thereof."""@en;
	rdfs:subPropertyOf knora-base:hasLinkToValue;
	knora-base:subjectClassConstraint text:Text;
	knora-base:objectClassConstraint knora-base:LinkValue.

textedit:hasDerivedTextExpression
	a owl:ObjectProperty;
	rdfs:label "has derived text expression"@en, "hat abgeleitete Textexpression"@de;
	rdfs:comment "Relating a text expression to another one derived from it."@en;
	rdfs:domain text:Expression;
	rdfs:range textedit:DerivedTextExpression;
	rdfs:subPropertyOf knora-base:hasLinkTo;
	knora-base:subjectClassConstraint text:Expression;
	knora-base:objectClassConstraint textedit:DerivedTextExpression.

textedit:hasDerivedTextExpressionValue
	a owl:ObjectProperty;
	rdfs:label "has derived text expression - statement"@en, "hat abgeleitete Textexpression - Festlegung"@de;
	rdfs:comment "Relating a text expression to a reification statement of the relation between the text expression and another one derived from it."@en;
	rdfs:subPropertyOf knora-base:hasLinkToValue;
	knora-base:subjectClassConstraint text:Expression;
	knora-base:objectClassConstraint knora-base:LinkValue.

textedit:hasScientificEdition
	a owl:ObjectProperty;
	rdfs:label "has scientific text edition"@en, "hat wissenschaftliche Textedition"@de;
	rdfs:comment "Relating a text expression to a scientific edition thereof."@en;
	rdfs:domain text:Expression;
	rdfs:range textedit:ScientificEdition;
	rdfs:subPropertyOf textedit:hasDerivedTextExpression;
	knora-base:subjectClassConstraint text:Expression;
	knora-base:objectClassConstraint textedit:ScientificEdition.

textedit:hasScientificEditionValue
	a owl:ObjectProperty;
	rdfs:label "has scientific text edition - statement"@en, "hat wissenschaftliche Textedition - Festlegung"@de;
	rdfs:comment "Relating a text expression to a reification statement of the relation between the text expression and a scientific edition thereof."@en;
	rdfs:subPropertyOf textedit:hasDerivedTextExpressionValue;
	knora-base:subjectClassConstraint text:Expression;
	knora-base:objectClassConstraint knora-base:LinkValue.

textedit:hasScientificEditor
	a owl:ObjectProperty;
	rdfs:label "scientific edition has scientific editor"@en, "wissenschaftliche Edition hat wissenschaftliche Editor"@de;
	rdfs:comment "Relating a scientific edition to a scientific editor who created it."@en;
	rdfs:domain textedit:ScientificEdition;
#	rdfs:range [rdfs:subClassOf human:Person, [a owl:Restriction; owl:onProperty human:personHasRole; owl:someValuesFrom textedit:ScientificEditor]];
	rdfs:subPropertyOf knora-base:hasLinkTo; # textedit:hasEditor
	knora-base:subjectClassConstraint textedit:ScientificEdition;
	knora-base:objectClassConstraint human:Person.

textedit:hasScientificEditorValue
	a owl:ObjectProperty;
	rdfs:label "scientific edition has scientific editor - statement"@en, "wissenschaftliche Edition hat wissenschaftliche Editor - Festlegung"@de;
	rdfs:comment "Relating a scientific edition to a reification statement of the relation between the scientific edition and a scientific editor who created it."@en;
	rdfs:subPropertyOf knora-base:hasLinkToValue;
	knora-base:subjectClassConstraint textedit:ScientificEdition;
	knora-base:objectClassConstraint knora-base:LinkValue.

textedit:hasDiplomaticTranscription
	a owl:ObjectProperty;
	rdfs:label "has diplomatic transcription"@en, "hat diplomatische Umschrift"@de;
	rdfs:comment "Relating a text to a diplomatic transcription thereof."@en;
	rdfs:domain text:Expression;
	rdfs:range textedit:DiplomaticTranscription;
	rdfs:subPropertyOf textedit:hasScientificEdition;
	knora-base:subjectClassConstraint text:Expression;
	knora-base:objectClassConstraint textedit:DiplomaticTranscription.

textedit:hasDiplomaticTranscriptionValue
	a owl:ObjectProperty;
	rdfs:label "has diplomatic transcription - statement"@en, "hat diplomatische Umschrift - Festlegung"@de;
	rdfs:comment "Relating a text to a reification statement of the relation between the text and a diplomatic transcription thereof."@en;
	rdfs:subPropertyOf textedit:hasScientificEditionValue;
	knora-base:subjectClassConstraint text:Expression;
	knora-base:objectClassConstraint knora-base:LinkValue.

textedit:hasPageIndicator
	a owl:ObjectProperty;
	rdfs:label "has page indicator"@en, "hat Seite-Indikator"@de;
	rdfs:comment """Relating a derived text expression to a diacritical sign that indicates where a page starts."""@en;
	rdfs:subPropertyOf textedit:hasEditorialSymbol;
	knora-base:subjectClassConstraint textedit:DiplomaticTranscription;
	knora-base:objectClassConstraint knora-base:TextValue.

textedit:hasPageNumberIndicator
	a owl:ObjectProperty;
	rdfs:label "has page number indicator"@en, "hat Seitennummer-Indikator"@de;
	rdfs:comment """Relating a derived text expression to a diacritical sign that indicates the number of a page."""@en;
	rdfs:subPropertyOf textedit:hasEditorialSymbol;
	knora-base:subjectClassConstraint textedit:DiplomaticTranscription;
	knora-base:objectClassConstraint knora-base:TextValue.

textedit:hasColumnIndicator
	a owl:ObjectProperty;
	rdfs:label "has column indicator"@en, "hat Spalte-Indikator"@de;
	rdfs:comment """Relating a derived text expression to a diacritical sign that indicates where on a page a column starts."""@en;
	rdfs:subPropertyOf textedit:hasEditorialSymbol;
	knora-base:subjectClassConstraint textedit:DiplomaticTranscription;
	knora-base:objectClassConstraint knora-base:TextValue.

textedit:isDiplomaticTranscriptionOfTextOnPage
	a owl:ObjectProperty;
	rdfs:label "is diplomatic transcription of text on page"@en, "ist diplomatische Umschrift des Textes auf Seite"@de;
	rdfs:comment "Relating a diplomatic transcription to a page its source text is on."@en;
	rdfs:domain textedit:DiplomaticTranscription;
	rdfs:range infocar:Page;
	rdfs:subPropertyOf knora-base:hasLinkTo;
	knora-base:subjectClassConstraint textedit:DiplomaticTranscription;
	knora-base:objectClassConstraint infocar:Page.

textedit:isDiplomaticTranscriptionOfTextOnPageValue
	a owl:ObjectProperty;
	rdfs:label "is diplomatic transcription of text on page - statement"@en, "ist diplomatische Umschrift des Textes auf Seite - Festlegung"@de;
	rdfs:comment "Relating a diplomatic transcription to a reification statement of the relation between the diplomatic transcription and a page its source text is on."@en;
	rdfs:subPropertyOf knora-base:hasLinkToValue;
	knora-base:subjectClassConstraint textedit:DiplomaticTranscription;
	knora-base:objectClassConstraint knora-base:LinkValue.

textedit:hasCriticalEdition
	a owl:ObjectProperty;
	rdfs:label "has critical text edition"@en, "hat kritische Textedition"@de;
	rdfs:comment "Relating a text expression to a critical edition thereof."@en;
	rdfs:domain text:Expression;
	rdfs:range textedit:CriticalEdition;
	rdfs:subPropertyOf textedit:hasScientificEdition;
	knora-base:subjectClassConstraint text:Expression;
	knora-base:objectClassConstraint textedit:CriticalEdition.

textedit:hasCriticalEditionValue
	a owl:ObjectProperty;
	rdfs:label "has critical text edition - statement"@en, "hat kritische Textedition - Festlegung"@de;
	rdfs:comment "Relating a text expression to a reification statement of the relation between the text and a critical edition thereof."@en;
	rdfs:subPropertyOf textedit:hasScientificEditionValue;
	knora-base:subjectClassConstraint text:Expression;
	knora-base:objectClassConstraint knora-base:LinkValue.

textedit:hasCriticalEditor
	a owl:ObjectProperty;
	rdfs:label "has critical editor"@en, "hat kritische Editor"@de;
	rdfs:comment "Relating a critical edition to a critical editor who created it."@en;
	rdfs:domain textedit:CriticalEdition;
#	rdfs:range [rdfs:subClassOf human:Person, [a owl:Restriction; owl:onProperty human:personHasRole; owl:someValuesFrom textedit:CriticalEditor]];
	rdfs:subPropertyOf knora-base:hasLinkTo; # textedit:hasScientificEditor
	knora-base:subjectClassConstraint textedit:CriticalEdition;
	knora-base:objectClassConstraint human:Person.

textedit:hasCriticalEditorValue
	a owl:ObjectProperty;
	rdfs:label "has critical editor - statement"@en, "hat kritische Editor - Festlegung"@de;
	rdfs:comment "Relating a critical edition to a reification statement of the relation between the critical edition and a critical editor who created it."@en;
	rdfs:subPropertyOf knora-base:hasLinkToValue;
	knora-base:subjectClassConstraint textedit:CriticalEdition;
	knora-base:objectClassConstraint knora-base:LinkValue.

textedit:hasSiglum
	a owl:ObjectProperty;
	rdfs:label "editiorial text structure has siglum"@en, "editorische Textstruktur hat Siglum"@de;
	rdfs:comment """Relating an editiorial text structure to a siglum it has."""@en;
	rdfs:domain textedit:EditorialStructure;
	rdfs:range textedit:Siglum;
	rdfs:subPropertyOf document:hasExpressionReference;
	knora-base:subjectClassConstraint textedit:EditorialStructure;
	knora-base:objectClassConstraint textedit:Siglum.

textedit:hasSiglumValue
	a owl:ObjectProperty;
	rdfs:label "editiorial text structure has siglum - statement"@en, "editorische Textstruktur hat Siglum - Festlegung"@de;
	rdfs:comment """Relating an editiorial text structure to a reification statement of the relation between the structure and a siglum it has."""@en;
	rdfs:subPropertyOf document:hasExpressionReferenceValue;
	knora-base:subjectClassConstraint textedit:EditorialStructure;
	knora-base:objectClassConstraint knora-base:LinkValue.

textedit:isSiglumOfEntry
	a owl:ObjectProperty;
	rdfs:label "îs siglum of apparatus entry"@en, "ist Siglum eines Apparateintrages"@de;
	rdfs:comment """Relating a siglum to an apparatus entry."""@en;
	rdfs:domain textedit:Siglum;
	rdfs:range textedit:ApparatusEntry;
	rdfs:subPropertyOf concept:isPartOf;
	knora-base:subjectClassConstraint textedit:Siglum;
	knora-base:objectClassConstraint textedit:ApparatusEntry.

textedit:isSiglumOfEntryValue
	a owl:ObjectProperty;
	rdfs:label "îs siglum of apparatus entry - statement"@en, "ist Siglum eines Apparateintrages - Festlegung"@de;
	rdfs:comment """Relating a siglum to a reification statement of the relation between the siglum and an apparatus entry."""@en;
	rdfs:subPropertyOf concept:isPartOfValue;
	knora-base:subjectClassConstraint textedit:Siglum;
	knora-base:objectClassConstraint knora-base:LinkValue.

textedit:isSiglumOfScientificEdition
	a owl:ObjectProperty;
	rdfs:label "îs siglum of scientific edition"@en, "ist Siglum einer wissenschaftliche Edition"@de;
	rdfs:comment """Relating a siglum to its scientific edition."""@en;
	rdfs:domain textedit:Siglum;
	rdfs:range textedit:ScientificEdition;
	rdfs:subPropertyOf document:isStructureOfDocument;
	knora-base:subjectClassConstraint textedit:Siglum;
	knora-base:objectClassConstraint textedit:ScientificEdition.

textedit:isSiglumOfScientificEditionValue
	a owl:ObjectProperty;
	rdfs:label "îs siglum of scientific edition - statement"@en, "ist Siglum einer wissenschaftliche Edition - Festlegung"@de;
	rdfs:comment """Relating a siglum to a reification statement of the relation between the siglum and its scientific edition."""@en;
	rdfs:subPropertyOf document:isStructureOfDocumentValue;
	knora-base:subjectClassConstraint textedit:Siglum;
	knora-base:objectClassConstraint knora-base:LinkValue.

textedit:siglumHasIdentifier
	a owl:ObjectProperty;
	rdfs:label "siglum has identifier"@en, "Siglum hat Identifikator"@de;
	rdfs:comment """Relating a siglum to the identifier of a text that is subject to the siglum's critical edition."""@en;
	rdfs:domain textedit:Siglum;
	rdfs:range document:ExpressionIdentifier;
	rdfs:subPropertyOf document:expressionReferenceHasIdentifier;
	knora-base:subjectClassConstraint textedit:Siglum;
	knora-base:objectClassConstraint document:ExpressionIdentifier.

textedit:siglumHasIdentifierValue
	a owl:ObjectProperty;
	rdfs:label "siglum has identifier - statement"@en, "Siglum hat Identifikator - Festlegung"@de;
	rdfs:comment """Relating a siglum to a reification statement of the relation between the siglum and the identifier of a text that is subject to the siglum's critical edition."""@en;
	rdfs:subPropertyOf document:expressionReferenceHasIdentifierValue;
	knora-base:subjectClassConstraint textedit:Siglum;
	knora-base:objectClassConstraint knora-base:LinkValue.

textedit:siglumHasWitnessIdentifier
	a owl:ObjectProperty;
	rdfs:label "siglum has witness identifier"@en, "Siglum hat Textzeugeidentifikator"@de;
	rdfs:comment """Relating a siglum to the identifier of its witness."""@en;
	rdfs:domain textedit:Siglum;
	rdfs:range textedit:WitnessIdentifier;
	rdfs:subPropertyOf document:expressionReferenceHasIdentifier;
	knora-base:subjectClassConstraint textedit:Siglum;
	knora-base:objectClassConstraint textedit:WitnessIdentifier.

textedit:siglumHasWitnessIdentifierValue
	a owl:ObjectProperty;
	rdfs:label "siglum has witness identifier - statement"@en, "Siglum hat Textzeugeidentifikator - Festlegung"@de;
	rdfs:comment """Relating a siglum to a reification statement of the relation between the siglum and the identifier of its witness."""@en;
	rdfs:subPropertyOf document:expressionReferenceHasIdentifierValue;
	knora-base:subjectClassConstraint textedit:Siglum;
	knora-base:objectClassConstraint knora-base:LinkValue.

textedit:witnessHasIdentifier
	a owl:ObjectProperty;
	rdfs:label "witness text has identifier"@en, "Textzeuge hat Identifikator"@de;
	rdfs:comment """Relating a witness text expression to its identifier."""@en;
	rdfs:domain textedit:Witness;
	rdfs:range textedit:WitnessIdentifier;
	rdfs:subPropertyOf document:expressionHasIdentifier;
	knora-base:subjectClassConstraint textedit:Witness;
	knora-base:objectClassConstraint textedit:WitnessIdentifier.

textedit:witnessHasIdentifierValue
	a owl:ObjectProperty;
	rdfs:label "witness text has identifier - statement"@en, "Textzeuge hat Identifikator - Festlegung"@de;
	rdfs:comment """Relating a witness text expression to a reification statement of the relation between the witness and its identifier."""@en;
	rdfs:subPropertyOf document:expressionHasIdentifierValue;
	knora-base:subjectClassConstraint textedit:Witness;
	knora-base:objectClassConstraint knora-base:LinkValue.

textedit:isWitnessOf
	a owl:ObjectProperty;
	rdfs:label "is witness of"@en, "ist Textzeuge von"@de;
	rdfs:comment """Relating a witness text expression to its original."""@en;
	rdfs:domain textedit:Witness;
	rdfs:range text:Expression;
	rdfs:subPropertyOf knora-base:hasLinkTo;
	knora-base:subjectClassConstraint textedit:Witness;
	knora-base:objectClassConstraint text:Expression.

textedit:isWitnessOfValue
	a owl:ObjectProperty;
	rdfs:label "is witness of - statement"@en, "ist Textzeuge von - Festlegung"@de;
	rdfs:comment """Relating a witness text expression to a reification statement of the relation between the witness and its original."""@en;
	rdfs:subPropertyOf knora-base:hasLinkToValue;
	knora-base:subjectClassConstraint textedit:Witness;
	knora-base:objectClassConstraint knora-base:LinkValue.

textedit:isApparatusOf
	a owl:ObjectProperty;
	rdfs:label "is apparatus of"@en, "ist Apparat von"@de;
	rdfs:comment """Relating an editing apparatus to its scientific edition."""@en;
	rdfs:domain textedit:Apparatus;
	rdfs:range textedit:ScientificEdition;
	rdfs:subPropertyOf text-structure:isPartOfTextExpression;
	knora-base:subjectClassConstraint textedit:Apparatus;
	knora-base:objectClassConstraint textedit:ScientificEdition.

textedit:isApparatusOfValue
	a owl:ObjectProperty;
	rdfs:label "is apparatus of - statement"@en, "ist Apparat von - Festlegung"@de;
	rdfs:comment """Relating a editing apparatus to a reification statement of the relation between the apparatus and its scientific edition."""@en;
	rdfs:subPropertyOf text-structure:isPartOfTextExpressionValue;
	knora-base:subjectClassConstraint textedit:Apparatus;
	knora-base:objectClassConstraint knora-base:LinkValue.

textedit:isEntryOfApparatus
	a owl:ObjectProperty;
	rdfs:label "is entry of apparatus"@en, "ist Eintrag eines Apparates"@de;
	rdfs:comment """Relating an entry to its editing apparatus."""@en;
	rdfs:domain textedit:ApparatusEntry;
	rdfs:range textedit:Apparatus;
	rdfs:subPropertyOf concept:isPartOf;
	knora-base:subjectClassConstraint textedit:ApparatusEntry;
	knora-base:objectClassConstraint textedit:Apparatus.

textedit:isEntryOfApparatusValue
	a owl:ObjectProperty;
	rdfs:label "is entry of apparatus - statement"@en, "ist Eintrag eines Apparates - Festlegung"@de;
	rdfs:comment """Relating an entry to a reification statement of the relation between the entry and its editing apparatus."""@en;
	rdfs:subPropertyOf concept:isPartOfValue;
	knora-base:subjectClassConstraint textedit:ApparatusEntry;
	knora-base:objectClassConstraint knora-base:LinkValue.

textedit:hasApparatusEnteringDate
	a owl:ObjectProperty;
	rdfs:label "has apparatus entering date"@en, "hat Apparatuseintragsdatum"@de;
	rdfs:comment """Relating an entry to its date of entering in an apparatus."""@en;
	rdfs:domain textedit:ApparatusEntry;
	rdfs:range xsd:date;
	rdfs:subPropertyOf human:creationHasDate;
	knora-base:subjectClassConstraint textedit:ApparatusEntry;
	knora-base:objectClassConstraint knora-base:DateValue.

textedit:isDoctrinalApparatusOf
	a owl:ObjectProperty;
	rdfs:label "is doctrinal apparatus of"@en, "ist doktrinaler Apparat von"@de;
	rdfs:comment """Relating a doctrinal apparatus to its scientific edition."""@en;
	rdfs:domain textedit:DoctrinalApparatus;
	rdfs:range textedit:ScientificEdition;
	rdfs:subPropertyOf textedit:isApparatusOf;
	knora-base:subjectClassConstraint textedit:DoctrinalApparatus;
	knora-base:objectClassConstraint textedit:ScientificEdition.

textedit:isDoctrinalApparatusOfValue
	a owl:ObjectProperty;
	rdfs:label "is doctrinal apparatus of - statement"@en, "ist doktrinaler Apparat von - Festlegung"@de;
	rdfs:comment """Relating a doctrinal apparatus to a reification statement of the relation between the apparatus and its scientific edition."""@en;
	rdfs:subPropertyOf textedit:isApparatusOfValue;
	knora-base:subjectClassConstraint textedit:DoctrinalApparatus;
	knora-base:objectClassConstraint knora-base:LinkValue.

textedit:isEntryOfDoctrinalApparatus
	a owl:ObjectProperty;
	rdfs:label "is entry of doctrinal apparatus"@en, "ist Eintrag eines doktrinalen Apparates"@de;
	rdfs:comment """Relating an entry to its doctrinal apparatus."""@en;
	rdfs:domain textedit:DoctrinalApparatusEntry;
	rdfs:range textedit:DoctrinalApparatus;
	rdfs:subPropertyOf textedit:isEntryOfApparatus;
	knora-base:subjectClassConstraint textedit:DoctrinalApparatusEntry;
	knora-base:objectClassConstraint textedit:DoctrinalApparatus.

textedit:isEntryOfDoctrinalApparatusValue
	a owl:ObjectProperty;
	rdfs:label "is entry of doctrinal apparatus - statement"@en, "ist Eintrag eines doktrinalen Apparates - Festlegung"@de;
	rdfs:comment """Relating an entry to a reification statement of the relation between the entry and its doctrinal apparatus."""@en;
	rdfs:subPropertyOf textedit:isEntryOfApparatusValue;
	knora-base:subjectClassConstraint textedit:DoctrinalApparatusEntry;
	knora-base:objectClassConstraint knora-base:LinkValue.

textedit:isApparatusFontiumOf
	a owl:ObjectProperty;
	rdfs:label "is apparatus fontium of"@en, "ist Apparatus Fontium von"@de;
	rdfs:comment """Relating an apparatus fontium to its scientific edition."""@en;
	rdfs:domain textedit:ApparatusFontium;
	rdfs:range textedit:ScientificEdition;
	rdfs:subPropertyOf textedit:isApparatusOf;
	knora-base:subjectClassConstraint textedit:ApparatusFontium;
	knora-base:objectClassConstraint textedit:ScientificEdition.

textedit:isApparatusFontiumOfValue
	a owl:ObjectProperty;
	rdfs:label "is apparatus fontium of - statement"@en, "ist Apparatus Fontium von - Festlegung"@de;
	rdfs:comment """Relating an apparatus fontium to a reification statement of the relation between the apparatus and its scientific edition."""@en;
	rdfs:subPropertyOf textedit:isApparatusOfValue;
	knora-base:subjectClassConstraint textedit:ApparatusFontium;
	knora-base:objectClassConstraint knora-base:LinkValue.

textedit:isEntryOfApparatusFontium
	a owl:ObjectProperty;
	rdfs:label "is entry of apparatus fontium"@en, "ist Eintrag eines Apparatus Fontium"@de;
	rdfs:comment """Relating an entry to its apparatus fontium."""@en;
	rdfs:domain textedit:ApparatusFontiumEntry;
	rdfs:range textedit:ApparatusFontium;
	rdfs:subPropertyOf textedit:isEntryOfApparatus;
	knora-base:subjectClassConstraint textedit:ApparatusFontiumEntry;
	knora-base:objectClassConstraint textedit:ApparatusFontium.

textedit:isEntryOfApparatusFontiumValue
	a owl:ObjectProperty;
	rdfs:label "is entry of apparatus fontium - statement"@en, "ist Eintrag eines Apparatus Fontium - Festlegung"@de;
	rdfs:comment """Relating an entry to a reification statement of the relation between the entry and its apparatus fontium."""@en;
	rdfs:subPropertyOf textedit:isEntryOfApparatusValue;
	knora-base:subjectClassConstraint textedit:ApparatusFontiumEntry;
	knora-base:objectClassConstraint knora-base:LinkValue.

textedit:isCriticalApparatusOf
	a owl:ObjectProperty;
	rdfs:label "is critical apparatus of"@en, "ist textkritischer Apparat von"@de;
	rdfs:comment """Relating a critical apparatus to its edition."""@en;
	rdfs:domain textedit:CriticalApparatus;
	rdfs:range textedit:CriticalEdition;
	rdfs:subPropertyOf textedit:isApparatusOf;
	knora-base:subjectClassConstraint textedit:CriticalApparatus;
	knora-base:objectClassConstraint textedit:CriticalEdition.

textedit:isCriticalApparatusOfValue
	a owl:ObjectProperty;
	rdfs:label "is critical apparatus of - statement"@en, "ist textkritischer Apparat von - Festlegung"@de;
	rdfs:comment """Relating a critical apparatus to a reification statement of the relation between the apparatus and its edition."""@en;
	rdfs:subPropertyOf textedit:isApparatusOfValue;
	knora-base:subjectClassConstraint textedit:CriticalApparatus;
	knora-base:objectClassConstraint knora-base:LinkValue.

textedit:isEntryOfCriticalApparatus
	a owl:ObjectProperty;
	rdfs:label "is entry of critical apparatus"@en, "ist Eintrag eines textkritischen Apparates"@de;
	rdfs:comment """Relating an entry to its critical apparatus."""@en;
	rdfs:domain textedit:CriticalApparatusEntry;
	rdfs:range textedit:CriticalApparatus;
	rdfs:subPropertyOf textedit:isEntryOfApparatus;
	knora-base:subjectClassConstraint textedit:CriticalApparatusEntry;
	knora-base:objectClassConstraint textedit:CriticalApparatus.

textedit:isEntryOfCriticalApparatusValue
	a owl:ObjectProperty;
	rdfs:label "is entry of critical apparatus - statement"@en, "ist Eintrag eines textkritischen Apparates - Festlegung"@de;
	rdfs:comment """Relating an entry to a reification statement of the relation between the entry and its critical apparatus."""@en;
	rdfs:subPropertyOf textedit:isEntryOfApparatusValue;
	knora-base:subjectClassConstraint textedit:CriticalApparatusEntry;
	knora-base:objectClassConstraint knora-base:LinkValue.

textedit:isEntryOfStructureApparatus
	a owl:ObjectProperty;
	rdfs:label "is entry of text structure apparatus"@en, "ist Eintrag eines Textstruktur-Apparates"@de;
	rdfs:comment """Relating an entry to its text structure apparatus."""@en;
	rdfs:domain textedit:StructureApparatusEntry;
	rdfs:range textedit:StructureApparatus;
	rdfs:subPropertyOf textedit:isEntryOfApparatus;
	knora-base:subjectClassConstraint textedit:StructureApparatusEntry;
	knora-base:objectClassConstraint textedit:StructureApparatus.

textedit:isEntryOfStructureApparatusValue
	a owl:ObjectProperty;
	rdfs:label "is entry of text structure apparatus - statement"@en, "ist Eintrag eines Textstruktur-Apparates - Festlegung"@de;
	rdfs:comment """Relating an entry to a reification statement of the relation between the entry and its text structure apparatus."""@en;
	rdfs:subPropertyOf textedit:isEntryOfApparatusValue;
	knora-base:subjectClassConstraint textedit:StructureApparatusEntry;
	knora-base:objectClassConstraint knora-base:LinkValue.

textedit:isStructureDescriptionOfEntry
	a owl:ObjectProperty;
	rdfs:label "is structure description of apparatus entry"@en, "ist Strukturbeschreibung eines Apparateintrages"@de;
	rdfs:comment """Relating a text structure description to a text structure apparatus entry."""@en;
	rdfs:domain textedit:StructureDescription;
	rdfs:range textedit:StructureApparatusEntry;
	rdfs:subPropertyOf concept:isPartOf;
	knora-base:subjectClassConstraint textedit:StructureDescription;
	knora-base:objectClassConstraint textedit:StructureApparatusEntry.

textedit:isStructureDescriptionOfEntryValue
	a owl:ObjectProperty;
	rdfs:label "is structure description of apparatus entry - statement"@en, "ist Strukturbeschreibung eines Apparateintrages - Festlegung"@de;
	rdfs:comment """Relating a text structure description to a reification statement of the relation between the description and a text structure apparatus entry."""@en;
	rdfs:subPropertyOf concept:isPartOfValue;
	knora-base:subjectClassConstraint textedit:StructureDescription;
	knora-base:objectClassConstraint knora-base:LinkValue.

textedit:structureDescriptionHasContent
	a owl:ObjectProperty;
	rdfs:label "structure description has content"@en, "Strukturbeschreibung hat Inhalt"@de;
	rdfs:comment """Relating structure description to its content."""@en;
	rdfs:domain textedit:StructureDescription;
#	rdfs:range ling:Literal;
	rdfs:subPropertyOf language:hasContent;
	knora-base:subjectClassConstraint textedit:StructureDescription;
	knora-base:objectClassConstraint knora-base:TextValue.

textedit:hasWitness
	a owl:ObjectProperty;
	rdfs:label "has witness"@en, "hat Textzeuge"@de;
	rdfs:comment """Relating a reading to its witness."""@en;
	rdfs:domain textedit:Reading;
	rdfs:range textedit:Witness;
	rdfs:subPropertyOf concept:isPartOf;
	knora-base:subjectClassConstraint textedit:Reading;
	knora-base:objectClassConstraint textedit:Witness.

textedit:hasWitnessValue
	a owl:ObjectProperty;
	rdfs:label "has witness - statement"@en, "hat Textzeuge - Festlegung"@de;
	rdfs:comment """Relating a reading to a reification statement of the relation between the reading and its witness."""@en;
	rdfs:subPropertyOf concept:isPartOfValue;
	knora-base:subjectClassConstraint textedit:Reading;
	knora-base:objectClassConstraint knora-base:LinkValue.

textedit:isLemmaOfCriticalEntry
	a owl:ObjectProperty;
	rdfs:label "is lemma of critical apparatus entry"@en, "ist Lemma eines textkritischen Apparateintrages"@de;
	rdfs:comment """Relating a lemma to its critical apparatus entry."""@en;
	rdfs:domain textedit:Lemma;
	rdfs:range textedit:CriticalApparatusEntry;
	rdfs:subPropertyOf concept:isPartOf;
	knora-base:subjectClassConstraint textedit:Lemma;
	knora-base:objectClassConstraint textedit:CriticalApparatusEntry.

textedit:isLemmaOfCriticalEntryValue
	a owl:ObjectProperty;
	rdfs:label "is lemma of critical apparatus entry - statement"@en, "ist Lemma eines textkritischen Apparateintrages - Festlegung"@de;
	rdfs:comment """Relating a lemma to a reification statement of the relation between the lemma and its critical apparatus entry."""@en;
	rdfs:subPropertyOf concept:isPartOfValue;
	knora-base:subjectClassConstraint textedit:Lemma;
	knora-base:objectClassConstraint knora-base:LinkValue.

textedit:isLemmaOfDoctrinalEntry
	a owl:ObjectProperty;
	rdfs:label "is lemma of doctrinal apparatus entry"@en, "ist Lemma eines doktrinalen Apparateintrages"@de;
	rdfs:comment """Relating a lemma to its doctrinal apparatus entry."""@en;
	rdfs:domain textedit:Lemma;
	rdfs:range textedit:DoctrinalApparatusEntry;
	rdfs:subPropertyOf concept:isPartOf;
	knora-base:subjectClassConstraint textedit:Lemma;
	knora-base:objectClassConstraint textedit:DoctrinalApparatusEntry.

textedit:isLemmaOfDoctrinalEntryValue
	a owl:ObjectProperty;
	rdfs:label "is lemma of doctrinal apparatus entry - statement"@en, "ist Lemma eines doktrinalen Apparateintrages - Festlegung"@de;
	rdfs:comment """Relating a lemma to a reification statement of the relation between the lemma and its doctrinal apparatus entry."""@en;
	rdfs:subPropertyOf concept:isPartOfValue;
	knora-base:subjectClassConstraint textedit:Lemma;
	knora-base:objectClassConstraint knora-base:LinkValue.

textedit:lemmaHasReference
	a owl:ObjectProperty;
	rdfs:label "lemma has reference"@en, "Lemma hat Referenz"@de;
	rdfs:comment """Relating a lemma to its reference."""@en;
	rdfs:domain textedit:Lemma;
	rdfs:range document:TextStructureReference;
	rdfs:subPropertyOf document:hasTextReference;
	knora-base:subjectClassConstraint textedit:Lemma;
	knora-base:objectClassConstraint document:TextStructureReference.

textedit:lemmaHasReferenceValue
	a owl:ObjectProperty;
	rdfs:label "lemma has text reference - statement"@en, "Lemma hat Textreferenz - Festlegung"@de;
	rdfs:comment """Relating a lemma to a reification statement of the relation between the lemma and its text reference."""@en;
	rdfs:subPropertyOf document:hasTextReferenceValue;
	knora-base:subjectClassConstraint textedit:Lemma;
	knora-base:objectClassConstraint knora-base:LinkValue.

textedit:lemmaHasVariant
	a owl:ObjectProperty;
	rdfs:label "lemma has variant"@en, "Lemma hat Variant"@de;
	rdfs:comment """Relating a lemma to a variant it has."""@en;
	rdfs:domain textedit:Lemma;
	rdfs:range textedit:Variant;
	rdfs:subPropertyOf knora-base:hasLinkTo;
	knora-base:subjectClassConstraint textedit:Lemma;
	knora-base:objectClassConstraint textedit:Variant.

textedit:lemmaHasVariantValue
	a owl:ObjectProperty;
	rdfs:label "lemma has variant - statement"@en, "Lemma hat Textinterpretation - Festlegung"@de;
	rdfs:comment """Relating a lemma to a reification statement of the relation between the lemma and a variant it has."""@en;
	rdfs:subPropertyOf knora-base:hasLinkToValue;
	knora-base:subjectClassConstraint textedit:Lemma;
	knora-base:objectClassConstraint knora-base:LinkValue.

textedit:lemmaHasComment
	a owl:ObjectProperty;
	rdfs:label "lemma has comment"@en, "Lemma hat Kommentar"@de;
	rdfs:comment """Relating a lemma to a comment it has."""@en;
	rdfs:domain textedit:Lemma;
	rdfs:range textedit:EditorialComment;
	rdfs:subPropertyOf knora-base:hasLinkTo;
	knora-base:subjectClassConstraint textedit:Lemma;
	knora-base:objectClassConstraint textedit:EditorialComment.

textedit:lemmaHasCommentValue
	a owl:ObjectProperty;
	rdfs:label "lemma has comment - statement"@en, "Lemma hat Kommentar - Festlegung"@de;
	rdfs:comment """Relating a lemma to a reification statement of the relation between the lemma and a comment it has."""@en;
	rdfs:subPropertyOf knora-base:hasLinkToValue;
	knora-base:subjectClassConstraint textedit:Lemma;
	knora-base:objectClassConstraint knora-base:LinkValue.

textedit:isVariantOfEntry
	a owl:ObjectProperty;
	rdfs:label "is variant of apparatus entry"@en, "ist Variant eines Apparateintrages"@de;
	rdfs:comment """Relating a variant to its critical apparatus entry."""@en;
	rdfs:domain textedit:Variant;
	rdfs:range textedit:CriticalApparatusEntry;
	rdfs:subPropertyOf concept:isPartOf;
	knora-base:subjectClassConstraint textedit:Variant;
	knora-base:objectClassConstraint textedit:CriticalApparatusEntry.

textedit:isVariantOfEntryValue
	a owl:ObjectProperty;
	rdfs:label "is variant of apparatus entry - statement"@en, "ist Variant eines Apparateintrages - Festlegung"@de;
	rdfs:comment """Relating a variant to a reification statement of the relation between the variant and its critical apparatus entry."""@en;
	rdfs:subPropertyOf concept:isPartOfValue;
	knora-base:subjectClassConstraint textedit:Variant;
	knora-base:objectClassConstraint knora-base:LinkValue.

textedit:variantHasReference
	a owl:ObjectProperty;
	rdfs:label "variant has text reference"@en, "Variant hat Textreferenz"@de;
	rdfs:comment """Relating a variant to its text reference."""@en;
	rdfs:domain textedit:Variant;
	rdfs:range document:TextStructureReference;
	rdfs:subPropertyOf document:hasTextReference;
	knora-base:subjectClassConstraint textedit:Variant;
	knora-base:objectClassConstraint document:TextStructureReference.

textedit:variantHasReferenceValue
	a owl:ObjectProperty;
	rdfs:label "variant has text reference - statement"@en, "Variant hat Textreferenz - Festlegung"@de;
	rdfs:comment """Relating a variant to a reification statement of the relation between the variant and its text reference."""@en;
	rdfs:subPropertyOf document:hasTextReferenceValue;
	knora-base:subjectClassConstraint textedit:Variant;
	knora-base:objectClassConstraint knora-base:LinkValue.

textedit:variantHasComment
	a owl:ObjectProperty;
	rdfs:label "variant has comment"@en, "Variant hat Kommentar"@de;
	rdfs:comment """Relating a variant to an editorial comment."""@en;
	rdfs:domain textedit:Variant;
	rdfs:range textedit:EditorialComment;
	rdfs:subPropertyOf knora-base:hasLinkTo;
	knora-base:subjectClassConstraint textedit:Variant;
	knora-base:objectClassConstraint textedit:EditorialComment.

textedit:variantHasCommentValue
	a owl:ObjectProperty;
	rdfs:label "variant has comment - statement"@en, "Variant hat Kommentar - Festlegung"@de;
	rdfs:comment """Relating a variant to a reification statement of the relation between the variant and an editorial comment."""@en;
	rdfs:subPropertyOf knora-base:hasLinkToValue;
	knora-base:subjectClassConstraint textedit:Variant;
	knora-base:objectClassConstraint knora-base:LinkValue.

textedit:isCommentOn
	a owl:ObjectProperty;
	rdfs:label "is comment on"@en, "ist Kommentar zu"@de;
	rdfs:comment """Relating an editorial comment to a text expression it is a comment on."""@en;
	rdfs:domain textedit:EditorialComment;
	rdfs:range text:Expression;
	rdfs:subPropertyOf knora-base:hasLinkTo;
	knora-base:subjectClassConstraint textedit:EditorialComment;
	knora-base:objectClassConstraint text:Expression.

textedit:isCommentOnValue
	a owl:ObjectProperty;
	rdfs:label "is comment on - statement"@en, "ist Kommentar zu - Festlegung"@de;
	rdfs:comment """Relating an editorial comment to a reification statement of the relation between the comment and a text expression it is a comment on."""@en;
	rdfs:subPropertyOf knora-base:hasLinkToValue;
	knora-base:subjectClassConstraint textedit:EditorialComment;
	knora-base:objectClassConstraint knora-base:LinkValue.

textedit:isCommentOfScientificEdition
	a owl:ObjectProperty;
	rdfs:label "is comment of scientific edition"@en, "ist Kommentar der wissenschaftlichen Edition"@de;
	rdfs:comment """Relating an editorial comment to its scientific edition."""@en;
	rdfs:domain textedit:EditorialComment;
	rdfs:range textedit:ScientificEdition;
	rdfs:subPropertyOf text-structure:isPartOfTextExpression;
	knora-base:subjectClassConstraint textedit:EditorialComment;
	knora-base:objectClassConstraint textedit:ScientificEdition.

textedit:isCommentOfScientificEditionValue
	a owl:ObjectProperty;
	rdfs:label "is comment of scientific edition - statement"@en, "ist Kommentar der wissenschaftlichen Edition - Festlegung"@de;
	rdfs:comment """Relating an editorial comment to a reification statement of the relation between the comment and its scientific edition."""@en;
	rdfs:subPropertyOf text-structure:isPartOfTextExpressionValue;
	knora-base:subjectClassConstraint textedit:EditorialComment;
	knora-base:objectClassConstraint knora-base:LinkValue.

textedit:isCommentOfEntry
	a owl:ObjectProperty;
	rdfs:label "is comment of entry"@en, "ist Kommentar eines Eintrages"@de;
	rdfs:comment """Relating an editorial comment to its apparatus entry."""@en;
	rdfs:domain textedit:EditorialComment;
	rdfs:range textedit:ApparatusEntry;
	rdfs:subPropertyOf concept:isPartOf;
	knora-base:subjectClassConstraint textedit:EditorialComment;
	knora-base:objectClassConstraint textedit:ApparatusEntry.

textedit:isCommentOfEntryValue
	a owl:ObjectProperty;
	rdfs:label "is comment of entry - statement"@en, "ist Kommentar eines Eintrages - Festlegung"@de;
	rdfs:comment """Relating an editorial comment to a reification statement of the relation between the comment and its apparatus entry."""@en;
	rdfs:subPropertyOf concept:isPartOfValue;
	knora-base:subjectClassConstraint textedit:EditorialComment;
	knora-base:objectClassConstraint knora-base:LinkValue.

textedit:commentHasReference
	a owl:ObjectProperty;
	rdfs:label "comment has text reference"@en, "Kommentar hat Textreferenz"@de;
	rdfs:comment """Relating an editorial comment to its text reference."""@en;
	rdfs:domain textedit:EditorialComment;
	rdfs:range document:TextStructureReference;
	rdfs:subPropertyOf document:hasTextReference;
	knora-base:subjectClassConstraint textedit:EditorialComment;
	knora-base:objectClassConstraint document:TextStructureReference.

textedit:commentHasReferenceValue
	a owl:ObjectProperty;
	rdfs:label "comment has text reference - statement"@en, "Kommentar hat Textreferenz - Festlegung"@de;
	rdfs:comment """Relating an editorial comment to a reification statement of the relation between the comment and its text reference."""@en;
	rdfs:subPropertyOf document:hasTextReferenceValue;
	knora-base:subjectClassConstraint textedit:EditorialComment;
	knora-base:objectClassConstraint knora-base:LinkValue.

textedit:commentHasContent
	a owl:ObjectProperty;
	rdfs:label "editorial comment has content"@en, "editorischer Kommentar hat Inhalt"@de;
	rdfs:comment """Relating an editorial comment to its content."""@en;
	rdfs:domain textedit:EditorialComment;
#	rdfs:range rdfs:Literal;
	rdfs:subPropertyOf language:hasContent;
	knora-base:subjectClassConstraint textedit:EditorialComment;
	knora-base:objectClassConstraint knora-base:TextValue.