@prefix rdfs: <http://www.w3.org/2000/01/rdf-schema#>.
@prefix owl: <http://www.w3.org/2002/07/owl#>.
@prefix xsd: <http://www.w3.org/2001/XMLSchema#>.
@prefix skos: <http://www.w3.org/2004/02/skos/core#>.
@prefix dct: <http://purl.org/dc/terms/>.
@prefix foaf: <http://xmlns.com/foaf/0.1/>.
@prefix cidoc: <http://www.cidoc-crm.org/cidoc-crm/>.
@prefix frbroo: <http://iflastandards.info/ns/fr/frbr/frbroo/>.
@prefix event: <http://www.knora.org/ontology/shared/event#>.
@prefix human: <http://www.knora.org/ontology/shared/human#>.
@prefix language: <http://www.knora.org/ontology/shared/language#>.
@prefix concept: <http://www.knora.org/ontology/shared/concept#>.
@prefix math: <http://www.knora.org/ontology/shared/mathematics#>.
@prefix document: <http://www.knora.org/ontology/shared/document#>.
@prefix text: <http://www.knora.org/ontology/shared/text#>.
@prefix text-expression: <http://www.knora.org/ontology/shared/text-expression#>.
@prefix prosodic-structure: <http://www.knora.org/ontology/shared/prosodic-structure#>.
@prefix publish: <http://www.knora.org/ontology/shared/publishing#>.
@prefix litera: <http://www.knora.org/ontology/shared/literature#>.
@prefix ling: <http://www.knora.org/ontology/shared/linguistics#>.
@prefix lingmor: <http://www.knora.org/ontology/shared/linguistic-morphology#>.
@prefix knora-base: <http://www.knora.org/ontology/knora-base#>.

@base <http://www.knora.org/ontology/shared/text-structure>.
@prefix text-structure: <http://www.knora.org/ontology/shared/text-structure#>.

<http://www.knora.org/ontology/shared/text-structure>
	a owl:Ontology;
	dct:license <http://creativecommons.org/licenses/by/3.0/>;
	dct:title "An ontology about text structure"@en;
	dct:description """Formal description of text structure, subclasses, related classes, and properties."""@en;
	skos:note """Text and text editing are described in other ontologies"""@en;
	skos:note """Prosodic structure and note structure are described in other ontologies"""@en;
	dct:creator "Hans Cools, MD, knowledge engineer, ontologist, software developer, NIE-INE, Basel University, Switzerland"@en;
	dct:contributor "Roberta Padlina, tool coordinator and software developer, NIE-INE, Basel University, Switzerland"@en;
	dct:contributor "Reto Baumgartner, tool coordinator and software developer, NIE-INE, University of ZÃ¼rich, Switzerland"@en;
	dct:publisher "Basel University, Switzerland"@en;
	rdfs:seeAlso <https://files.ifi.uzh.ch/cl/siclemat/lehre/hs09/ecl1/script/html/script.html>;

	knora-base:attachedToProject <http://www.knora.org/ontology/knora-base#DefaultSharedOntologiesProject>.

#
# CLASSES
#

text-structure:Structure
	a owl:Class;
	rdfs:label "text structure"@en, "Textstruktur"@de;
	rdfs:comment """Text as structure abstracted from its carrier, e.g. a word, sentence, text line, paragraph, section, verse, strophe."""@en;
	skos:note """Making up a text expression, without necessarily being one itself."""@en;
	rdfs:subClassOf text:Text, document:ContentStructure, [
		a owl:Restriction; owl:onProperty text-structure:isPartOfTextExpression; owl:minCardinality "0"^^xsd:nonNegativeInteger], [
		a owl:Restriction; owl:onProperty text-structure:isPartOfTextExpressionValue; owl:minCardinality "0"^^xsd:nonNegativeInteger], [
		a owl:Restriction; owl:onProperty text-structure:hasIdentifier; owl:minCardinality "0"^^xsd:nonNegativeInteger], [
		a owl:Restriction; owl:onProperty text-structure:hasIdentifierValue; owl:minCardinality "0"^^xsd:nonNegativeInteger].

text-structure:Identifier
	a owl:Class;
	rdfs:label "text structure identifier"@en, "Textstrukturidentifikator"@de;
	rdfs:comment """Identifier of a text structure."""@en;
	rdfs:subClassOf document:ContentStructureIdentifier.

text-structure:SyntacticStructure
	a owl:Class;
	rdfs:label "syntactic text structure"@en, "syntaktische Textstruktur"@de;
	rdfs:comment """Text structure depending on natural language-specific syntax, e.g. a word, sentence."""@en;
	rdfs:subClassOf text-structure:Structure.

text-structure:CompositionalStructure
	a owl:Class;
	rdfs:label "compositional text structure"@en, "kompositionelle Textstruktur"@de;
	rdfs:comment """Text structure depending on text composition in a two-dimensional plane, e.g. a line, paragraph, section, page."""@en;
	rdfs:subClassOf text-structure:Structure.

text-structure:ContentStructure
	a owl:Class;
	rdfs:label "content text structure"@en, "inhaltliche Textstruktur"@de;
	rdfs:comment """Text structure depending on text content, e.g. a paragraph, section, prose, citation."""@en;
	rdfs:subClassOf text-structure:Structure.

text-structure:SentenceStructure
	a owl:Class;
	rdfs:label "sentence structure"@en, "Satzstruktur"@de;
	rdfs:comment """Content structure depending on sentences, e.g. a paragraph, section, prose"""@en;
	rdfs:subClassOf text-structure:ContentStructure.

text-structure:CompositionalContentStructure
	a owl:Class;
	rdfs:label "compositional content text structure"@en, "kompositionelle inhaltliche Textstruktur"@de;
	rdfs:comment """Content text structure depending on text composition, e.g. a paragraph, section."""@en;
	rdfs:subClassOf text-structure:ContentStructure, text-structure:CompositionalStructure.

text-structure:ScientificStructure
	a owl:Class;
	rdfs:label "scientific text structure"@en, "wissenschaftliche Textstruktur"@de;
	rdfs:comment """Content text structure depending on scientific purpose, e.g. a critical apparatus."""@en;
	rdfs:subClassOf text-structure:ContentStructure.

text-structure:ReadabilityStructure
	a owl:Class;
	rdfs:label "text readability structure"@en, "Textlesbarkeitstruktur"@de;
	rdfs:comment """Compositional text structure providing text readability, e.g. a line, column, page."""@en;
	rdfs:subClassOf text:WrittenText, text-structure:CompositionalStructure.

text-structure:SyntacticWord
	a owl:Class;
	rdfs:label "syntactic word"@en, "syntaktisches Wort"@de;
	rdfs:comment """Smallest independent syntactic structure composed of symbols that can be replaced in a sentence or verse."""@en;
	rdfs:subClassOf text-structure:SyntacticStructure, ling:Concept, [
#		a owl:Restriction; owl:onProperty concept:hasLiteral; owl:minCardinality "0"^^xsd:nonNegativeInteger], [
#		a owl:Restriction; owl:onProperty ling:hasLanguage; owl:minCardinality "0"^^xsd:nonNegativeInteger], [
		a owl:Restriction; owl:onProperty text-structure:syntacticWordHasForm; owl:minCardinality "0"^^xsd:nonNegativeInteger], [
		a owl:Restriction; owl:onProperty text-structure:syntacticWordHasFormValue; owl:minCardinality "0"^^xsd:nonNegativeInteger], [
		a owl:Restriction; owl:onProperty text-structure:isWordBeforePunctuation; owl:minCardinality "0"^^xsd:nonNegativeInteger], [
		a owl:Restriction; owl:onProperty text-structure:isWordBeforePunctuationValue; owl:minCardinality "0"^^xsd:nonNegativeInteger], [
		a owl:Restriction; owl:onProperty text-structure:isWordOfSentence; owl:minCardinality "0"^^xsd:nonNegativeInteger], [
		a owl:Restriction; owl:onProperty text-structure:isWordOfSentenceValue; owl:minCardinality "0"^^xsd:nonNegativeInteger], [
#		a owl:Restriction; owl:onProperty prosodic-structure:isWordOfVerse; owl:allValuesFrom prosodic-structure:Verse], [
		a owl:Restriction; owl:onProperty prosodic-structure:isWordOfVerse; owl:minCardinality "0"^^xsd:nonNegativeInteger], [
		a owl:Restriction; owl:onProperty prosodic-structure:isWordOfVerseValue; owl:minCardinality "0"^^xsd:nonNegativeInteger].

text-structure:Sentence
	a owl:Class;
	rdfs:label "sentence"@en, "Satz"@de;
	rdfs:comment """Syntactic structure comprising one or more linked syntactic words, typically a subject and predicate."""@en;
	rdfs:subClassOf text-structure:SyntacticStructure, text-structure:ContentStructure, [
#		a owl:Restriction; owl:onProperty text-structure:isSentenceOfParagraph; owl:allValuesFrom text-structure:Paragraph], [
		a owl:Restriction; owl:onProperty text-structure:isSentenceOfParagraph; owl:minCardinality "0"^^xsd:nonNegativeInteger], [
		a owl:Restriction; owl:onProperty text-structure:isSentenceOfParagraphValue; owl:minCardinality "0"^^xsd:nonNegativeInteger], [
#		a owl:Restriction; owl:onProperty text-structure:isSentenceOfProse; owl:allValuesFrom text-structure:Prose], [
		a owl:Restriction; owl:onProperty text-structure:isSentenceOfProse; owl:minCardinality "0"^^xsd:nonNegativeInteger], [
		a owl:Restriction; owl:onProperty text-structure:isSentenceOfProseValue; owl:minCardinality "0"^^xsd:nonNegativeInteger].

text-structure:Prose
	a owl:Class;
	rdfs:label "prose"@en, "Prosa"@de;
	rdfs:comment """Syntactic structure with a sentence as unit, in a natural flow of speech."""@en;
	rdfs:subClassOf text-structure:SentenceStructure, [
#		a owl:Restriction; owl:onProperty text-structure:isProseOfExpression; owl:allValuesFrom text:Text], [
		a owl:Restriction; owl:onProperty text-structure:isProseOfExpression; owl:minCardinality "0"^^xsd:nonNegativeInteger], [
		a owl:Restriction; owl:onProperty text-structure:isProseOfExpressionValue; owl:minCardinality "0"^^xsd:nonNegativeInteger].

text-structure:Paragraph
	a owl:Class;
	rdfs:label "paragraph"@en, "Paragraf"@de;
	rdfs:comment """Composition of sentences ending with a line break."""@en; #*
	rdfs:subClassOf text-structure:SentenceStructure, text-structure:CompositionalContentStructure, [
#		a owl:Restriction; owl:onProperty text-structure:isParagraphOfSection; owl:allValuesFrom text-structure:Section], [
		a owl:Restriction; owl:onProperty text-structure:isParagraphOfSection; owl:minCardinality "0"^^xsd:nonNegativeInteger], [
		a owl:Restriction; owl:onProperty text-structure:isParagraphOfSectionValue; owl:minCardinality "0"^^xsd:nonNegativeInteger], [
		a owl:Restriction; owl:onProperty text-structure:paragraphHasTitle; owl:minCardinality "0"^^xsd:nonNegativeInteger], [
		a owl:Restriction; owl:onProperty text-structure:paragraphHasNumber; owl:minCardinality "0"^^xsd:nonNegativeInteger].

text-structure:Section
	a owl:Class;
	rdfs:label "text section"@en, "Textabschnitt"@de;
	rdfs:comment """Composition of paragraphs, mostly about a certain topic."""@en;
	rdfs:subClassOf text-structure:SentenceStructure, text-structure:CompositionalContentStructure, [
#		a owl:Restriction; owl:onProperty text-structure:isSectionOfExpression; owl:allValuesFrom text-structure:Section], [
		a owl:Restriction; owl:onProperty text-structure:isSectionOfExpression; owl:minCardinality "0"^^xsd:nonNegativeInteger], [
		a owl:Restriction; owl:onProperty text-structure:isSectionOfExpressionValue; owl:minCardinality "0"^^xsd:nonNegativeInteger], [
		a owl:Restriction; owl:onProperty text-structure:sectionHasTitle; owl:minCardinality "0"^^xsd:nonNegativeInteger], [
		a owl:Restriction; owl:onProperty text-structure:sectionHasNumber; owl:minCardinality "0"^^xsd:nonNegativeInteger].

text-structure:OrthographicWord
	a owl:Class;
	rdfs:label "orthographic word"@en, "orthographisches Wort"@de;
	rdfs:comment """Smallest independent orthographic entity composed of symbols, surrounded by whitespace in a written text line."""@en;
	rdfs:subClassOf text:WrittenText, ling:Concept, [
#		a owl:Restriction; owl:onProperty text-structure:isWordBeforeSpace; owl:allValuesFrom text-structure:LineSpace], [
		a owl:Restriction; owl:onProperty text-structure:isWordBeforeSpace; owl:minCardinality "0"^^xsd:nonNegativeInteger], [
		a owl:Restriction; owl:onProperty text-structure:isWordBeforeSpaceValue; owl:minCardinality "0"^^xsd:nonNegativeInteger], [
#		a owl:Restriction; owl:onProperty text-structure:isWordOfLine; owl:allValuesFrom text-structure:Line], [
		a owl:Restriction; owl:onProperty text-structure:isWordOfLine; owl:minCardinality "0"^^xsd:nonNegativeInteger], [
		a owl:Restriction; owl:onProperty text-structure:isWordOfLineValue; owl:minCardinality "0"^^xsd:nonNegativeInteger].

text-structure:OrthographoSyntacticWord
	a owl:Class;
	rdfs:label "orthographo-syntactic word"@en, "orthographosyntaktisches Wort"@de;
	rdfs:comment """Word being orthographic and syntactic."""@en;
	skos:note """Common word."""@en;
	rdfs:subClassOf text-structure:OrthographicWord, text-structure:SyntacticWord.

text-structure:LineSpace
	a owl:Class;
	rdfs:label "text line space"@en, "Leerzeichen einer Textzeile"@de;
	rdfs:comment """Empty space between orthographic words in a text line."""@en;
	rdfs:subClassOf text-structure:ReadabilityStructure, [
#		a owl:Restriction; owl:onProperty text-structure:isSpaceBeforeWord; owl:allValuesFrom text-structure:OrthographicWord], [
		a owl:Restriction; owl:onProperty text-structure:isSpaceBeforeWord; owl:minCardinality "0"^^xsd:nonNegativeInteger], [
		a owl:Restriction; owl:onProperty text-structure:isSpaceBeforeWordValue; owl:minCardinality "0"^^xsd:nonNegativeInteger], [
#		a owl:Restriction; owl:onProperty text-structure:isSpaceOfLine; owl:allValuesFrom text-structure:Line], [
		a owl:Restriction; owl:onProperty text-structure:isSpaceOfLine; owl:minCardinality "0"^^xsd:nonNegativeInteger], [
		a owl:Restriction; owl:onProperty text-structure:isSpaceOfLineValue; owl:minCardinality "0"^^xsd:nonNegativeInteger].

text-structure:Punctuation
	a owl:Class;
	rdfs:label "punctuation"@en, "Interpunktion"@de;
	rdfs:comment """One or more language symbols in written text, different from a letter, to help interpret semantics of a sentence."""@en;
	rdfs:subClassOf text-structure:ReadabilityStructure, text-structure:SyntacticStructure, ling:Symbol, [
		a owl:Restriction; owl:onProperty text-structure:isPunctuationBeforeSpace; owl:minCardinality "0"^^xsd:nonNegativeInteger], [
		a owl:Restriction; owl:onProperty text-structure:isPunctuationBeforeSpaceValue; owl:minCardinality "0"^^xsd:nonNegativeInteger], [	
		a owl:Restriction; owl:onProperty text-structure:isPunctuationBeforeWord; owl:minCardinality "0"^^xsd:nonNegativeInteger], [
		a owl:Restriction; owl:onProperty text-structure:isPunctuationBeforeWordValue; owl:minCardinality "0"^^xsd:nonNegativeInteger], [
		a owl:Restriction; owl:onProperty text-structure:isPunctuationOfSentence; owl:minCardinality "0"^^xsd:nonNegativeInteger], [
		a owl:Restriction; owl:onProperty text-structure:isPunctuationOfSentenceValue; owl:minCardinality "0"^^xsd:nonNegativeInteger].

text-structure:Line # :hasEndOfLine
	a owl:Class;
	rdfs:label "text line"@en, "Textzeile"@de, "ligne de texte"@fr, "riga di testo"@it;
	rdfs:comment """Text structured as a line."""@en;
	rdfs:subClassOf text-structure:ReadabilityStructure, [
		a owl:Restriction; owl:onProperty text-structure:lineHasNumber; owl:minCardinality "0"^^xsd:nonNegativeInteger].

# page text line

# page text line

# horizontal page text line (max. length = page width - L/R margins)

# vertical page text line (max. length (or height) = page height - top/bottom margins)

text-structure:Column
	a owl:Class;
	rdfs:label "text column"@en, "Textspalte"@de, "colonne de texte"@fr, "colonna di testo"@it;
	rdfs:comment """Text structured as a column."""@en;
	rdfs:subClassOf text-structure:ReadabilityStructure, [
#		a owl:Restriction; owl:onProperty text-structure:isTextOfColumn; owl:allValuesFrom document:Column], [
		a owl:Restriction; owl:onProperty text-structure:isTextOfColumn; owl:minCardinality "0"^^xsd:nonNegativeInteger], [
		a owl:Restriction; owl:onProperty text-structure:isTextOfColumnValue; owl:minCardinality "0"^^xsd:nonNegativeInteger], [
#		a owl:Restriction; owl:onProperty text-structure:isColumnOfPage; owl:allValuesFrom document:Page], [
		a owl:Restriction; owl:onProperty text-structure:isColumnOfPage; owl:minCardinality "0"^^xsd:nonNegativeInteger], [
		a owl:Restriction; owl:onProperty text-structure:isColumnOfPageValue; owl:minCardinality "0"^^xsd:nonNegativeInteger].

text-structure:ColumnLine
	a owl:Class;
	rdfs:label "text column line"@en, "Textspaltezeile"@de, "ligne de colonne de texte"@fr, "riga di colonna di testo"@it;
	rdfs:comment """Text line of a text column."""@en;
	skos:note """Maximum length of a column line equals the column width."""@en;
	rdfs:subClassOf text-structure:Line, [
#		a owl:Restriction; owl:onProperty text-structure:isLineOfColumn; owl:allValuesFrom document:Column], [
		a owl:Restriction; owl:onProperty text-structure:isLineOfColumn; owl:minCardinality "0"^^xsd:nonNegativeInteger], [
		a owl:Restriction; owl:onProperty text-structure:isLineOfColumnValue; owl:minCardinality "0"^^xsd:nonNegativeInteger].

text-structure:Page
	a owl:Class;
	rdfs:label "text page"@en, "Textseite"@de, "page de texte"@fr, "pagina di testo"@it;
	rdfs:comment """Text structured as a page."""@en;
	rdfs:subClassOf text-structure:ReadabilityStructure, [
		a owl:Restriction; owl:onProperty text-structure:isTextOfPage; owl:minCardinality "0"^^xsd:nonNegativeInteger], [
		a owl:Restriction; owl:onProperty text-structure:isTextOfPageValue; owl:minCardinality "0"^^xsd:nonNegativeInteger], [
		a owl:Restriction; owl:onProperty text-structure:isPageOfExpression; owl:minCardinality "0"^^xsd:nonNegativeInteger], [
		a owl:Restriction; owl:onProperty text-structure:isPageOfExpressionValue; owl:minCardinality "0"^^xsd:nonNegativeInteger].

text-structure:PageLine
	a owl:Class;
	rdfs:label "text page line"@en, "Textseitezeile"@de, "ligne de page de texte"@fr, "riga di pagina di testo"@it;
	rdfs:comment """Text line of a text page."""@en;
	skos:note """Maximum length of a page line equals the page width minus margins."""@en;
	rdfs:subClassOf text-structure:Line, [
#		a owl:Restriction; owl:onProperty text-structure:isLineOfColumn; owl:allValuesFrom document:Column], [
		a owl:Restriction; owl:onProperty text-structure:isLineOfPage; owl:minCardinality "0"^^xsd:nonNegativeInteger], [
		a owl:Restriction; owl:onProperty text-structure:isLineOfPageValue; owl:minCardinality "0"^^xsd:nonNegativeInteger].

text-structure:Table #Â° tableHasTitle, tableHasField, tableHasRow, tableHasColumn
	a owl:Class;
	rdfs:label "text table"@en, "Texttabelle"@de;
	rdfs:comment """Two-dimensional structure composed of one or more fields containing text, and  being part of a vertical column and a horizontal row, both with own identifier."""@en;
	rdfs:subClassOf text-structure:CompositionalContentStructure, document:Table.

text-structure:Rhyme
	a owl:Class;
	rdfs:label "rhyme"@en, "Reim"@de;
	rdfs:comment """Words or phrases with whole or end corresponding sound, especially when involving the last stressed vowel and all succeeding sounds."""@en;
	rdfs:subClassOf text-structure:ContentStructure.

text-structure:Dialogue
	a owl:Class;
	rdfs:label "dialogue"@en, "Dialog"@de;
	rdfs:comment """Text with dialogue structure."""@en;
	rdfs:subClassOf text-structure:CompositionalContentStructure.

text-structure:Diary
	a owl:Class;
	rdfs:label "diary structure"@en, "Tagebuch-Struktur"@de;
	rdfs:comment """Text with diary structure."""@en;
	rdfs:subClassOf text-structure:CompositionalContentStructure, [
		a owl:Restriction; owl:onProperty text-structure:isDiaryStructureOfExpression; owl:minCardinality "0"^^xsd:nonNegativeInteger], [
		a owl:Restriction; owl:onProperty text-structure:isDiaryStructureOfExpressionValue; owl:minCardinality "0"^^xsd:nonNegativeInteger].

text-structure:Postcard
	a owl:Class;
	rdfs:label "postcard structure"@en, "Postkarte-Struktur"@de;
	rdfs:comment """Text with postcard structure."""@en;
	rdfs:subClassOf text-structure:CompositionalContentStructure, [
		a owl:Restriction; owl:onProperty text-structure:isPostcardStructureOfExpression; owl:minCardinality "0"^^xsd:nonNegativeInteger], [
		a owl:Restriction; owl:onProperty text-structure:isPostcardStructureOfExpressionValue; owl:minCardinality "0"^^xsd:nonNegativeInteger].

#
# PROPERTIES
#

text-structure:isPartOfTextExpression
	a owl:ObjectProperty;
	rdfs:label "is part of text expression"@en, "ist Teil einer Textexpression"@de;
	rdfs:comment """Relating a text structure to a text expression it is part of."""@en;
	rdfs:domain text-structure:Structure;
	rdfs:range text-expression:Expression;
	rdfs:subPropertyOf concept:isPartOf;
	knora-base:subjectClassConstraint text-structure:Structure;
	knora-base:objectClassConstraint text-expression:Expression.

text-structure:isPartOfTextExpressionValue
	a owl:ObjectProperty;
	rdfs:label "is part of text expression - statement"@en, "ist Teil einer Textexpression - Festlegung"@de;
	rdfs:comment """Relating a text structure to a reification statement of the relation between the text structure and a text expression it is part of."""@en;
	rdfs:subPropertyOf concept:isPartOfValue;
	knora-base:subjectClassConstraint text-structure:Structure;
	knora-base:objectClassConstraint knora-base:LinkValue.

text-structure:hasIdentifier
	a owl:ObjectProperty;
	rdfs:label "text structure has identifier"@en, "Textstruktur hat Identifikator"@de;
	rdfs:comment """Relating a text structure to its identifier."""@en;
	rdfs:domain text-structure:Structure;
	rdfs:range text-structure:Identifier;
	rdfs:subPropertyOf document:contentStructureHasIdentifier;
	knora-base:subjectClassConstraint text-structure:Structure;
	knora-base:objectClassConstraint text-structure:Identifier.

text-structure:hasIdentifierValue
	a owl:ObjectProperty;
	rdfs:label "text structure has identifier - statement"@en, "Textstruktur hat Identifikator - Festlegung"@de;
	rdfs:comment """Relating a text structure to a reification statement of the relation between the structure and its identifier."""@en;
	rdfs:subPropertyOf document:contentStructureHasIdentifierValue;
	knora-base:subjectClassConstraint text-structure:Structure;
	knora-base:objectClassConstraint knora-base:LinkValue.

text-structure:syntacticWordHasForm
	a owl:ObjectProperty;
	rdfs:label "syntactic word has form"@en, "syntaktisches Wort hat Form"@de;
	rdfs:comment """Relating a syntactic word to its form."""@en;
	rdfs:domain text-structure:SyntacticWord;
	rdfs:range lingmor:SyntacticWordForm;
	rdfs:subPropertyOf knora-base:hasLinkTo;
	knora-base:subjectClassConstraint text-structure:SyntacticWord;
	knora-base:objectClassConstraint lingmor:SyntacticWordForm.

text-structure:syntacticWordHasFormValue
	a owl:ObjectProperty;
	rdfs:label "syntactic word has form - statement"@en, "syntaktisches Wort hat Form - Festlegung"@de;
	rdfs:comment """Relating a syntactic word to a reification statement of the relation between the word and its form."""@en;
	rdfs:subPropertyOf knora-base:hasLinkToValue;
	knora-base:subjectClassConstraint text-structure:SyntacticWord;
	knora-base:objectClassConstraint knora-base:LinkValue.

text-structure:isWordBeforePunctuation
	a owl:ObjectProperty;
	rdfs:label "is word before punctuation"@en, "ist Wort vor einer Interpunktion"@de;
	rdfs:comment """Relating a syntactic word to the punctuation it precedes."""@en;
	rdfs:domain text-structure:SyntacticWord;
	rdfs:range text-structure:Punctuation;
	rdfs:subPropertyOf knora-base:hasLinkTo;
	knora-base:subjectClassConstraint text-structure:SyntacticWord;
	knora-base:objectClassConstraint text-structure:Punctuation.

text-structure:isWordBeforePunctuationValue
	a owl:ObjectProperty;
	rdfs:label "is word before punctuation - statement"@en, "ist Wort vor einer Interpunktion - Festlegung"@de;
	rdfs:comment """Relating a syntactic word to a reification statement of the relation between the word and the punctuation it precedes."""@en;
	rdfs:subPropertyOf knora-base:hasLinkToValue;
	knora-base:subjectClassConstraint text-structure:SyntacticWord;
	knora-base:objectClassConstraint knora-base:LinkValue.

text-structure:isWordOfSentence
	a owl:ObjectProperty;
	rdfs:label "is word of sentence"@en, "ist Wort eines Satzes"@de;
	rdfs:comment """Relating a syntactic word to the sentence it is part of."""@en;
	rdfs:domain text-structure:SyntacticWord;
	rdfs:range text-structure:Sentence;
	rdfs:subPropertyOf concept:isPartOf;
	knora-base:subjectClassConstraint text-structure:SyntacticWord;
	knora-base:objectClassConstraint text-structure:Sentence.

text-structure:isWordOfSentenceValue
	a owl:ObjectProperty;
	rdfs:label "is word of sentence - statement"@en, "ist Wort eines Satzes - Festlegung"@de;
	rdfs:comment """Relating a syntactic word to a reification statement of the relation between the word and the sentence it is part of."""@en;
	rdfs:subPropertyOf concept:isPartOfValue;
	knora-base:subjectClassConstraint text-structure:SyntacticWord;
	knora-base:objectClassConstraint knora-base:LinkValue.

text-structure:isSentenceOfParagraph
	a owl:ObjectProperty;
	rdfs:label "is sentence of paragraph"@en, "ist Satz eines Paragrafen"@de;
	rdfs:comment """Relating a sentence to a paragraph it is part of."""@en;
	rdfs:domain text-structure:Sentence;
	rdfs:range text-structure:Paragraph;
	rdfs:subPropertyOf concept:isPartOf;
	knora-base:subjectClassConstraint text-structure:Sentence;
	knora-base:objectClassConstraint text-structure:Paragraph.

text-structure:isSentenceOfParagraphValue
	a owl:ObjectProperty;
	rdfs:label "is sentence of paragraph - statement"@en, "ist Satz eines Paragrafen - Festlegung"@de;
	rdfs:comment """Relating a sentence to a reification statement of the relation between the sentence and a paragraph it is part of."""@en;
	rdfs:subPropertyOf concept:isPartOfValue;
	knora-base:subjectClassConstraint text-structure:Sentence;
	knora-base:objectClassConstraint knora-base:LinkValue.

text-structure:isSentenceOfProse
	a owl:ObjectProperty;
	rdfs:label "is sentence of prose"@en, "ist Satz einer Prosa"@de;
	rdfs:comment """Relating a sentence to a prose it is part of."""@en;
	rdfs:domain text-structure:Sentence;
	rdfs:range text-structure:Prose;
	rdfs:subPropertyOf concept:isPartOf;
	knora-base:subjectClassConstraint text-structure:Sentence;
	knora-base:objectClassConstraint text-structure:Prose.

text-structure:isSentenceOfProseValue
	a owl:ObjectProperty;
	rdfs:label "is sentence of prose - statement"@en, "ist Satz einer Prosa - Festlegung"@de;
	rdfs:comment """Relating a sentence to a reification statement of the relation between the sentence and a prose it is part of."""@en;
	rdfs:subPropertyOf concept:isPartOfValue;
	knora-base:subjectClassConstraint text-structure:Sentence;
	knora-base:objectClassConstraint knora-base:LinkValue.

text-structure:isProseOfExpression
	a owl:ObjectProperty;
	rdfs:label "is prose of sentence expression"@en, "ist Prosa einer Satz-Expression"@de;
	rdfs:comment """Relating a prose to a sentence expression it is part of."""@en;
	rdfs:domain text-structure:Prose;
	rdfs:range text-expression:SentenceExpression;
	rdfs:subPropertyOf text-structure:isPartOfTextExpression;
	knora-base:subjectClassConstraint text-structure:Prose;
	knora-base:objectClassConstraint text-expression:SentenceExpression.

text-structure:isProseOfExpressionValue
	a owl:ObjectProperty;
	rdfs:label "is prose of sentence expression - statement"@en, "ist Prosa einer Satz-Expression - Festlegung"@de;
	rdfs:comment """Relating a prose to a reification statement of the relation between the prose and a sentence expression it is part of."""@en;
	rdfs:subPropertyOf text-structure:isPartOfTextExpressionValue;
	knora-base:subjectClassConstraint text-structure:Prose;
	knora-base:objectClassConstraint knora-base:LinkValue.

text-structure:isParagraphOfSection
	a owl:ObjectProperty;
	rdfs:label "is paragraph of section"@en, "ist Paragraf eines Textabschnittes"@de;
	rdfs:comment """Relating a paragraph to a section it is part of."""@en;
	rdfs:domain text-structure:Paragraph;
	rdfs:range text-structure:Section;
	rdfs:subPropertyOf concept:isPartOf;
	knora-base:subjectClassConstraint text-structure:Paragraph;
	knora-base:objectClassConstraint text-structure:Section.

text-structure:isParagraphOfSectionValue
	a owl:ObjectProperty;
	rdfs:label "is paragraph of section - statement"@en, "ist Paragraf eines Textabschnittes - Festlegung"@de;
	rdfs:comment """Relating a paragraph to a reification statement of the relation between the paragraph and a section it is part of."""@en;
	rdfs:subPropertyOf concept:isPartOfValue;
	knora-base:subjectClassConstraint text-structure:Paragraph;
	knora-base:objectClassConstraint knora-base:LinkValue.

text-structure:paragraphHasTitle
	a owl:ObjectProperty;
	rdfs:label "paragraph has title"@en, "Paragraf hat Titel"@de;
	rdfs:comment """Relating a paragraph to its title."""@en;
	rdfs:domain text-structure:Paragraph;
	rdfs:range rdfs:Literal;
	rdfs:subPropertyOf text:hasTitle;
	knora-base:subjectClassConstraint text-structure:Paragraph;
	knora-base:objectClassConstraint knora-base:TextValue.

text-structure:paragraphHasNumber
	a owl:ObjectProperty;
	rdfs:label "paragraph has number"@en, "Paragraf hat Nummer"@de;
	rdfs:comment """Relating a paragraph to its number."""@en;
	rdfs:domain text-structure:Paragraph;
	rdfs:range xsd:nonNegativeInteger;
	rdfs:subPropertyOf knora-base:hasValue;
	knora-base:subjectClassConstraint text-structure:Paragraph;
	knora-base:objectClassConstraint knora-base:IntValue.

text-structure:isSectionOfExpression
	a owl:ObjectProperty;
	rdfs:label "is section of sentence expression"@en, "ist Textabschnitt eines Satz-Expression"@de;
	rdfs:comment """Relating a section to a sentence expression it is part of."""@en;
	rdfs:domain text-structure:Section;
	rdfs:range text-expression:SentenceExpression;
	rdfs:subPropertyOf text-structure:isPartOfTextExpression;
	knora-base:subjectClassConstraint text-structure:Section;
	knora-base:objectClassConstraint text-expression:SentenceExpression.

text-structure:isSectionOfExpressionValue
	a owl:ObjectProperty;
	rdfs:label "is section of sentence expression - statement"@en, "ist Textabschnitt eines Satz-Expression - Festlegung"@de;
	rdfs:comment """Relating a section to a reification statement of the relation between the section and a sentence expression it is part of."""@en;
	rdfs:subPropertyOf text-structure:isPartOfTextExpressionValue;
	knora-base:subjectClassConstraint text-structure:Section;
	knora-base:objectClassConstraint knora-base:LinkValue.

text-structure:sectionHasTitle
	a owl:ObjectProperty;
	rdfs:label "section has title"@en, "Textabschnitt hat Titel"@de;
	rdfs:comment """Relating a section to its title."""@en;
	rdfs:domain text-structure:Section;
	rdfs:range rdfs:Literal;
	rdfs:subPropertyOf text:hasTitle;
	knora-base:subjectClassConstraint text-structure:Section;
	knora-base:objectClassConstraint knora-base:TextValue.

text-structure:sectionHasNumber
	a owl:ObjectProperty;
	rdfs:label "section has number"@en, "Textabschnitt hat Nummer"@de;
	rdfs:comment """Relating a section to its number."""@en;
	rdfs:domain text-structure:Section;
	rdfs:range xsd:nonNegativeInteger;
	rdfs:subPropertyOf knora-base:hasValue;
	knora-base:subjectClassConstraint text-structure:Section;
	knora-base:objectClassConstraint knora-base:IntValue.

text-structure:isWordBeforeSpace
	a owl:ObjectProperty;
	rdfs:label "is word before space"@en, "ist Wort vor einem Leerzeichen"@de;
	rdfs:comment """Relating an orthographic word to the text line space it precedes."""@en;
	rdfs:domain text-structure:OrthographicWord;
	rdfs:range text-structure:LineSpace;
	rdfs:subPropertyOf knora-base:hasLinkTo;
	knora-base:subjectClassConstraint text-structure:OrthographicWord;
	knora-base:objectClassConstraint text-structure:LineSpace.

text-structure:isWordBeforeSpaceValue
	a owl:ObjectProperty;
	rdfs:label "is word before space - statement"@en, "ist Wort vor einem Leerzeichen - Festlegung"@de;
	rdfs:comment """Relating an orthographic word to a reification statement of the relation between the word and the text line space it precedes."""@en;
	rdfs:subPropertyOf knora-base:hasLinkToValue;
	knora-base:subjectClassConstraint text-structure:OrthographicWord;
	knora-base:objectClassConstraint knora-base:LinkValue.

text-structure:isWordOfLine
	a owl:ObjectProperty;
	rdfs:label "is word of line"@en, "ist Wort einer Zeile"@de;
	rdfs:comment """Relating an orthographic word to the text line it is part of."""@en;
	rdfs:domain text-structure:OrthographicWord;
	rdfs:range text-structure:Line;
	rdfs:subPropertyOf concept:isPartOf;
	knora-base:subjectClassConstraint text-structure:OrthographicWord;
	knora-base:objectClassConstraint text-structure:Line.

text-structure:isWordOfLineValue
	a owl:ObjectProperty;
	rdfs:label "is word of line - statement"@en, "ist Wort einer Zeile - Festlegung"@de;
	rdfs:comment """Relating an orthographic word to a reification statement of the relation between the word and the text line it is part of."""@en;
	rdfs:subPropertyOf concept:isPartOfValue;
	knora-base:subjectClassConstraint text-structure:OrthographicWord;
	knora-base:objectClassConstraint knora-base:LinkValue.

text-structure:isSpaceBeforeWord
	a owl:ObjectProperty;
	rdfs:label "is space before word"@en, "ist Leerzeichen vor einem Wort"@de;
	rdfs:comment """Relating a text line space to the orthographic word it precedes."""@en;
	rdfs:domain text-structure:LineSpace;
	rdfs:range text-structure:OrthographicWord;
	rdfs:subPropertyOf knora-base:hasLinkTo;
	knora-base:subjectClassConstraint text-structure:LineSpace;
	knora-base:objectClassConstraint text-structure:OrthographicWord.

text-structure:isSpaceBeforeWordValue
	a owl:ObjectProperty;
	rdfs:label "is space before word - statement"@en, "ist Leerzeichen vor einem Wort - Festlegung"@de;
	rdfs:comment """Relating a text line space to a reification statement of the relation between the space and the orthographic word it precedes."""@en;
	rdfs:subPropertyOf knora-base:hasLinkToValue;
	knora-base:subjectClassConstraint text-structure:LineSpace;
	knora-base:objectClassConstraint knora-base:LinkValue.

text-structure:isSpaceOfLine
	a owl:ObjectProperty;
	rdfs:label "is space of line"@en, "ist Leerzeichen einer Zeile"@de;
	rdfs:comment """Relating a space to a text line it is part of."""@en;
	rdfs:domain text-structure:LineSpace;
	rdfs:range text-structure:Line;
	rdfs:subPropertyOf concept:isPartOf;
	knora-base:subjectClassConstraint text-structure:LineSpace;
	knora-base:objectClassConstraint text-structure:Line.

text-structure:isSpaceOfLineValue
	a owl:ObjectProperty;
	rdfs:label "is space of line - statement"@en, "ist Leerzeichen einer Zeile - Festlegung"@de;
	rdfs:comment """Relating a space to a reification statement of the relation between the space and a text line it is part of."""@en;
	rdfs:subPropertyOf concept:isPartOfValue;
	knora-base:subjectClassConstraint text-structure:LineSpace;
	knora-base:objectClassConstraint knora-base:LinkValue.

text-structure:isPunctuationBeforeSpace
	a owl:ObjectProperty;
	rdfs:label "is punctuation before space"@en, "ist Interpunktion vor einem Leerzeichen"@de;
	rdfs:comment """Relating a punctuation to the space it precedes."""@en;
	rdfs:domain text-structure:Punctuation;
	rdfs:range text-structure:LineSpace;
	rdfs:subPropertyOf knora-base:hasLinkTo;
	knora-base:subjectClassConstraint text-structure:Punctuation;
	knora-base:objectClassConstraint text-structure:LineSpace.

text-structure:isPunctuationBeforeSpaceValue
	a owl:ObjectProperty;
	rdfs:label "is punctuation before space - statement"@en, "ist Interpunktion vor einem Leerzeichen - Festlegung"@de;
	rdfs:comment """Relating a punctuation to a reification statement of the relation between the punctuation and the space it precedes."""@en;
	rdfs:subPropertyOf knora-base:hasLinkToValue;
	knora-base:subjectClassConstraint text-structure:Punctuation;
	knora-base:objectClassConstraint knora-base:LinkValue.

text-structure:isPunctuationBeforeWord
	a owl:ObjectProperty;
	rdfs:label "is punctuation before word"@en, "ist Interpunktion vor einem Wort"@de;
	rdfs:comment """Relating a punctuation to the word it precedes."""@en;
	rdfs:domain text-structure:Punctuation;
	rdfs:range text-structure:SyntacticWord;
	rdfs:subPropertyOf knora-base:hasLinkTo;
	knora-base:subjectClassConstraint text-structure:Punctuation;
	knora-base:objectClassConstraint text-structure:SyntacticWord.

text-structure:isPunctuationBeforeWordValue
	a owl:ObjectProperty;
	rdfs:label "is punctuation before word - statement"@en, "ist Interpunktion vor einem Wort - Festlegung"@de;
	rdfs:comment """Relating a punctuation to a reification statement of the relation between the punctuation and the word it precedes."""@en;
	rdfs:subPropertyOf knora-base:hasLinkToValue;
	knora-base:subjectClassConstraint text-structure:Punctuation;
	knora-base:objectClassConstraint knora-base:LinkValue.

text-structure:isPunctuationOfSentence
	a owl:ObjectProperty;
	rdfs:label "is punctuation of sentence"@en, "ist Interpunktion eines Satzes"@de;
	rdfs:comment """Relating a punctuation to the sentence it is part of."""@en;
	rdfs:domain text-structure:Punctuation;
	rdfs:range text-structure:Sentence;
	rdfs:subPropertyOf concept:isPartOf;
	knora-base:subjectClassConstraint text-structure:Punctuation;
	knora-base:objectClassConstraint text-structure:Sentence.

text-structure:isPunctuationOfSentenceValue
	a owl:ObjectProperty;
	rdfs:label "is punctuation of sentence - statement"@en, "ist Interpunktion eines Satzes - Festlegung"@de;
	rdfs:comment """Relating a punctuation to a reification statement of the relation between the punctuation and the sentence it is part of."""@en;
	rdfs:subPropertyOf concept:isPartOfValue;
	knora-base:subjectClassConstraint text-structure:Punctuation;
	knora-base:objectClassConstraint knora-base:LinkValue.

text-structure:lineHasNumber
	a owl:ObjectProperty;
	rdfs:label "line has number"@en, "Linie hat Nummer"@de;
	rdfs:comment """Relating a line to a number it has."""@en;
	rdfs:domain text-structure:Line;
	rdfs:range xsd:nonNegativeInteger;
	rdfs:subPropertyOf knora-base:hasValue;
	knora-base:subjectClassConstraint text-structure:Line;
	knora-base:objectClassConstraint knora-base:IntValue.

text-structure:isLineOfColumn
	a owl:ObjectProperty;
	rdfs:label "is line of column"@en, "ist Zeile einer Spalte"@de;
	rdfs:comment """Relating a text line to a column it is part of."""@en;
	rdfs:domain text-structure:ColumnLine;
	rdfs:range text-structure:Column;
	rdfs:subPropertyOf concept:isPartOf;
	knora-base:subjectClassConstraint text-structure:ColumnLine;
	knora-base:objectClassConstraint text-structure:Column.

text-structure:isLineOfColumnValue
	a owl:ObjectProperty;
	rdfs:label "is line of column - statement"@en, "ist Zeile einer Spalte - Festlegung"@de;
	rdfs:comment """Relating a text line to a reification statement of the relation between the line and a column it is part of."""@en;
	rdfs:subPropertyOf concept:isPartOfValue;
	knora-base:subjectClassConstraint text-structure:ColumnLine;
	knora-base:objectClassConstraint knora-base:LinkValue.

text-structure:isTextOfColumn
	a owl:ObjectProperty;
	rdfs:label "is text of column"@en, "ist Text einer Spalte"@de;
	rdfs:comment """Relating text to a column it is part of."""@en;
	rdfs:domain text-structure:Column;
	rdfs:range document:Column;
	rdfs:subPropertyOf concept:isPartOf;
	knora-base:subjectClassConstraint text-structure:Column;
	knora-base:objectClassConstraint document:Column.

text-structure:isTextOfColumnValue
	a owl:ObjectProperty;
	rdfs:label "is text of column - statement"@en, "ist Text einer Spalte - Festlegung"@de;
	rdfs:comment """Relating a text to a reification statement of the relation between the text and a column it is part of."""@en;
	rdfs:subPropertyOf concept:isPartOfValue;
	knora-base:subjectClassConstraint text-structure:Column;
	knora-base:objectClassConstraint knora-base:LinkValue.

text-structure:isColumnOfPage
	a owl:ObjectProperty;
	rdfs:label "is column of text page"@en, "ist Spalte einer Textseite"@de;
	rdfs:comment """Relating a column to a text page it is part of."""@en;
	rdfs:domain text-structure:Column;
	rdfs:range text-structure:Page;
	rdfs:subPropertyOf concept:isPartOf;
	knora-base:subjectClassConstraint text-structure:Column;
	knora-base:objectClassConstraint text-structure:Page.

text-structure:isColumnOfPageValue
	a owl:ObjectProperty;
	rdfs:label "is column of text page - statement"@en, "ist Spalte einer Textseite - Festlegung"@de;
	rdfs:comment """Relating a column to a reification statement of the relation between the column and a text page it is part of."""@en;
	rdfs:subPropertyOf concept:isPartOfValue;
	knora-base:subjectClassConstraint text-structure:Column;
	knora-base:objectClassConstraint knora-base:LinkValue.

text-structure:isTextOfPage
	a owl:ObjectProperty;
	rdfs:label "is text of page"@en, "ist Text einer Seite"@de;
	rdfs:comment """Relating a text page to a document page it is part of."""@en;
	rdfs:domain text-structure:Page;
	rdfs:range document:Page;
	rdfs:subPropertyOf concept:isPartOf;
	knora-base:subjectClassConstraint text-structure:Page;
	knora-base:objectClassConstraint document:Page.

text-structure:isTextOfPageValue
	a owl:ObjectProperty;
	rdfs:label "is text of page - statement"@en, "ist Text einer Seite - Festlegung"@de;
	rdfs:comment """Relating a text page to a reification statement of the relation between the text page and a document page it is part of."""@en;
	rdfs:subPropertyOf concept:isPartOfValue;
	knora-base:subjectClassConstraint text-structure:Page;
	knora-base:objectClassConstraint knora-base:LinkValue.

text-structure:isPageOfExpression
	a owl:ObjectProperty;
	rdfs:label "is page of text expression"@en, "ist Seite einer Textexpression"@de;
	rdfs:comment """Relating a text page to a text expression it is part of."""@en;
	rdfs:domain text-structure:Page;
	rdfs:range text-expression:Expression;
	rdfs:subPropertyOf concept:isPartOf;
	knora-base:subjectClassConstraint text-structure:Page;
	knora-base:objectClassConstraint text-expression:Expression.

text-structure:isPageOfExpressionValue
	a owl:ObjectProperty;
	rdfs:label "is text page of expression - statement"@en, "ist Seite einer Textexpression - Festlegung"@de;
	rdfs:comment """Relating a text page to a reification statement of the relation between the page and a text expression it is part of."""@en;
	rdfs:subPropertyOf concept:isPartOfValue;
	knora-base:subjectClassConstraint text-structure:Page;
	knora-base:objectClassConstraint knora-base:LinkValue.

text-structure:isLineOfPage
	a owl:ObjectProperty;
	rdfs:label "is line of page"@en, "ist Zeile einer Seite"@de;
	rdfs:comment """Relating a text line to a page it is part of."""@en;
	rdfs:domain text-structure:PageLine;
	rdfs:range text-structure:Page;
	rdfs:subPropertyOf concept:isPartOf;
	knora-base:subjectClassConstraint text-structure:PageLine;
	knora-base:objectClassConstraint text-structure:Page.

text-structure:isLineOfPageValue
	a owl:ObjectProperty;
	rdfs:label "is line of page - statement"@en, "ist Zeile einer Seite - Festlegung"@de;
	rdfs:comment """Relating a text line to a reification statement of the relation between the line and a page it is part of."""@en;
	rdfs:subPropertyOf concept:isPartOfValue;
	knora-base:subjectClassConstraint text-structure:PageLine;
	knora-base:objectClassConstraint knora-base:LinkValue.

text-structure:isPostcardStructureOfExpression
	a owl:ObjectProperty;
	rdfs:label "is postcard structure of expression"@en, "ist Postkarte-Struktur einer Expression"@de;
	rdfs:comment """Relating a postcard structure to a text expression it is part of."""@en;
	rdfs:domain text-structure:Postcard;
	rdfs:range text-expression:Expression;
	rdfs:subPropertyOf text-structure:isPartOfTextExpression;
	knora-base:subjectClassConstraint text-structure:Postcard;
	knora-base:objectClassConstraint text-expression:Expression.

text-structure:isPostcardStructureOfExpressionValue
	a owl:ObjectProperty;
	rdfs:label "is postcard structure of expression - statement"@en, "ist Postkarte-Struktur einer Expression - Festlegung"@de;
	rdfs:comment """Relating a postcard structure to a reification statement of the relation between the postcard structure and a text expression it is part of."""@en;
	rdfs:subPropertyOf text-structure:isPartOfTextExpressionValue;
	knora-base:subjectClassConstraint text-structure:Postcard;
	knora-base:objectClassConstraint knora-base:LinkValue.

text-structure:isDiaryStructureOfExpression
	a owl:ObjectProperty;
	rdfs:label "is diary structure of expression"@en, "ist Tagebuch-Struktur einer Expression"@de;
	rdfs:comment """Relating a diary structure to a text expression it is part of."""@en;
	rdfs:domain text-structure:Diary;
	rdfs:range text-expression:Expression;
	rdfs:subPropertyOf text-structure:isPartOfTextExpression;
	knora-base:subjectClassConstraint text-structure:Diary;
	knora-base:objectClassConstraint text-expression:Expression.

text-structure:isDiaryStructureOfExpressionValue
	a owl:ObjectProperty;
	rdfs:label "is diary structure of expression - statement"@en, "ist Tagebuch-Struktur einer Expression - Festlegung"@de;
	rdfs:comment """Relating a diary structure to a reification statement of the relation between the diary structure and a text expression it is part of."""@en;
	rdfs:subPropertyOf text-structure:isPartOfTextExpressionValue;
	knora-base:subjectClassConstraint text-structure:Diary;
	knora-base:objectClassConstraint knora-base:LinkValue.