@prefix rdfs: <http://www.w3.org/2000/01/rdf-schema#>.
@prefix owl: <http://www.w3.org/2002/07/owl#>.
@prefix xsd: <http://www.w3.org/2001/XMLSchema#>.
@prefix skos: <http://www.w3.org/2004/02/skos/core#>.
@prefix dct: <http://purl.org/dc/terms/>.
@prefix foaf: <http://xmlns.com/foaf/0.1/>.
@prefix cidoc: <http://www.cidoc-crm.org/cidoc-crm/>.
@prefix frbroo: <http://iflastandards.info/ns/fr/frbr/frbroo/>.
@prefix event: <http://www.knora.org/ontology/shared/event#>.
@prefix human: <http://www.knora.org/ontology/shared/human#>.
@prefix org: <http://www.knora.org/ontology/shared/organization#>.
@prefix language: <http://www.knora.org/ontology/shared/language#>.
@prefix concept: <http://www.knora.org/ontology/shared/concept#>.
@prefix math: <http://www.knora.org/ontology/shared/mathematics#>.
@prefix document: <http://www.knora.org/ontology/shared/document#>.
@prefix text-structure: <http://www.knora.org/ontology/shared/text-structure#>.
@prefix textedit: <http://www.knora.org/ontology/shared/text-editing#>.
@prefix infocar: <http://www.knora.org/ontology/shared/information-carrier#>.
@prefix publish: <http://www.knora.org/ontology/shared/publishing#>.
@prefix litera: <http://www.knora.org/ontology/shared/literature#>.
@prefix knora-base: <http://www.knora.org/ontology/knora-base#>.

@base <http://www.knora.org/ontology/shared/text>.
@prefix text: <http://www.knora.org/ontology/shared/text#>.

<http://www.knora.org/ontology/shared/text>
	a owl:Ontology;
	dct:title "An ontology about text"@en;
	dct:description """Formal description of text in broadest sense, general subclasses, related classes, and properties."""@en;
	skos:note """Text editing is described in a seperate ontology"""@en;
	dct:creator "Hans Cools, MD, knowledge engineer, ontologist, software developer, NIE-INE, Basel University, Switzerland"@en;
	dct:contributor "Roberta Padlina, tool coordinator, software developer, NIE-INE, Basel University, Switzerland"@en;
	dct:publisher "Basel University, Switzerland"@en;
#	skos:note """Representation of an otherwise literal data element as object enabling relating it to other data"""@en.

	knora-base:attachedToProject <http://www.knora.org/ontology/knora-base#DefaultSharedOntologiesProject>. # <http://rdfh.ch/projects/0059>.

#
# CLASSES
#

text:Text
	a owl:Class;
	rdfs:label "text"@en, "Text"@de, "texte"@fr, "testo"@it;
	rdfs:comment """Human natural language expression serialized in writable form."""@en; # what can be learned by heart
	rdfs:subClassOf language:HumanNaturalLanguageExpression, [
		a owl:Restriction; owl:onProperty text:hasLineNumber; owl:minCardinality "0"^^xsd:nonNegativeInteger], [
		a owl:Restriction; owl:onProperty text:hasVersionIndicator; owl:minCardinality "0"^^xsd:nonNegativeInteger], [
		a owl:Restriction; owl:onProperty text:hasPageNumberDescription; owl:minCardinality "0"^^xsd:nonNegativeInteger], [
		a owl:Restriction; owl:onProperty text:hasReferenceText; owl:minCardinality "0"^^xsd:nonNegativeInteger], [
		a owl:Restriction; owl:onProperty text:hasReferenceTextValue; owl:minCardinality "0"^^xsd:nonNegativeInteger], [
		a owl:Restriction; owl:onProperty text:hasRevisor; owl:minCardinality "0"^^xsd:nonNegativeInteger], [
		a owl:Restriction; owl:onProperty text:hasRevisorValue; owl:minCardinality "0"^^xsd:nonNegativeInteger], [
		a owl:Restriction; owl:onProperty text:hasTranscriber; owl:minCardinality "0"^^xsd:nonNegativeInteger], [
		a owl:Restriction; owl:onProperty text:hasTranscriberValue; owl:minCardinality "0"^^xsd:nonNegativeInteger], [
		a owl:Restriction; owl:onProperty text:hasVulgarizer; owl:minCardinality "0"^^xsd:nonNegativeInteger], [
		a owl:Restriction; owl:onProperty text:hasVulgarizerValue; owl:minCardinality "0"^^xsd:nonNegativeInteger], [
		a owl:Restriction; owl:onProperty text:hasCiter; owl:minCardinality "0"^^xsd:nonNegativeInteger], [
		a owl:Restriction; owl:onProperty text:hasCiterValue; owl:minCardinality "0"^^xsd:nonNegativeInteger], [
		a owl:Restriction; owl:onProperty text:hasCitation; owl:minCardinality "0"^^xsd:nonNegativeInteger], [
		a owl:Restriction; owl:onProperty text:hasCitationValue; owl:minCardinality "0"^^xsd:nonNegativeInteger], [
		a owl:Restriction; owl:onProperty text:hasCitationReference; owl:minCardinality "0"^^xsd:nonNegativeInteger], [
		a owl:Restriction; owl:onProperty text:hasCitationReferenceValue; owl:minCardinality "0"^^xsd:nonNegativeInteger], [
		a owl:Restriction; owl:onProperty text:isCitedIn; owl:minCardinality "0"^^xsd:nonNegativeInteger], [
		a owl:Restriction; owl:onProperty text:isCitedInValue; owl:minCardinality "0"^^xsd:nonNegativeInteger], [
		a owl:Restriction; owl:onProperty text:hasEditor; owl:minCardinality "0"^^xsd:nonNegativeInteger], [
		a owl:Restriction; owl:onProperty text:hasEditorValue; owl:minCardinality "0"^^xsd:nonNegativeInteger], [
		a owl:Restriction; owl:onProperty textedit:hasEdition; owl:minCardinality "0"^^xsd:nonNegativeInteger], [
		a owl:Restriction; owl:onProperty textedit:hasEditionValue; owl:minCardinality "0"^^xsd:nonNegativeInteger], [
		a owl:Restriction; owl:onProperty textedit:hasTransliteration; owl:minCardinality "0"^^xsd:nonNegativeInteger], [
		a owl:Restriction; owl:onProperty textedit:hasTransliterationValue; owl:minCardinality "0"^^xsd:nonNegativeInteger], [
		a owl:Restriction; owl:onProperty textedit:hasGlossator; owl:minCardinality "0"^^xsd:nonNegativeInteger], [
		a owl:Restriction; owl:onProperty textedit:hasGlossatorValue; owl:minCardinality "0"^^xsd:nonNegativeInteger], [
		a owl:Restriction; owl:onProperty textedit:hasAbbreviator; owl:minCardinality "0"^^xsd:nonNegativeInteger], [
		a owl:Restriction; owl:onProperty textedit:hasAbbreviatorValue; owl:minCardinality "0"^^xsd:nonNegativeInteger], [
		a owl:Restriction; owl:onProperty textedit:hasRedactor; owl:minCardinality "0"^^xsd:nonNegativeInteger], [
		a owl:Restriction; owl:onProperty textedit:hasRedactorValue; owl:minCardinality "0"^^xsd:nonNegativeInteger], [
		a owl:Restriction; owl:onProperty textedit:hasSameEditionAs; owl:minCardinality "0"^^xsd:nonNegativeInteger], [
		a owl:Restriction; owl:onProperty textedit:hasSameEditionAsValue; owl:minCardinality "0"^^xsd:nonNegativeInteger], [
		a owl:Restriction; owl:onProperty infocar:isTextOnPage; owl:minCardinality "0"^^xsd:nonNegativeInteger], [
		a owl:Restriction; owl:onProperty infocar:isTextOnPageValue; owl:minCardinality "0"^^xsd:nonNegativeInteger].

text:Draft
	a owl:Class;
	rdfs:label "draft"@en, "Entwurf"@de;
	rdfs:comment """Developmental text expression."""@en;
	rdfs:subClassOf text:Text, human:CreationVersion.

text:Development
	a owl:Class;
	rdfs:label "text development"@en, "Text-Entwicklung"@de;
	rdfs:comment """Action wherein a person(s) creates text resulting in different manifestation, e.g. from notebook to manuscript to typescript to published print."""@en;
	rdfs:subClassOf human:Creating, [
		a owl:Restriction; owl:onProperty event:hasStage; owl:minCardinality "0"^^xsd:nonNegativeInteger], [
		a owl:Restriction; owl:onProperty event:hasStageValue; owl:minCardinality "0"^^xsd:nonNegativeInteger].

text:WrittenText
	a owl:Class;
	rdfs:label "written text"@en, "geschriebener Text"@de, "texte écrit"@fr, "testo scritto"@it;
	rdfs:comment """Text written by any method, e.g. manually, with an analogue or digital typewriter, or on a computer, abstracted from its carrier."""@en;
	rdfs:subClassOf text:Text, [
		a owl:Restriction; owl:onProperty infocar:isWrittenWith; owl:minCardinality "0"^^xsd:nonNegativeInteger], [
		a owl:Restriction; owl:onProperty infocar:isWrittenWithValue; owl:minCardinality "0"^^xsd:nonNegativeInteger].

text:HandwrittenText
	a owl:Class;
	rdfs:label "handwritten text"@en, "handgeschriebener Text"@de, "texte manuscrit"@fr, "testo scritto a mano"@it;
	rdfs:comment """Text written by hand."""@en;
	rdfs:subClassOf text:WrittenText, [
		a owl:Restriction; owl:onProperty infocar:isInManuscript; owl:minCardinality "0"^^xsd:nonNegativeInteger], [
		a owl:Restriction; owl:onProperty infocar:isInManuscriptValue; owl:minCardinality "0"^^xsd:nonNegativeInteger].

text:TypewrittenText
	a owl:Class;
	rdfs:label "typewritten text"@en, "maschinengeschriebener Text"@de, "texte dactylographié"@fr, "testo dattiloscritto"@it;
	rdfs:comment """Text written with a typewriter."""@en;
	rdfs:subClassOf text:WrittenText, [
		a owl:Restriction; owl:onProperty infocar:isInTypescript; owl:minCardinality "0"^^xsd:nonNegativeInteger], [
		a owl:Restriction; owl:onProperty infocar:isInTypescriptValue; owl:minCardinality "0"^^xsd:nonNegativeInteger].

text:CopiedText
	a owl:Class;
	rdfs:label "copied text"@en, "kopierter Text"@de, "texte copié"@fr, "testo copiato"@it;
	rdfs:comment """Text copied by any method, abstracted from its carrier."""@en;
	rdfs:subClassOf text:Text, [
		a owl:Restriction; owl:onProperty infocar:isInTextCopy; owl:minCardinality "0"^^xsd:nonNegativeInteger], [
		a owl:Restriction; owl:onProperty infocar:isInTextCopyValue; owl:minCardinality "0"^^xsd:nonNegativeInteger].

text:TranscribedText
	a owl:Class;
	rdfs:label "transcribed text"@en, "transkribierter Text"@de, "texte transcrit"@fr, "testo trascritto"@it;
	rdfs:comment """Text copied by character by any method."""@en;
	rdfs:subClassOf text:CopiedText, [
		a owl:Restriction; owl:onProperty infocar:isInTranscript; owl:minCardinality "0"^^xsd:nonNegativeInteger], [
		a owl:Restriction; owl:onProperty infocar:isInTranscriptValue; owl:minCardinality "0"^^xsd:nonNegativeInteger].

text:PrintedText
	a owl:Class;
	rdfs:label "printed text"@en, "gedruckter Text"@de, "texte imprimé"@fr, "testo stampato"@it;
	rdfs:comment """Text printed by any method, abstracted from its carrier."""@en;
	rdfs:subClassOf text:Text, [
		a owl:Restriction; owl:onProperty infocar:isInPrint; owl:minCardinality "0"^^xsd:nonNegativeInteger], [
		a owl:Restriction; owl:onProperty infocar:isInPrintValue; owl:minCardinality "0"^^xsd:nonNegativeInteger].

text:Translation
	a owl:Class;
	rdfs:label "text translation"@en, "Textübersetzung"@de, "traduction de texte"@fr, "traduzione di testi"@it;
	rdfs:comment """Translation from text to text."""@en;
	rdfs:subClassOf text:Text, language:Translation. #, event:Output.

text:Nonfiction
	a owl:Class;
	rdfs:label "nonfiction text"@en, "Sachtext"@de;
	rdfs:comment """Text having content based on fact."""@en;
	rdfs:subClassOf text:Text, concept:Nonfiction.

text:Fiction
	a owl:Class;
	rdfs:label "fiction text"@en, "Fiktiontext"@de;
	rdfs:comment """Text having content derived from imagination."""@en;
	rdfs:subClassOf text:Text, concept:Fiction.

text:Expression
	a owl:Class;
	rdfs:label "text expression"@en, "Text-Expression"@de, "expression textuelle"@fr, "espressione testuale"@it;
	rdfs:comment """Document expression as text."""@en;
	rdfs:subClassOf document:Expression, text:Text, [
		a owl:Restriction; owl:onProperty text:expressionHasTitle; owl:minCardinality "0"^^xsd:nonNegativeInteger], [
		a owl:Restriction; owl:onProperty text:hasIncipit; owl:minCardinality "0"^^xsd:nonNegativeInteger], [
		a owl:Restriction; owl:onProperty text:hasExplicit; owl:minCardinality "0"^^xsd:nonNegativeInteger], [
		a owl:Restriction; owl:onProperty text:hasAuthor; owl:minCardinality "0"^^xsd:nonNegativeInteger], [
		a owl:Restriction; owl:onProperty text:hasAuthorValue; owl:minCardinality "0"^^xsd:nonNegativeInteger], [
		a owl:Restriction; owl:onProperty text:hasCommentator; owl:minCardinality "0"^^xsd:nonNegativeInteger], [
		a owl:Restriction; owl:onProperty text:hasCommentatorValue; owl:minCardinality "0"^^xsd:nonNegativeInteger], [
		a owl:Restriction; owl:onProperty text:hasScientificEditor; owl:minCardinality "0"^^xsd:nonNegativeInteger], [
		a owl:Restriction; owl:onProperty text:hasScientificEditorValue; owl:minCardinality "0"^^xsd:nonNegativeInteger], [
		a owl:Restriction; owl:onProperty text:hasCriticalEditor; owl:minCardinality "0"^^xsd:nonNegativeInteger], [
		a owl:Restriction; owl:onProperty text:hasCriticalEditorValue; owl:minCardinality "0"^^xsd:nonNegativeInteger], [
		a owl:Restriction; owl:onProperty textedit:hasDerivedTextExpression; owl:minCardinality "0"^^xsd:nonNegativeInteger], [
		a owl:Restriction; owl:onProperty textedit:hasDerivedTextExpressionValue; owl:minCardinality "0"^^xsd:nonNegativeInteger], [
		a owl:Restriction; owl:onProperty textedit:hasScientificEdition; owl:minCardinality "0"^^xsd:nonNegativeInteger], [
		a owl:Restriction; owl:onProperty textedit:hasScientificEditionValue; owl:minCardinality "0"^^xsd:nonNegativeInteger], [
		a owl:Restriction; owl:onProperty textedit:hasDiplomaticTranscription; owl:minCardinality "0"^^xsd:nonNegativeInteger], [
		a owl:Restriction; owl:onProperty textedit:hasDiplomaticTranscriptionValue; owl:minCardinality "0"^^xsd:nonNegativeInteger], [
		a owl:Restriction; owl:onProperty textedit:hasCriticalEdition; owl:minCardinality "0"^^xsd:nonNegativeInteger], [
		a owl:Restriction; owl:onProperty textedit:hasCriticalEditionValue; owl:minCardinality "0"^^xsd:nonNegativeInteger].

text:PolyAuthorExpression
	a owl:Class;
	rdfs:label "poly-author text expression"@en, "Mehrautorentext-Expression"@de;
	rdfs:comment """Text expression by different authors."""@en;
	rdfs:subClassOf text:Expression, [
		a owl:Restriction; owl:onProperty text:hasMainAuthor; owl:minCardinality "0"^^xsd:nonNegativeInteger], [
		a owl:Restriction; owl:onProperty text:hasMainAuthorValue; owl:minCardinality "0"^^xsd:nonNegativeInteger].

text:IndividualExpression
	a owl:Class;
	rdfs:label "individual text expression"@en, "individuelle Text-Expression"@de;
	rdfs:comment """Text as individual expression."""@en;
	rdfs:subClassOf text:Expression, document:IndividualExpression.

text:ExpressionPart
	a owl:Class;
	rdfs:label "text expression part"@en, "Text-Expressionsteil"@de;
	rdfs:comment """Part of an individual text expression, considered as incomplete."""@en;
	rdfs:subClassOf text:Expression, document:ExpressionPart, [
		a owl:Restriction; owl:onProperty text:isPartOfIndividualExpression; owl:minCardinality "0"^^xsd:nonNegativeInteger], [
		a owl:Restriction; owl:onProperty text:isPartOfIndividualExpressionValue; owl:minCardinality "0"^^xsd:nonNegativeInteger].

text:Introduction
	a owl:Class;
	rdfs:label "text introduction"@en, "Texteinleitung"@de;
	rdfs:comment """Beginning section of a text expression, usually written by the (main) author, stating e.g. the subject, purpose and limits of its main section; usually remaining unchanged."""@en;
#	rdfs:seeAlso <https://www.abc-clio.com/ODLIS/odlis_f.aspx>;
	rdfs:subClassOf text-structure:CompositionalContentStructure, text:ExpressionPart.

text:Body
	a owl:Class;
	rdfs:label "text body"@en, "Texthauptteil"@de;
	rdfs:comment """Main section of a text expression, e.g. including footnotes and illustrations but excluding the front matter and back matter."""@en;
#	rdfs:seeAlso <https://www.abc-clio.com/ODLIS/odlis_f.aspx>;
	rdfs:subClassOf text-structure:CompositionalContentStructure, text:ExpressionPart.

text:Conclusion
	a owl:Class;
	rdfs:label "text conclusion"@en, "Textkonklusion"@de;
	rdfs:comment """Concluding section of a text expression."""@en;
	rdfs:subClassOf text-structure:CompositionalContentStructure, text:ExpressionPart.

text:Author
	a owl:Class;
	rdfs:label "text author"@en, "Textautor"@de, "auteur du texte"@fr, "autore di testo"@it;
	rdfs:comment """Role of a person being responsible for a text expression."""@en;
	skos:note """Often an author is also the creator of a text expression."""@en;
	rdfs:subClassOf human:Author.

text:MainAuthor
	a owl:Class;
	rdfs:label "main text author"@en, "Haupttextautor"@de; # , "auteur du texte"@fr, "autore di testo"@it;
	rdfs:comment """Role of a person being the main responsible person for a text expression."""@en;
	rdfs:subClassOf text:Author.

text:ManOfLetters
	a owl:Class;
	rdfs:label "man of letters"@en, "Literat"@de, "homme de lettres"@fr, "uomo di lettere"@it;
	rdfs:comment """Role of a man devoted to literary activity."""@en;
	rdfs:subClassOf human:PersonRole.

text:WomanOfLetters
	a owl:Class;
	rdfs:label "woman of letters"@en, "Literatin"@de, "femme de lettres"@fr, "donna di lettere"@it;
	rdfs:comment """Role of a woman devoted to literary activity."""@en;
	rdfs:subClassOf human:PersonRole.

text:Revisor
	a owl:Class;
	rdfs:label "revisor"@en, "Revisor"@de, "réviseur"@fr, "revisore"@it;
	rdfs:comment """Role of a person checking on certain aspects of a text."""@en;
	rdfs:subClassOf human:PersonRole.

text:Translator
	a owl:Class;
	rdfs:label "translator"@en, "ÜbersetzerIn"@de, "traduct-eur/rice"@fr, "tradutt-ore/rice"@it;
	rdfs:comment """Role of a person translating text by writing or printing."""@en;
	rdfs:subClassOf language:PersonTranslator.

text:Copyist
	a owl:Class;
	rdfs:label "copyist"@en, "Kopist"@de, "copiste"@fr, "copista"@it, "scribes"@la; # "scribe"@en, "Schreiber"@de;
#	ling:hasSynonym "transcriber"@de;
	rdfs:comment """Role of a person copying text by writing."""@en;
	rdfs:subClassOf human:PersonCreator.

text:Vulgarizer
	a owl:Class;
	rdfs:label "text vulgarizer"@en, "Text-VulgarisatorIn"@de, "vulgarisat-eur/rice du texte"@fr;
	rdfs:comment """Role of a person vulgarizing a text, e.g. a scientific one, or creating one using vulgarizing terminology."""@en;
	rdfs:subClassOf human:Vulgarizer.

text:AgentCiter
	a owl:Class;
	rdfs:label "agent citer"@en, "Agent-Zitierer"@de;
	rdfs:comment """Role of a human agent, person or group, citing a text."""@en;
	rdfs:subClassOf human:AgentRole.

text:PersonCiter
	a owl:Class;
	rdfs:label "person citer"@en, "Person-ZitiererIn"@de;
	rdfs:comment """Citer as role of a person."""@en;
	rdfs:subClassOf text:AgentCiter, human:PersonRole.

text:OrganizationCiter
	a owl:Class;
	rdfs:label "organization citer"@en, "Organisation-Zitiererin"@de;
	rdfs:comment """Citer as role of an organization."""@en;
	rdfs:subClassOf text:AgentCiter, org:Role.

text:Citation
	a owl:Class;
	rdfs:label "citation"@en, "Zitat"@de, "citation"@fr, "citazione"@it;
	rdfs:comment """Copy of a text expression, or part of it, in another text expression, with reference to the first expression."""@en;
	skos:note """A citation can also be referred to from the source text, having an identifier linked to both the source reference and the citation."""@en;
	rdfs:subClassOf text-structure:ContentStructure, [
		a owl:Restriction; owl:onProperty text:citationHasReference; owl:minCardinality "0"^^xsd:nonNegativeInteger], [
		a owl:Restriction; owl:onProperty text:citationHasReferenceValue; owl:minCardinality "0"^^xsd:nonNegativeInteger], [
		a owl:Restriction; owl:onProperty text:citationHasIdentifier; owl:minCardinality "0"^^xsd:nonNegativeInteger], [
		a owl:Restriction; owl:onProperty text:citationHasIdentifierValue; owl:minCardinality "0"^^xsd:nonNegativeInteger], [
		a owl:Restriction; owl:onProperty text:citationHasNumber; owl:minCardinality "0"^^xsd:nonNegativeInteger], [
		a owl:Restriction; owl:onProperty text:citationHasNumberValue; owl:minCardinality "0"^^xsd:nonNegativeInteger], [
		a owl:Restriction; owl:onProperty text:citationIsPartOf; owl:minCardinality "0"^^xsd:nonNegativeInteger], [
		a owl:Restriction; owl:onProperty text:citationIsPartOfValue; owl:minCardinality "0"^^xsd:nonNegativeInteger].

text:CitationReference
	a owl:Class;
	rdfs:label "citation reference"@en, "Zitatreferenz"@de;
	rdfs:comment """Reference of a citation to the referred."""@en;
	rdfs:subClassOf document:TextReference, [
		a owl:Restriction; owl:onProperty text:hasCitationIdentifier; owl:minCardinality "0"^^xsd:nonNegativeInteger], [
		a owl:Restriction; owl:onProperty text:hasCitationIdentifierValue; owl:minCardinality "0"^^xsd:nonNegativeInteger].

text:CitationIdentifier
	a owl:Class;
	rdfs:label "citation identifier"@en, "Zitatidentifikator"@de;
	rdfs:comment """Identifier of a citation."""@en;
	rdfs:subClassOf concept:Identifier, document:Structure.

text:CitationNumber
	a owl:Class;
	rdfs:label "citation number"@en, "Zitatnummer"@de;
	rdfs:comment """Number of a citation."""@en;
	rdfs:subClassOf text:CitationIdentifier, math:Number.

text:SentenceExpression
	a owl:Class;
	rdfs:label "sentence expression"@en, "Satz-Expression"@de, "expression de phrases"@fr, "espressione di frase"@it;
	rdfs:comment """Text expression with sentence structure."""@en;
	rdfs:subClassOf text:Expression.

text:DiaryEntry
	a owl:Class;
	rdfs:label "diary entry"@en, "Tagebucheintrag"@de, "entrée du journal"@fr, "iscrizione del diario"@it;
	rdfs:comment """Periodical, usually daily description of a personal experience or observation written in a diary."""@en;
	rdfs:subClassOf text-structure:CompositionalContentStructure, text:IndividualExpression, [
		a owl:Restriction; owl:onProperty text:isEntryOfDiaryExpression; owl:minCardinality "0"^^xsd:nonNegativeInteger], [
		a owl:Restriction; owl:onProperty text:isEntryOfDiaryExpressionValue; owl:minCardinality "0"^^xsd:nonNegativeInteger], [
		a owl:Restriction; owl:onProperty infocar:entryIsInDiary; owl:minCardinality "0"^^xsd:nonNegativeInteger], [
		a owl:Restriction; owl:onProperty infocar:entryIsInDiaryValue; owl:minCardinality "0"^^xsd:nonNegativeInteger], [
		a owl:Restriction; owl:onProperty infocar:hasDiaryEnteringDate; owl:minCardinality "0"^^xsd:nonNegativeInteger].

text:DiaryExpression
	a owl:Class;
	rdfs:label "diary expression"@en, "Tagebuch-Expression"@de, "expression d'un journal"@fr, "expression del diario"@it;
	rdfs:comment """Text expression with a diary content and possibly structure."""@en;
	rdfs:subClassOf text:IndividualExpression, [
		a owl:Restriction; owl:onProperty infocar:isInDiary; owl:minCardinality "0"^^xsd:nonNegativeInteger], [
		a owl:Restriction; owl:onProperty infocar:isInDiaryValue; owl:minCardinality "0"^^xsd:nonNegativeInteger].

text:LetterExpression
	a owl:Class;
	rdfs:label "letter expression"@en, "Brief-Expression"@de;
	rdfs:comment """Text expression with a letter content and possibly structure."""@en;
	rdfs:subClassOf text:IndividualExpression, [
		a owl:Restriction; owl:onProperty infocar:isInLetter; owl:minCardinality "0"^^xsd:nonNegativeInteger], [
		a owl:Restriction; owl:onProperty infocar:isInLetterValue; owl:minCardinality "0"^^xsd:nonNegativeInteger].

text:Commentator
	a owl:Class;
	rdfs:label "commentator"@en, "KommentatorIn"@de;
	rdfs:comment """Role of a person commenting on a text expression."""@en;
	rdfs:subClassOf human:PersonRole.

text:Commentary
	a owl:Class;
	rdfs:label "commentary"@en, "Kommentar"@de;
	rdfs:comment """Text expression in the form of a series of comments as analysis, interpretation or explanation of another text expression."""@en;
	rdfs:subClassOf text:IndividualExpression, [
		a owl:Restriction; owl:onProperty text:isCommentaryOn; owl:minCardinality "0"^^xsd:nonNegativeInteger], [
		a owl:Restriction; owl:onProperty text:isCommentaryOnValue; owl:minCardinality "0"^^xsd:nonNegativeInteger].

text:Article
	a owl:Class;
	rdfs:label "article"@en, "Artikel"@de, "article"@fr, "articolo"@it;
	rdfs:comment """Text expression about a defined (main) subject."""@en;
	rdfs:subClassOf text:IndividualExpression, [
		a owl:Restriction; owl:onProperty text:isArticleAbout; owl:minCardinality "0"^^xsd:nonNegativeInteger], [
		a owl:Restriction; owl:onProperty text:isArticleAboutValue; owl:minCardinality "0"^^xsd:nonNegativeInteger].

text:Biography
	a owl:Class;
	rdfs:label "biography"@en, "Biographie"@de; #*
	rdfs:comment """Text expression about a person's life."""@en;
	rdfs:subClassOf text:IndividualExpression.

text:Manual
	a owl:Class;
	rdfs:label "manual"@en, "Handbuch"@de, "manuel"@fr, "manuale"@it;
	rdfs:comment """Text expression providing procedural infromation."""@en;
	rdfs:subClassOf text:IndividualExpression.

text:ScientificExpression
	a owl:Class;
	rdfs:label "scientific expression"@en, "wissenschaftliche Expression"@de;
	rdfs:comment """Text expression with scientific content."""@en;
	rdfs:subClassOf text:IndividualExpression.

text:VulgarizedScientificExpression
	a owl:Class;
	rdfs:label "vulgarized scientific expression"@en, "vulgarisierte wissenschaftliche Expression"@de;
	rdfs:comment """Text expression with vulgarized scientific content."""@en;
	rdfs:subClassOf text:ScientificExpression.

text:Dictionary
	a owl:Class;
	rdfs:label "dictionary"@en, "Wörterbuch"@de;
	rdfs:comment """List of brief explanatory entries for terms of a human natural language, belonging to a certain domain, providing their meaning, mostly ordered, e.g. alphabetically."""@en;
#	rdfs:seeAlso <https://www.abc-clio.com/ODLIS/odlis_f.aspx>;
	rdfs:subClassOf text:IndividualExpression. # text:ReferenceExpression

#
# PROPERTIES
#

text:hasText
	a owl:ObjectProperty;
	rdfs:label "has text"@en, "hat Text"@de;
	rdfs:comment """Relating a resource to a text as a writable coherent set of signs representing semantics in a language."""@en;
	rdfs:domain rdfs:Resource;
#	rdfs:range text:Text ling:Literal;
	rdfs:subPropertyOf knora-base:hasValue;
	knora-base:subjectClassConstraint knora-base:Resource;
	knora-base:objectClassConstraint knora-base:TextValue.

text:hasName
	a owl:ObjectProperty;
	rdfs:label "has name"@en, "hat Name"@de;
	rdfs:comment """Relating a resource to a name as a textual identifier of the resource."""@en;
	rdfs:subPropertyOf text:hasText; #° rdfs:label, foaf:name
	knora-base:subjectClassConstraint knora-base:Resource;
	knora-base:objectClassConstraint knora-base:TextValue.

text:hasPreferredName
	a owl:ObjectProperty;
	rdfs:label "has preferred name"@en, "hat bevorzugter Name"@de;
	rdfs:comment """Relating a resource to a preferred name."""@en;
	rdfs:subPropertyOf text:hasName;
	knora-base:subjectClassConstraint knora-base:Resource;
	knora-base:objectClassConstraint knora-base:TextValue.

text:hasAlias
	a owl:ObjectProperty;
	rdfs:label "has alias"@en, "hat Alias"@de;
	rdfs:comment """Relating a resource to an alias as an alternative name of the resource."""@en;
	rdfs:subPropertyOf text:hasName;
	knora-base:subjectClassConstraint knora-base:Resource;
	knora-base:objectClassConstraint knora-base:TextValue.

text:hasIdentifier
	a owl:ObjectProperty;
	rdfs:label "has identifier"@en, "hat Kennzeichen"@de;
	rdfs:comment """Relating a resource to an identifier as a unique and permanent textual reference to the resource within a given context, and conforming to a formal identification system."""@en;
	rdfs:subPropertyOf text:hasText; #° cf. dcterms:identifier
	knora-base:subjectClassConstraint knora-base:Resource;
	knora-base:objectClassConstraint knora-base:TextValue.

text:hasTitle
	a owl:ObjectProperty;
	rdfs:label "has title"@en, "hat Titel"@de;
	rdfs:comment """Relating a resource to a title as a textual identifier of the resource."""@en;
	rdfs:subPropertyOf text:hasText;
	knora-base:subjectClassConstraint knora-base:Resource;
	knora-base:objectClassConstraint knora-base:TextValue.

text:hasComment
	a owl:ObjectProperty;
	rdfs:label "has comment"@en, "hat Kommentar"@de;
	rdfs:comment """Relating a resource to a comment as a textual statement about the resource."""@en;
	rdfs:subPropertyOf text:hasText;
	knora-base:subjectClassConstraint knora-base:Resource;
	knora-base:objectClassConstraint knora-base:TextValue.

text:hasDescription
	a owl:ObjectProperty;
	rdfs:label "has description"@en, "hat Beschreibung"@de;
	rdfs:comment """Relating a resource to a description as a textual statement about features of the resource."""@en;
	rdfs:subPropertyOf text:hasText;
	knora-base:subjectClassConstraint knora-base:Resource;
	knora-base:objectClassConstraint knora-base:TextValue.

text:hasDefinition
	a owl:ObjectProperty;
	rdfs:label "has definition"@en, "hat Definition"@de;
	rdfs:comment """Relating a resource to a definition as a textual statement about the essential features of the resource."""@en;
	rdfs:subPropertyOf text:hasDescription;
	knora-base:subjectClassConstraint knora-base:Resource;
	knora-base:objectClassConstraint knora-base:TextValue.

text:hasDetailDescription
	a owl:ObjectProperty;
	rdfs:label "has detail description"@en, "hat Detail-Beschreibung"@de;
	rdfs:comment """Relating a resource to a description of its detail. E.g. in the case of a text a detail can be a passage variant or an emendation"""@en;
	rdfs:subPropertyOf text:hasDescription;
	knora-base:subjectClassConstraint knora-base:Resource;
	knora-base:objectClassConstraint knora-base:TextValue.

text:hasSpecialDescription
	a owl:ObjectProperty;
	rdfs:label "has special description"@en, "hat Besonderes-Beschreibung"@de;
	rdfs:comment """Relating a resource to a description of (a) certain feature(s)."""@en;
	rdfs:subPropertyOf text:hasDescription;
	knora-base:subjectClassConstraint knora-base:Resource;
	knora-base:objectClassConstraint knora-base:TextValue.

text:hasLineNumber
	a owl:ObjectProperty;
	rdfs:label "has line number"@en, "hat Liniennummer"@de;
	rdfs:comment """Relating a text to the number of a line of the text expression."""@en;
	rdfs:domain text:Text;
	rdfs:range rdfs:Literal;	
	rdfs:subPropertyOf text:hasText;
	knora-base:subjectClassConstraint text:Text;
	knora-base:objectClassConstraint knora-base:TextValue.

text:hasVersionIndicator
	a owl:ObjectProperty;
	rdfs:label "has version indicator"@en, "hat Version-Indikator"@de;
	rdfs:comment """Relating a text to a textual element that indicates its version."""@en;
	rdfs:domain text:Text;
	rdfs:range rdfs:Literal;
	rdfs:subPropertyOf text:hasText;
	knora-base:subjectClassConstraint text:Text;
	knora-base:objectClassConstraint knora-base:TextValue.

text:hasPageNumberDescription
	a owl:ObjectProperty;
	rdfs:label "text has page number description"@en, "Text hat Seitennummerbeschreibung"@de;
	rdfs:comment """Relating a text to a description of the number(s) of and possibly a location on (a) pages it is on; examples of the string of its value: "001-002", "01 recto", "O2 (bottom)"."""@en;
	rdfs:domain text:Text;
	rdfs:range rdfs:Literal;
	rdfs:subPropertyOf knora-base:hasValue;
	knora-base:subjectClassConstraint text:Text;
	knora-base:objectClassConstraint knora-base:TextValue.

text:hasReferenceText
	a owl:ObjectProperty;
	rdfs:label "has reference text"@en, "hat Bezugstext"@de;
	rdfs:comment "Relating a text to another one as its reference."@en;
	rdfs:subPropertyOf knora-base:hasLinkTo;
	knora-base:subjectClassConstraint text:Text;
	knora-base:objectClassConstraint text:Text.

text:hasReferenceTextValue
	a owl:ObjectProperty;
	rdfs:label "has reference text - statement"@en, "hat Bezugstext - Festlegung"@de;
	rdfs:comment "Relating a text to a reification statement of the relation between the text and another one as its reference."@en;
	rdfs:subPropertyOf knora-base:hasLinkToValue;
	knora-base:subjectClassConstraint text:Text;
	knora-base:objectClassConstraint knora-base:LinkValue.

text:hasRevisor
	a owl:ObjectProperty;
	rdfs:label "has revisor"@en, "hat Revisor"@de;
	rdfs:comment """Relating a text to a person who revised it."""@en;
	rdfs:domain text:Text;
#	rdfs:range [rdfs:subClassOf human:Person, [a owl:Restriction; owl:onProperty human:personHasRole; owl:someValuesFrom text:Revisor]];
	rdfs:subPropertyOf knora-base:hasLinkTo;
	knora-base:subjectClassConstraint text:Text;
	knora-base:objectClassConstraint human:Person.

text:hasRevisorValue
	a owl:ObjectProperty;
	rdfs:label "has revisor - statement"@en, "hat Revisor - Festlegung"@de;
	rdfs:comment """Relating a text to a reification statement of the relation between the text and a person who revised it."""@en;
	rdfs:subPropertyOf knora-base:hasLinkToValue;
	knora-base:subjectClassConstraint text:Text;
	knora-base:objectClassConstraint knora-base:LinkValue.

text:hasTranscriber
	a owl:ObjectProperty;
	rdfs:label "has transcriber"@en, "hat TranskribiererIn"@de;
	rdfs:comment """Relating a text to a person who transcribed it."""@en;
	rdfs:domain text:Text;
#	rdfs:range [rdfs:subClassOf human:Person, [a owl:Restriction; owl:onProperty human:personHasRole; owl:someValuesFrom text:Transcriber]];
	rdfs:subPropertyOf knora-base:hasLinkTo;
	knora-base:subjectClassConstraint text:Text;
	knora-base:objectClassConstraint human:Person.

text:hasTranscriberValue
	a owl:ObjectProperty;
	rdfs:label "has transcriber - statement"@en, "hat TranskribiererIn - Festlegung"@de;
	rdfs:comment """Relating a text to a reification statement of the relation between the text and a person who transcribed it."""@en;
	rdfs:subPropertyOf knora-base:hasLinkToValue;
	knora-base:subjectClassConstraint text:Text;
	knora-base:objectClassConstraint knora-base:LinkValue.

text:hasVulgarizer
	a owl:ObjectProperty;
	rdfs:label "text has vulgarizer"@en, "Text hat VulgarisatorIn"@de;
	rdfs:comment """Relating a text to a person who vulgarized it."""@en;
	rdfs:domain text:Text;
#	rdfs:range [rdfs:subClassOf human:Person, [a owl:Restriction; owl:onProperty human:personHasRole; owl:someValuesFrom text:Vulgarizer]];
	rdfs:subPropertyOf knora-base:hasLinkTo;
	knora-base:subjectClassConstraint text:Text;
	knora-base:objectClassConstraint human:Person.

text:hasVulgarizerValue
	a owl:ObjectProperty;
	rdfs:label "text has vulgarizer - statement"@en, "Text hat VulgarisatorIn - Festlegung"@de;
	rdfs:comment """Relating a text to a reification statement of the relation between the text and a person who vulgarized it."""@en;
	rdfs:subPropertyOf knora-base:hasLinkToValue;
	knora-base:subjectClassConstraint text:Text;
	knora-base:objectClassConstraint knora-base:LinkValue.

text:hasCiter
	a owl:ObjectProperty;
	rdfs:label "has citer"@en, "hat ZitiererIn"@de;
	rdfs:comment """Relating a text to a human agent - person or group - citing it."""@en;
	rdfs:domain text:Text;
#	rdfs:range [rdfs:subClassOf human:Agent, [a owl:Restriction; owl:onProperty human:agentHasRole; owl:someValuesFrom text:AgentCiter]];
	rdfs:subPropertyOf knora-base:hasLinkTo;
	knora-base:subjectClassConstraint text:Text;
	knora-base:objectClassConstraint human:Agent.

text:hasCiterValue
	a owl:ObjectProperty;
	rdfs:label "has citer - statement"@en, "hat ZitiererIn - Festlegung"@de;
	rdfs:comment """Relating a text to a reification statement of the relation between the text and a human agent - person or group - citing it."""@en;
	rdfs:subPropertyOf knora-base:hasLinkToValue;
	knora-base:subjectClassConstraint text:Text;
	knora-base:objectClassConstraint knora-base:LinkValue.

text:hasCitation
	a owl:ObjectProperty;
	rdfs:label "has citation"@en, "hat Zitat"@de;
	rdfs:comment "Relating a text to a citation thereof."@en;
	rdfs:domain text:Text;
	rdfs:range text:Citation;
	rdfs:subPropertyOf knora-base:hasLinkTo;
	knora-base:subjectClassConstraint text:Text;
	knora-base:objectClassConstraint text:Citation.

text:hasCitationValue
	a owl:ObjectProperty;
	rdfs:label "has citation - statement"@en, "hat Zitat - Festlegung"@de;
	rdfs:comment "Relating a text to a reification statement of the relation between the text and a citation thereof."@en;
	rdfs:subPropertyOf knora-base:hasLinkToValue;
	knora-base:subjectClassConstraint text:Text;
	knora-base:objectClassConstraint knora-base:LinkValue.

text:hasCitationReference
	a owl:ObjectProperty;
	rdfs:label "has citation reference"@en, "hat Zitatreferenz"@de;
	rdfs:comment "Relating a text to a citation reference thereof."@en;
	rdfs:domain text:Text;
	rdfs:range text:CitationReference;
	rdfs:subPropertyOf knora-base:hasLinkTo;
	knora-base:subjectClassConstraint text:Text;
	knora-base:objectClassConstraint text:CitationReference.

text:hasCitationReferenceValue
	a owl:ObjectProperty;
	rdfs:label "has citation reference - statement"@en, "hat Zitatreferenz - Festlegung"@de;
	rdfs:comment "Relating a text to a reification statement of the relation between the text and a citation reference thereof."@en;
	rdfs:subPropertyOf knora-base:hasLinkToValue;
	knora-base:subjectClassConstraint text:Text;
	knora-base:objectClassConstraint knora-base:LinkValue.

text:isCitedIn
	a owl:ObjectProperty;
	rdfs:label "is cited in"@en, "ist zitiert in"@de;
	rdfs:comment "Relating a text to an expression wherein it is cited."@en;
	rdfs:domain text:Text;
	rdfs:range document:Expression;
	rdfs:subPropertyOf knora-base:hasLinkTo;
	knora-base:subjectClassConstraint text:Text;
	knora-base:objectClassConstraint document:Expression.

text:isCitedInValue
	a owl:ObjectProperty;
	rdfs:label "is cited in - statement"@en, "ist zitiert in - Festlegung"@de;
	rdfs:comment "Relating a text to a reification statement of the relation between the text and an expression wherein it is cited."@en;
	rdfs:subPropertyOf knora-base:hasLinkToValue;
	knora-base:subjectClassConstraint text:Text;
	knora-base:objectClassConstraint knora-base:LinkValue.

text:hasEditor
	a owl:ObjectProperty;
	rdfs:label "text has editor"@en, "Text hat Editor"@de;
	rdfs:comment """Relating a text to a person who edited it."""@en;
	rdfs:domain text:Text;
#	rdfs:range [rdfs:subClassOf human:Person, [a owl:Restriction; owl:onProperty human:personHasRole; owl:someValuesFrom textedit:Editor]];
	rdfs:subPropertyOf knora-base:hasLinkTo;
	knora-base:subjectClassConstraint text:Text;
	knora-base:objectClassConstraint human:Person.

text:hasEditorValue
	a owl:ObjectProperty;
	rdfs:label "text has editor - statement"@en, "Text hat Editor - Festlegung"@de;
	rdfs:comment """Relating a text to a reification statement of the relation between the text and a person who edited it."""@en;
	rdfs:subPropertyOf knora-base:hasLinkToValue;
	knora-base:subjectClassConstraint text:Text;
	knora-base:objectClassConstraint knora-base:LinkValue.

text:expressionHasTitle
	a owl:ObjectProperty;
	rdfs:label "text expression has title"@en, "Text-Expression hat Titel"@de;
	rdfs:comment """Relating a text expression to a title it has."""@en;
	rdfs:domain text:Expression;
#	rdfs:range rdfs:Literal;
	rdfs:subPropertyOf text:hasTitle;
	knora-base:subjectClassConstraint text:Expression;
	knora-base:objectClassConstraint knora-base:TextValue.

text:hasIncipit
	a owl:ObjectProperty;
	rdfs:label "has incipit"@en, "hat Incipit"@de;
	rdfs:comment """Relating an untitled individual text expression to a beginning part thereof to identify the text."""@en;
	rdfs:domain text:Expression;
#	rdfs:range rdfs:Literal;
	rdfs:subPropertyOf text:hasText;
	knora-base:subjectClassConstraint text:Expression;
	knora-base:objectClassConstraint knora-base:TextValue.

text:hasExplicit
	a owl:ObjectProperty;
	rdfs:label "has explicit"@en, "hat Explicit"@de;
	rdfs:comment """Relating an untitled individual text expression to an end part thereof to identify the text."""@en;
	rdfs:domain text:Expression;
#	rdfs:range rdfs:Literal;
	rdfs:subPropertyOf text:hasText;
	knora-base:subjectClassConstraint text:Expression;
	knora-base:objectClassConstraint knora-base:TextValue.

text:hasAuthor
	a owl:ObjectProperty;
	rdfs:label "text has author"@en, "Text hat Autor"@de;
	rdfs:comment """Relating a text expression to a person who authored it."""@en;
	skos:note """A text can have more than one author."""@en;
	rdfs:domain text:Expression;
#	rdfs:range [rdfs:subClassOf human:Person, [a owl:Restriction; owl:onProperty human:personHasRole; owl:someValuesFrom text:Author]];
	rdfs:subPropertyOf human:hasAuthor;
	knora-base:subjectClassConstraint text:Expression;
	knora-base:objectClassConstraint human:Person.

text:hasAuthorValue
	a owl:ObjectProperty;
	rdfs:label "text has author - statement"@en, "Text hat Autor - Festlegung"@de;
	rdfs:comment """Relating a text expression to a reification statement of the relation between the text and a person who authored it."""@en;
	rdfs:subPropertyOf human:hasAuthorValue;
	knora-base:subjectClassConstraint text:Expression;
	knora-base:objectClassConstraint knora-base:LinkValue.

text:hasCommentator
	a owl:ObjectProperty;
	rdfs:label "text expression has commentator"@en, "Text-Expression hat KommentatorIn"@de;
	rdfs:comment "Relating a text expression to a person who commented on it."@en;
	rdfs:domain text:Expression;
#	rdfs:range [rdfs:subClassOf human:Person, [a owl:Restriction; owl:onProperty human:personHasRole; owl:someValuesFrom text:Commentator]];
	rdfs:subPropertyOf knora-base:hasLinkTo;
	knora-base:subjectClassConstraint text:Expression;
	knora-base:objectClassConstraint human:Person.

text:hasCommentatorValue
	a owl:ObjectProperty;
	rdfs:label "text expression has commentator - statement"@en, "Text-Expression hat KommentatorIn - Festlegung"@de;
	rdfs:comment "Relating a text expression to a reification statement of the relation between the expression and person who commented on it."@en;
	rdfs:subPropertyOf knora-base:hasLinkToValue;
	knora-base:subjectClassConstraint text:Expression;
	knora-base:objectClassConstraint knora-base:LinkValue.

text:hasScientificEditor
	a owl:ObjectProperty;
	rdfs:label "text expression has scientific editor"@en, "Text-Expression hat wissenschaftliche Editor"@de;
	rdfs:comment "Relating a text expression to a person who edited it scientifically."@en;
	rdfs:domain text:Expression;
#	rdfs:range [rdfs:subClassOf human:Person, [a owl:Restriction; owl:onProperty human:personHasRole; owl:someValuesFrom textedit:ScientificEditor]];
	rdfs:subPropertyOf knora-base:hasLinkTo;
	knora-base:subjectClassConstraint text:Expression;
	knora-base:objectClassConstraint human:Person.

text:hasScientificEditorValue
	a owl:ObjectProperty;
	rdfs:label "text expression has scientific editor - statement"@en, "Text-Expression hat wissenschaftliche Editor - Festlegung"@de;
	rdfs:comment "Relating a text expression to a reification statement of the relation between the expression and person who edited it scientifically."@en;
	rdfs:subPropertyOf knora-base:hasLinkToValue;
	knora-base:subjectClassConstraint text:Expression;
	knora-base:objectClassConstraint knora-base:LinkValue.

text:hasCriticalEditor
	a owl:ObjectProperty;
	rdfs:label "text expression has critical editor"@en, "Text-Expression hat kritische Editor"@de;
	rdfs:comment "Relating a text expression to a person who edited it critically."@en;
	rdfs:domain text:Expression;
#	rdfs:range [rdfs:subClassOf human:Person, [a owl:Restriction; owl:onProperty human:personHasRole; owl:someValuesFrom textedit:CriticalEditor]];
	rdfs:subPropertyOf knora-base:hasLinkTo;
	knora-base:subjectClassConstraint text:Expression;
	knora-base:objectClassConstraint human:Person.

text:hasCriticalEditorValue
	a owl:ObjectProperty;
	rdfs:label "text expression has critical editor - statement"@en, "Text-Expression hat kritische Editor - Festlegung"@de;
	rdfs:comment "Relating a text expression to a reification statement of the relation between the expression and person who edited it critically."@en;
	rdfs:subPropertyOf knora-base:hasLinkToValue;
	knora-base:subjectClassConstraint text:Expression;
	knora-base:objectClassConstraint knora-base:LinkValue.

text:hasMainAuthor
	a owl:ObjectProperty;
	rdfs:label "has main author"@en, "hat Hauptautor"@de;
	rdfs:comment """Relating a poly-author text expression to its main author."""@en;
	rdfs:domain text:PolyAuthorExpression;
#	rdfs:range [rdfs:subClassOf human:Person, [a owl:Restriction; owl:onProperty human:personHasRole; owl:someValuesFrom text:MainAuthor]];
	rdfs:subPropertyOf knora-base:hasLinkTo;
	knora-base:subjectClassConstraint text:PolyAuthorExpression;
	knora-base:objectClassConstraint human:Person.

text:hasMainAuthorValue
	a owl:ObjectProperty;
	rdfs:label "has main author - statement"@en, "hat  Hauptautor - Festlegung"@de;
	rdfs:comment """Relating a poly-author text expression to a reification statement of the relation between the expression and its main author."""@en;
	rdfs:subPropertyOf knora-base:hasLinkToValue;
	knora-base:subjectClassConstraint text:PolyAuthorExpression;
	knora-base:objectClassConstraint knora-base:LinkValue.

text:isPartOfIndividualExpression
	a owl:ObjectProperty;
	rdfs:label "is part of individual text expression"@en, "ist Teil einer individuellen Text-Expression"@de;
	rdfs:comment """Relating a text expression part to an individual expression it is part of."""@en;
	rdfs:domain text:ExpressionPart;
	rdfs:range text:IndividualExpression;
	rdfs:subPropertyOf concept:isPartOf;
	knora-base:subjectClassConstraint text:ExpressionPart;
	knora-base:objectClassConstraint text:IndividualExpression.

text:isPartOfIndividualExpressionValue
	a owl:ObjectProperty;
	rdfs:label "is part of individual text expression - statement"@en, "ist Teil einer individuellen Text-Expression - Festlegung"@de;
	rdfs:comment """Relating a text expression part to a reification statement of the relation between the part and an individual expression it is part of."""@en;
	rdfs:subPropertyOf concept:isPartOfValue;
	knora-base:subjectClassConstraint text:ExpressionPart;
	knora-base:objectClassConstraint knora-base:LinkValue.

text:citationHasReference
	a owl:ObjectProperty;
	rdfs:label "citation has reference"@en, "Zitat hat Referenz"@de;
	rdfs:comment """Relating a citation to its reference."""@en;
	rdfs:domain text:Citation;
	rdfs:range document:TextReference;
	rdfs:subPropertyOf document:hasTextReference;
	knora-base:subjectClassConstraint text:Citation;
	knora-base:objectClassConstraint document:TextReference.

text:citationHasReferenceValue
	a owl:ObjectProperty;
	rdfs:label "citation has reference - statement"@en, "Zitat hat Referenz - Festlegung"@de;
	rdfs:comment """Relating a citation to a reification statement of the relation between the citation and its reference."""@en;
	rdfs:subPropertyOf document:hasTextReferenceValue;
	knora-base:subjectClassConstraint text:Citation;
	knora-base:objectClassConstraint knora-base:LinkValue.

text:citationHasIdentifier
	a owl:ObjectProperty;
	rdfs:label "citation has identifier"@en, "Zitat hat Identifikator"@de;
	rdfs:comment """Relating a citation to its identifier."""@en;
	rdfs:domain text:Citation;
	rdfs:range text:CitationIdentifier;
	rdfs:subPropertyOf knora-base:hasLinkTo; # text-structure:hasIdentifier
	knora-base:subjectClassConstraint text:Citation;
	knora-base:objectClassConstraint text:CitationIdentifier.

text:citationHasIdentifierValue
	a owl:ObjectProperty;
	rdfs:label "citation has identifier - statement"@en, "Zitat hat Identifikator - Festlegung"@de;
	rdfs:comment """Relating a citation to a reification statement of the relation between the citation and its identifier."""@en;
	rdfs:subPropertyOf knora-base:hasLinkToValue; # text-structure:hasIdentifierValue
	knora-base:subjectClassConstraint text:Citation;
	knora-base:objectClassConstraint knora-base:LinkValue.

text:citationHasNumber
	a owl:ObjectProperty;
	rdfs:label "citation has number"@en, "Zitat hat Nummer"@de;
	rdfs:comment """Relating a citation to its number."""@en;
	rdfs:domain text:Citation;
	rdfs:range text:CitationNumber;
	rdfs:subPropertyOf text:citationHasIdentifier;
	knora-base:subjectClassConstraint text:Citation;
	knora-base:objectClassConstraint text:CitationNumber.

text:citationHasNumberValue
	a owl:ObjectProperty;
	rdfs:label "citation has number - statement"@en, "Zitat hat Nummer - Festlegung"@de;
	rdfs:comment """Relating a citation to a reification statement of the relation between the citation and its number."""@en;
	rdfs:subPropertyOf text:citationHasIdentifierValue;
	knora-base:subjectClassConstraint text:Citation;
	knora-base:objectClassConstraint knora-base:LinkValue.

text:citationIsPartOf
	a owl:ObjectProperty;
	rdfs:label "citation is part of text expression"@en, "Zitat ist Teil einer Text-Expression"@de;
	rdfs:comment """Relating a citation to a text expression it is part of."""@en;
	rdfs:domain text:Citation;
	rdfs:range text:Expression;
	rdfs:subPropertyOf concept:isPartOf;
	knora-base:subjectClassConstraint text:Citation;
	knora-base:objectClassConstraint text:Expression.

text:citationIsPartOfValue
	a owl:ObjectProperty;
	rdfs:label "citation is part of text expression - statement"@en, "Zitat ist Teil einer Text-Expression - Festlegung"@de;
	rdfs:comment """Relating a citation to a reification statement of the relation between the citation and a text expression it is part of."""@en;
	rdfs:subPropertyOf concept:isPartOfValue;
	knora-base:subjectClassConstraint text:Citation;
	knora-base:objectClassConstraint knora-base:LinkValue.

text:hasCitationIdentifier
	a owl:ObjectProperty;
	rdfs:label "has citation identifier"@en, "hat Zitatidentifikator"@de;
	rdfs:comment """Relating a citation reference to its citation identifier."""@en;
	rdfs:domain text:CitationReference;
	rdfs:range text:CitationIdentifier;
	rdfs:subPropertyOf knora-base:hasLinkTo; #°
	knora-base:subjectClassConstraint text:CitationReference;
	knora-base:objectClassConstraint text:CitationIdentifier.

text:hasCitationIdentifierValue
	a owl:ObjectProperty;
	rdfs:label "has citation identifier - statement"@en, "hat Zitatidentifikator - Festlegung"@de;
	rdfs:comment """Relating a citation reference to a reification statement of the relation between that reference and its citation identifier."""@en;
	rdfs:subPropertyOf knora-base:hasLinkToValue; #°
	knora-base:subjectClassConstraint text:CitationReference;
	knora-base:objectClassConstraint knora-base:LinkValue.

text:isEntryOfDiaryExpression
	a owl:ObjectProperty;
	rdfs:label "is entry of diary expression"@en, "ist Eingabe einer Tagebuch-Expression"@de;
	rdfs:comment """Relating a diary entry to its diary expression."""@en;
	rdfs:domain text:DiaryEntry;
	rdfs:range text:DiaryExpression;
	rdfs:subPropertyOf concept:isPartOf;
	knora-base:subjectClassConstraint text:DiaryEntry;
	knora-base:objectClassConstraint text:DiaryExpression.

text:isEntryOfDiaryExpressionValue
	a owl:ObjectProperty;
	rdfs:label "is entry of diary expression - statement"@en, "ist Eingabe einer Tagebuch-Expression - Festlegung"@de;
	rdfs:comment """Relating a diary entry to a reification statement of the relation between that entry and its diary expression."""@en;
	rdfs:subPropertyOf concept:isPartOfValue;
	knora-base:subjectClassConstraint text:DiaryEntry;
	knora-base:objectClassConstraint knora-base:LinkValue.

text:isCommentaryOn
	a owl:ObjectProperty;
	rdfs:label "is commentary on"@en, "ist Kommentar zu"@de;
	rdfs:comment """Relating a commentary to a text expression it comments on."""@en;
	rdfs:domain text:Commentary;
	rdfs:range text:Expression;
	rdfs:subPropertyOf knora-base:hasLinkTo;
	knora-base:subjectClassConstraint text:Commentary;
	knora-base:objectClassConstraint text:Expression.

text:isCommentaryOnValue
	a owl:ObjectProperty;
	rdfs:label "is commentary on - statement"@en, "ist Kommentar zu - Festlegung"@de;
	rdfs:comment """Relating a commentary to a reification statement of the relation between the commentary and a text expression it comments on."""@en;
	rdfs:subPropertyOf knora-base:hasLinkToValue;
	knora-base:subjectClassConstraint text:Commentary;
	knora-base:objectClassConstraint knora-base:LinkValue.

text:isArticleAbout
	a owl:ObjectProperty;
	rdfs:label "is article about"@en, "ist Artikel über"@de;
	rdfs:comment """Relating an article to a subject it is about."""@en;
	rdfs:domain text:Article;
	rdfs:range rdfs:Resource;
	rdfs:subPropertyOf concept:informationHasSubject;
	knora-base:subjectClassConstraint text:Article;
	knora-base:objectClassConstraint knora-base:Resource.

text:isArticleAboutValue
	a owl:ObjectProperty;
	rdfs:label "is article about - statement"@en, "ist Artikel über - Festlegung"@de;
	rdfs:comment """Relating an article to a reification statement of the relation between the article and a subject it is about."""@en;
	rdfs:subPropertyOf concept:informationHasSubjectValue;
	knora-base:subjectClassConstraint text:Article;
	knora-base:objectClassConstraint knora-base:LinkValue.