@prefix rdfs: <http://www.w3.org/2000/01/rdf-schema#>.
@prefix owl: <http://www.w3.org/2002/07/owl#>.
@prefix xsd: <http://www.w3.org/2001/XMLSchema#>.
@prefix skos: <http://www.w3.org/2004/02/skos/core#>.
@prefix dct: <http://purl.org/dc/terms/>.
@prefix foaf: <http://xmlns.com/foaf/0.1/>.
@prefix cidoc: <http://www.cidoc-crm.org/cidoc-crm/>.
@prefix frbroo: <http://iflastandards.info/ns/fr/frbr/frbroo/>.
@prefix event: <http://www.knora.org/ontology/shared/event#>.
@prefix human: <http://www.knora.org/ontology/shared/human#>.
@prefix creating: <http://www.knora.org/ontology/shared/creating#>.
@prefix org: <http://www.knora.org/ontology/shared/organization#>.
@prefix language: <http://www.knora.org/ontology/shared/language#>.
@prefix concept: <http://www.knora.org/ontology/shared/concept#>.
@prefix math: <http://www.knora.org/ontology/shared/mathematics#>.
@prefix document: <http://www.knora.org/ontology/shared/document#>.
@prefix text-expression: <http://www.knora.org/ontology/shared/text-expression#>.
@prefix text-structure: <http://www.knora.org/ontology/shared/text-structure#>.
@prefix textedit: <http://www.knora.org/ontology/shared/text-editing#>.
@prefix infocar: <http://www.knora.org/ontology/shared/information-carrier#>.
@prefix publish: <http://www.knora.org/ontology/shared/publishing#>.
@prefix litera: <http://www.knora.org/ontology/shared/literature#>.
@prefix knora-base: <http://www.knora.org/ontology/knora-base#>.

@base <http://www.knora.org/ontology/shared/text>.
@prefix text: <http://www.knora.org/ontology/shared/text#>.

<http://www.knora.org/ontology/shared/text>
	a owl:Ontology;
	dct:license <http://creativecommons.org/licenses/by/3.0/>;
	dct:title "An ontology about text"@en;
	dct:description """Formal description of text in broadest sense, general subclasses, related classes, and properties."""@en;
	skos:note """Text structure, text editing, and text roles are described in respective ontologies"""@en;
	dct:creator "Hans Cools, MD, knowledge engineer, ontologist, software developer, NIE-INE, Basel University, Switzerland"@en;
	dct:contributor "Roberta Padlina, tool coordinator, software developer, NIE-INE, Basel University, Switzerland"@en;
	dct:publisher "Basel University, Switzerland"@en;
#	skos:note """Representation of text as an otherwise literal data element as object enabling relating it to other information"""@en.

	knora-base:attachedToProject <http://www.knora.org/ontology/knora-base#DefaultSharedOntologiesProject>.

#
# CLASSES
#

text:Text
	a owl:Class;
	rdfs:label "text"@en, "Text"@de, "texte"@fr, "testo"@it;
	rdfs:comment """Human natural language expression serialized in writable form."""@en; # coherent set of signs representing semantics in a language
	rdfs:subClassOf language:HumanNaturalLanguageExpression, [
		a owl:Restriction; owl:onProperty text:isTextOfDocument; owl:minCardinality "0"^^xsd:nonNegativeInteger], [
		a owl:Restriction; owl:onProperty text:isTextOfDocumentValue; owl:minCardinality "0"^^xsd:nonNegativeInteger], [
		a owl:Restriction; owl:onProperty text:hasContentNature; owl:minCardinality "0"^^xsd:nonNegativeInteger], [
		a owl:Restriction; owl:onProperty text:hasContentNatureValue; owl:minCardinality "0"^^xsd:nonNegativeInteger], [
		a owl:Restriction; owl:onProperty text:hasLineNumber; owl:minCardinality "0"^^xsd:nonNegativeInteger], [
		a owl:Restriction; owl:onProperty text:hasVersionIndicator; owl:minCardinality "0"^^xsd:nonNegativeInteger], [
		a owl:Restriction; owl:onProperty text:hasPageNumberDescription; owl:minCardinality "0"^^xsd:nonNegativeInteger], [
		a owl:Restriction; owl:onProperty text:hasNumberOfPages; owl:minCardinality "0"^^xsd:nonNegativeInteger], [
		a owl:Restriction; owl:onProperty text:hasReferenceText; owl:minCardinality "0"^^xsd:nonNegativeInteger], [
		a owl:Restriction; owl:onProperty text:hasReferenceTextValue; owl:minCardinality "0"^^xsd:nonNegativeInteger], [
		a owl:Restriction; owl:onProperty text:hasTranscriber; owl:minCardinality "0"^^xsd:nonNegativeInteger], [
		a owl:Restriction; owl:onProperty text:hasTranscriberValue; owl:minCardinality "0"^^xsd:nonNegativeInteger], [
		a owl:Restriction; owl:onProperty text:hasVulgarizer; owl:minCardinality "0"^^xsd:nonNegativeInteger], [
		a owl:Restriction; owl:onProperty text:hasVulgarizerValue; owl:minCardinality "0"^^xsd:nonNegativeInteger], [
		a owl:Restriction; owl:onProperty text:hasCiter; owl:minCardinality "0"^^xsd:nonNegativeInteger], [
		a owl:Restriction; owl:onProperty text:hasCiterValue; owl:minCardinality "0"^^xsd:nonNegativeInteger], [
		a owl:Restriction; owl:onProperty text:hasCitation; owl:minCardinality "0"^^xsd:nonNegativeInteger], [
		a owl:Restriction; owl:onProperty text:hasCitationValue; owl:minCardinality "0"^^xsd:nonNegativeInteger], [
		a owl:Restriction; owl:onProperty text:hasCitationReference; owl:minCardinality "0"^^xsd:nonNegativeInteger], [
		a owl:Restriction; owl:onProperty text:hasCitationReferenceValue; owl:minCardinality "0"^^xsd:nonNegativeInteger], [
		a owl:Restriction; owl:onProperty text:isCitedIn; owl:minCardinality "0"^^xsd:nonNegativeInteger], [
		a owl:Restriction; owl:onProperty text:isCitedInValue; owl:minCardinality "0"^^xsd:nonNegativeInteger], [
		a owl:Restriction; owl:onProperty text:hasEditor; owl:minCardinality "0"^^xsd:nonNegativeInteger], [
		a owl:Restriction; owl:onProperty text:hasEditorValue; owl:minCardinality "0"^^xsd:nonNegativeInteger], [
		a owl:Restriction; owl:onProperty text:hasRevisor; owl:minCardinality "0"^^xsd:nonNegativeInteger], [
		a owl:Restriction; owl:onProperty text:hasRevisorValue; owl:minCardinality "0"^^xsd:nonNegativeInteger], [
		a owl:Restriction; owl:onProperty text:hasAnnotator; owl:minCardinality "0"^^xsd:nonNegativeInteger], [
		a owl:Restriction; owl:onProperty text:hasAnnotatorValue; owl:minCardinality "0"^^xsd:nonNegativeInteger], [
		a owl:Restriction; owl:onProperty text:hasGlossator; owl:minCardinality "0"^^xsd:nonNegativeInteger], [
		a owl:Restriction; owl:onProperty text:hasGlossatorValue; owl:minCardinality "0"^^xsd:nonNegativeInteger], [
		a owl:Restriction; owl:onProperty text:hasAbbreviator; owl:minCardinality "0"^^xsd:nonNegativeInteger], [
		a owl:Restriction; owl:onProperty text:hasAbbreviatorValue; owl:minCardinality "0"^^xsd:nonNegativeInteger], [
		a owl:Restriction; owl:onProperty text:hasCompiler; owl:minCardinality "0"^^xsd:nonNegativeInteger], [
		a owl:Restriction; owl:onProperty text:hasCompilerValue; owl:minCardinality "0"^^xsd:nonNegativeInteger], [
		a owl:Restriction; owl:onProperty textedit:hasEdition; owl:minCardinality "0"^^xsd:nonNegativeInteger], [
		a owl:Restriction; owl:onProperty textedit:hasEditionValue; owl:minCardinality "0"^^xsd:nonNegativeInteger], [
		a owl:Restriction; owl:onProperty textedit:hasSameEditionAs; owl:minCardinality "0"^^xsd:nonNegativeInteger], [
		a owl:Restriction; owl:onProperty textedit:hasSameEditionAsValue; owl:minCardinality "0"^^xsd:nonNegativeInteger], [
		a owl:Restriction; owl:onProperty textedit:hasTransliteration; owl:minCardinality "0"^^xsd:nonNegativeInteger], [
		a owl:Restriction; owl:onProperty textedit:hasTransliterationValue; owl:minCardinality "0"^^xsd:nonNegativeInteger], [
		a owl:Restriction; owl:onProperty infocar:isTextOnPage; owl:minCardinality "0"^^xsd:nonNegativeInteger], [
		a owl:Restriction; owl:onProperty infocar:isTextOnPageValue; owl:minCardinality "0"^^xsd:nonNegativeInteger].

text:ContentNature
	a owl:Class;
	rdfs:label "text content nature"@en, "textinhaltliche Art"@de;
	rdfs:comment """Nature of the content of a text."""@en;
	rdfs:subClassOf text:Text.

text:Nonfiction
	a owl:Class;
	rdfs:label "nonfiction text"@en, "Sachtext"@de;
	rdfs:comment """Text having content based on fact."""@en;
	rdfs:subClassOf text:ContentNature, concept:Nonfiction.

text:Fiction
	a owl:Class;
	rdfs:label "fiction text"@en, "Fiktiontext"@de;
	rdfs:comment """Text having content derived from imagination."""@en;
	rdfs:subClassOf text:ContentNature, concept:Fiction.

text:Developing
	a owl:Class;
	rdfs:label "text developing"@en, "Textentwicklung"@de;
	rdfs:comment """Action wherein a person(s) creates text resulting in different manifestation, e.g. from notebook to manuscript to typescript to published print."""@en;
	rdfs:subClassOf creating:Creating, [
		a owl:Restriction; owl:onProperty event:hasStage; owl:minCardinality "0"^^xsd:nonNegativeInteger], [
		a owl:Restriction; owl:onProperty event:hasStageValue; owl:minCardinality "0"^^xsd:nonNegativeInteger].

text:SurfaceText
	a owl:Class;
	rdfs:label "surface text"@en, "Flächetext"@de, "texte surfacique"@fr, "testo superficiale"@it;
	rdfs:comment """Text applied to any surface in any way, abstracted from its carrier."""@en;
	skos:note """Groups written and printed text."""@en;
	rdfs:subClassOf text:Text.

text:WrittenText
	a owl:Class;
	rdfs:label "written text"@en, "geschriebener Text"@de, "texte écrit"@fr, "testo scritto"@it;
	rdfs:comment """Text written by symbol, by any method, e.g. manually, with a typewriter, or on a computer, abstracted from its carrier."""@en;
	rdfs:subClassOf text:SurfaceText, [
		a owl:Restriction; owl:onProperty infocar:isWrittenWith; owl:minCardinality "0"^^xsd:nonNegativeInteger], [
		a owl:Restriction; owl:onProperty infocar:isWrittenWithValue; owl:minCardinality "0"^^xsd:nonNegativeInteger].

text:Handwriter
	a owl:Class;
	rdfs:label "handwriter"@en, "Handschreiber"@de, "écrivain"@fr, "manoscrittore"@it;
	rdfs:comment """Role of a person writing text symbols by hand."""@en;
	rdfs:subClassOf creating:PersonCreator.

text:HandwrittenText
	a owl:Class;
	rdfs:label "handwritten text"@en, "handgeschriebener Text"@de, "texte manuscrit"@fr, "testo scritto a mano"@it;
	rdfs:comment """Text with symbols formed by hand, abstracted from its manuscript."""@en;
	rdfs:subClassOf text:WrittenText, [
		a owl:Restriction; owl:onProperty text:hasHandwriter; owl:minCardinality "0"^^xsd:nonNegativeInteger], [
		a owl:Restriction; owl:onProperty text:hasHandwriterValue; owl:minCardinality "0"^^xsd:nonNegativeInteger], [
		a owl:Restriction; owl:onProperty infocar:isInManuscript; owl:minCardinality "0"^^xsd:nonNegativeInteger], [
		a owl:Restriction; owl:onProperty infocar:isInManuscriptValue; owl:minCardinality "0"^^xsd:nonNegativeInteger].

text:TypewrittenText
	a owl:Class;
	rdfs:label "typewritten text"@en, "maschinengeschriebener Text"@de, "texte dactylographié"@fr, "testo dattiloscritto"@it;
	rdfs:comment """Text written with a typewriter."""@en;
	rdfs:subClassOf text:WrittenText, [
		a owl:Restriction; owl:onProperty infocar:isInTypescript; owl:minCardinality "0"^^xsd:nonNegativeInteger], [
		a owl:Restriction; owl:onProperty infocar:isInTypescriptValue; owl:minCardinality "0"^^xsd:nonNegativeInteger].

text:PrintedText
	a owl:Class;
	rdfs:label "printed text"@en, "gedruckter Text"@de, "texte imprimé"@fr, "testo stampato"@it;
	rdfs:comment """Text printed by any method, abstracted from its carrier."""@en;
	rdfs:subClassOf text:Text, [
		a owl:Restriction; owl:onProperty infocar:isInPrint; owl:minCardinality "0"^^xsd:nonNegativeInteger], [
		a owl:Restriction; owl:onProperty infocar:isInPrintValue; owl:minCardinality "0"^^xsd:nonNegativeInteger].

text:CopiedText
	a owl:Class;
	rdfs:label "copied text"@en, "kopierter Text"@de, "texte copié"@fr, "testo copiato"@it;
	rdfs:comment """Text copied by any method; text abstracted from its carrier."""@en;
	rdfs:subClassOf text:Text, [
		a owl:Restriction; owl:onProperty infocar:isInTextCopy; owl:minCardinality "0"^^xsd:nonNegativeInteger], [
		a owl:Restriction; owl:onProperty infocar:isInTextCopyValue; owl:minCardinality "0"^^xsd:nonNegativeInteger].

text:Transcriber
	a owl:Class;
	rdfs:label "text transcriber"@en, "TexttranskribiererIn"@de, "scribe de texte"@fr, "scriba di testo"@it;
	rdfs:comment """Role of a person copying a text by writing, creating a transcribed text in a transcript."""@en;
	rdfs:subClassOf creating:PersonCreator.

text:TranscribedText
	a owl:Class;
	rdfs:label "transcribed text"@en, "transkribierter Text"@de, "texte transcrit"@fr, "testo trascritto"@it;
	rdfs:comment """Text copied by character by any writing method; text abstracted from its carrier."""@en;
	rdfs:subClassOf text:CopiedText, [
		a owl:Restriction; owl:onProperty infocar:isInTranscript; owl:minCardinality "0"^^xsd:nonNegativeInteger], [
		a owl:Restriction; owl:onProperty infocar:isInTranscriptValue; owl:minCardinality "0"^^xsd:nonNegativeInteger].

text:Scribe
	a owl:Class;
	rdfs:label "scribe"@en, "TextKopist"@de, "scribe"@fr, "scriba"@it, "scribes"@la;
	rdfs:comment """Role of a person copying a text by handwriting, creating a transcribed text in a manual transcript."""@en;
	rdfs:subClassOf text:Transcriber.

text:PhotocopiedText
	a owl:Class;
	rdfs:label "photocopied text"@en, "fotokopierter Text"@de; #, "texte copié"@fr, "testo copiato"@it;
	rdfs:comment """Text photocopied, abstracted from its carrier."""@en;
	rdfs:subClassOf text:CopiedText, [
		a owl:Restriction; owl:onProperty infocar:isTextInPhotocopy; owl:minCardinality "0"^^xsd:nonNegativeInteger], [
		a owl:Restriction; owl:onProperty infocar:isTextInPhotocopyValue; owl:minCardinality "0"^^xsd:nonNegativeInteger].

text:AgentCiter
	a owl:Class;
	rdfs:label "agent citer"@en, "Agent-Zitierer"@de;
	rdfs:comment """Role of a human agent, person or group, citing a text."""@en;
	rdfs:subClassOf human:AgentRole.

text:PersonCiter
	a owl:Class;
	rdfs:label "person citer"@en, "Person-ZitiererIn"@de;
	rdfs:comment """Citer as role of a person."""@en;
	rdfs:subClassOf text:AgentCiter, human:PersonRole.

text:OrganizationCiter
	a owl:Class;
	rdfs:label "organization citer"@en, "Organisation-Zitiererin"@de;
	rdfs:comment """Citer as role of an organization."""@en;
	rdfs:subClassOf text:AgentCiter, org:Role.

text:Citation
	a owl:Class;
	rdfs:label "citation"@en, "Zitat"@de, "citation"@fr, "citazione"@it;
	rdfs:comment """Copy of a text expression, mostly a part of it, in another text expression, with reference to the first expression."""@en;
	skos:note """A citation can also be referred to from the source text, having an identifier linked to both the source reference and the citation."""@en;
	rdfs:subClassOf text:CopiedText, text-structure:ContentStructure, [
		a owl:Restriction; owl:onProperty text:citationHasReference; owl:minCardinality "0"^^xsd:nonNegativeInteger], [
		a owl:Restriction; owl:onProperty text:citationHasReferenceValue; owl:minCardinality "0"^^xsd:nonNegativeInteger], [
		a owl:Restriction; owl:onProperty text:citationHasIdentifier; owl:minCardinality "0"^^xsd:nonNegativeInteger], [
		a owl:Restriction; owl:onProperty text:citationHasIdentifierValue; owl:minCardinality "0"^^xsd:nonNegativeInteger], [
		a owl:Restriction; owl:onProperty text:citationHasNumber; owl:minCardinality "0"^^xsd:nonNegativeInteger], [
		a owl:Restriction; owl:onProperty text:citationHasNumberValue; owl:minCardinality "0"^^xsd:nonNegativeInteger], [
		a owl:Restriction; owl:onProperty text:citationIsPartOf; owl:minCardinality "0"^^xsd:nonNegativeInteger], [
		a owl:Restriction; owl:onProperty text:citationIsPartOfValue; owl:minCardinality "0"^^xsd:nonNegativeInteger].

text:CitationReference
	a owl:Class;
	rdfs:label "citation reference"@en, "Zitatreferenz"@de;
	rdfs:comment """Reference of a citation to the referred."""@en;
	rdfs:subClassOf document:TextStructureReference, [
		a owl:Restriction; owl:onProperty text:hasCitationIdentifier; owl:minCardinality "0"^^xsd:nonNegativeInteger], [
		a owl:Restriction; owl:onProperty text:hasCitationIdentifierValue; owl:minCardinality "0"^^xsd:nonNegativeInteger].

text:CitationIdentifier
	a owl:Class;
	rdfs:label "citation identifier"@en, "Zitatidentifikator"@de;
	rdfs:comment """Identifier of a citation."""@en;
	rdfs:subClassOf concept:Identifier, document:Structure.

text:CitationNumber
	a owl:Class;
	rdfs:label "citation number"@en, "Zitatnummer"@de;
	rdfs:comment """Number of a citation."""@en;
	rdfs:subClassOf text:CitationIdentifier, math:Number.

text:Normalization
	a owl:Class;
	rdfs:label "text normalization"@en, "Textnormalisation"@de;
	rdfs:comment """Derivative of a text of which it is a normalization along a certain procedure."""@en;
	rdfs:subClassOf text:Text, creating:CreationDerivative,
		a owl:Restriction; owl:onProperty text:isNormalizationOf; owl:minCardinality "0"^^xsd:nonNegativeInteger], [
		a owl:Restriction; owl:onProperty text:isNormalizationOfValue; owl:minCardinality "0"^^xsd:nonNegativeInteger].

text:Compiler
	a owl:Class;
	rdfs:label "compiler"@en, "Kompilator"@de, "compilator"@la;
	rdfs:comment """Role of a person assembling texts to a new whole."""@en;
	rdfs:subClassOf creating:PersonCreator.

text:CompiledText
	a owl:Class;
	rdfs:label "compiled text"@en, "zusammengestellte Text"@de, "texte compilé"@fr, "testo compilato"@it;
	rdfs:comment """Text assembled from previously separate texts."""@en;
	rdfs:subClassOf text:Text, [
		a owl:Restriction; owl:onProperty infocar:isInCompilation; owl:minCardinality "0"^^xsd:nonNegativeInteger], [
		a owl:Restriction; owl:onProperty infocar:isInCompilationValue; owl:minCardinality "0"^^xsd:nonNegativeInteger].

text:Translation
	a owl:Class;
	rdfs:label "text translation"@en, "Textübersetzung"@de, "traduction de texte"@fr, "traduzione di testi"@it;
	rdfs:comment """Translation from text to text."""@en;
	rdfs:subClassOf text:Text, language:Translation.

#
# PROPERTIES
#

text:hasText
	a owl:ObjectProperty;
	rdfs:label "has text"@en, "hat Text"@de;
	rdfs:comment """Relating a resource to a text as a writable coherent set of signs representing semantics in a language."""@en;
	rdfs:subPropertyOf knora-base:hasValue;
	knora-base:subjectClassConstraint knora-base:Resource;
	knora-base:objectClassConstraint knora-base:TextValue.

text:hasName
	a owl:ObjectProperty;
	rdfs:label "has name"@en, "hat Name"@de;
	rdfs:comment """Relating a resource to a name as a textual identifier of the resource."""@en;
	rdfs:subPropertyOf text:hasText; #° rdfs:label, foaf:name
	knora-base:subjectClassConstraint knora-base:Resource;
	knora-base:objectClassConstraint knora-base:TextValue.

text:hasPreferredName
	a owl:ObjectProperty;
	rdfs:label "has preferred name"@en, "hat bevorzugter Name"@de;
	rdfs:comment """Relating a resource to a preferred name."""@en;
	rdfs:subPropertyOf text:hasName;
	knora-base:subjectClassConstraint knora-base:Resource;
	knora-base:objectClassConstraint knora-base:TextValue.

text:hasAlias
	a owl:ObjectProperty;
	rdfs:label "has alias"@en, "hat Alias"@de;
	rdfs:comment """Relating a resource to an alias as an alternative name of the resource."""@en;
	rdfs:subPropertyOf text:hasName;
	knora-base:subjectClassConstraint knora-base:Resource;
	knora-base:objectClassConstraint knora-base:TextValue.

text:hasIdentifier
	a owl:ObjectProperty;
	rdfs:label "has identifier"@en, "hat Kennzeichen"@de;
	rdfs:comment """Relating a resource to an identifier as a unique and permanent textual reference to the resource within a given context, and conforming to a formal identification system."""@en;
	rdfs:subPropertyOf text:hasText; #° cf. dcterms:identifier
	knora-base:subjectClassConstraint knora-base:Resource;
	knora-base:objectClassConstraint knora-base:TextValue.

text:hasTitle
	a owl:ObjectProperty;
	rdfs:label "has title"@en, "hat Titel"@de;
	rdfs:comment """Relating a resource to a title as a textual identifier of the resource."""@en;
	rdfs:subPropertyOf text:hasText;
	knora-base:subjectClassConstraint knora-base:Resource;
	knora-base:objectClassConstraint knora-base:TextValue.

text:hasSubtitle
	a owl:ObjectProperty;
	rdfs:label "has subtitle"@en, "hat Untertitel"@de;
	rdfs:comment """Relating a resource to a subtitle as additional, usually explanatory to the title."""@en;
	rdfs:subPropertyOf text:hasText;
	knora-base:subjectClassConstraint knora-base:Resource;
	knora-base:objectClassConstraint knora-base:TextValue.

text:hasComment
	a owl:ObjectProperty;
	rdfs:label "has comment"@en, "hat Kommentar"@de;
	rdfs:comment """Relating a resource to a comment as a textual statement about the resource."""@en;
	rdfs:subPropertyOf text:hasText;
	knora-base:subjectClassConstraint knora-base:Resource;
	knora-base:objectClassConstraint knora-base:TextValue.

text:hasDescription
	a owl:ObjectProperty;
	rdfs:label "has description"@en, "hat Beschreibung"@de;
	rdfs:comment """Relating a resource to a description as a textual statement about features of the resource."""@en;
	rdfs:subPropertyOf text:hasText;
	knora-base:subjectClassConstraint knora-base:Resource;
	knora-base:objectClassConstraint knora-base:TextValue.

text:hasDefinition
	a owl:ObjectProperty;
	rdfs:label "has definition"@en, "hat Definition"@de;
	rdfs:comment """Relating a resource to a definition as a textual statement about the essential features of the resource."""@en;
	rdfs:subPropertyOf text:hasDescription;
	knora-base:subjectClassConstraint knora-base:Resource;
	knora-base:objectClassConstraint knora-base:TextValue.

text:hasDetailDescription
	a owl:ObjectProperty;
	rdfs:label "has detail description"@en, "hat Detail-Beschreibung"@de;
	rdfs:comment """Relating a resource to a description of its detail. E.g. in the case of a text a detail can be a passage variant or an emendation"""@en;
	rdfs:subPropertyOf text:hasDescription;
	knora-base:subjectClassConstraint knora-base:Resource;
	knora-base:objectClassConstraint knora-base:TextValue.

text:hasSpecialDescription
	a owl:ObjectProperty;
	rdfs:label "has special description"@en, "hat Besonderes-Beschreibung"@de;
	rdfs:comment """Relating a resource to a description of (a) certain feature(s)."""@en;
	rdfs:subPropertyOf text:hasDescription;
	knora-base:subjectClassConstraint knora-base:Resource;
	knora-base:objectClassConstraint knora-base:TextValue.

text:isTextOfDocument
	a owl:ObjectProperty;
	rdfs:label "is text of document"@en, "ist Text eines Dokumentes"@de;
	rdfs:comment "Relating a text to the document it is part of."@en;
	rdfs:subPropertyOf concept:isPartOf;
	knora-base:subjectClassConstraint text:Text;
	knora-base:objectClassConstraint document:Document.

text:isTextOfDocumentValue
	a owl:ObjectProperty;
	rdfs:label "is text of document - statement"@en, "ist Text eines Dokumentes - Festlegung"@de;
	rdfs:comment "Relating a text to a reification statement of the relation between the text and the document it is part of."@en;
	rdfs:subPropertyOf concept:isPartOfValue;
	knora-base:subjectClassConstraint text:Text;
	knora-base:objectClassConstraint knora-base:LinkValue.

text:hasContentNature
	a owl:ObjectProperty;
	rdfs:label "has content nature"@en, "hat textinhaltliche Art"@de;
	rdfs:comment """Relating a text to a content nature it has."""@en;
	rdfs:subPropertyOf knora-base:hasLinkTo;
	knora-base:subjectClassConstraint text:Text;
	knora-base:objectClassConstraint text:ContentNature.

text:hasContentNatureValue
	a owl:ObjectProperty;
	rdfs:label "has content nature - statement"@en, "hat textinhaltliche Art - Festlegung"@de;
	rdfs:comment """Relating a text to a reification statement of the relation between the text and a content nature it has."""@en;
	rdfs:subPropertyOf knora-base:hasLinkToValue;
	knora-base:subjectClassConstraint text:Text;
	knora-base:objectClassConstraint knora-base:LinkValue.

text:hasLineNumber
	a owl:ObjectProperty;
	rdfs:label "has line number"@en, "hat Liniennummer"@de;
	rdfs:comment """Relating a text to the number of a line of the text expression."""@en;
	rdfs:subPropertyOf text:hasText;
	knora-base:subjectClassConstraint text:Text;
	knora-base:objectClassConstraint knora-base:TextValue.

text:hasVersionIndicator
	a owl:ObjectProperty;
	rdfs:label "has version indicator"@en, "hat Version-Indikator"@de;
	rdfs:comment """Relating a text to a textual element that indicates its version."""@en;
	rdfs:subPropertyOf text:hasText;
	knora-base:subjectClassConstraint text:Text;
	knora-base:objectClassConstraint knora-base:TextValue.

text:hasPageNumberDescription
	a owl:ObjectProperty;
	rdfs:label "text has page number description"@en, "Text hat Seitennummerbeschreibung"@de;
	rdfs:comment """Relating a text to a description of the number(s) of and possibly a location on (a) pages it is on; examples of the string of its value: "001-002", "01 recto", "O2 (bottom)"."""@en;
	rdfs:subPropertyOf knora-base:hasValue;
	knora-base:subjectClassConstraint text:Text;
	knora-base:objectClassConstraint knora-base:TextValue.

text:hasNumberOfPages
	a owl:ObjectProperty;
	rdfs:label "has number of pages"@en, "hat Seitenanzahl"@de;
	rdfs:comment """Relating a text to the number of pages it has."""@en;
	rdfs:subPropertyOf knora-base:hasValue;
	knora-base:subjectClassConstraint text:Text;
	knora-base:objectClassConstraint knora-base:TextValue.

text:hasReferenceText
	a owl:ObjectProperty;
	rdfs:label "has reference text"@en, "hat Bezugstext"@de;
	rdfs:comment "Relating a text to another one as its reference."@en;
	rdfs:subPropertyOf knora-base:hasLinkTo;
	knora-base:subjectClassConstraint text:Text;
	knora-base:objectClassConstraint text:Text.

text:hasReferenceTextValue
	a owl:ObjectProperty;
	rdfs:label "has reference text - statement"@en, "hat Bezugstext - Festlegung"@de;
	rdfs:comment "Relating a text to a reification statement of the relation between the text and another one as its reference."@en;
	rdfs:subPropertyOf knora-base:hasLinkToValue;
	knora-base:subjectClassConstraint text:Text;
	knora-base:objectClassConstraint knora-base:LinkValue.

text:hasTranscriber
	a owl:ObjectProperty;
	rdfs:label "has transcriber"@en, "hat TranskribiererIn"@de;
	rdfs:comment """Relating a text to a person who transcribed it; text abstracted from its carrier."""@en;
	rdfs:subPropertyOf knora-base:hasLinkTo;
	knora-base:subjectClassConstraint text:Text;
	knora-base:objectClassConstraint human:Person.

text:hasTranscriberValue
	a owl:ObjectProperty;
	rdfs:label "has transcriber - statement"@en, "hat TranskribiererIn - Festlegung"@de;
	rdfs:comment """Relating a text to a reification statement of the relation between the text and a person who transcribed it."""@en;
	rdfs:subPropertyOf knora-base:hasLinkToValue;
	knora-base:subjectClassConstraint text:Text;
	knora-base:objectClassConstraint knora-base:LinkValue.

text:hasVulgarizer
	a owl:ObjectProperty;
	rdfs:label "text has vulgarizer"@en, "Text hat VulgarisatorIn"@de;
	rdfs:comment """Relating a text to a person who vulgarized it."""@en;
	rdfs:subPropertyOf knora-base:hasLinkTo;
	knora-base:subjectClassConstraint text:Text;
	knora-base:objectClassConstraint human:Person.

text:hasVulgarizerValue
	a owl:ObjectProperty;
	rdfs:label "text has vulgarizer - statement"@en, "Text hat VulgarisatorIn - Festlegung"@de;
	rdfs:comment """Relating a text to a reification statement of the relation between the text and a person who vulgarized it."""@en;
	rdfs:subPropertyOf knora-base:hasLinkToValue;
	knora-base:subjectClassConstraint text:Text;
	knora-base:objectClassConstraint knora-base:LinkValue.

text:hasCiter
	a owl:ObjectProperty;
	rdfs:label "has citer"@en, "hat ZitiererIn"@de;
	rdfs:comment """Relating a text to a human agent - person or group - citing it."""@en;
	rdfs:subPropertyOf knora-base:hasLinkTo;
	knora-base:subjectClassConstraint text:Text;
	knora-base:objectClassConstraint human:Agent.

text:hasCiterValue
	a owl:ObjectProperty;
	rdfs:label "has citer - statement"@en, "hat ZitiererIn - Festlegung"@de;
	rdfs:comment """Relating a text to a reification statement of the relation between the text and a human agent - person or group - citing it."""@en;
	rdfs:subPropertyOf knora-base:hasLinkToValue;
	knora-base:subjectClassConstraint text:Text;
	knora-base:objectClassConstraint knora-base:LinkValue.

text:hasCitation
	a owl:ObjectProperty;
	rdfs:label "has citation"@en, "hat Zitat"@de;
	rdfs:comment "Relating a text to a citation thereof."@en;
	rdfs:subPropertyOf knora-base:hasLinkTo;
	knora-base:subjectClassConstraint text:Text;
	knora-base:objectClassConstraint text:Citation.

text:hasCitationValue
	a owl:ObjectProperty;
	rdfs:label "has citation - statement"@en, "hat Zitat - Festlegung"@de;
	rdfs:comment "Relating a text to a reification statement of the relation between the text and a citation thereof."@en;
	rdfs:subPropertyOf knora-base:hasLinkToValue;
	knora-base:subjectClassConstraint text:Text;
	knora-base:objectClassConstraint knora-base:LinkValue.

text:hasCitationReference
	a owl:ObjectProperty;
	rdfs:label "has citation reference"@en, "hat Zitatreferenz"@de;
	rdfs:comment "Relating a text to a citation reference thereof."@en;
	rdfs:subPropertyOf knora-base:hasLinkTo;
	knora-base:subjectClassConstraint text:Text;
	knora-base:objectClassConstraint text:CitationReference.

text:hasCitationReferenceValue
	a owl:ObjectProperty;
	rdfs:label "has citation reference - statement"@en, "hat Zitatreferenz - Festlegung"@de;
	rdfs:comment "Relating a text to a reification statement of the relation between the text and a citation reference thereof."@en;
	rdfs:subPropertyOf knora-base:hasLinkToValue;
	knora-base:subjectClassConstraint text:Text;
	knora-base:objectClassConstraint knora-base:LinkValue.

text:isCitedIn
	a owl:ObjectProperty;
	rdfs:label "is cited in"@en, "ist zitiert in"@de;
	rdfs:comment "Relating a text to an expression wherein it is cited."@en;
	rdfs:subPropertyOf knora-base:hasLinkTo;
	knora-base:subjectClassConstraint text:Text;
	knora-base:objectClassConstraint document:Expression.

text:isCitedInValue
	a owl:ObjectProperty;
	rdfs:label "is cited in - statement"@en, "ist zitiert in - Festlegung"@de;
	rdfs:comment "Relating a text to a reification statement of the relation between the text and an expression wherein it is cited."@en;
	rdfs:subPropertyOf knora-base:hasLinkToValue;
	knora-base:subjectClassConstraint text:Text;
	knora-base:objectClassConstraint knora-base:LinkValue.

text:hasEditor
	a owl:ObjectProperty;
	rdfs:label "text has editor"@en, "Text hat EditorIn"@de;
	rdfs:comment """Relating a text to a person who edited it."""@en;
	rdfs:subPropertyOf knora-base:hasLinkTo;
	knora-base:subjectClassConstraint text:Text;
	knora-base:objectClassConstraint human:Person.

text:hasEditorValue
	a owl:ObjectProperty;
	rdfs:label "text has editor - statement"@en, "Text hat EditorIn - Festlegung"@de;
	rdfs:comment """Relating a text to a reification statement of the relation between the text and a person who edited it."""@en;
	rdfs:subPropertyOf knora-base:hasLinkToValue;
	knora-base:subjectClassConstraint text:Text;
	knora-base:objectClassConstraint knora-base:LinkValue.

text:hasHandwriter
	a owl:ObjectProperty;
	rdfs:label "has handwriter"@en, "hat Handschreiber"@de;
	rdfs:comment """Relating a handwritten text to the person who wrote it."""@en;
	rdfs:subPropertyOf knora-base:hasLinkTo;
	knora-base:subjectClassConstraint text:HandwrittenText;
	knora-base:objectClassConstraint human:Person.

text:hasHandwriterValue
	a owl:ObjectProperty;
	rdfs:label "has handwriter - statement"@en, "hat Handschreiber - Festlegung"@de;
	rdfs:comment """Relating a handwritten text to a reification statement of the relation between the text and a person who wrote it."""@en;
	rdfs:subPropertyOf knora-base:hasLinkToValue;
	knora-base:subjectClassConstraint text:HandwrittenText;
	knora-base:objectClassConstraint knora-base:LinkValue.

text:citationHasReference
	a owl:ObjectProperty;
	rdfs:label "citation has reference"@en, "Zitat hat Referenz"@de;
	rdfs:comment """Relating a citation to its reference."""@en;
	rdfs:subPropertyOf document:hasTextReference;
	knora-base:subjectClassConstraint text:Citation;
	knora-base:objectClassConstraint document:TextStructureReference.

text:citationHasReferenceValue
	a owl:ObjectProperty;
	rdfs:label "citation has reference - statement"@en, "Zitat hat Referenz - Festlegung"@de;
	rdfs:comment """Relating a citation to a reification statement of the relation between the citation and its reference."""@en;
	rdfs:subPropertyOf document:hasTextReferenceValue;
	knora-base:subjectClassConstraint text:Citation;
	knora-base:objectClassConstraint knora-base:LinkValue.

text:citationHasIdentifier
	a owl:ObjectProperty;
	rdfs:label "citation has identifier"@en, "Zitat hat Identifikator"@de;
	rdfs:comment """Relating a citation to its identifier."""@en;
	rdfs:subPropertyOf knora-base:hasLinkTo; # text-structure:hasIdentifier
	knora-base:subjectClassConstraint text:Citation;
	knora-base:objectClassConstraint text:CitationIdentifier.

text:citationHasIdentifierValue
	a owl:ObjectProperty;
	rdfs:label "citation has identifier - statement"@en, "Zitat hat Identifikator - Festlegung"@de;
	rdfs:comment """Relating a citation to a reification statement of the relation between the citation and its identifier."""@en;
	rdfs:subPropertyOf knora-base:hasLinkToValue; # text-structure:hasIdentifierValue
	knora-base:subjectClassConstraint text:Citation;
	knora-base:objectClassConstraint knora-base:LinkValue.

text:citationHasNumber
	a owl:ObjectProperty;
	rdfs:label "citation has number"@en, "Zitat hat Nummer"@de;
	rdfs:comment """Relating a citation to its number."""@en;
	rdfs:subPropertyOf text:citationHasIdentifier;
	knora-base:subjectClassConstraint text:Citation;
	knora-base:objectClassConstraint text:CitationNumber.

text:citationHasNumberValue
	a owl:ObjectProperty;
	rdfs:label "citation has number - statement"@en, "Zitat hat Nummer - Festlegung"@de;
	rdfs:comment """Relating a citation to a reification statement of the relation between the citation and its number."""@en;
	rdfs:subPropertyOf text:citationHasIdentifierValue;
	knora-base:subjectClassConstraint text:Citation;
	knora-base:objectClassConstraint knora-base:LinkValue.

text:citationIsPartOf
	a owl:ObjectProperty;
	rdfs:label "citation is part of text expression"@en, "Zitat ist Teil einer Textexpression"@de;
	rdfs:comment """Relating a citation to a text expression it is part of."""@en;
	rdfs:subPropertyOf concept:isPartOf;
	knora-base:subjectClassConstraint text:Citation;
	knora-base:objectClassConstraint text-expression:Expression.

text:citationIsPartOfValue
	a owl:ObjectProperty;
	rdfs:label "citation is part of text expression - statement"@en, "Zitat ist Teil einer Textexpression - Festlegung"@de;
	rdfs:comment """Relating a citation to a reification statement of the relation between the citation and a text expression it is part of."""@en;
	rdfs:subPropertyOf concept:isPartOfValue;
	knora-base:subjectClassConstraint text:Citation;
	knora-base:objectClassConstraint knora-base:LinkValue.

text:hasCitationIdentifier
	a owl:ObjectProperty;
	rdfs:label "has citation identifier"@en, "hat Zitatidentifikator"@de;
	rdfs:comment """Relating a citation reference to its citation identifier."""@en;
	rdfs:subPropertyOf knora-base:hasLinkTo; #°
	knora-base:subjectClassConstraint text:CitationReference;
	knora-base:objectClassConstraint text:CitationIdentifier.

text:hasCitationIdentifierValue
	a owl:ObjectProperty;
	rdfs:label "has citation identifier - statement"@en, "hat Zitatidentifikator - Festlegung"@de;
	rdfs:comment """Relating a citation reference to a reification statement of the relation between that reference and its citation identifier."""@en;
	rdfs:subPropertyOf knora-base:hasLinkToValue; #°
	knora-base:subjectClassConstraint text:CitationReference;
	knora-base:objectClassConstraint knora-base:LinkValue.

text:hasRevisor
	a owl:ObjectProperty;
	rdfs:label "text has revisor"@en, "Text hat Revisor"@de;
	rdfs:comment """Relating a text to a person who revised it."""@en;
	rdfs:subPropertyOf knora-base:hasLinkTo;
	knora-base:subjectClassConstraint text:Text;
	knora-base:objectClassConstraint human:Person.

text:hasRevisorValue
	a owl:ObjectProperty;
	rdfs:label "text has revisor - statement"@en, "Text hat Revisor - Festlegung"@de;
	rdfs:comment """Relating a text to a reification statement of the relation between the text and a person who revised it."""@en;
	rdfs:subPropertyOf knora-base:hasLinkToValue;
	knora-base:subjectClassConstraint text:Text;
	knora-base:objectClassConstraint knora-base:LinkValue.

text:hasAnnotator
	a owl:ObjectProperty;
	rdfs:label "text has annotator"@en, "Text hat AnnotatorIn"@de;
	rdfs:comment """Relating a text to a person who annotated it."""@en;
	rdfs:subPropertyOf knora-base:hasLinkTo;
	knora-base:subjectClassConstraint text:Text;
	knora-base:objectClassConstraint human:Person.

text:hasAnnotatorValue
	a owl:ObjectProperty;
	rdfs:label "text has annotator - statement"@en, "Text hat AnnotatorIn - Festlegung"@de;
	rdfs:comment """Relating a text to a reification statement of the relation between the text and a person who annotated it."""@en;
	rdfs:subPropertyOf knora-base:hasLinkToValue;
	knora-base:subjectClassConstraint text:Text;
	knora-base:objectClassConstraint knora-base:LinkValue.

text:hasGlossator
	a owl:ObjectProperty;
	rdfs:label "has glossator"@en, "hat Glossator"@de;
	rdfs:comment """Relating a text to a person who glossed it."""@en;
	rdfs:subPropertyOf knora-base:hasLinkTo;
	knora-base:subjectClassConstraint text:Text;
	knora-base:objectClassConstraint human:Person.

text:hasGlossatorValue
	a owl:ObjectProperty;
	rdfs:label "has glossator - statement"@en, "hat Glossator - Festlegung"@de;
	rdfs:comment """Relating a text to a reification statement of the relation between the text and a person who glossed it."""@en;
	rdfs:subPropertyOf knora-base:hasLinkToValue;
	knora-base:subjectClassConstraint text:Text;
	knora-base:objectClassConstraint knora-base:LinkValue.

text:hasAbbreviator
	a owl:ObjectProperty;
	rdfs:label "has abbreviator"@en, "hat Abkurzer"@de;
	rdfs:comment """Relating a text to a person who abbreviated it."""@en;
	rdfs:subPropertyOf knora-base:hasLinkTo;
	knora-base:subjectClassConstraint text:Text;
	knora-base:objectClassConstraint human:Person.

text:hasAbbreviatorValue
	a owl:ObjectProperty;
	rdfs:label "has abbreviator - statement"@en, "hat Abkurzer - Festlegung"@de;
	rdfs:comment """Relating a text to a reification statement of the relation between the text and a person who abbreviated it."""@en;
	rdfs:subPropertyOf knora-base:hasLinkToValue;
	knora-base:subjectClassConstraint text:Text;
	knora-base:objectClassConstraint knora-base:LinkValue.

text:isNormalizedAs
	a owl:ObjectProperty;
	rdfs:label "is normalized as"@en, "ist normalisiert als"@de;
	rdfs:comment """Relating a text to a normalized derivative."""@en;
	rdfs:subPropertyOf knora-base:hasLinkTo;
	knora-base:subjectClassConstraint text:Text;
	knora-base:objectClassConstraint text:NormalizedDerivative.

text:isNormalizedAsValue
	a owl:ObjectProperty;
	rdfs:label "is normalized as - statement"@en, "ist normalisiert als - Festlegung"@de;
	rdfs:comment """Relating a text to a reification statement of the relation between the text and a a normalized derivative."""@en;
	rdfs:subPropertyOf knora-base:hasLinkToValue;
	knora-base:subjectClassConstraint text:Text;
	knora-base:objectClassConstraint knora-base:LinkValue.

text:hasCompiler
	a owl:ObjectProperty;
	rdfs:label "text has compiler"@en, "Text hat KompilatorIn"@de;
	rdfs:comment """Relating a text to a person who compiled it."""@en;
	rdfs:subPropertyOf knora-base:hasLinkTo;
	knora-base:subjectClassConstraint text:Text;
	knora-base:objectClassConstraint human:Person.

text:hasCompilerValue
	a owl:ObjectProperty;
	rdfs:label "text has compiler - statement"@en, "Text hat KompilatorIn - Festlegung"@de;
	rdfs:comment """Relating a text to a reification statement of the relation between the text and a person who compiled it."""@en;
	rdfs:subPropertyOf knora-base:hasLinkToValue;
	knora-base:subjectClassConstraint text:Text;
	knora-base:objectClassConstraint knora-base:LinkValue.

text:isNormalizationOf
	a owl:ObjectProperty;
	rdfs:label "is normalization of"@en, "ist Normalisierung von"@de;
	rdfs:comment """Relating a text normalization to its source text."""@en;
	rdfs:subPropertyOf knora-base:hasLinkTo;
	knora-base:subjectClassConstraint text:Normalization;
	knora-base:objectClassConstraint text:Text.

text:isNormalizationOfValue
	a owl:ObjectProperty;
	rdfs:label "is normalization of - statement"@en, "ist Normalisierung von - Festlegung"@de;
	rdfs:comment """Relating a text normalization to a reification statement of the relation between the text and its source text."""@en;
	rdfs:subPropertyOf knora-base:hasLinkToValue;
	knora-base:subjectClassConstraint text:Normalization;
	knora-base:objectClassConstraint knora-base:LinkValue.